@prefix cs: <https://example.org/test_> .
@prefix dcat: <http://www.w3.org/ns/dcat#> .
@prefix dcterms: <http://purl.org/dc/terms/> .
@prefix owl: <http://www.w3.org/2002/07/owl#> .
@prefix skos: <http://www.w3.org/2004/02/skos/core#> .
@prefix xsd: <http://www.w3.org/2001/XMLSchema#> .

<https://w3id.org/nfdi4cat/voc4cat_0000005> a skos:Concept ;
    dcterms:identifier "voc4cat_0000005"^^xsd:token ;
    dcterms:provenance "Self"@en ;
    skos:broader <https://w3id.org/nfdi4cat/voc4cat_0000004> ;
    skos:definition "A chemical compound formed by the reaction of a metal with oxygen."@en ;
    skos:inScheme cs: ;
    skos:prefLabel "metal oxide"@en .

<https://w3id.org/nfdi4cat/voc4cat_0000007> a skos:Concept ;
    dcterms:identifier "voc4cat_0000007"^^xsd:token ;
    dcterms:provenance "Self"@en ;
    skos:altLabel "EF"@en ;
    skos:broader <https://w3id.org/nfdi4cat/voc4cat_0000006> ;
    skos:definition "The energy level in a semiconductor where the probability of finding an electron is 0.5. "@en ;
    skos:inScheme cs: ;
    skos:prefLabel "Fermi level"@en .

<https://w3id.org/nfdi4cat/voc4cat_0000008> a skos:Concept ;
    dcterms:identifier "voc4cat_0000008"^^xsd:token ;
    dcterms:provenance "Self"@en ;
    skos:broader <https://w3id.org/nfdi4cat/voc4cat_0000006> ;
    skos:definition "The degree of a three-dimensional structural order of atoms which constitute the crystal lattice of a material."@en ;
    skos:inScheme cs: ;
    skos:prefLabel "crystallinity"@en .

<https://w3id.org/nfdi4cat/voc4cat_0000009> a skos:Concept ;
    dcterms:identifier "voc4cat_0000009"^^xsd:token ;
    dcterms:provenance "Self"@en ;
    skos:broader <https://w3id.org/nfdi4cat/voc4cat_0000006> ;
    skos:definition "Pore size distribution refers to the range of pore sizes in a material. "@en ;
    skos:inScheme cs: ;
    skos:prefLabel "pore size distribution"@en .

<https://w3id.org/nfdi4cat/voc4cat_0000010> a skos:Concept ;
    dcterms:identifier "voc4cat_0000010"^^xsd:token ;
    dcterms:provenance "Self"@en ;
    skos:altLabel "energy bandgap; Eg"@en ;
    skos:broader <https://w3id.org/nfdi4cat/voc4cat_0000006> ;
    skos:definition "The energy difference between a semiconductor’s valence band top and conduction band bottom, which is required to excite an electron from the former to the latter.  "@en ;
    skos:inScheme cs: ;
    skos:prefLabel "bandgap energy"@en .

<https://w3id.org/nfdi4cat/voc4cat_0000011> a skos:Concept ;
    dcterms:identifier "voc4cat_0000011"^^xsd:token ;
    dcterms:provenance "Self"@en ;
    skos:altLabel "VB"@en ;
    skos:broader <https://w3id.org/nfdi4cat/voc4cat_0000006> ;
    skos:definition "The band of energy levels in a solid fully occupied by electrons at 0 K (273.15 °C)."@en ;
    skos:inScheme cs: ;
    skos:prefLabel "valence band"@en .

<https://w3id.org/nfdi4cat/voc4cat_0000012> a skos:Concept ;
    dcterms:identifier "voc4cat_0000012"^^xsd:token ;
    dcterms:provenance "Self"@en ;
    skos:altLabel "CB"@en ;
    skos:broader <https://w3id.org/nfdi4cat/voc4cat_0000006> ;
    skos:definition "The energy band of electronic levels of partially or fully filled mobile electrons in a metal or a semiconductor. "@en ;
    skos:inScheme cs: ;
    skos:prefLabel "conduction band"@en .

<https://w3id.org/nfdi4cat/voc4cat_0000013> a skos:Concept ;
    dcterms:identifier "voc4cat_0000013"^^xsd:token ;
    dcterms:provenance "Self"@en ;
    skos:altLabel "SSA"@en ;
    skos:broader <https://w3id.org/nfdi4cat/voc4cat_0000006> ;
    skos:definition "Α measure of the total surface area of a material per unit mass or volume."@en ;
    skos:inScheme cs: ;
    skos:prefLabel "specific surface area"@en .

<https://w3id.org/nfdi4cat/voc4cat_0000015> a skos:Concept ;
    dcterms:identifier "voc4cat_0000015"^^xsd:token ;
    dcterms:provenance "Self"@en ;
    skos:broader <https://w3id.org/nfdi4cat/voc4cat_0000014> ;
    skos:definition "The introduction of foreign atoms into a semiconductor leading to the formation of new energy levels and charge concentrations."@en ;
    skos:inScheme cs: ;
    skos:prefLabel "doping"@en .

<https://w3id.org/nfdi4cat/voc4cat_0000018> a skos:Concept ;
    dcterms:identifier "voc4cat_0000018"^^xsd:token ;
    dcterms:provenance "Self"@en ;
    skos:broader <https://w3id.org/nfdi4cat/voc4cat_0000017> ;
    skos:definition "Mass of a powdered photocatalyst used for an experiment."@en ;
    skos:inScheme cs: ;
    skos:prefLabel "powder mass"@en .

<https://w3id.org/nfdi4cat/voc4cat_0000021> a skos:Concept ;
    dcterms:identifier "voc4cat_0000021"^^xsd:token ;
    dcterms:provenance "Self"@en ;
    skos:altLabel "spray-coating"@en ;
    skos:broader <https://w3id.org/nfdi4cat/voc4cat_0000020> ;
    skos:definition "A technique used to deposit uniform thin films onto a substrate by spraying a solution of the material onto the surface."@en ;
    skos:inScheme cs: ;
    skos:prefLabel "spray coating"@en .

<https://w3id.org/nfdi4cat/voc4cat_0000022> a skos:Concept ;
    dcterms:identifier "voc4cat_0000022"^^xsd:token ;
    dcterms:provenance "Self"@en ;
    skos:broader <https://w3id.org/nfdi4cat/voc4cat_0000020> ;
    skos:definition "A tape-casting method used to deposit thin films of a photocatalyst onto the surface of a substrate."@en ;
    skos:inScheme cs: ;
    skos:prefLabel "doctor blading"@en .

<https://w3id.org/nfdi4cat/voc4cat_0000023> a skos:Concept ;
    dcterms:identifier "voc4cat_0000023"^^xsd:token ;
    dcterms:provenance "Self"@en ;
    skos:altLabel "spin casting"@en,
        "spin-casting"@en,
        "spin-coating"@en ;
    skos:broader <https://w3id.org/nfdi4cat/voc4cat_0000020> ;
    skos:definition "A technique used to deposit uniform thin films onto a substrate (e.g., metal or glass) by spinning at high speeds a solution (paste) of the material onto the surface."@en ;
    skos:inScheme cs: ;
    skos:prefLabel "spin coating"@en .

<https://w3id.org/nfdi4cat/voc4cat_0000026> a skos:Concept ;
    dcterms:identifier "voc4cat_0000026"^^xsd:token ;
    dcterms:provenance "Self"@en ;
    skos:broader <https://w3id.org/nfdi4cat/voc4cat_0000025> ;
    skos:definition "A  flat surface made of a metal (e.g., titanium, stainless steel) serving as a substrate for the deposition of a photocatalyst."@en ;
    skos:inScheme cs: ;
    skos:prefLabel "metallic substrate"@en .

<https://w3id.org/nfdi4cat/voc4cat_0000028> a skos:Concept ;
    dcterms:identifier "voc4cat_0000028"^^xsd:token ;
    dcterms:provenance "Self"@en ;
    skos:altLabel "FTO; FTO glass"@en ;
    skos:broader <https://w3id.org/nfdi4cat/voc4cat_0000027> ;
    skos:definition "Transparent conductive metal oxide (fluorine doped tin oxide) that can be used in the fabrication of transparent electrodes for thin films."@en ;
    skos:inScheme cs: ;
    skos:prefLabel "fluorine doped tin oxide coated glass"@en .

<https://w3id.org/nfdi4cat/voc4cat_0000029> a skos:Concept ;
    dcterms:identifier "voc4cat_0000029"^^xsd:token ;
    dcterms:provenance "Self"@en ;
    skos:altLabel "ITO; ITO glass"@en ;
    skos:broader <https://w3id.org/nfdi4cat/voc4cat_0000027> ;
    skos:definition "Transparent conductive metal oxide (indium tin oxide) that can be used in the fabrication of transparent electrodes for thin films."@en ;
    skos:inScheme cs: ;
    skos:prefLabel "indium tin oxide coated glass"@en .

<https://w3id.org/nfdi4cat/voc4cat_0000030> a skos:Concept ;
    dcterms:identifier "voc4cat_0000030"^^xsd:token ;
    dcterms:provenance "Self"@en ;
    skos:broader <https://w3id.org/nfdi4cat/voc4cat_0000027> ;
    skos:definition "A resistant to thermal shock type of glass, composed mainly of silica and boron trioxide."@en ;
    skos:inScheme cs: ;
    skos:prefLabel "borosilicate glass"@en .

<https://w3id.org/nfdi4cat/voc4cat_0000031> a skos:Concept ;
    dcterms:identifier "voc4cat_0000031"^^xsd:token ;
    dcterms:provenance "Self"@en ;
    skos:altLabel "quartz"@en ;
    skos:broader <https://w3id.org/nfdi4cat/voc4cat_0000027> ;
    skos:definition "A type of pure silicon dioxide, highly crystalline glass that allows the transmission of light in the UV wavelength range."@en ;
    skos:inScheme cs: ;
    skos:prefLabel "quartz glass"@en .

<https://w3id.org/nfdi4cat/voc4cat_0000032> a skos:Concept ;
    dcterms:identifier "voc4cat_0000032"^^xsd:token ;
    dcterms:provenance "Self"@en ;
    skos:broader <https://w3id.org/nfdi4cat/voc4cat_0000025> ;
    skos:definition "A  surface made of a ceramic material (e.g., alumina) serving as a substrate for the deposition of a photocatalyst."@en ;
    skos:inScheme cs: ;
    skos:prefLabel "ceramic substrate"@en .

<https://w3id.org/nfdi4cat/voc4cat_0000034> a skos:Concept ;
    dcterms:identifier "voc4cat_0000034"^^xsd:token ;
    dcterms:provenance "Self"@en ;
    skos:broader <https://w3id.org/nfdi4cat/voc4cat_0000033> ;
    skos:definition "The width of the substrate."@en ;
    skos:inScheme cs: ;
    skos:prefLabel "substrate width"@en .

<https://w3id.org/nfdi4cat/voc4cat_0000035> a skos:Concept ;
    dcterms:identifier "voc4cat_0000035"^^xsd:token ;
    dcterms:provenance "Self"@en ;
    skos:broader <https://w3id.org/nfdi4cat/voc4cat_0000033> ;
    skos:definition "The depth of the substrate."@en ;
    skos:inScheme cs: ;
    skos:prefLabel "substrate depth"@en .

<https://w3id.org/nfdi4cat/voc4cat_0000036> a skos:Concept ;
    dcterms:identifier "voc4cat_0000036"^^xsd:token ;
    dcterms:provenance "Self"@en ;
    skos:broader <https://w3id.org/nfdi4cat/voc4cat_0000033> ;
    skos:definition "The thickness of the substrate."@en ;
    skos:inScheme cs: ;
    skos:prefLabel "substrate thickness"@en .

<https://w3id.org/nfdi4cat/voc4cat_0000037> a skos:Concept ;
    dcterms:identifier "voc4cat_0000037"^^xsd:token ;
    dcterms:provenance "Self"@en ;
    skos:altLabel "substrate surface area"@en ;
    skos:broader <https://w3id.org/nfdi4cat/voc4cat_0000033> ;
    skos:definition "The surface area of the substrate."@en ;
    skos:inScheme cs: ;
    skos:prefLabel "substrate area"@en .

<https://w3id.org/nfdi4cat/voc4cat_0000039> a skos:Concept ;
    dcterms:identifier "voc4cat_0000039"^^xsd:token ;
    dcterms:provenance "Self"@en ;
    skos:broader <https://w3id.org/nfdi4cat/voc4cat_0000038> ;
    skos:definition "Mass of catalyst deposited onto the surface of a substrate."@en ;
    skos:inScheme cs: ;
    skos:prefLabel "thin film mass"@en .

<https://w3id.org/nfdi4cat/voc4cat_0000041> a skos:Concept ;
    dcterms:identifier "voc4cat_0000041"^^xsd:token ;
    dcterms:provenance "Self"@en ;
    skos:broader <https://w3id.org/nfdi4cat/voc4cat_0000040> ;
    skos:definition "The width of the film of the deposited photocatalyst."@en ;
    skos:inScheme cs: ;
    skos:prefLabel "thin film width"@en .

<https://w3id.org/nfdi4cat/voc4cat_0000042> a skos:Concept ;
    dcterms:identifier "voc4cat_0000042"^^xsd:token ;
    dcterms:provenance "Self"@en ;
    skos:broader <https://w3id.org/nfdi4cat/voc4cat_0000040> ;
    skos:definition "The thickness of the film of the deposited photocatalyst. "@en ;
    skos:inScheme cs: ;
    skos:prefLabel "thin film thickness"@en .

<https://w3id.org/nfdi4cat/voc4cat_0000043> a skos:Concept ;
    dcterms:identifier "voc4cat_0000043"^^xsd:token ;
    dcterms:provenance "Self"@en ;
    skos:broader <https://w3id.org/nfdi4cat/voc4cat_0000040> ;
    skos:definition "The depth of the film of the deposited photocatalyst."@en ;
    skos:inScheme cs: ;
    skos:prefLabel "thin film depth"@en .

<https://w3id.org/nfdi4cat/voc4cat_0000044> a skos:Concept ;
    dcterms:identifier "voc4cat_0000044"^^xsd:token ;
    dcterms:provenance "Self"@en ;
    skos:broader <https://w3id.org/nfdi4cat/voc4cat_0000040> ;
    skos:definition "The area of the substrate covered by the deposited photocatalyst."@en ;
    skos:inScheme cs: ;
    skos:prefLabel "thin film area"@en .

<https://w3id.org/nfdi4cat/voc4cat_0000047> a skos:Concept ;
    dcterms:identifier "voc4cat_0000047"^^xsd:token ;
    dcterms:provenance "Self"@en ;
    skos:broader <https://w3id.org/nfdi4cat/voc4cat_0000046> ;
    skos:definition "Filtering of literature research to include only the most relevant sources of information for the application / experiment / catalysts of interest."@en ;
    skos:inScheme cs: ;
    skos:prefLabel "literature collection"@en .

<https://w3id.org/nfdi4cat/voc4cat_0000048> a skos:Concept ;
    dcterms:identifier "voc4cat_0000048"^^xsd:token ;
    dcterms:provenance "Self"@en ;
    skos:altLabel "literature organization; organization of literature; citation management software"@en ;
    skos:broader <https://w3id.org/nfdi4cat/voc4cat_0000046> ;
    skos:definition "Addition and organization of relevant literature of interest using a citation management software (e.g., Mendeley, Zotero, EndNote etc.) allowing for easy access and categorization."@en ;
    skos:inScheme cs: ;
    skos:prefLabel "literature organization"@en .

<https://w3id.org/nfdi4cat/voc4cat_0000050> a skos:Concept ;
    dcterms:identifier "voc4cat_0000050"^^xsd:token ;
    dcterms:provenance "Self"@en ;
    skos:broader <https://w3id.org/nfdi4cat/voc4cat_0000049> ;
    skos:definition "Duration of each synthesis step needed to synthesize the desired photocatalyst."@en ;
    skos:inScheme cs: ;
    skos:prefLabel "synthesis duration"@en .

<https://w3id.org/nfdi4cat/voc4cat_0000051> a skos:Concept ;
    dcterms:identifier "voc4cat_0000051"^^xsd:token ;
    dcterms:provenance "Self"@en ;
    skos:broader <https://w3id.org/nfdi4cat/voc4cat_0000049> ;
    skos:definition "Temperature externally applied (if necessary) in any of the synthesis step. Higher temperature values can be observed if an exothermic reaction takes place during the synthesis."@en ;
    skos:inScheme cs: ;
    skos:prefLabel "synthesis temperature"@en .

<https://w3id.org/nfdi4cat/voc4cat_0000052> a skos:Concept ;
    dcterms:identifier "voc4cat_0000052"^^xsd:token ;
    dcterms:provenance "Self"@en ;
    skos:broader <https://w3id.org/nfdi4cat/voc4cat_0000049> ;
    skos:definition "pH value in each of the synthesis steps"@en ;
    skos:inScheme cs: ;
    skos:prefLabel "synthesis pH"@en .

<https://w3id.org/nfdi4cat/voc4cat_0000053> a skos:Concept ;
    dcterms:identifier "voc4cat_0000053"^^xsd:token ;
    dcterms:provenance "Self"@en ;
    skos:broader <https://w3id.org/nfdi4cat/voc4cat_0000049> ;
    skos:definition "Pressure applied (if necessary) in any of the synthesis step. Changes in the pressure may be observed if variations in the temperature of the reaction occur (e.g., exothermic reaction) "@en ;
    skos:inScheme cs: ;
    skos:prefLabel "synthesis pressure"@en .

<https://w3id.org/nfdi4cat/voc4cat_0000055> a skos:Concept ;
    dcterms:identifier "voc4cat_0000055"^^xsd:token ;
    dcterms:provenance "Self"@en ;
    skos:broader <https://w3id.org/nfdi4cat/voc4cat_0000054> ;
    skos:definition "A gas flow under which the calcination step takes place (e,g,, Ar or synthetic air)"@en ;
    skos:inScheme cs: ;
    skos:prefLabel "gaseous environment in calcination"@en .

<https://w3id.org/nfdi4cat/voc4cat_0000056> a skos:Concept ;
    dcterms:identifier "voc4cat_0000056"^^xsd:token ;
    dcterms:provenance "Self"@en ;
    skos:broader <https://w3id.org/nfdi4cat/voc4cat_0000054> ;
    skos:definition "The flow of gas (usually in ml min-1) used in the calcination steps during synthesis"@en ;
    skos:inScheme cs: ;
    skos:prefLabel "gas flow rate in calcination"@en .

<https://w3id.org/nfdi4cat/voc4cat_0000057> a skos:Concept ;
    dcterms:identifier "voc4cat_0000057"^^xsd:token ;
    dcterms:provenance "Self"@en ;
    skos:broader <https://w3id.org/nfdi4cat/voc4cat_0000054> ;
    skos:definition "Initial temperature of the calcination step."@en ;
    skos:inScheme cs: ;
    skos:prefLabel "calcination initial temperature"@en .

<https://w3id.org/nfdi4cat/voc4cat_0000058> a skos:Concept ;
    dcterms:identifier "voc4cat_0000058"^^xsd:token ;
    dcterms:provenance "Self"@en ;
    skos:broader <https://w3id.org/nfdi4cat/voc4cat_0000054> ;
    skos:definition "Final temperature of the calcination step."@en ;
    skos:inScheme cs: ;
    skos:prefLabel "calcination final temperature"@en .

<https://w3id.org/nfdi4cat/voc4cat_0000059> a skos:Concept ;
    dcterms:identifier "voc4cat_0000059"^^xsd:token ;
    dcterms:provenance "Self"@en ;
    skos:broader <https://w3id.org/nfdi4cat/voc4cat_0000054> ;
    skos:definition "Rate of increasing or decreasing the temperature during the calcination step. Usually mentioned in K min-1."@en ;
    skos:inScheme cs: ;
    skos:prefLabel "calcination heating rate"@en .

<https://w3id.org/nfdi4cat/voc4cat_0000060> a skos:Concept ;
    dcterms:identifier "voc4cat_0000060"^^xsd:token ;
    dcterms:provenance "Self"@en ;
    skos:broader <https://w3id.org/nfdi4cat/voc4cat_0000054> ;
    skos:definition "Time (usually in h) for which a desired temperature is held."@en ;
    skos:inScheme cs: ;
    skos:prefLabel "calcination dwelling time"@en .

<https://w3id.org/nfdi4cat/voc4cat_0000061> a skos:Concept ;
    dcterms:identifier "voc4cat_0000061"^^xsd:token ;
    dcterms:provenance "Self"@en ;
    skos:broader <https://w3id.org/nfdi4cat/voc4cat_0000049> ;
    skos:definition "Equipment used in each step of the synthesis of the photocatalysts. The equipment can incude (but not limited to): crucibles, pH meters, condensers, volumetric cylinders, centrifuges, test tubes, flasks, beakers, mechanical shakers, pipettes, syringes, magenetic stirrers, heating plates, fitlers, funnels and digital balances."@en ;
    skos:inScheme cs: ;
    skos:prefLabel "synthesis equipment"@en .

<https://w3id.org/nfdi4cat/voc4cat_0000063> a skos:Concept ;
    dcterms:identifier "voc4cat_0000063"^^xsd:token ;
    dcterms:provenance "Self"@en ;
    skos:broader <https://w3id.org/nfdi4cat/voc4cat_0000062> ;
    skos:definition "Mass of chemicals used for synthesis"@en ;
    skos:inScheme cs: ;
    skos:prefLabel "mass of chemical substance for synthesis"@en .

<https://w3id.org/nfdi4cat/voc4cat_0000064> a skos:Concept ;
    dcterms:identifier "voc4cat_0000064"^^xsd:token ;
    dcterms:provenance "Self"@en ;
    skos:broader <https://w3id.org/nfdi4cat/voc4cat_0000062> ;
    skos:definition "Volume of chemicals used for synthesis"@en ;
    skos:inScheme cs: ;
    skos:prefLabel "volume chemical substance for synthesis"@en .

<https://w3id.org/nfdi4cat/voc4cat_0000065> a skos:Concept ;
    dcterms:identifier "voc4cat_0000065"^^xsd:token ;
    dcterms:provenance "Self"@en ;
    skos:broader <https://w3id.org/nfdi4cat/voc4cat_0000062> ;
    skos:definition "Concentration of chemicals used for synthesis"@en ;
    skos:inScheme cs: ;
    skos:prefLabel "concentration chemical substance for synthesis"@en .

<https://w3id.org/nfdi4cat/voc4cat_0000085> a skos:Concept ;
    dcterms:identifier "voc4cat_0000085"^^xsd:token ;
    dcterms:provenance "Self"@en ;
    skos:broader <https://w3id.org/nfdi4cat/voc4cat_0000084> ;
    skos:definition "Τhe lowest energy state of a system. "@en ;
    skos:inScheme cs: ;
    skos:prefLabel "ground state"@en .

<https://w3id.org/nfdi4cat/voc4cat_0000086> a skos:Concept ;
    dcterms:identifier "voc4cat_0000086"^^xsd:token ;
    dcterms:provenance "Self"@en ;
    skos:broader <https://w3id.org/nfdi4cat/voc4cat_0000084> ;
    skos:definition "Τhe temporary state of a system with higher energy than its ground state caused by an external factor. "@en ;
    skos:inScheme cs: ;
    skos:prefLabel "excited state"@en .

<https://w3id.org/nfdi4cat/voc4cat_0000088> a skos:Concept ;
    dcterms:identifier "voc4cat_0000088"^^xsd:token ;
    dcterms:provenance "Self"@en ;
    skos:broader <https://w3id.org/nfdi4cat/voc4cat_0000087> ;
    skos:definition "The transfer of an electron initiated by the absorption of a photon of sufficient energy. "@en ;
    skos:inScheme cs: ;
    skos:prefLabel "photoinduced electron transfer"@en .

<https://w3id.org/nfdi4cat/voc4cat_0000089> a skos:Concept ;
    dcterms:identifier "voc4cat_0000089"^^xsd:token ;
    dcterms:provenance "Self"@en ;
    skos:broader <https://w3id.org/nfdi4cat/voc4cat_0000087> ;
    skos:definition "The transfer of a hole initiated by the absorption of a photon of sufficient energy. "@en ;
    skos:inScheme cs: ;
    skos:prefLabel "photoinduced hole transfer"@en .

<https://w3id.org/nfdi4cat/voc4cat_0000090> a skos:Concept ;
    dcterms:identifier "voc4cat_0000090"^^xsd:token ;
    dcterms:provenance "Self"@en ;
    skos:altLabel "charge photogeneration; photogenerated charges; charge photo-generation; electron excitation; electron-hole pair;"@en ;
    skos:broader <https://w3id.org/nfdi4cat/voc4cat_0000087> ;
    skos:definition "The generation of electron - hole pairs in a semiconductor as a result of light absorption of sufficient energy to overcome the bandgap energy. Electrons (negative charge) get excited to the conduction band, while holes (positive charge) remain in the valence band. "@en ;
    skos:inScheme cs: ;
    skos:prefLabel "photoinduced charge generation"@en .

<https://w3id.org/nfdi4cat/voc4cat_0000091> a skos:Concept ;
    dcterms:identifier "voc4cat_0000091"^^xsd:token ;
    dcterms:provenance "Self"@en ;
    skos:broader <https://w3id.org/nfdi4cat/voc4cat_0000087> ;
    skos:definition "The process by which photogenerated charges (electrons and holes) in a semiconductor recombine, resulting in the dissipation of energy in the form of e.g., heat or light. "@en ;
    skos:inScheme cs: ;
    skos:prefLabel "charge recombination"@en .

<https://w3id.org/nfdi4cat/voc4cat_0000092> a skos:Concept ;
    dcterms:identifier "voc4cat_0000092"^^xsd:token ;
    dcterms:provenance "Self"@en ;
    skos:broader <https://w3id.org/nfdi4cat/voc4cat_0000087> ;
    skos:definition "Absorption is the process in which energy (e.g., photons) or an absorbent (e.g., a gas) is taken up by an absorbate. "@en ;
    skos:inScheme cs: ;
    skos:prefLabel "absorption"@en .

<https://w3id.org/nfdi4cat/voc4cat_0000093> a skos:Concept ;
    dcterms:identifier "voc4cat_0000093"^^xsd:token ;
    dcterms:provenance "Self"@en ;
    skos:broader <https://w3id.org/nfdi4cat/voc4cat_0000087> ;
    skos:definition "The binding (strong or weak) of a pollutant or a reactant molecule on the surface of a photocatalyst which facilitates the performance of photocatalytic reactions."@en ;
    skos:inScheme cs: ;
    skos:prefLabel "adsorption"@en .

<https://w3id.org/nfdi4cat/voc4cat_0000094> a skos:Concept ;
    dcterms:identifier "voc4cat_0000094"^^xsd:token ;
    dcterms:provenance "Self"@en ;
    skos:broader <https://w3id.org/nfdi4cat/voc4cat_0000087> ;
    skos:definition "The process under which reactants, intermediates and products are released from the surface of the photocatalyst. Desoprtion can be faciliated by an increase in temparature or a change in the pH."@en ;
    skos:inScheme cs: ;
    skos:prefLabel "desorption"@en .

<https://w3id.org/nfdi4cat/voc4cat_0000095> a skos:Concept ;
    dcterms:identifier "voc4cat_0000095"^^xsd:token ;
    dcterms:provenance "Self"@en ;
    skos:broader <https://w3id.org/nfdi4cat/voc4cat_0000087> ;
    skos:definition "The process of separating positive and negative charges in a semiconductor, typically as a result of an external force, (e.g., photoexcitation). "@en ;
    skos:inScheme cs: ;
    skos:prefLabel "charge separation"@en .

<https://w3id.org/nfdi4cat/voc4cat_0000096> a skos:Concept ;
    dcterms:identifier "voc4cat_0000096"^^xsd:token ;
    dcterms:provenance "Self"@en ;
    skos:altLabel "photo-excitation"@en ;
    skos:broader <https://w3id.org/nfdi4cat/voc4cat_0000087> ;
    skos:definition "The state caused by the transition of electrons from the valence band top to the conduction band bottom by absorption of photons of sufficient energy.  "@en ;
    skos:inScheme cs: ;
    skos:prefLabel "photoexcitation"@en .

<https://w3id.org/nfdi4cat/voc4cat_0000097> a skos:Concept ;
    dcterms:identifier "voc4cat_0000097"^^xsd:token ;
    dcterms:provenance "Self"@en ;
    skos:broader <https://w3id.org/nfdi4cat/voc4cat_0000087> ;
    skos:definition "The loss of electrons or an increase in the oxidation state of a species. "@en ;
    skos:inScheme cs: ;
    skos:prefLabel "oxidation"@en .

<https://w3id.org/nfdi4cat/voc4cat_0000099> a skos:Concept ;
    dcterms:identifier "voc4cat_0000099"^^xsd:token ;
    dcterms:provenance "Self"@en ;
    skos:altLabel "photocatalytic carbon dioxide reduction; CO2 photoreduction; carbon dioxide photoreduction; artificial photosynthesis"@en ;
    skos:broader <https://w3id.org/nfdi4cat/voc4cat_0000098> ;
    skos:definition "The light-driven reduction (conversion) of carbon dioxide (CO2) to hydrocarbons and / or platform chemicals in presence of water. The absorption of light and the adsorption of the reactants is performed by a photocatalyst (usually a metal oxide). "@en ;
    skos:inScheme cs: ;
    skos:prefLabel "photocatalytic CO2 reduction"@en .

<https://w3id.org/nfdi4cat/voc4cat_0000102> a skos:Concept ;
    dcterms:identifier "voc4cat_0000102"^^xsd:token ;
    dcterms:provenance "Self"@en ;
    skos:broader <https://w3id.org/nfdi4cat/voc4cat_0000101> ;
    skos:definition "Concentration of the reactants (e.g., CO2 and H2O) used in the photocatalytic CO2 reduction experiments"@en ;
    skos:inScheme cs: ;
    skos:prefLabel "reactant concentration"@en .

<https://w3id.org/nfdi4cat/voc4cat_0000103> a skos:Concept ;
    dcterms:identifier "voc4cat_0000103"^^xsd:token ;
    dcterms:provenance "Self"@en ;
    skos:broader <https://w3id.org/nfdi4cat/voc4cat_0000101> ;
    skos:definition "Purity of reactants (e.g., CO2, H2O, He) used in the photocatalytic CO2 reduction experiments. Purity is measure of the impurities contained in the reactants' supply. The highest purity reactants should be used to ensure the collection of reliable results. "@en ;
    skos:inScheme cs: ;
    skos:prefLabel "reactant purity"@en .

<https://w3id.org/nfdi4cat/voc4cat_0000104> a skos:Concept ;
    dcterms:identifier "voc4cat_0000104"^^xsd:token ;
    dcterms:provenance "Self"@en ;
    skos:broader <https://w3id.org/nfdi4cat/voc4cat_0000101> ;
    skos:definition "The rate of flow of reactants (often in ml per min) in the photoreactor. Flow rates are usually controlled by mass flow controllers (MFCs)  "@en ;
    skos:inScheme cs: ;
    skos:prefLabel "reactant flow rate"@en .

<https://w3id.org/nfdi4cat/voc4cat_0000106> a skos:Concept ;
    dcterms:identifier "voc4cat_0000106"^^xsd:token ;
    dcterms:provenance "Self"@en ;
    skos:broader <https://w3id.org/nfdi4cat/voc4cat_0000105> ;
    skos:definition "A molecule that accepts electrons from photoexcited species in a redox reaction and is subsequently consumed or degraded."@en ;
    skos:inScheme cs: ;
    skos:prefLabel "sacrificial acceptor"@en .

<https://w3id.org/nfdi4cat/voc4cat_0000107> a skos:Concept ;
    dcterms:identifier "voc4cat_0000107"^^xsd:token ;
    dcterms:provenance "Self"@en ;
    skos:broader <https://w3id.org/nfdi4cat/voc4cat_0000105> ;
    skos:definition "A molecule that donates electrons from photoexcited species in a redox reaction and is subsequently consumed or degraded."@en ;
    skos:inScheme cs: ;
    skos:prefLabel "sacrificial donor"@en .

<https://w3id.org/nfdi4cat/voc4cat_0000109> a skos:Concept ;
    dcterms:identifier "voc4cat_0000109"^^xsd:token ;
    dcterms:provenance "Self"@en ;
    skos:altLabel "continuous flow mode"@en,
        "continuous-flow mode"@en,
        "flow-mode"@en ;
    skos:broader <https://w3id.org/nfdi4cat/voc4cat_0000108> ;
    skos:definition " Under flow conditions, a continuous flow of reactants is supplied to the reaction chamber and the formed products are removed and identified by an appropriate technique."@en ;
    skos:inScheme cs: ;
    skos:prefLabel "flow mode"@en .

<https://w3id.org/nfdi4cat/voc4cat_0000110> a skos:Concept ;
    dcterms:identifier "voc4cat_0000110"^^xsd:token ;
    dcterms:provenance "Self"@en ;
    skos:altLabel "batch-mode"@en ;
    skos:broader <https://w3id.org/nfdi4cat/voc4cat_0000108> ;
    skos:definition "Operation mode in which the reaction chamber is filled with the (reactant) gas(es) up to a certain pressure, and the photoreaction products acummulate over time."@en ;
    skos:inScheme cs: ;
    skos:prefLabel "batch mode"@en .

<https://w3id.org/nfdi4cat/voc4cat_0000112> a skos:Concept ;
    dcterms:identifier "voc4cat_0000112"^^xsd:token ;
    dcterms:provenance "Self"@en ;
    skos:broader <https://w3id.org/nfdi4cat/voc4cat_0000111> ;
    skos:definition "Time for which a gas is purged through the reaction chamber."@en ;
    skos:inScheme cs: ;
    skos:prefLabel "purging duration"@en .

<https://w3id.org/nfdi4cat/voc4cat_0000113> a skos:Concept ;
    dcterms:identifier "voc4cat_0000113"^^xsd:token ;
    dcterms:provenance "Self"@en ;
    skos:broader <https://w3id.org/nfdi4cat/voc4cat_0000111> ;
    skos:definition "The time in between the collection of two data points."@en ;
    skos:inScheme cs: ;
    skos:prefLabel "sampling interval"@en .

<https://w3id.org/nfdi4cat/voc4cat_0000114> a skos:Concept ;
    dcterms:identifier "voc4cat_0000114"^^xsd:token ;
    dcterms:provenance "Self"@en ;
    skos:broader <https://w3id.org/nfdi4cat/voc4cat_0000111> ;
    skos:definition "The total duration in which the photocatalyst was under irradiation by the selected light source. "@en ;
    skos:inScheme cs: ;
    skos:prefLabel "irradiation duration"@en .

<https://w3id.org/nfdi4cat/voc4cat_0000116> a skos:Concept ;
    dcterms:identifier "voc4cat_0000116"^^xsd:token ;
    dcterms:provenance "Self"@en ;
    skos:broader <https://w3id.org/nfdi4cat/voc4cat_0000115> ;
    skos:definition "The temperature at the initiaton of the experiment."@en ;
    skos:inScheme cs: ;
    skos:prefLabel "experiment initial temperature"@en .

<https://w3id.org/nfdi4cat/voc4cat_0000117> a skos:Concept ;
    dcterms:identifier "voc4cat_0000117"^^xsd:token ;
    dcterms:provenance "Self"@en ;
    skos:broader <https://w3id.org/nfdi4cat/voc4cat_0000115> ;
    skos:definition "The temperature at the end of the experiment."@en ;
    skos:inScheme cs: ;
    skos:prefLabel "experiment final temperature"@en .

<https://w3id.org/nfdi4cat/voc4cat_0000119> a skos:Concept ;
    dcterms:identifier "voc4cat_0000119"^^xsd:token ;
    dcterms:provenance "Self"@en ;
    skos:broader <https://w3id.org/nfdi4cat/voc4cat_0000118> ;
    skos:definition "The pressure at the initiaton of the experiment or before a sampling event."@en ;
    skos:inScheme cs: ;
    skos:prefLabel "experiment initial pressure"@en .

<https://w3id.org/nfdi4cat/voc4cat_0000120> a skos:Concept ;
    dcterms:identifier "voc4cat_0000120"^^xsd:token ;
    dcterms:provenance "Self"@en ;
    skos:broader <https://w3id.org/nfdi4cat/voc4cat_0000118> ;
    skos:definition "The pressure at the end of the experiment or after a sampling event."@en ;
    skos:inScheme cs: ;
    skos:prefLabel "experiment final pressure"@en .

<https://w3id.org/nfdi4cat/voc4cat_0000121> a skos:Concept ;
    dcterms:identifier "voc4cat_0000121"^^xsd:token ;
    dcterms:provenance "Self"@en ;
    skos:broader <https://w3id.org/nfdi4cat/voc4cat_0000100> ;
    skos:definition "The pressure drop occuring when collecting a gaseous sample for the reaction chamber. This pressure drop should be taken into consideration when caluclation the concentration of formed products. "@en ;
    skos:inScheme cs: ;
    skos:prefLabel "experiment pressure drop"@en .

<https://w3id.org/nfdi4cat/voc4cat_0000122> a skos:Concept ;
    dcterms:identifier "voc4cat_0000122"^^xsd:token ;
    dcterms:provenance "Self"@en ;
    skos:broader <https://w3id.org/nfdi4cat/voc4cat_0000100> ;
    skos:definition "Pretreatment of the photocatalyst before its intoduction to the reaction chamber."@en ;
    skos:inScheme cs: ;
    skos:prefLabel "sample pre-treatment"@en .

<https://w3id.org/nfdi4cat/voc4cat_0000123> a skos:Concept ;
    dcterms:identifier "voc4cat_0000123"^^xsd:token ;
    dcterms:provenance "Self"@en ;
    skos:altLabel "control experiment"@en ;
    skos:broader <https://w3id.org/nfdi4cat/voc4cat_0000100> ;
    skos:definition "Measurements performed to ensure that the studied photocatalytic reaction occurs because of the interaction of the photocatalyst with the reactants, and not from the environment or the photoreactor. Such blank experiment incude experiments under dark conditions, experiments with light but without a photocatalyst and experiments under light in the presence of the photocatalyst but without the targeted reactants."@en ;
    skos:inScheme cs: ;
    skos:prefLabel "blank experiment"@en .

<https://w3id.org/nfdi4cat/voc4cat_0000125> a skos:Concept ;
    dcterms:identifier "voc4cat_0000125"^^xsd:token ;
    dcterms:provenance "Self"@en ;
    skos:broader <https://w3id.org/nfdi4cat/voc4cat_0000124> ;
    skos:definition "In photocatalytic processes where product formation is expected, selectivity describes the ability of a photocatalyst to produce only the desired product with minimal (or none) of byproducts."@en ;
    skos:inScheme cs: ;
    skos:prefLabel "selectivity"@en .

<https://w3id.org/nfdi4cat/voc4cat_0000126> a skos:Concept ;
    dcterms:identifier "voc4cat_0000126"^^xsd:token ;
    dcterms:provenance "Self"@en ;
    skos:altLabel "AQY"@en,
        "AQY%"@en,
        "apparent photonic yield"@en ;
    skos:broader <https://w3id.org/nfdi4cat/voc4cat_0000124> ;
    skos:definition "A measure of the efficiency of a photocatalytic reaction. It is expressed as the number of consumed charge carriers divided by the number of incident photons."@en ;
    skos:inScheme cs: ;
    skos:prefLabel "apparent quantum yield"@en .

<https://w3id.org/nfdi4cat/voc4cat_0000127> a skos:Concept ;
    dcterms:identifier "voc4cat_0000127"^^xsd:token ;
    dcterms:provenance "Self"@en ;
    skos:broader <https://w3id.org/nfdi4cat/voc4cat_0000124> ;
    skos:definition "The concentration (usually in ppm or mol) of the products formed during a photocatalytic reaction."@en ;
    skos:inScheme cs: ;
    skos:prefLabel "product concentration"@en .

<https://w3id.org/nfdi4cat/voc4cat_0000132> a skos:Concept ;
    dcterms:identifier "voc4cat_0000132"^^xsd:token ;
    dcterms:provenance "Self"@en ;
    skos:altLabel "FID"@en ;
    skos:broader <https://w3id.org/nfdi4cat/voc4cat_0000131> ;
    skos:definition "A type of gas chromatography detector that detects and quantifies the concentration of organic compounds in a gas sample emerging from a column, by measuring the electrical current generated by ionized gas constituents in a hydrogen flame."@en ;
    skos:inScheme cs: ;
    skos:prefLabel "flame ionization detector"@en .

<https://w3id.org/nfdi4cat/voc4cat_0000133> a skos:Concept ;
    dcterms:identifier "voc4cat_0000133"^^xsd:token ;
    dcterms:provenance "Self"@en ;
    skos:altLabel "TCD"@en ;
    skos:broader <https://w3id.org/nfdi4cat/voc4cat_0000131> ;
    skos:definition "A type of gas chromatography detector that measures the thermal conductivity of a gas sample and identifies its constituent molecules through changes in a filament’s temperature."@en ;
    skos:inScheme cs: ;
    skos:prefLabel "thermal conductivity detector"@en .

<https://w3id.org/nfdi4cat/voc4cat_0000134> a skos:Concept ;
    dcterms:identifier "voc4cat_0000134"^^xsd:token ;
    dcterms:provenance "Self"@en ;
    skos:altLabel "BID"@en ;
    skos:broader <https://w3id.org/nfdi4cat/voc4cat_0000131> ;
    skos:definition "Detector incorporating Ionization via a new dielectric barrier discharge He plasma."@en ;
    skos:inScheme cs: ;
    skos:prefLabel "dielectric-barrier discharge ionization detector"@en .

<https://w3id.org/nfdi4cat/voc4cat_0000135> a skos:Concept ;
    dcterms:identifier "voc4cat_0000135"^^xsd:token ;
    dcterms:provenance "Self"@en ;
    skos:broader <https://w3id.org/nfdi4cat/voc4cat_0000130> ;
    skos:definition "The minimum concentration of a product or intermediate that the gas chromatograph can identify. "@en ;
    skos:inScheme cs: ;
    skos:prefLabel "gas chromatograph sensitivity"@en .

<https://w3id.org/nfdi4cat/voc4cat_0000136> a skos:Concept ;
    dcterms:identifier "voc4cat_0000136"^^xsd:token ;
    dcterms:provenance "Self"@en ;
    skos:broader <https://w3id.org/nfdi4cat/voc4cat_0000130> ;
    skos:definition "A process in which gaseous substances of known purity and concentration are introduced to the gas chromatograph and the respective area and retention time of the resulting peaks are identified. This process when concluded, allows for the calculation of concentrations of products and intermediates of the photoreaction."@en ;
    skos:inScheme cs: ;
    skos:prefLabel "gas chromatograph calibration"@en .

<https://w3id.org/nfdi4cat/voc4cat_0000138> a skos:Concept ;
    dcterms:identifier "voc4cat_0000138"^^xsd:token ;
    dcterms:provenance "Self"@en ;
    skos:broader <https://w3id.org/nfdi4cat/voc4cat_0000137> ;
    skos:definition "Detectors of the mass spectrometer used to identify the reaction products and intemediates."@en ;
    skos:inScheme cs: ;
    skos:prefLabel "mass spectrometer detector"@en .

<https://w3id.org/nfdi4cat/voc4cat_0000139> a skos:Concept ;
    dcterms:identifier "voc4cat_0000139"^^xsd:token ;
    dcterms:provenance "Self"@en ;
    skos:broader <https://w3id.org/nfdi4cat/voc4cat_0000137> ;
    skos:definition "The minimum concentration of a product or intermediate that the mass spectrometer can identify. "@en ;
    skos:inScheme cs: ;
    skos:prefLabel "mass spectrometer sensitivity"@en .

<https://w3id.org/nfdi4cat/voc4cat_0000140> a skos:Concept ;
    dcterms:identifier "voc4cat_0000140"^^xsd:token ;
    dcterms:provenance "Self"@en ;
    skos:broader <https://w3id.org/nfdi4cat/voc4cat_0000137> ;
    skos:definition "A process in which gaseous substances of known purity and concentration are introduced to the mass spectrometer and the respective mass-to-charge ratios are identified. This process when concluded, allows for the calculation of concentrations of products and intermediates of the photoreaction."@en ;
    skos:inScheme cs: ;
    skos:prefLabel "mass spectrometer calibration"@en .

<https://w3id.org/nfdi4cat/voc4cat_0000144> a skos:Concept ;
    dcterms:identifier "voc4cat_0000144"^^xsd:token ;
    dcterms:provenance "Self"@en ;
    skos:broader <https://w3id.org/nfdi4cat/voc4cat_0000143> ;
    skos:definition "Maximum of operation pressure range within the reactor can operate safely. "@en ;
    skos:inScheme cs: ;
    skos:prefLabel "maximum operation pressure"@en .

<https://w3id.org/nfdi4cat/voc4cat_0000145> a skos:Concept ;
    dcterms:identifier "voc4cat_0000145"^^xsd:token ;
    dcterms:provenance "Self"@en ;
    skos:broader <https://w3id.org/nfdi4cat/voc4cat_0000143> ;
    skos:definition "Minimum of operation pressure range within the reactor can operate safely. "@en ;
    skos:inScheme cs: ;
    skos:prefLabel "minimum operation pressure"@en .

<https://w3id.org/nfdi4cat/voc4cat_0000147> a skos:Concept ;
    dcterms:identifier "voc4cat_0000147"^^xsd:token ;
    dcterms:provenance "Self"@en ;
    skos:broader <https://w3id.org/nfdi4cat/voc4cat_0000146> ;
    skos:definition "Α mechanical device that removes gas molecules from a sealed chamber reaching pressures lower than the atmospheric pressure. "@en ;
    skos:inScheme cs: ;
    skos:prefLabel "vacuum pump"@en .

<https://w3id.org/nfdi4cat/voc4cat_0000149> a skos:Concept ;
    dcterms:identifier "voc4cat_0000149"^^xsd:token ;
    dcterms:provenance "Self"@en ;
    skos:broader <https://w3id.org/nfdi4cat/voc4cat_0000148> ;
    skos:definition "Maximum of operation temperature range within the reactor can operate safely."@en ;
    skos:inScheme cs: ;
    skos:prefLabel "maximum operation temperature"@en .

<https://w3id.org/nfdi4cat/voc4cat_0000150> a skos:Concept ;
    dcterms:identifier "voc4cat_0000150"^^xsd:token ;
    dcterms:provenance "Self"@en ;
    skos:broader <https://w3id.org/nfdi4cat/voc4cat_0000148> ;
    skos:definition "Minimum of operation temperature range within the reactor can operate safely."@en ;
    skos:inScheme cs: ;
    skos:prefLabel "minimum operation temperature"@en .

<https://w3id.org/nfdi4cat/voc4cat_0000151> a skos:Concept ;
    dcterms:identifier "voc4cat_0000151"^^xsd:token ;
    dcterms:provenance "Self"@en ;
    skos:altLabel "temperature controller; temperature gauge; temperature monitor; heating device; cooling device"@en ;
    skos:broader <https://w3id.org/nfdi4cat/voc4cat_0000148> ;
    skos:definition "Equipment used for controlling and/or monitoring the temperature in various parts of a photoreactor. This can include hot plates, heating elements and cryostats. Light sources in operation can also affect the temperature in the reaction chamber."@en ;
    skos:inScheme cs: ;
    skos:prefLabel "temperature controller and monitor"@en .

<https://w3id.org/nfdi4cat/voc4cat_0000153> a skos:Concept ;
    dcterms:identifier "voc4cat_0000153"^^xsd:token ;
    dcterms:provenance "Self"@en ;
    skos:broader <https://w3id.org/nfdi4cat/voc4cat_0000152> ;
    skos:definition "Volume of the reaction chamber, calculated by its dimensions. Volume of pipes and valves connected to the reaction chamber should also be calculated and added to the total volume. "@en ;
    skos:inScheme cs: ;
    skos:prefLabel "reaction chamber volume"@en .

<https://w3id.org/nfdi4cat/voc4cat_0000154> a skos:Concept ;
    dcterms:identifier "voc4cat_0000154"^^xsd:token ;
    dcterms:provenance "Self"@en ;
    skos:broader <https://w3id.org/nfdi4cat/voc4cat_0000152> ;
    skos:definition "Height, width and depth (in cubic- or rectangular- shaped reaction chambers) or diameter and height (in cylindrer - shaped reaction chambers)"@en ;
    skos:inScheme cs: ;
    skos:prefLabel "reaction chamber dimension"@en .

<https://w3id.org/nfdi4cat/voc4cat_0000155> a skos:Concept ;
    dcterms:identifier "voc4cat_0000155"^^xsd:token ;
    dcterms:provenance "Self"@en ;
    skos:broader <https://w3id.org/nfdi4cat/voc4cat_0000152> ;
    skos:definition "The shape of the reaction chamber. In gas-phase reactions, reaction chambers have usually a cylindrical, cubical or rectangular shape."@en ;
    skos:inScheme cs: ;
    skos:prefLabel "reaction chamber shape"@en .

<https://w3id.org/nfdi4cat/voc4cat_0000156> a skos:Concept ;
    dcterms:identifier "voc4cat_0000156"^^xsd:token ;
    dcterms:provenance "Self"@en ;
    skos:broader <https://w3id.org/nfdi4cat/voc4cat_0000152> ;
    skos:definition "Material used for the construction of the main body of the reaction chamber."@en ;
    skos:inScheme cs: ;
    skos:prefLabel "reaction chamber material"@en .

<https://w3id.org/nfdi4cat/voc4cat_0000158> a skos:Concept ;
    dcterms:identifier "voc4cat_0000158"^^xsd:token ;
    dcterms:provenance "Self"@en ;
    skos:broader <https://w3id.org/nfdi4cat/voc4cat_0000157> ;
    skos:definition "Material that the window is made of. The window, usually attached to the lid sealing the reaction chamber, allows for the incoming light to enter the reaction chamber and interact with the photocatalyst. The material of the window influences the wavelenth range the the photocatalyst experieneces. "@en ;
    skos:inScheme cs: ;
    skos:prefLabel "optical window material"@en .

<https://w3id.org/nfdi4cat/voc4cat_0000160> a skos:Concept ;
    dcterms:identifier "voc4cat_0000160"^^xsd:token ;
    dcterms:provenance "Self"@en ;
    skos:broader <https://w3id.org/nfdi4cat/voc4cat_0000159> ;
    skos:definition "Diameter of the optical window allowing the incoming light to enter the reaction chamber and interact with the photocatalyst."@en ;
    skos:inScheme cs: ;
    skos:prefLabel "optical window diameter"@en .

<https://w3id.org/nfdi4cat/voc4cat_0000161> a skos:Concept ;
    dcterms:identifier "voc4cat_0000161"^^xsd:token ;
    dcterms:provenance "Self"@en ;
    skos:broader <https://w3id.org/nfdi4cat/voc4cat_0000159> ;
    skos:definition "Thickness of the optical window allowing the incoming light to enter the reaction chamber and interact with the photocatalyst."@en ;
    skos:inScheme cs: ;
    skos:prefLabel "optical window thickness"@en .

<https://w3id.org/nfdi4cat/voc4cat_0000164> a skos:Concept ;
    dcterms:identifier "voc4cat_0000164"^^xsd:token ;
    dcterms:provenance "Self"@en ;
    skos:altLabel "MFC"@en,
        "MFCs"@en ;
    skos:broader <https://w3id.org/nfdi4cat/voc4cat_0000163> ;
    skos:definition "Devices used to control and monitor gas or liquid flow rates."@en ;
    skos:inScheme cs: ;
    skos:prefLabel "mass flow controller"@en .

<https://w3id.org/nfdi4cat/voc4cat_0000167> a skos:Concept ;
    dcterms:identifier "voc4cat_0000167"^^xsd:token ;
    dcterms:provenance "Self"@en ;
    skos:altLabel "Hg-Xe lamp"@en,
        "Hg/Xe lamp"@en,
        "mercury xenon lamp"@en ;
    skos:broader <https://w3id.org/nfdi4cat/voc4cat_0000166> ;
    skos:definition "A lamp containg a mixture of mercury (Hg) and xenon (Xe) gases. Under electric current, the gas mixture gets ionized through a discharge electric charge creating a plasma generating UV and visible light. "@en ;
    skos:inScheme cs: ;
    skos:prefLabel "mercury-xenon lamp"@en .

<https://w3id.org/nfdi4cat/voc4cat_0000168> a skos:Concept ;
    dcterms:identifier "voc4cat_0000168"^^xsd:token ;
    dcterms:provenance "Self"@en ;
    skos:altLabel "Xe lamp"@en,
        "Xe-lamp"@en ;
    skos:broader <https://w3id.org/nfdi4cat/voc4cat_0000166> ;
    skos:definition "A lamp containg pure xenon (Xe) gas. Under electric current, the gas mixture gets ionized through a discharge electric charge creating a plasma generating UV and visible light. "@en ;
    skos:inScheme cs: ;
    skos:prefLabel "xenon lamp"@en .

<https://w3id.org/nfdi4cat/voc4cat_0000169> a skos:Concept ;
    dcterms:identifier "voc4cat_0000169"^^xsd:token ;
    dcterms:provenance "Self"@en ;
    skos:altLabel "LED"@en,
        "light-emitting diode"@en ;
    skos:broader <https://w3id.org/nfdi4cat/voc4cat_0000166> ;
    skos:definition "A solid-state semiconductor emitting light at highly controllable (narrow) wavelength ranges."@en ;
    skos:inScheme cs: ;
    skos:prefLabel "light emitting diode"@en .

<https://w3id.org/nfdi4cat/voc4cat_0000171> a skos:Concept ;
    dcterms:identifier "voc4cat_0000171"^^xsd:token ;
    dcterms:provenance "Self"@en ;
    skos:broader <https://w3id.org/nfdi4cat/voc4cat_0000170> ;
    skos:definition "The distance of the light source from the reaction chamber and the photocatalyst."@en ;
    skos:inScheme cs: ;
    skos:prefLabel "light source distance"@en .

<https://w3id.org/nfdi4cat/voc4cat_0000172> a skos:Concept ;
    dcterms:identifier "voc4cat_0000172"^^xsd:token ;
    dcterms:provenance "Self"@en ;
    skos:broader <https://w3id.org/nfdi4cat/voc4cat_0000170> ;
    skos:definition "The value of current (usually in A or mA) used to operate the selected light source."@en ;
    skos:inScheme cs: ;
    skos:prefLabel "light operation current"@en .

<https://w3id.org/nfdi4cat/voc4cat_0000173> a skos:Concept ;
    dcterms:identifier "voc4cat_0000173"^^xsd:token ;
    dcterms:provenance "Self"@en ;
    skos:broader <https://w3id.org/nfdi4cat/voc4cat_0000170> ;
    skos:definition "The value of voltage  (usually in V or mV) used to operate the selected light source."@en ;
    skos:inScheme cs: ;
    skos:prefLabel "light operation voltage"@en .

<https://w3id.org/nfdi4cat/voc4cat_0000174> a skos:Concept ;
    dcterms:identifier "voc4cat_0000174"^^xsd:token ;
    dcterms:provenance "Self"@en ;
    skos:broader <https://w3id.org/nfdi4cat/voc4cat_0000170> ;
    skos:definition "The power of the light source (usually in W or mW). The power can be calculated by the multiplication of the current and voltage used to operate the light source,"@en ;
    skos:inScheme cs: ;
    skos:prefLabel "light power output"@en .

<https://w3id.org/nfdi4cat/voc4cat_0000175> a skos:Concept ;
    dcterms:identifier "voc4cat_0000175"^^xsd:token ;
    dcterms:provenance "Self"@en ;
    skos:broader <https://w3id.org/nfdi4cat/voc4cat_0000170> ;
    skos:definition "The light intensity (usually in mW cm-2) of the selected light source. The light intensity should be measured at the same distance as the one between the light source and the reaction chamber / sample."@en ;
    skos:inScheme cs: ;
    skos:prefLabel "light intensity"@en .

<https://w3id.org/nfdi4cat/voc4cat_0000177> a skos:Concept ;
    dcterms:identifier "voc4cat_0000177"^^xsd:token ;
    dcterms:provenance "Self"@en ;
    skos:altLabel "IR; Ir"@en ;
    skos:broader <https://w3id.org/nfdi4cat/voc4cat_0000176> ;
    skos:definition "Electromagnetic radiation with wavelengths typically in the range of 800 nm - 20000 nm."@en ;
    skos:inScheme cs: ;
    skos:prefLabel "infrared"@en .

<https://w3id.org/nfdi4cat/voc4cat_0000178> a skos:Concept ;
    dcterms:identifier "voc4cat_0000178"^^xsd:token ;
    dcterms:provenance "Self"@en ;
    skos:altLabel "Vis; VIS"@en ;
    skos:broader <https://w3id.org/nfdi4cat/voc4cat_0000176> ;
    skos:definition "Electromagnetic radiation with wavelengths visible to the human eye, typically in the range of 400-800 nm. "@en ;
    skos:inScheme cs: ;
    skos:prefLabel "visible"@en .

<https://w3id.org/nfdi4cat/voc4cat_0000179> a skos:Concept ;
    dcterms:identifier "voc4cat_0000179"^^xsd:token ;
    dcterms:provenance "Self"@en ;
    skos:altLabel "UV"@en,
        "UV-A"@en,
        "UV-B"@en,
        "UV-C"@en,
        "VUV"@en ;
    skos:broader <https://w3id.org/nfdi4cat/voc4cat_0000176> ;
    skos:definition "Electromagnetic radiation with a wavelength typically in the range of 100-400 nanometers."@en ;
    skos:inScheme cs: ;
    skos:prefLabel "ultraviolet"@en .

<https://w3id.org/nfdi4cat/voc4cat_0001900> a skos:Collection ;
    dcterms:identifier "voc4cat_0001900"^^xsd:token ;
    dcterms:isPartOf cs: ;
    dcterms:provenance "Self"@en ;
    skos:definition "A collection of concepts referring to material  characterization techniques and methods to evaluate their efficiency in photocatalysis."@en ;
    skos:member <https://w3id.org/nfdi4cat/voc4cat_0000067>,
        <https://w3id.org/nfdi4cat/voc4cat_0000068>,
        <https://w3id.org/nfdi4cat/voc4cat_0000069>,
        <https://w3id.org/nfdi4cat/voc4cat_0000070>,
        <https://w3id.org/nfdi4cat/voc4cat_0000071>,
        <https://w3id.org/nfdi4cat/voc4cat_0000072>,
        <https://w3id.org/nfdi4cat/voc4cat_0000073>,
        <https://w3id.org/nfdi4cat/voc4cat_0000074>,
        <https://w3id.org/nfdi4cat/voc4cat_0000075>,
        <https://w3id.org/nfdi4cat/voc4cat_0000076>,
        <https://w3id.org/nfdi4cat/voc4cat_0000077>,
        <https://w3id.org/nfdi4cat/voc4cat_0000078>,
        <https://w3id.org/nfdi4cat/voc4cat_0000079>,
        <https://w3id.org/nfdi4cat/voc4cat_0000080>,
        <https://w3id.org/nfdi4cat/voc4cat_0000081>,
        <https://w3id.org/nfdi4cat/voc4cat_0000082>,
        <https://w3id.org/nfdi4cat/voc4cat_0000083>,
        <https://w3id.org/nfdi4cat/voc4cat_0000130>,
        <https://w3id.org/nfdi4cat/voc4cat_0000137>,
        <https://w3id.org/nfdi4cat/voc4cat_0000141> ;
    skos:prefLabel "Characterization and evaluation techniques"@en .

<https://w3id.org/nfdi4cat/voc4cat_0001901> a skos:Collection ;
    dcterms:identifier "voc4cat_0001901"^^xsd:token ;
    dcterms:isPartOf cs: ;
    dcterms:provenance "Self"@en ;
    skos:definition "A collection of concepts referring to photocatalysis."@en ;
    skos:member <https://w3id.org/nfdi4cat/voc4cat_00000001>,
        <https://w3id.org/nfdi4cat/voc4cat_00000002>,
        <https://w3id.org/nfdi4cat/voc4cat_00000003>,
        <https://w3id.org/nfdi4cat/voc4cat_00000004>,
        <https://w3id.org/nfdi4cat/voc4cat_00000005>,
        <https://w3id.org/nfdi4cat/voc4cat_00000006>,
        <https://w3id.org/nfdi4cat/voc4cat_00000007>,
        <https://w3id.org/nfdi4cat/voc4cat_00000008>,
        <https://w3id.org/nfdi4cat/voc4cat_00000009>,
        <https://w3id.org/nfdi4cat/voc4cat_00000010>,
        <https://w3id.org/nfdi4cat/voc4cat_00000011>,
        <https://w3id.org/nfdi4cat/voc4cat_00000012>,
        <https://w3id.org/nfdi4cat/voc4cat_00000013>,
        <https://w3id.org/nfdi4cat/voc4cat_00000014>,
        <https://w3id.org/nfdi4cat/voc4cat_00000015>,
        <https://w3id.org/nfdi4cat/voc4cat_00000016>,
        <https://w3id.org/nfdi4cat/voc4cat_00000017>,
        <https://w3id.org/nfdi4cat/voc4cat_00000018>,
        <https://w3id.org/nfdi4cat/voc4cat_00000019>,
        <https://w3id.org/nfdi4cat/voc4cat_00000020>,
        <https://w3id.org/nfdi4cat/voc4cat_00000021>,
        <https://w3id.org/nfdi4cat/voc4cat_00000022>,
        <https://w3id.org/nfdi4cat/voc4cat_00000023>,
        <https://w3id.org/nfdi4cat/voc4cat_00000024>,
        <https://w3id.org/nfdi4cat/voc4cat_00000025>,
        <https://w3id.org/nfdi4cat/voc4cat_00000026>,
        <https://w3id.org/nfdi4cat/voc4cat_00000027>,
        <https://w3id.org/nfdi4cat/voc4cat_00000028>,
        <https://w3id.org/nfdi4cat/voc4cat_00000029>,
        <https://w3id.org/nfdi4cat/voc4cat_00000030>,
        <https://w3id.org/nfdi4cat/voc4cat_00000031>,
        <https://w3id.org/nfdi4cat/voc4cat_00000032>,
        <https://w3id.org/nfdi4cat/voc4cat_00000033>,
        <https://w3id.org/nfdi4cat/voc4cat_00000034>,
        <https://w3id.org/nfdi4cat/voc4cat_00000035>,
        <https://w3id.org/nfdi4cat/voc4cat_00000036>,
        <https://w3id.org/nfdi4cat/voc4cat_00000037>,
        <https://w3id.org/nfdi4cat/voc4cat_00000038>,
        <https://w3id.org/nfdi4cat/voc4cat_00000039>,
        <https://w3id.org/nfdi4cat/voc4cat_00000040>,
        <https://w3id.org/nfdi4cat/voc4cat_00000041>,
        <https://w3id.org/nfdi4cat/voc4cat_00000042>,
        <https://w3id.org/nfdi4cat/voc4cat_00000043>,
        <https://w3id.org/nfdi4cat/voc4cat_00000044>,
        <https://w3id.org/nfdi4cat/voc4cat_00000045>,
        <https://w3id.org/nfdi4cat/voc4cat_00000046>,
        <https://w3id.org/nfdi4cat/voc4cat_00000047>,
        <https://w3id.org/nfdi4cat/voc4cat_00000048>,
        <https://w3id.org/nfdi4cat/voc4cat_00000049>,
        <https://w3id.org/nfdi4cat/voc4cat_00000050>,
        <https://w3id.org/nfdi4cat/voc4cat_00000051>,
        <https://w3id.org/nfdi4cat/voc4cat_00000052>,
        <https://w3id.org/nfdi4cat/voc4cat_00000053>,
        <https://w3id.org/nfdi4cat/voc4cat_00000054>,
        <https://w3id.org/nfdi4cat/voc4cat_00000055>,
        <https://w3id.org/nfdi4cat/voc4cat_00000056>,
        <https://w3id.org/nfdi4cat/voc4cat_00000057>,
        <https://w3id.org/nfdi4cat/voc4cat_00000058>,
        <https://w3id.org/nfdi4cat/voc4cat_00000059>,
        <https://w3id.org/nfdi4cat/voc4cat_00000060>,
        <https://w3id.org/nfdi4cat/voc4cat_00000061>,
        <https://w3id.org/nfdi4cat/voc4cat_00000062>,
        <https://w3id.org/nfdi4cat/voc4cat_00000063>,
        <https://w3id.org/nfdi4cat/voc4cat_00000064>,
        <https://w3id.org/nfdi4cat/voc4cat_00000065>,
        <https://w3id.org/nfdi4cat/voc4cat_00000066>,
        <https://w3id.org/nfdi4cat/voc4cat_00000067>,
        <https://w3id.org/nfdi4cat/voc4cat_00000068>,
        <https://w3id.org/nfdi4cat/voc4cat_00000069>,
        <https://w3id.org/nfdi4cat/voc4cat_00000070>,
        <https://w3id.org/nfdi4cat/voc4cat_00000071>,
        <https://w3id.org/nfdi4cat/voc4cat_00000072>,
        <https://w3id.org/nfdi4cat/voc4cat_00000073>,
        <https://w3id.org/nfdi4cat/voc4cat_00000074>,
        <https://w3id.org/nfdi4cat/voc4cat_00000075>,
        <https://w3id.org/nfdi4cat/voc4cat_00000076>,
        <https://w3id.org/nfdi4cat/voc4cat_00000077>,
        <https://w3id.org/nfdi4cat/voc4cat_00000078>,
        <https://w3id.org/nfdi4cat/voc4cat_00000079>,
        <https://w3id.org/nfdi4cat/voc4cat_00000080>,
        <https://w3id.org/nfdi4cat/voc4cat_00000081>,
        <https://w3id.org/nfdi4cat/voc4cat_00000082>,
        <https://w3id.org/nfdi4cat/voc4cat_00000083>,
        <https://w3id.org/nfdi4cat/voc4cat_00000084>,
        <https://w3id.org/nfdi4cat/voc4cat_00000085>,
        <https://w3id.org/nfdi4cat/voc4cat_00000086>,
        <https://w3id.org/nfdi4cat/voc4cat_00000087>,
        <https://w3id.org/nfdi4cat/voc4cat_00000088>,
        <https://w3id.org/nfdi4cat/voc4cat_00000089>,
        <https://w3id.org/nfdi4cat/voc4cat_00000090>,
        <https://w3id.org/nfdi4cat/voc4cat_00000091>,
        <https://w3id.org/nfdi4cat/voc4cat_00000092>,
        <https://w3id.org/nfdi4cat/voc4cat_00000093>,
        <https://w3id.org/nfdi4cat/voc4cat_00000094>,
        <https://w3id.org/nfdi4cat/voc4cat_00000095>,
        <https://w3id.org/nfdi4cat/voc4cat_00000096>,
        <https://w3id.org/nfdi4cat/voc4cat_00000097>,
        <https://w3id.org/nfdi4cat/voc4cat_00000098>,
        <https://w3id.org/nfdi4cat/voc4cat_00000099>,
        <https://w3id.org/nfdi4cat/voc4cat_00000100>,
        <https://w3id.org/nfdi4cat/voc4cat_00000101>,
        <https://w3id.org/nfdi4cat/voc4cat_00000102>,
        <https://w3id.org/nfdi4cat/voc4cat_00000103>,
        <https://w3id.org/nfdi4cat/voc4cat_00000104>,
        <https://w3id.org/nfdi4cat/voc4cat_00000105>,
        <https://w3id.org/nfdi4cat/voc4cat_00000106>,
        <https://w3id.org/nfdi4cat/voc4cat_00000107>,
        <https://w3id.org/nfdi4cat/voc4cat_00000108>,
        <https://w3id.org/nfdi4cat/voc4cat_00000109>,
        <https://w3id.org/nfdi4cat/voc4cat_00000110>,
        <https://w3id.org/nfdi4cat/voc4cat_00000111>,
        <https://w3id.org/nfdi4cat/voc4cat_00000112>,
        <https://w3id.org/nfdi4cat/voc4cat_00000113>,
        <https://w3id.org/nfdi4cat/voc4cat_00000114>,
        <https://w3id.org/nfdi4cat/voc4cat_00000115>,
        <https://w3id.org/nfdi4cat/voc4cat_00000116>,
        <https://w3id.org/nfdi4cat/voc4cat_00000117>,
        <https://w3id.org/nfdi4cat/voc4cat_00000118>,
        <https://w3id.org/nfdi4cat/voc4cat_00000119>,
        <https://w3id.org/nfdi4cat/voc4cat_00000120>,
        <https://w3id.org/nfdi4cat/voc4cat_00000121>,
        <https://w3id.org/nfdi4cat/voc4cat_00000122>,
        <https://w3id.org/nfdi4cat/voc4cat_00000123>,
        <https://w3id.org/nfdi4cat/voc4cat_00000124>,
        <https://w3id.org/nfdi4cat/voc4cat_00000125>,
        <https://w3id.org/nfdi4cat/voc4cat_00000126>,
        <https://w3id.org/nfdi4cat/voc4cat_00000127>,
        <https://w3id.org/nfdi4cat/voc4cat_00000128>,
        <https://w3id.org/nfdi4cat/voc4cat_00000129>,
        <https://w3id.org/nfdi4cat/voc4cat_00000130>,
        <https://w3id.org/nfdi4cat/voc4cat_00000131>,
        <https://w3id.org/nfdi4cat/voc4cat_00000132>,
        <https://w3id.org/nfdi4cat/voc4cat_00000133>,
        <https://w3id.org/nfdi4cat/voc4cat_00000134>,
        <https://w3id.org/nfdi4cat/voc4cat_00000135>,
        <https://w3id.org/nfdi4cat/voc4cat_00000136>,
        <https://w3id.org/nfdi4cat/voc4cat_00000137>,
        <https://w3id.org/nfdi4cat/voc4cat_00000138>,
        <https://w3id.org/nfdi4cat/voc4cat_00000139>,
        <https://w3id.org/nfdi4cat/voc4cat_00000140>,
        <https://w3id.org/nfdi4cat/voc4cat_00000141>,
        <https://w3id.org/nfdi4cat/voc4cat_00000142>,
        <https://w3id.org/nfdi4cat/voc4cat_00000143>,
        <https://w3id.org/nfdi4cat/voc4cat_00000144>,
        <https://w3id.org/nfdi4cat/voc4cat_00000145>,
        <https://w3id.org/nfdi4cat/voc4cat_00000146>,
        <https://w3id.org/nfdi4cat/voc4cat_00000147>,
        <https://w3id.org/nfdi4cat/voc4cat_00000148>,
        <https://w3id.org/nfdi4cat/voc4cat_00000149>,
        <https://w3id.org/nfdi4cat/voc4cat_00000150>,
        <https://w3id.org/nfdi4cat/voc4cat_00000151>,
        <https://w3id.org/nfdi4cat/voc4cat_00000152>,
        <https://w3id.org/nfdi4cat/voc4cat_00000153>,
        <https://w3id.org/nfdi4cat/voc4cat_00000154>,
        <https://w3id.org/nfdi4cat/voc4cat_00000155>,
        <https://w3id.org/nfdi4cat/voc4cat_00000156>,
        <https://w3id.org/nfdi4cat/voc4cat_00000157>,
        <https://w3id.org/nfdi4cat/voc4cat_00000158>,
        <https://w3id.org/nfdi4cat/voc4cat_00000159>,
        <https://w3id.org/nfdi4cat/voc4cat_00000160>,
        <https://w3id.org/nfdi4cat/voc4cat_00000161>,
        <https://w3id.org/nfdi4cat/voc4cat_00000162>,
        <https://w3id.org/nfdi4cat/voc4cat_00000163>,
        <https://w3id.org/nfdi4cat/voc4cat_00000164>,
        <https://w3id.org/nfdi4cat/voc4cat_00000165>,
        <https://w3id.org/nfdi4cat/voc4cat_00000166>,
        <https://w3id.org/nfdi4cat/voc4cat_00000167>,
        <https://w3id.org/nfdi4cat/voc4cat_00000168>,
        <https://w3id.org/nfdi4cat/voc4cat_00000169>,
        <https://w3id.org/nfdi4cat/voc4cat_00000170>,
        <https://w3id.org/nfdi4cat/voc4cat_00000171>,
        <https://w3id.org/nfdi4cat/voc4cat_00000172>,
        <https://w3id.org/nfdi4cat/voc4cat_00000173>,
        <https://w3id.org/nfdi4cat/voc4cat_00000174>,
        <https://w3id.org/nfdi4cat/voc4cat_00000175>,
        <https://w3id.org/nfdi4cat/voc4cat_00000176>,
        <https://w3id.org/nfdi4cat/voc4cat_00000177>,
        <https://w3id.org/nfdi4cat/voc4cat_00000178>,
        <https://w3id.org/nfdi4cat/voc4cat_00000179> ;
    skos:prefLabel "Photocatalysis collection"@en .

<https://w3id.org/nfdi4cat/voc4cat_0000004> a skos:Concept ;
    dcterms:identifier "voc4cat_0000004"^^xsd:token ;
    dcterms:provenance "self"@en ;
    skos:broader <https://w3id.org/nfdi4cat/voc4cat_0000003> ;
    skos:definition "Broad families of semiconduction materials (e.g., metal oxides) that can be used as photocatalysts in various applications."@en ;
    skos:inScheme cs: ;
    skos:narrower <https://w3id.org/nfdi4cat/voc4cat_0000005> ;
    skos:prefLabel "categories of semiconductors"@en .

<https://w3id.org/nfdi4cat/voc4cat_0000014> a skos:Concept ;
    dcterms:identifier "voc4cat_0000014"^^xsd:token ;
    dcterms:provenance "Self"@en ;
    skos:broader <https://w3id.org/nfdi4cat/voc4cat_0000003> ;
    skos:definition "Tecniques used to modify the properties of a photocatalyst, with the aim to increase its efficiency in a photocatalytic application. "@en ;
    skos:inScheme cs: ;
    skos:narrower <https://w3id.org/nfdi4cat/voc4cat_0000015> ;
    skos:prefLabel "modification technique"@en .

<https://w3id.org/nfdi4cat/voc4cat_0000017> a skos:Concept ;
    dcterms:identifier "voc4cat_0000017"^^xsd:token ;
    dcterms:provenance "Self"@en ;
    skos:broader <https://w3id.org/nfdi4cat/voc4cat_0000016> ;
    skos:definition "A photocatalyst introduced to the reaction chamber in the form of a powder. Usually the powdered photocatalyst is spread inside a quartz / glass plate."@en ;
    skos:inScheme cs: ;
    skos:narrower <https://w3id.org/nfdi4cat/voc4cat_0000018> ;
    skos:prefLabel "powdered photocatalyst"@en .

<https://w3id.org/nfdi4cat/voc4cat_0000067> a skos:Concept ;
    dcterms:identifier "voc4cat_0000067"^^xsd:token ;
    dcterms:provenance "Self"@en ;
    skos:altLabel "X-ray emission spectrometry"@en,
        "X-ray fluorescence spectrometry; X-ray fluorescence spectroscopy"@en,
        "XES"@en,
        "XRES"@en,
        "XRF"@en,
        "XRF spectrometry"@en,
        "XRF spectroscopy"@en ;
    skos:broader <https://w3id.org/nfdi4cat/voc4cat_0000066> ;
    skos:definition "A non-destructive analytical technique which uses a high-energy X-ray source to expose a material and monitors the emitted characteristic fluorescent X-Rays.  "@en ;
    skos:inScheme cs: ;
    skos:prefLabel "X-ray fluorescence"@en .

<https://w3id.org/nfdi4cat/voc4cat_0000068> a skos:Concept ;
    dcterms:identifier "voc4cat_0000068"^^xsd:token ;
    dcterms:provenance "Self"@en ;
    skos:altLabel "EELS"@en ;
    skos:broader <https://w3id.org/nfdi4cat/voc4cat_0000066> ;
    skos:definition "An analytical technique used to measure the energy loss of electrons passing through a sample. "@en ;
    skos:inScheme cs: ;
    skos:prefLabel "electron energy loss spectroscopy"@en .

<https://w3id.org/nfdi4cat/voc4cat_0000069> a skos:Concept ;
    dcterms:identifier "voc4cat_0000069"^^xsd:token ;
    dcterms:provenance "Self"@en ;
    skos:altLabel "RAMAN"@en,
        "Raman"@en,
        "Raman scattering spectrometry"@en,
        "Raman spectrometry"@en,
        "raman scattering spectroscopy"@en ;
    skos:broader <https://w3id.org/nfdi4cat/voc4cat_0000066> ;
    skos:definition "A spectroscopy technique studying the vibrational modes of molecules, by measuring the intensity and frequency of scattered by the sample of monochromatic light. "@en ;
    skos:inScheme cs: ;
    skos:prefLabel "Raman spectroscopy"@en .

<https://w3id.org/nfdi4cat/voc4cat_0000070> a skos:Concept ;
    dcterms:identifier "voc4cat_0000070"^^xsd:token ;
    dcterms:provenance "Self"@en ;
    skos:altLabel "AFM"@en,
        "SFM"@en,
        "atomic force imaging"@en,
        "atomic-force microscopy"@en,
        "scanning force microscopy"@en ;
    skos:broader <https://w3id.org/nfdi4cat/voc4cat_0000066> ;
    skos:definition "A high-resolution imaging technique that measures the interaction between a sharp probe and the sample’s surface to create a three-dimensional image of the surface’s morphology.  "@en ;
    skos:inScheme cs: ;
    skos:prefLabel "atomic force microscopy"@en .

<https://w3id.org/nfdi4cat/voc4cat_0000071> a skos:Concept ;
    dcterms:identifier "voc4cat_0000071"^^xsd:token ;
    dcterms:provenance "Self"@en ;
    skos:altLabel "DSC"@en,
        "differential scanning calorimetric (DSC) analysis"@en,
        "differential scanning calorimetric analysis"@en ;
    skos:broader <https://w3id.org/nfdi4cat/voc4cat_0000066> ;
    skos:definition "A thermal analysis technique which compares the heat flow in a sample and a reference material under controlled applied temperature profiles. "@en ;
    skos:inScheme cs: ;
    skos:prefLabel "differential scanning calorimetry"@en .

<https://w3id.org/nfdi4cat/voc4cat_0000072> a skos:Concept ;
    dcterms:identifier "voc4cat_0000072"^^xsd:token ;
    dcterms:provenance "Self"@en ;
    skos:altLabel "TG"@en,
        "TG analysis"@en,
        "TG measurements"@en,
        "TGA"@en,
        "thermal gravimetric analysis"@en,
        "thermo-gravimetric analysis"@en,
        "thermogravimetric (TG) analyses"@en,
        "thermogravimetric (TG) analysis"@en ;
    skos:broader <https://w3id.org/nfdi4cat/voc4cat_0000066> ;
    skos:definition "A thermal analysis technique used to measure the change of a sample’s mass under the influence of controlled applied temperature profiles."@en ;
    skos:inScheme cs: ;
    skos:prefLabel "thermogravimetric analysis"@en .

<https://w3id.org/nfdi4cat/voc4cat_0000073> a skos:Concept ;
    dcterms:identifier "voc4cat_0000073"^^xsd:token ;
    dcterms:provenance "Self"@en ;
    skos:altLabel "NMR"@en ;
    skos:broader <https://w3id.org/nfdi4cat/voc4cat_0000066> ;
    skos:definition "A spectroscopic technique that uses a static magnetic field and radiofrequency radiation to measure the magnetic resonance of atomic nuclei protons or electrons."@en ;
    skos:inScheme cs: ;
    skos:prefLabel "nuclear magnetic resonance spectroscopy"@en .

<https://w3id.org/nfdi4cat/voc4cat_0000074> a skos:Concept ;
    dcterms:identifier "voc4cat_0000074"^^xsd:token ;
    dcterms:provenance "Self"@en ;
    skos:altLabel "PL"@en ;
    skos:broader <https://w3id.org/nfdi4cat/voc4cat_0000066> ;
    skos:definition "Light emission of lower energy photons from a sample upon its photoexcitation. "@en ;
    skos:inScheme cs: ;
    skos:prefLabel "photoluminescence"@en .

<https://w3id.org/nfdi4cat/voc4cat_0000075> a skos:Concept ;
    dcterms:identifier "voc4cat_0000075"^^xsd:token ;
    dcterms:provenance "Self"@en ;
    skos:altLabel "SEM"@en ;
    skos:broader <https://w3id.org/nfdi4cat/voc4cat_0000066> ;
    skos:definition "An electron microscopy technique that produces high-resolution images under high magnification of a sample's surface by assessing the secondary and back-scattered electrons produced by a focused electron beam."@en ;
    skos:inScheme cs: ;
    skos:prefLabel "scanning electron microscopy"@en .

<https://w3id.org/nfdi4cat/voc4cat_0000076> a skos:Concept ;
    dcterms:identifier "voc4cat_0000076"^^xsd:token ;
    dcterms:provenance "Self"@en ;
    skos:altLabel "XPS"@en ;
    skos:broader <https://w3id.org/nfdi4cat/voc4cat_0000066> ;
    skos:definition "A technique that analyzes the chemical composition of an X-ray irradiated sample by measuring the energies of the emitted electrons."@en ;
    skos:inScheme cs: ;
    skos:prefLabel "X-ray photoelectron spectroscopy"@en .

<https://w3id.org/nfdi4cat/voc4cat_0000077> a skos:Concept ;
    dcterms:identifier "voc4cat_0000077"^^xsd:token ;
    dcterms:provenance "Self"@en ;
    skos:altLabel "X-ray analysis"@en,
        "X-ray crystallographic analysis"@en,
        "X-ray crystallography"@en,
        "X-ray diffraction analysis"@en,
        "X-ray diffractometry"@en,
        "X-ray structure determination"@en,
        "XRD"@en ;
    skos:broader <https://w3id.org/nfdi4cat/voc4cat_0000066> ;
    skos:definition "A technique which analyses the diffraction pattern produced when X-rays are scattered by a sample bombarded by a focused electron beam."@en ;
    skos:inScheme cs: ;
    skos:prefLabel "X-ray diffraction"@en .

<https://w3id.org/nfdi4cat/voc4cat_0000078> a skos:Concept ;
    dcterms:identifier "voc4cat_0000078"^^xsd:token ;
    dcterms:provenance "Self"@en ;
    skos:altLabel "TEM"@en ;
    skos:broader <https://w3id.org/nfdi4cat/voc4cat_0000066> ;
    skos:definition "Transmission electron microscopy is a technique that produces high-resolution images if the internal structure of a sample by using a beam of electrons to bombard the thin sample and measuring the intensity of the scattered transmitted electrons."@en ;
    skos:inScheme cs: ;
    skos:prefLabel "transmission electron microscopy"@en .

<https://w3id.org/nfdi4cat/voc4cat_0000079> a skos:Concept ;
    dcterms:identifier "voc4cat_0000079"^^xsd:token ;
    dcterms:provenance "Self"@en ;
    skos:altLabel "UV-Vis"@en ;
    skos:broader <https://w3id.org/nfdi4cat/voc4cat_0000066> ;
    skos:definition "A technique used to measure the absorption, transmission or reflectance of light by a sample in the ultraviolet and visible regions of the electromagnetic spectrum."@en ;
    skos:inScheme cs: ;
    skos:prefLabel "ultraviolet-visible spectroscopy"@en .

<https://w3id.org/nfdi4cat/voc4cat_0000080> a skos:Concept ;
    dcterms:identifier "voc4cat_0000080"^^xsd:token ;
    dcterms:provenance "Self"@en ;
    skos:altLabel "FT-IR"@en,
        "FT-IR spectroscopy"@en,
        "FTIR"@en,
        "FTIR spectrometry"@en,
        "FTIR spectroscopy"@en,
        "Fourier transform infra-red absoprtion spectroscopy"@en,
        "Fourier transform infra-red spectrometry"@en,
        "Fourier transform infrared (FT-IR)"@en,
        "Fourier transform infrared (FT-IR) spectroscopy"@en,
        "Fourier-transform infra-red absorption spectrometry"@en,
        "Fourier-transform infrared (FTIR) absorption spectroscopy"@en ;
    skos:broader <https://w3id.org/nfdi4cat/voc4cat_0000066> ;
    skos:definition "A spectroscopic technique used to study the vibrational modes of chemical bonds of a sample using infrared radiation."@en ;
    skos:inScheme cs: ;
    skos:prefLabel "fourier transform infrared spectroscopy"@en .

<https://w3id.org/nfdi4cat/voc4cat_0000081> a skos:Concept ;
    dcterms:identifier "voc4cat_0000081"^^xsd:token ;
    dcterms:provenance "Self"@en ;
    skos:altLabel "BET"@en ;
    skos:broader <https://w3id.org/nfdi4cat/voc4cat_0000066> ;
    skos:definition "The study of physical adsorption of gas molecules on a solid surface for the calculation of the specific surface area of materials."@en ;
    skos:inScheme cs: ;
    skos:prefLabel "Brunauer-Emmett-Teller surface area analysis"@en .

<https://w3id.org/nfdi4cat/voc4cat_0000082> a skos:Concept ;
    dcterms:identifier "voc4cat_0000082"^^xsd:token ;
    dcterms:provenance "Self"@en ;
    skos:altLabel "CV"@en,
        "cyclovoltammetry"@en ;
    skos:broader <https://w3id.org/nfdi4cat/voc4cat_0000066> ;
    skos:definition "An electrochemical technique used to study the redox properties of a sample by measuring the current produced by an applied voltage sweep."@en ;
    skos:inScheme cs: ;
    skos:prefLabel "cyclic voltammetry"@en .

<https://w3id.org/nfdi4cat/voc4cat_0000083> a skos:Concept ;
    dcterms:identifier "voc4cat_0000083"^^xsd:token ;
    dcterms:provenance "Self"@en ;
    skos:broader <https://w3id.org/nfdi4cat/voc4cat_0000066> ;
    skos:definition "A method used in cyclic voltammetry to determine the charge carrier concentration and the flat-band potential of an electrochemical system by measuring the capacitance as a function of applied voltage."@en ;
    skos:inScheme cs: ;
    skos:prefLabel "Mott-Schottky analysis"@en .

<https://w3id.org/nfdi4cat/voc4cat_0000098> a skos:Concept ;
    dcterms:identifier "voc4cat_0000098"^^xsd:token ;
    dcterms:provenance "Self"@en ;
    skos:broader <https://w3id.org/nfdi4cat/voc4cat_0000087> ;
    skos:definition "The gain of electrons or a decrease in the oxidation state of a species. "@en ;
    skos:inScheme cs: ;
    skos:narrower <https://w3id.org/nfdi4cat/voc4cat_0000099> ;
    skos:prefLabel "reduction"@en .

<https://w3id.org/nfdi4cat/voc4cat_0000141> a skos:Concept ;
    dcterms:identifier "voc4cat_0000141"^^xsd:token ;
    dcterms:provenance "Self"@en ;
    skos:altLabel "LC"@en ;
    skos:broader <https://w3id.org/nfdi4cat/voc4cat_0000129> ;
    skos:definition "A sepation technique that uses a liquid mobile phase to separate the components of a mixture based on their interactions with a stationary phase and a mobile phase. "@en ;
    skos:inScheme cs: ;
    skos:prefLabel "liquid chromatography"@en .

<https://w3id.org/nfdi4cat/voc4cat_0000146> a skos:Concept ;
    dcterms:identifier "voc4cat_0000146"^^xsd:token ;
    dcterms:provenance "Self"@en ;
    skos:altLabel "pressure controller; pressure gauge; pressure monitor"@en ;
    skos:broader <https://w3id.org/nfdi4cat/voc4cat_0000143> ;
    skos:definition "Equipment used for controlling and / or monitoring the pressure in various parts of a photoreactor. A vaccum pump is a typical example of such equipment."@en ;
    skos:inScheme cs: ;
    skos:narrower <https://w3id.org/nfdi4cat/voc4cat_0000147> ;
    skos:prefLabel "pressure controller and monitor"@en .

<https://w3id.org/nfdi4cat/voc4cat_0000162> a skos:Concept ;
    dcterms:identifier "voc4cat_0000162"^^xsd:token ;
    dcterms:provenance "Self"@en ;
    skos:altLabel "gas flow"@en ;
    skos:broader <https://w3id.org/nfdi4cat/voc4cat_0000128> ;
    skos:definition "Flow rates of gases used in an experiment. Gases can have either the role of a reactant (e.g., CO2) or be inert (e.g., Ar, He). "@en ;
    skos:inScheme cs: ;
    skos:narrower <https://w3id.org/nfdi4cat/voc4cat_0000163> ;
    skos:prefLabel "gas feed"@en .

<https://w3id.org/nfdi4cat/voc4cat_0000163> a skos:Concept ;
    dcterms:identifier "voc4cat_0000163"^^xsd:token ;
    dcterms:provenance "Self"@en ;
    skos:broader <https://w3id.org/nfdi4cat/voc4cat_0000162> ;
    skos:definition "Equipment used for controlling and / or monitoring the flow of gases (reactant or inert) needed for a photocatalytic experiment. Mass flow controllers (MFCs) are commonly used to controll gas flows."@en ;
    skos:inScheme cs: ;
    skos:narrower <https://w3id.org/nfdi4cat/voc4cat_0000164> ;
    skos:prefLabel "gas flow controller and monitor"@en .

<https://w3id.org/nfdi4cat/voc4cat_0000016> a skos:Concept ;
    dcterms:identifier "voc4cat_0000016"^^xsd:token ;
    dcterms:provenance "Self"@en ;
    skos:broader <https://w3id.org/nfdi4cat/voc4cat_0000002> ;
    skos:definition "The form in which the photocatalyst is introduced to the reaction chamber. This can include e.g., powders, pellets or thin films deposited on a substrate. "@en ;
    skos:inScheme cs: ;
    skos:narrower <https://w3id.org/nfdi4cat/voc4cat_0000017>,
        <https://w3id.org/nfdi4cat/voc4cat_0000019> ;
    skos:prefLabel "sample form"@en .

<https://w3id.org/nfdi4cat/voc4cat_0000024> a skos:Concept ;
    dcterms:identifier "voc4cat_0000024"^^xsd:token ;
    dcterms:provenance "Self"@en ;
    skos:broader <https://w3id.org/nfdi4cat/voc4cat_0000019> ;
    skos:definition "The substate onto which a (powdered) photocatalyst is deposited. Such substrates incude glass surfaces (e.g., borosilicate glass or conductive glass like ITO and FTO), ceramic substrates (e.g., alumina) or metal substrates (e.g., Ti foils, stainless steel etc.) "@en ;
    skos:inScheme cs: ;
    skos:narrower <https://w3id.org/nfdi4cat/voc4cat_0000025>,
        <https://w3id.org/nfdi4cat/voc4cat_0000033> ;
    skos:prefLabel "substrate"@en .

<https://w3id.org/nfdi4cat/voc4cat_0000038> a skos:Concept ;
    dcterms:identifier "voc4cat_0000038"^^xsd:token ;
    dcterms:provenance "Self"@en ;
    skos:broader <https://w3id.org/nfdi4cat/voc4cat_0000019> ;
    skos:definition "A thin film of the photocatalyst deposited on an appropiate for the application substrate."@en ;
    skos:inScheme cs: ;
    skos:narrower <https://w3id.org/nfdi4cat/voc4cat_0000039>,
        <https://w3id.org/nfdi4cat/voc4cat_0000040> ;
    skos:prefLabel "deposited sample"@en .

<https://w3id.org/nfdi4cat/voc4cat_0000045> a skos:Concept ;
    dcterms:identifier "voc4cat_0000045"^^xsd:token ;
    dcterms:provenance "Self"@en ;
    skos:broader <https://w3id.org/nfdi4cat/voc4cat_0000002> ;
    skos:definition "The process by which one or more chemical reactions are performed with the aim of converting a reactant or starting material into a product or multiple products."@en ;
    skos:inScheme cs: ;
    skos:narrower <https://w3id.org/nfdi4cat/voc4cat_0000046>,
        <https://w3id.org/nfdi4cat/voc4cat_0000049> ;
    skos:prefLabel "synthesis"@en .

<https://w3id.org/nfdi4cat/voc4cat_0000046> a skos:Concept ;
    dcterms:identifier "voc4cat_0000046"^^xsd:token ;
    dcterms:provenance "Self"@en ;
    skos:altLabel "publications; papers; manuscripts;"@en ;
    skos:broader <https://w3id.org/nfdi4cat/voc4cat_0000045> ;
    skos:definition "Thorough search of available literature on the research topic of interest using online research platforms (e.g, Scopus, Google Scholar, Web of Science, Research Gate etc.) and / or libraries. Relevant literature can be found in the form of publications, books, abstracts and conference presentations. "@en ;
    skos:inScheme cs: ;
    skos:narrower <https://w3id.org/nfdi4cat/voc4cat_0000047>,
        <https://w3id.org/nfdi4cat/voc4cat_0000048> ;
    skos:prefLabel "literature research"@en .

<https://w3id.org/nfdi4cat/voc4cat_0000084> a skos:Concept ;
    dcterms:identifier "voc4cat_0000084"^^xsd:token ;
    dcterms:provenance "Self"@en ;
    skos:broader <https://w3id.org/nfdi4cat/voc4cat_0000001> ;
    skos:definition "The energy state occupied by an electron in a photocatalyst. This state cab affect the electron's ability to participate in a photocatalytic reaction. "@en ;
    skos:inScheme cs: ;
    skos:narrower <https://w3id.org/nfdi4cat/voc4cat_0000085>,
        <https://w3id.org/nfdi4cat/voc4cat_0000086> ;
    skos:prefLabel "electronic state"@en .

<https://w3id.org/nfdi4cat/voc4cat_0000105> a skos:Concept ;
    dcterms:identifier "voc4cat_0000105"^^xsd:token ;
    dcterms:provenance "Self"@en ;
    skos:broader <https://w3id.org/nfdi4cat/voc4cat_0000101> ;
    skos:definition "Electron donors or hole scavengers used to reduce the recombination tendency of electrons and holes. Sacrificial reagents are used in photocatalysis to study an oxidation or reduction reaction seperately."@en ;
    skos:inScheme cs: ;
    skos:narrower <https://w3id.org/nfdi4cat/voc4cat_0000106>,
        <https://w3id.org/nfdi4cat/voc4cat_0000107> ;
    skos:prefLabel "sacrificial reagant"@en .

<https://w3id.org/nfdi4cat/voc4cat_0000108> a skos:Concept ;
    dcterms:identifier "voc4cat_0000108"^^xsd:token ;
    dcterms:provenance "Self"@en ;
    skos:broader <https://w3id.org/nfdi4cat/voc4cat_0000100> ;
    skos:definition "Operation mode under the which the experiment takes place: batch of continuous flow mode."@en ;
    skos:inScheme cs: ;
    skos:narrower <https://w3id.org/nfdi4cat/voc4cat_0000109>,
        <https://w3id.org/nfdi4cat/voc4cat_0000110> ;
    skos:prefLabel "operation mode"@en .

<https://w3id.org/nfdi4cat/voc4cat_0000115> a skos:Concept ;
    dcterms:identifier "voc4cat_0000115"^^xsd:token ;
    dcterms:provenance "Self"@en ;
    skos:broader <https://w3id.org/nfdi4cat/voc4cat_0000100> ;
    skos:definition "The temperature (range) under which the photocatalytic reaction takes place."@en ;
    skos:inScheme cs: ;
    skos:narrower <https://w3id.org/nfdi4cat/voc4cat_0000116>,
        <https://w3id.org/nfdi4cat/voc4cat_0000117> ;
    skos:prefLabel "experiment temperature"@en .

<https://w3id.org/nfdi4cat/voc4cat_0000118> a skos:Concept ;
    dcterms:identifier "voc4cat_0000118"^^xsd:token ;
    dcterms:provenance "Self"@en ;
    skos:broader <https://w3id.org/nfdi4cat/voc4cat_0000100> ;
    skos:definition "The pressure (range) under which the photocatalytic reaction takes place."@en ;
    skos:inScheme cs: ;
    skos:narrower <https://w3id.org/nfdi4cat/voc4cat_0000119>,
        <https://w3id.org/nfdi4cat/voc4cat_0000120> ;
    skos:prefLabel "experiment pressure"@en .

<https://w3id.org/nfdi4cat/voc4cat_0000142> a skos:Concept ;
    dcterms:identifier "voc4cat_0000142"^^xsd:token ;
    dcterms:provenance "Self"@en ;
    skos:broader <https://w3id.org/nfdi4cat/voc4cat_0000128> ;
    skos:definition "The range of critical for the safe operation of the photoreactor parameters."@en ;
    skos:inScheme cs: ;
    skos:narrower <https://w3id.org/nfdi4cat/voc4cat_0000143>,
        <https://w3id.org/nfdi4cat/voc4cat_0000148> ;
    skos:prefLabel "operation parameters"@en .

<https://w3id.org/nfdi4cat/voc4cat_0000157> a skos:Concept ;
    dcterms:identifier "voc4cat_0000157"^^xsd:token ;
    dcterms:provenance "Self"@en ;
    skos:broader <https://w3id.org/nfdi4cat/voc4cat_0000152> ;
    skos:definition "A transparent material optimized to allow the transmission of electromagnetic radiation with low reflectance and scattering. "@en ;
    skos:inScheme cs: ;
    skos:narrower <https://w3id.org/nfdi4cat/voc4cat_0000158>,
        <https://w3id.org/nfdi4cat/voc4cat_0000159> ;
    skos:prefLabel "optical window"@en .

<https://w3id.org/nfdi4cat/voc4cat_0000159> a skos:Concept ;
    dcterms:identifier "voc4cat_0000159"^^xsd:token ;
    dcterms:provenance "Self"@en ;
    skos:broader <https://w3id.org/nfdi4cat/voc4cat_0000157> ;
    skos:definition "The dimension of the optical window (diameter / thickness) allowing the incoming light to enter the reaction chamber and interact with the photocatalyst."@en ;
    skos:inScheme cs: ;
    skos:narrower <https://w3id.org/nfdi4cat/voc4cat_0000160>,
        <https://w3id.org/nfdi4cat/voc4cat_0000161> ;
    skos:prefLabel "optical window dimensions"@en .

<https://w3id.org/nfdi4cat/voc4cat_0000165> a skos:Concept ;
    dcterms:identifier "voc4cat_0000165"^^xsd:token ;
    dcterms:provenance "Self"@en ;
    skos:broader <https://w3id.org/nfdi4cat/voc4cat_0000128> ;
    skos:definition "The irradiation system includes all the necessary equipment needed to perform a photocatalytic experiment. The system apart from the light source can include, filters, power units, lamp cooling devices etc."@en ;
    skos:inScheme cs: ;
    skos:narrower <https://w3id.org/nfdi4cat/voc4cat_0000166>,
        <https://w3id.org/nfdi4cat/voc4cat_0000170> ;
    skos:prefLabel "irradiation system"@en .

<https://w3id.org/nfdi4cat/voc4cat_0000003> a skos:Concept ;
    dcterms:identifier "voc4cat_0000003"^^xsd:token ;
    dcterms:provenance "Self"@en ;
    skos:broader <https://w3id.org/nfdi4cat/voc4cat_0000002> ;
    skos:definition "A material with electrical conductivity between that of a conductor and an insulator."@en ;
    skos:inScheme cs: ;
    skos:narrower <https://w3id.org/nfdi4cat/voc4cat_0000004>,
        <https://w3id.org/nfdi4cat/voc4cat_0000006>,
        <https://w3id.org/nfdi4cat/voc4cat_0000014> ;
    skos:prefLabel "semiconductor"@en .

<https://w3id.org/nfdi4cat/voc4cat_0000019> a skos:Concept ;
    dcterms:identifier "voc4cat_0000019"^^xsd:token ;
    dcterms:provenance "Self"@en ;
    skos:broader <https://w3id.org/nfdi4cat/voc4cat_0000016> ;
    skos:definition "A photocatalyst introduced to the reaction chamber in the form of a thin film. To form a thin film, a (powdered) photocatalyst is deposited on a substrate (e.g., glass or metal) using an appropriate deposition technique. "@en ;
    skos:inScheme cs: ;
    skos:narrower <https://w3id.org/nfdi4cat/voc4cat_0000020>,
        <https://w3id.org/nfdi4cat/voc4cat_0000024>,
        <https://w3id.org/nfdi4cat/voc4cat_0000038> ;
    skos:prefLabel "thin film"@en .

<https://w3id.org/nfdi4cat/voc4cat_0000020> a skos:Concept ;
    dcterms:identifier "voc4cat_0000020"^^xsd:token ;
    dcterms:provenance "Self"@en ;
    skos:broader <https://w3id.org/nfdi4cat/voc4cat_0000019> ;
    skos:definition "A technique used to deposit (immobilize) a (powdered) photocatalyst on a substate. These techniques indlude (but are not limited to): doctor blading, spin coating, spray coating, etc."@en ;
    skos:inScheme cs: ;
    skos:narrower <https://w3id.org/nfdi4cat/voc4cat_0000021>,
        <https://w3id.org/nfdi4cat/voc4cat_0000022>,
        <https://w3id.org/nfdi4cat/voc4cat_0000023> ;
    skos:prefLabel "deposition technique"@en .

<https://w3id.org/nfdi4cat/voc4cat_0000025> a skos:Concept ;
    dcterms:identifier "voc4cat_0000025"^^xsd:token ;
    dcterms:provenance "Self"@en ;
    skos:broader <https://w3id.org/nfdi4cat/voc4cat_0000024> ;
    skos:definition "The material that the substrate is made of. Common materials include: glass (conductive or not), ceramics and metal."@en ;
    skos:inScheme cs: ;
    skos:narrower <https://w3id.org/nfdi4cat/voc4cat_0000026>,
        <https://w3id.org/nfdi4cat/voc4cat_0000027>,
        <https://w3id.org/nfdi4cat/voc4cat_0000032> ;
    skos:prefLabel "substrate material"@en .

<https://w3id.org/nfdi4cat/voc4cat_0000062> a skos:Concept ;
    dcterms:identifier "voc4cat_0000062"^^xsd:token ;
    dcterms:provenance "Self"@en ;
    skos:broader <https://w3id.org/nfdi4cat/voc4cat_0000049> ;
    skos:definition "Chemical substances used in the synthesis process of a desired photocatalyst."@en ;
    skos:inScheme cs: ;
    skos:narrower <https://w3id.org/nfdi4cat/voc4cat_0000063>,
        <https://w3id.org/nfdi4cat/voc4cat_0000064>,
        <https://w3id.org/nfdi4cat/voc4cat_0000065> ;
    skos:prefLabel "chemical substance for synthesis"@en .

<https://w3id.org/nfdi4cat/voc4cat_0000111> a skos:Concept ;
    dcterms:identifier "voc4cat_0000111"^^xsd:token ;
    dcterms:provenance "Self"@en ;
    skos:broader <https://w3id.org/nfdi4cat/voc4cat_0000100> ;
    skos:definition "The total duration of an experiment"@en ;
    skos:inScheme cs: ;
    skos:narrower <https://w3id.org/nfdi4cat/voc4cat_0000112>,
        <https://w3id.org/nfdi4cat/voc4cat_0000113>,
        <https://w3id.org/nfdi4cat/voc4cat_0000114> ;
    skos:prefLabel "experiment duration"@en .

<https://w3id.org/nfdi4cat/voc4cat_0000124> a skos:Concept ;
    dcterms:identifier "voc4cat_0000124"^^xsd:token ;
    dcterms:provenance "Self"@en ;
    skos:broader <https://w3id.org/nfdi4cat/voc4cat_0000100> ;
    skos:definition "Quantitative and qualitative evaluation of the outcome of a photocatalytic reaction (e.g., product formation from the photoreduction of CO2). The evaluation can lead to changes in the synthesis of the photocatalyst and / or selecting different experimental parameters."@en ;
    skos:inScheme cs: ;
    skos:narrower <https://w3id.org/nfdi4cat/voc4cat_0000125>,
        <https://w3id.org/nfdi4cat/voc4cat_0000126>,
        <https://w3id.org/nfdi4cat/voc4cat_0000127> ;
    skos:prefLabel "evaluation"@en .

<https://w3id.org/nfdi4cat/voc4cat_0000129> a skos:Concept ;
    dcterms:identifier "voc4cat_0000129"^^xsd:token ;
    dcterms:provenance "Self"@en ;
    skos:broader <https://w3id.org/nfdi4cat/voc4cat_0000128> ;
    skos:definition "Spectroscopic or chromatographic methods used to qualitatively and quantitatively identify the products of the photoreaction. Such devices are usually attached to the photoreactor, or a sample is being trasfered to an identification method via another medium (e.g., gastight syringes)."@en ;
    skos:inScheme cs: ;
    skos:narrower <https://w3id.org/nfdi4cat/voc4cat_0000130>,
        <https://w3id.org/nfdi4cat/voc4cat_0000137>,
        <https://w3id.org/nfdi4cat/voc4cat_0000141> ;
    skos:prefLabel "product identification method"@en .

<https://w3id.org/nfdi4cat/voc4cat_0000131> a skos:Concept ;
    dcterms:identifier "voc4cat_0000131"^^xsd:token ;
    dcterms:provenance "Self"@en ;
    skos:broader <https://w3id.org/nfdi4cat/voc4cat_0000130> ;
    skos:definition "Detectors of the gas chromatogragh used to identify the reaction products and intemediates."@en ;
    skos:inScheme cs: ;
    skos:narrower <https://w3id.org/nfdi4cat/voc4cat_0000132>,
        <https://w3id.org/nfdi4cat/voc4cat_0000133>,
        <https://w3id.org/nfdi4cat/voc4cat_0000134> ;
    skos:prefLabel "gas chromatograph detector"@en .

<https://w3id.org/nfdi4cat/voc4cat_0000143> a skos:Concept ;
    dcterms:identifier "voc4cat_0000143"^^xsd:token ;
    dcterms:provenance "Self"@en ;
    skos:altLabel "range of operation pressure; operation pressure range; \\Ppressure range"@en ;
    skos:broader <https://w3id.org/nfdi4cat/voc4cat_0000142> ;
    skos:definition "Maximum and minimum of operation pressure range within the reactor can operate safely. Higher operation temperatures can lead to higher pressure values."@en ;
    skos:inScheme cs: ;
    skos:narrower <https://w3id.org/nfdi4cat/voc4cat_0000144>,
        <https://w3id.org/nfdi4cat/voc4cat_0000145>,
        <https://w3id.org/nfdi4cat/voc4cat_0000146> ;
    skos:prefLabel "operation pressure"@en .

<https://w3id.org/nfdi4cat/voc4cat_0000148> a skos:Concept ;
    dcterms:identifier "voc4cat_0000148"^^xsd:token ;
    dcterms:provenance "Self"@en ;
    skos:altLabel "range of operation temperature; operation temperature range; temparature range"@en ;
    skos:broader <https://w3id.org/nfdi4cat/voc4cat_0000142> ;
    skos:definition "Maximum and minimum of operation temperature range within the reactor can operate safely."@en ;
    skos:inScheme cs: ;
    skos:narrower <https://w3id.org/nfdi4cat/voc4cat_0000149>,
        <https://w3id.org/nfdi4cat/voc4cat_0000150>,
        <https://w3id.org/nfdi4cat/voc4cat_0000151> ;
    skos:prefLabel "operation temperature"@en .

<https://w3id.org/nfdi4cat/voc4cat_0000166> a skos:Concept ;
    dcterms:identifier "voc4cat_0000166"^^xsd:token ;
    dcterms:provenance "Self"@en ;
    skos:broader <https://w3id.org/nfdi4cat/voc4cat_0000165> ;
    skos:definition "Light source used to irradiate a photocatalyst in a reaction chamber. These include sources with various intensities, powers and wavelength ranges,  including Hg/Xe lamps, Xe lamps and LEDs. "@en ;
    skos:inScheme cs: ;
    skos:narrower <https://w3id.org/nfdi4cat/voc4cat_0000167>,
        <https://w3id.org/nfdi4cat/voc4cat_0000168>,
        <https://w3id.org/nfdi4cat/voc4cat_0000169> ;
    skos:prefLabel "light source"@en .

<https://w3id.org/nfdi4cat/voc4cat_0000176> a skos:Concept ;
    dcterms:identifier "voc4cat_0000176"^^xsd:token ;
    dcterms:provenance "Self"@en ;
    skos:altLabel "λ"@en ;
    skos:broader <https://w3id.org/nfdi4cat/voc4cat_0000170> ;
    skos:definition "The distance between two successive peaks or troughs in a wave."@en ;
    skos:inScheme cs: ;
    skos:narrower <https://w3id.org/nfdi4cat/voc4cat_0000177>,
        <https://w3id.org/nfdi4cat/voc4cat_0000178>,
        <https://w3id.org/nfdi4cat/voc4cat_0000179> ;
    skos:prefLabel "light wavelength"@en .

<https://w3id.org/nfdi4cat/voc4cat_0000002> a skos:Concept ;
    dcterms:identifier "voc4cat_0000002"^^xsd:token ;
    dcterms:provenance "Self"@en ;
    skos:altLabel "photocatalytic material"@en ;
    skos:broader <https://w3id.org/nfdi4cat/voc4cat_0000001> ;
    skos:definition "A material that absorbs photons (light) of appropriate energy and initiates or accelerates a photochemical reaction, while it regenerates itself after each reaction cycle. "@en ;
    skos:inScheme cs: ;
    skos:narrower <https://w3id.org/nfdi4cat/voc4cat_0000003>,
        <https://w3id.org/nfdi4cat/voc4cat_0000016>,
        <https://w3id.org/nfdi4cat/voc4cat_0000045>,
        <https://w3id.org/nfdi4cat/voc4cat_0000066> ;
    skos:prefLabel "photocatalyst"@en .

<https://w3id.org/nfdi4cat/voc4cat_0000027> a skos:Concept ;
    dcterms:identifier "voc4cat_0000027"^^xsd:token ;
    dcterms:provenance "Self"@en ;
    skos:broader <https://w3id.org/nfdi4cat/voc4cat_0000025> ;
    skos:definition "A flat surface made of glass serving as a substrate for the deposition of a photocatalyst."@en ;
    skos:inScheme cs: ;
    skos:narrower <https://w3id.org/nfdi4cat/voc4cat_0000028>,
        <https://w3id.org/nfdi4cat/voc4cat_0000029>,
        <https://w3id.org/nfdi4cat/voc4cat_0000030>,
        <https://w3id.org/nfdi4cat/voc4cat_0000031> ;
    skos:prefLabel "glass substrate"@en .

<https://w3id.org/nfdi4cat/voc4cat_0000033> a skos:Concept ;
    dcterms:identifier "voc4cat_0000033"^^xsd:token ;
    dcterms:provenance "Self"@en ;
    skos:broader <https://w3id.org/nfdi4cat/voc4cat_0000024> ;
    skos:definition "The diamensions of the substrate."@en ;
    skos:inScheme cs: ;
    skos:narrower <https://w3id.org/nfdi4cat/voc4cat_0000034>,
        <https://w3id.org/nfdi4cat/voc4cat_0000035>,
        <https://w3id.org/nfdi4cat/voc4cat_0000036>,
        <https://w3id.org/nfdi4cat/voc4cat_0000037> ;
    skos:prefLabel "substrate dimension"@en .

<https://w3id.org/nfdi4cat/voc4cat_0000040> a skos:Concept ;
    dcterms:identifier "voc4cat_0000040"^^xsd:token ;
    dcterms:provenance "Self"@en ;
    skos:broader <https://w3id.org/nfdi4cat/voc4cat_0000038> ;
    skos:definition "The diamensions of the - deposited on the substrate - thin film"@en ;
    skos:inScheme cs: ;
    skos:narrower <https://w3id.org/nfdi4cat/voc4cat_0000041>,
        <https://w3id.org/nfdi4cat/voc4cat_0000042>,
        <https://w3id.org/nfdi4cat/voc4cat_0000043>,
        <https://w3id.org/nfdi4cat/voc4cat_0000044> ;
    skos:prefLabel "thin film dimension"@en .

<https://w3id.org/nfdi4cat/voc4cat_0000101> a skos:Concept ;
    dcterms:identifier "voc4cat_0000101"^^xsd:token ;
    dcterms:provenance "Self"@en ;
    skos:broader <https://w3id.org/nfdi4cat/voc4cat_0000100> ;
    skos:definition "The starting substances that undergo a chemical reaction to produce a desired product."@en ;
    skos:inScheme cs: ;
    skos:narrower <https://w3id.org/nfdi4cat/voc4cat_0000102>,
        <https://w3id.org/nfdi4cat/voc4cat_0000103>,
        <https://w3id.org/nfdi4cat/voc4cat_0000104>,
        <https://w3id.org/nfdi4cat/voc4cat_0000105> ;
    skos:prefLabel "reactant"@en .

<https://w3id.org/nfdi4cat/voc4cat_0000130> a skos:Concept ;
    dcterms:identifier "voc4cat_0000130"^^xsd:token ;
    dcterms:provenance "Self"@en ;
    skos:altLabel "GC"@en ;
    skos:broader <https://w3id.org/nfdi4cat/voc4cat_0000129> ;
    skos:definition "An analytical technique that separates and analyzes the components of a gas mixture by passing it though a stationary phase."@en ;
    skos:inScheme cs: ;
    skos:narrower <https://w3id.org/nfdi4cat/voc4cat_0000131>,
        <https://w3id.org/nfdi4cat/voc4cat_0000135>,
        <https://w3id.org/nfdi4cat/voc4cat_0000136> ;
    skos:prefLabel "gas chromatography"@en .

<https://w3id.org/nfdi4cat/voc4cat_0000137> a skos:Concept ;
    dcterms:identifier "voc4cat_0000137"^^xsd:token ;
    dcterms:provenance "Self"@en ;
    skos:altLabel "MS"@en ;
    skos:broader <https://w3id.org/nfdi4cat/voc4cat_0000129> ;
    skos:definition "An analytical technique which determines the mass-to-charge ratio of ions in a sample to give information about the composition of the sample."@en ;
    skos:inScheme cs: ;
    skos:narrower <https://w3id.org/nfdi4cat/voc4cat_0000138>,
        <https://w3id.org/nfdi4cat/voc4cat_0000139>,
        <https://w3id.org/nfdi4cat/voc4cat_0000140> ;
    skos:prefLabel "mass spectrometry"@en .

<https://w3id.org/nfdi4cat/voc4cat_0000001> a skos:Concept ;
    dcterms:identifier "voc4cat_0000001"^^xsd:token ;
    dcterms:provenance "Self"@en ;
    skos:altLabel "photocatalytic reaction"@en ;
    skos:definition "A process which catalyzes a chemical reaction through the absorption of sufficient light energy by a photocatalyst. "@en ;
    skos:inScheme cs: ;
    skos:narrower <https://w3id.org/nfdi4cat/voc4cat_0000002>,
        <https://w3id.org/nfdi4cat/voc4cat_0000084>,
        <https://w3id.org/nfdi4cat/voc4cat_0000087>,
        <https://w3id.org/nfdi4cat/voc4cat_0000100>,
        <https://w3id.org/nfdi4cat/voc4cat_0000128> ;
    skos:prefLabel "photocatalysis"@en ;
    skos:topConceptOf cs: .

<https://w3id.org/nfdi4cat/voc4cat_0000128> a skos:Concept ;
    dcterms:identifier "voc4cat_0000128"^^xsd:token ;
    dcterms:provenance "Self"@en ;
    skos:altLabel "reactor design; reactor engineering; photoreactor engineering"@en ;
    skos:broader <https://w3id.org/nfdi4cat/voc4cat_0000001> ;
    skos:definition "Details describing the construction, physical dimensions, and operation of the photoreactor used to perform a photocatalytic reaction."@en ;
    skos:inScheme cs: ;
    skos:narrower <https://w3id.org/nfdi4cat/voc4cat_0000129>,
        <https://w3id.org/nfdi4cat/voc4cat_0000142>,
        <https://w3id.org/nfdi4cat/voc4cat_0000152>,
        <https://w3id.org/nfdi4cat/voc4cat_0000162>,
        <https://w3id.org/nfdi4cat/voc4cat_0000165> ;
    skos:prefLabel "photoreactor design"@en .

<https://w3id.org/nfdi4cat/voc4cat_0000152> a skos:Concept ;
    dcterms:identifier "voc4cat_0000152"^^xsd:token ;
    dcterms:provenance "Self"@en ;
    skos:altLabel "photoreaction chamber"@en ;
    skos:broader <https://w3id.org/nfdi4cat/voc4cat_0000128> ;
    skos:definition "A construction inside of which the photocatalyst and the reactants coexist and the photoreaction takes place."@en ;
    skos:inScheme cs: ;
    skos:narrower <https://w3id.org/nfdi4cat/voc4cat_0000153>,
        <https://w3id.org/nfdi4cat/voc4cat_0000154>,
        <https://w3id.org/nfdi4cat/voc4cat_0000155>,
        <https://w3id.org/nfdi4cat/voc4cat_0000156>,
        <https://w3id.org/nfdi4cat/voc4cat_0000157> ;
    skos:prefLabel "reaction chamber"@en .

<https://w3id.org/nfdi4cat/voc4cat_0000054> a skos:Concept ;
    dcterms:identifier "voc4cat_0000054"^^xsd:token ;
    dcterms:provenance "self"@en ;
    skos:altLabel "heat treatment; heat-treatment; calcination"@en ;
    skos:broader <https://w3id.org/nfdi4cat/voc4cat_0000049> ;
    skos:definition "Heat treatment to reach the desired final photocatalyst. The parameters of the heat treatment can vary between each calcination step. "@en ;
    skos:inScheme cs: ;
    skos:narrower <https://w3id.org/nfdi4cat/voc4cat_0000055>,
        <https://w3id.org/nfdi4cat/voc4cat_0000056>,
        <https://w3id.org/nfdi4cat/voc4cat_0000057>,
        <https://w3id.org/nfdi4cat/voc4cat_0000058>,
        <https://w3id.org/nfdi4cat/voc4cat_0000059>,
        <https://w3id.org/nfdi4cat/voc4cat_0000060> ;
    skos:prefLabel "calcination step"@en .

<https://w3id.org/nfdi4cat/voc4cat_0000170> a skos:Concept ;
    dcterms:identifier "voc4cat_0000170"^^xsd:token ;
    dcterms:provenance "Self"@en ;
    skos:broader <https://w3id.org/nfdi4cat/voc4cat_0000165> ;
    skos:definition "Specific of roperties of the light source dictaning its operation and its adequacy in the studied photocatalytic reaction. "@en ;
    skos:inScheme cs: ;
    skos:narrower <https://w3id.org/nfdi4cat/voc4cat_0000171>,
        <https://w3id.org/nfdi4cat/voc4cat_0000172>,
        <https://w3id.org/nfdi4cat/voc4cat_0000173>,
        <https://w3id.org/nfdi4cat/voc4cat_0000174>,
        <https://w3id.org/nfdi4cat/voc4cat_0000175>,
        <https://w3id.org/nfdi4cat/voc4cat_0000176> ;
    skos:prefLabel "light source property"@en .

<https://w3id.org/nfdi4cat/voc4cat_0000006> a skos:Concept ;
    dcterms:identifier "voc4cat_0000006"^^xsd:token ;
    dcterms:provenance "Self"@en ;
    skos:broader <https://w3id.org/nfdi4cat/voc4cat_0000003> ;
    skos:definition "Characteristic properties of a semiconductor used in the field of photocatalysis. These properties determine its performance in the studied photocatalytic application."@en ;
    skos:inScheme cs: ;
    skos:narrower <https://w3id.org/nfdi4cat/voc4cat_0000007>,
        <https://w3id.org/nfdi4cat/voc4cat_0000008>,
        <https://w3id.org/nfdi4cat/voc4cat_0000009>,
        <https://w3id.org/nfdi4cat/voc4cat_0000010>,
        <https://w3id.org/nfdi4cat/voc4cat_0000011>,
        <https://w3id.org/nfdi4cat/voc4cat_0000012>,
        <https://w3id.org/nfdi4cat/voc4cat_0000013> ;
    skos:prefLabel "semiconductor property"@en .

<https://w3id.org/nfdi4cat/voc4cat_0000049> a skos:Concept ;
    dcterms:identifier "voc4cat_0000049"^^xsd:token ;
    dcterms:provenance "Self"@en ;
    skos:broader <https://w3id.org/nfdi4cat/voc4cat_0000045> ;
    skos:definition "Necessary steps needed to follow in order to reach the desired photocatalyst."@en ;
    skos:inScheme cs: ;
    skos:narrower <https://w3id.org/nfdi4cat/voc4cat_0000050>,
        <https://w3id.org/nfdi4cat/voc4cat_0000051>,
        <https://w3id.org/nfdi4cat/voc4cat_0000052>,
        <https://w3id.org/nfdi4cat/voc4cat_0000053>,
        <https://w3id.org/nfdi4cat/voc4cat_0000054>,
        <https://w3id.org/nfdi4cat/voc4cat_0000061>,
        <https://w3id.org/nfdi4cat/voc4cat_0000062> ;
    skos:prefLabel "synthesis procedure"@en .

<https://w3id.org/nfdi4cat/voc4cat_0000100> a skos:Concept ;
    dcterms:identifier "voc4cat_0000100"^^xsd:token ;
    dcterms:provenance "Self"@en ;
    skos:broader <https://w3id.org/nfdi4cat/voc4cat_0000001> ;
    skos:definition "A lab-scale experiment performed to test the efficiency of a studied photocatalyst in a photocatalytic application (e.g., dye degradation, CO2 photoreduction e.t.c.)."@en ;
    skos:inScheme cs: ;
    skos:narrower <https://w3id.org/nfdi4cat/voc4cat_0000101>,
        <https://w3id.org/nfdi4cat/voc4cat_0000108>,
        <https://w3id.org/nfdi4cat/voc4cat_0000111>,
        <https://w3id.org/nfdi4cat/voc4cat_0000115>,
        <https://w3id.org/nfdi4cat/voc4cat_0000118>,
        <https://w3id.org/nfdi4cat/voc4cat_0000121>,
        <https://w3id.org/nfdi4cat/voc4cat_0000122>,
        <https://w3id.org/nfdi4cat/voc4cat_0000123>,
        <https://w3id.org/nfdi4cat/voc4cat_0000124> ;
    skos:prefLabel "photocatalytic experiment"@en .

<https://w3id.org/nfdi4cat/voc4cat_0000087> a skos:Concept ;
    dcterms:identifier "voc4cat_0000087"^^xsd:token ;
    dcterms:provenance "Self"@en ;
    skos:broader <https://w3id.org/nfdi4cat/voc4cat_0000001> ;
    skos:definition "A multi-step process iniatiated by the absorption of photons by a photocatalyst. This process involves various sub-processes that include the photogeneration and transfer of electron and hole pairs. "@en ;
    skos:inScheme cs: ;
    skos:narrower <https://w3id.org/nfdi4cat/voc4cat_0000088>,
        <https://w3id.org/nfdi4cat/voc4cat_0000089>,
        <https://w3id.org/nfdi4cat/voc4cat_0000090>,
        <https://w3id.org/nfdi4cat/voc4cat_0000091>,
        <https://w3id.org/nfdi4cat/voc4cat_0000092>,
        <https://w3id.org/nfdi4cat/voc4cat_0000093>,
        <https://w3id.org/nfdi4cat/voc4cat_0000094>,
        <https://w3id.org/nfdi4cat/voc4cat_0000095>,
        <https://w3id.org/nfdi4cat/voc4cat_0000096>,
        <https://w3id.org/nfdi4cat/voc4cat_0000097>,
        <https://w3id.org/nfdi4cat/voc4cat_0000098> ;
    skos:prefLabel "photocatalytic process"@en .

<https://w3id.org/nfdi4cat/voc4cat_0000066> a skos:Concept ;
    dcterms:identifier "voc4cat_0000066"^^xsd:token ;
    dcterms:provenance "Self"@en ;
    skos:broader <https://w3id.org/nfdi4cat/voc4cat_0000002> ;
    skos:definition "A collection of techniques used to identify the (physico)chemical, morphological, structural, mechanical, optical and electrical properties of the syntesized photocatalysts. Characterization is performed after the synthesis of the photocatalysts to evaluate the success of the synthetic approach, but also after the completion of the evaluation of the materials in CO2 photoreduction to ensure their stability under the selected experimental parameters."@en ;
    skos:inScheme cs: ;
    skos:narrower <https://w3id.org/nfdi4cat/voc4cat_0000067>,
        <https://w3id.org/nfdi4cat/voc4cat_0000068>,
        <https://w3id.org/nfdi4cat/voc4cat_0000069>,
        <https://w3id.org/nfdi4cat/voc4cat_0000070>,
        <https://w3id.org/nfdi4cat/voc4cat_0000071>,
        <https://w3id.org/nfdi4cat/voc4cat_0000072>,
        <https://w3id.org/nfdi4cat/voc4cat_0000073>,
        <https://w3id.org/nfdi4cat/voc4cat_0000074>,
        <https://w3id.org/nfdi4cat/voc4cat_0000075>,
        <https://w3id.org/nfdi4cat/voc4cat_0000076>,
        <https://w3id.org/nfdi4cat/voc4cat_0000077>,
        <https://w3id.org/nfdi4cat/voc4cat_0000078>,
        <https://w3id.org/nfdi4cat/voc4cat_0000079>,
        <https://w3id.org/nfdi4cat/voc4cat_0000080>,
        <https://w3id.org/nfdi4cat/voc4cat_0000081>,
        <https://w3id.org/nfdi4cat/voc4cat_0000082>,
        <https://w3id.org/nfdi4cat/voc4cat_0000083> ;
    skos:prefLabel "characterization"@en .

cs: a skos:ConceptScheme ;
    dcterms:created "2023-06-29"^^xsd:date ;
    dcterms:creator <http://example.org/nfdi4cat/> ;
    dcterms:hasPart <https://w3id.org/nfdi4cat/voc4cat_0001900>,
        <https://w3id.org/nfdi4cat/voc4cat_0001901> ;
    dcterms:identifier "test_"^^xsd:token ;
    dcterms:modified "2023-06-29"^^xsd:date ;
    dcterms:provenance "David Linke (orcid:0000-0002-5898-1820), Nikolaos G. Moustakas (orcid:0000-0002-6242-2167)"@en ;
    dcterms:publisher <http://example.org/nfdi4cat/> ;
    owl:versionInfo "v2023-06-29" ;
    skos:definition "A vocabulary for all areas of catalysis initiated in NFDI4Cat. Starting with photocatalysis we add more and more terms from other areas of catalysis and related disciplines like chemical enineering or material science."@en ;
    skos:hasTopConcept <https://w3id.org/nfdi4cat/voc4cat_0000001> ;
    skos:prefLabel "Voc4Cat - A SKOS vocabulary for Catalysis."@en ;
    dcat:contactPoint "David Linke (orcid:0000-0002-5898-1820), Nikolaos G. Moustakas (orcid:0000-0002-6242-2167)" .

