@prefix dcat: <http://www.w3.org/ns/dcat#> .
@prefix dcterms: <http://purl.org/dc/terms/> .
@prefix owl: <http://www.w3.org/2002/07/owl#> .
@prefix rdfs: <http://www.w3.org/2000/01/rdf-schema#> .
@prefix schema: <https://schema.org/> .
@prefix skos: <http://www.w3.org/2004/02/skos/core#> .
@prefix xsd: <http://www.w3.org/2001/XMLSchema#> .

<https://w3id.org/nfdi4cat/voc4cat_0000016> a skos:Concept ;
    dcterms:identifier "voc4cat_0000016"^^xsd:token ;
    skos:broader <https://w3id.org/nfdi4cat/voc4cat_0000186> ;
    skos:definition "The form in which the catalyst is introduced to the reaction chamber. This can include e.g., powders, pellets or thin films deposited on a substrate."@en ;
    skos:historyNote "0000-0002-6242-2167 Nikolaos G. Moustakas created the resource, 0000-0002-4041-0165 Julia Schumann generalized the definition"@en ;
    skos:inScheme <https://w3id.org/nfdi4cat/voc4cat> ;
    skos:prefLabel "catalyst form"@en .

<https://w3id.org/nfdi4cat/voc4cat_0000019> a skos:Concept ;
    dcterms:identifier "voc4cat_0000019"^^xsd:token ;
    skos:broader <https://w3id.org/nfdi4cat/voc4cat_0000194> ;
    skos:definition "A catalyst introduced to the reaction chamber in the form of a thin film. To form a thin film, a (powdered) catalyst is deposited on a substrate (e.g., glass or metal) using an appropriate deposition technique."@en ;
    skos:historyNote "0000-0002-6242-2167 Nikolaos G. Moustakas created the resource, 0000-0002-4041-0165 Julia Schumann generalized the definition"@en ;
    skos:inScheme <https://w3id.org/nfdi4cat/voc4cat> ;
    skos:prefLabel "thin film"@en .

<https://w3id.org/nfdi4cat/voc4cat_0000193> a skos:Concept ;
    dcterms:identifier "voc4cat_0000193"^^xsd:token ;
    skos:broader <https://w3id.org/nfdi4cat/voc4cat_0007017> ;
    skos:definition "A reactor used to perform and study electrochemical reactions."@en ;
    skos:historyNote "0000-0002-6242-2167 Nikolaos G. Moustakas created the resource"@en ;
    skos:inScheme <https://w3id.org/nfdi4cat/voc4cat> ;
    skos:prefLabel "electrochemical reactor"@en .

<https://w3id.org/nfdi4cat/voc4cat_0000195> a skos:Collection ;
    dcterms:identifier "voc4cat_0000195"^^xsd:token ;
    dcterms:isPartOf <https://w3id.org/nfdi4cat/voc4cat> ;
    rdfs:isDefinedBy <https://w3id.org/nfdi4cat/voc4cat> ;
    skos:definition "A collection of concepts most often appearing as publication keywords in the journal ChemCatChem (Wiley)."@en ;
    skos:historyNote "0000-0002-6242-2167 Nikolaos G. Moustakas created the collection"@en ;
    skos:inScheme <https://w3id.org/nfdi4cat/voc4cat> ;
    skos:member <https://w3id.org/nfdi4cat/voc4cat_0000001>,
        <https://w3id.org/nfdi4cat/voc4cat_0000002>,
        <https://w3id.org/nfdi4cat/voc4cat_0000015>,
        <https://w3id.org/nfdi4cat/voc4cat_0000020>,
        <https://w3id.org/nfdi4cat/voc4cat_0000049>,
        <https://w3id.org/nfdi4cat/voc4cat_0000069>,
        <https://w3id.org/nfdi4cat/voc4cat_0000073>,
        <https://w3id.org/nfdi4cat/voc4cat_0000080>,
        <https://w3id.org/nfdi4cat/voc4cat_0000093>,
        <https://w3id.org/nfdi4cat/voc4cat_0000097>,
        <https://w3id.org/nfdi4cat/voc4cat_0000098>,
        <https://w3id.org/nfdi4cat/voc4cat_0000125>,
        <https://w3id.org/nfdi4cat/voc4cat_0000178>,
        <https://w3id.org/nfdi4cat/voc4cat_0000194>,
        <https://w3id.org/nfdi4cat/voc4cat_0000197>,
        <https://w3id.org/nfdi4cat/voc4cat_0000198>,
        <https://w3id.org/nfdi4cat/voc4cat_0000199>,
        <https://w3id.org/nfdi4cat/voc4cat_0000200>,
        <https://w3id.org/nfdi4cat/voc4cat_0000201>,
        <https://w3id.org/nfdi4cat/voc4cat_0000202>,
        <https://w3id.org/nfdi4cat/voc4cat_0000203>,
        <https://w3id.org/nfdi4cat/voc4cat_0000204>,
        <https://w3id.org/nfdi4cat/voc4cat_0000205>,
        <https://w3id.org/nfdi4cat/voc4cat_0000206>,
        <https://w3id.org/nfdi4cat/voc4cat_0000207>,
        <https://w3id.org/nfdi4cat/voc4cat_0000208>,
        <https://w3id.org/nfdi4cat/voc4cat_0000209>,
        <https://w3id.org/nfdi4cat/voc4cat_0000210>,
        <https://w3id.org/nfdi4cat/voc4cat_0000211>,
        <https://w3id.org/nfdi4cat/voc4cat_0000212>,
        <https://w3id.org/nfdi4cat/voc4cat_0000213>,
        <https://w3id.org/nfdi4cat/voc4cat_0000214>,
        <https://w3id.org/nfdi4cat/voc4cat_0000215>,
        <https://w3id.org/nfdi4cat/voc4cat_0000216>,
        <https://w3id.org/nfdi4cat/voc4cat_0000217>,
        <https://w3id.org/nfdi4cat/voc4cat_0000218>,
        <https://w3id.org/nfdi4cat/voc4cat_0000219>,
        <https://w3id.org/nfdi4cat/voc4cat_0000220>,
        <https://w3id.org/nfdi4cat/voc4cat_0000221>,
        <https://w3id.org/nfdi4cat/voc4cat_0000222>,
        <https://w3id.org/nfdi4cat/voc4cat_0000223>,
        <https://w3id.org/nfdi4cat/voc4cat_0000224>,
        <https://w3id.org/nfdi4cat/voc4cat_0000225>,
        <https://w3id.org/nfdi4cat/voc4cat_0000226>,
        <https://w3id.org/nfdi4cat/voc4cat_0000227>,
        <https://w3id.org/nfdi4cat/voc4cat_0000228>,
        <https://w3id.org/nfdi4cat/voc4cat_0000229>,
        <https://w3id.org/nfdi4cat/voc4cat_0000230>,
        <https://w3id.org/nfdi4cat/voc4cat_0000231>,
        <https://w3id.org/nfdi4cat/voc4cat_0000232>,
        <https://w3id.org/nfdi4cat/voc4cat_0000233>,
        <https://w3id.org/nfdi4cat/voc4cat_0000234>,
        <https://w3id.org/nfdi4cat/voc4cat_0000235>,
        <https://w3id.org/nfdi4cat/voc4cat_0000236>,
        <https://w3id.org/nfdi4cat/voc4cat_0000237>,
        <https://w3id.org/nfdi4cat/voc4cat_0000238>,
        <https://w3id.org/nfdi4cat/voc4cat_0000239>,
        <https://w3id.org/nfdi4cat/voc4cat_0000240>,
        <https://w3id.org/nfdi4cat/voc4cat_0000241>,
        <https://w3id.org/nfdi4cat/voc4cat_0000242>,
        <https://w3id.org/nfdi4cat/voc4cat_0000243>,
        <https://w3id.org/nfdi4cat/voc4cat_0000244>,
        <https://w3id.org/nfdi4cat/voc4cat_0000245>,
        <https://w3id.org/nfdi4cat/voc4cat_0000246>,
        <https://w3id.org/nfdi4cat/voc4cat_0000247>,
        <https://w3id.org/nfdi4cat/voc4cat_0000248>,
        <https://w3id.org/nfdi4cat/voc4cat_0000249>,
        <https://w3id.org/nfdi4cat/voc4cat_0000250>,
        <https://w3id.org/nfdi4cat/voc4cat_0000251>,
        <https://w3id.org/nfdi4cat/voc4cat_0000252>,
        <https://w3id.org/nfdi4cat/voc4cat_0000253>,
        <https://w3id.org/nfdi4cat/voc4cat_0000254>,
        <https://w3id.org/nfdi4cat/voc4cat_0000255>,
        <https://w3id.org/nfdi4cat/voc4cat_0000256>,
        <https://w3id.org/nfdi4cat/voc4cat_0000257>,
        <https://w3id.org/nfdi4cat/voc4cat_0000258>,
        <https://w3id.org/nfdi4cat/voc4cat_0000259>,
        <https://w3id.org/nfdi4cat/voc4cat_0000260>,
        <https://w3id.org/nfdi4cat/voc4cat_0000261>,
        <https://w3id.org/nfdi4cat/voc4cat_0000262>,
        <https://w3id.org/nfdi4cat/voc4cat_0000263>,
        <https://w3id.org/nfdi4cat/voc4cat_0000264>,
        <https://w3id.org/nfdi4cat/voc4cat_0000265>,
        <https://w3id.org/nfdi4cat/voc4cat_0000266>,
        <https://w3id.org/nfdi4cat/voc4cat_0000267>,
        <https://w3id.org/nfdi4cat/voc4cat_0000268>,
        <https://w3id.org/nfdi4cat/voc4cat_0000269>,
        <https://w3id.org/nfdi4cat/voc4cat_0000270>,
        <https://w3id.org/nfdi4cat/voc4cat_0000271>,
        <https://w3id.org/nfdi4cat/voc4cat_0000272>,
        <https://w3id.org/nfdi4cat/voc4cat_0000273>,
        <https://w3id.org/nfdi4cat/voc4cat_0000274>,
        <https://w3id.org/nfdi4cat/voc4cat_0000275>,
        <https://w3id.org/nfdi4cat/voc4cat_0000276>,
        <https://w3id.org/nfdi4cat/voc4cat_0000277>,
        <https://w3id.org/nfdi4cat/voc4cat_0000278>,
        <https://w3id.org/nfdi4cat/voc4cat_0000279>,
        <https://w3id.org/nfdi4cat/voc4cat_0000280>,
        <https://w3id.org/nfdi4cat/voc4cat_0000281>,
        <https://w3id.org/nfdi4cat/voc4cat_0000282>,
        <https://w3id.org/nfdi4cat/voc4cat_0000283>,
        <https://w3id.org/nfdi4cat/voc4cat_0000284>,
        <https://w3id.org/nfdi4cat/voc4cat_0000285>,
        <https://w3id.org/nfdi4cat/voc4cat_0000286>,
        <https://w3id.org/nfdi4cat/voc4cat_0000287>,
        <https://w3id.org/nfdi4cat/voc4cat_0000288>,
        <https://w3id.org/nfdi4cat/voc4cat_0000289>,
        <https://w3id.org/nfdi4cat/voc4cat_0000290>,
        <https://w3id.org/nfdi4cat/voc4cat_0000291>,
        <https://w3id.org/nfdi4cat/voc4cat_0000292>,
        <https://w3id.org/nfdi4cat/voc4cat_0000293>,
        <https://w3id.org/nfdi4cat/voc4cat_0000294>,
        <https://w3id.org/nfdi4cat/voc4cat_0000295>,
        <https://w3id.org/nfdi4cat/voc4cat_0000296>,
        <https://w3id.org/nfdi4cat/voc4cat_0000297>,
        <https://w3id.org/nfdi4cat/voc4cat_0000298>,
        <https://w3id.org/nfdi4cat/voc4cat_0000299>,
        <https://w3id.org/nfdi4cat/voc4cat_0000300>,
        <https://w3id.org/nfdi4cat/voc4cat_0000301>,
        <https://w3id.org/nfdi4cat/voc4cat_0000302>,
        <https://w3id.org/nfdi4cat/voc4cat_0000303>,
        <https://w3id.org/nfdi4cat/voc4cat_0000304>,
        <https://w3id.org/nfdi4cat/voc4cat_0000305>,
        <https://w3id.org/nfdi4cat/voc4cat_0000306>,
        <https://w3id.org/nfdi4cat/voc4cat_0000307>,
        <https://w3id.org/nfdi4cat/voc4cat_0000308>,
        <https://w3id.org/nfdi4cat/voc4cat_0000309>,
        <https://w3id.org/nfdi4cat/voc4cat_0007001>,
        <https://w3id.org/nfdi4cat/voc4cat_0007002>,
        <https://w3id.org/nfdi4cat/voc4cat_0007003>,
        <https://w3id.org/nfdi4cat/voc4cat_0007034> ;
    skos:prefLabel "ChemCatChem keyword collection"@en .

<https://w3id.org/nfdi4cat/voc4cat_0001900> a skos:Collection ;
    dcterms:identifier "voc4cat_0001900"^^xsd:token ;
    dcterms:isPartOf <https://w3id.org/nfdi4cat/voc4cat> ;
    rdfs:isDefinedBy <https://w3id.org/nfdi4cat/voc4cat> ;
    skos:definition "A collection of concepts referring to material  characterization techniques and methods to evaluate their efficiency in photocatalysis."@en ;
    skos:historyNote "0000-0002-6242-2167 Nikolaos G. Moustakas created the resource"@en ;
    skos:inScheme <https://w3id.org/nfdi4cat/voc4cat> ;
    skos:member <https://w3id.org/nfdi4cat/voc4cat_0000067>,
        <https://w3id.org/nfdi4cat/voc4cat_0000068>,
        <https://w3id.org/nfdi4cat/voc4cat_0000069>,
        <https://w3id.org/nfdi4cat/voc4cat_0000070>,
        <https://w3id.org/nfdi4cat/voc4cat_0000071>,
        <https://w3id.org/nfdi4cat/voc4cat_0000072>,
        <https://w3id.org/nfdi4cat/voc4cat_0000073>,
        <https://w3id.org/nfdi4cat/voc4cat_0000074>,
        <https://w3id.org/nfdi4cat/voc4cat_0000075>,
        <https://w3id.org/nfdi4cat/voc4cat_0000076>,
        <https://w3id.org/nfdi4cat/voc4cat_0000077>,
        <https://w3id.org/nfdi4cat/voc4cat_0000078>,
        <https://w3id.org/nfdi4cat/voc4cat_0000079>,
        <https://w3id.org/nfdi4cat/voc4cat_0000080>,
        <https://w3id.org/nfdi4cat/voc4cat_0000081>,
        <https://w3id.org/nfdi4cat/voc4cat_0000082>,
        <https://w3id.org/nfdi4cat/voc4cat_0000083>,
        <https://w3id.org/nfdi4cat/voc4cat_0000130>,
        <https://w3id.org/nfdi4cat/voc4cat_0000137>,
        <https://w3id.org/nfdi4cat/voc4cat_0000141> ;
    skos:prefLabel "Characterization and evaluation techniques"@en .

<https://w3id.org/nfdi4cat/voc4cat_0001901> a skos:Collection ;
    dcterms:identifier "voc4cat_0001901"^^xsd:token ;
    dcterms:isPartOf <https://w3id.org/nfdi4cat/voc4cat> ;
    rdfs:isDefinedBy <https://w3id.org/nfdi4cat/voc4cat> ;
    skos:definition "A collection of concepts referring to photocatalysis."@en ;
    skos:historyNote "0000-0002-6242-2167 Nikolaos G. Moustakas created the collection, 0000-0002-5898-1820 David Linke updated members"@en ;
    skos:inScheme <https://w3id.org/nfdi4cat/voc4cat> ;
    skos:member <https://w3id.org/nfdi4cat/voc4cat_0000001>,
        <https://w3id.org/nfdi4cat/voc4cat_0000002>,
        <https://w3id.org/nfdi4cat/voc4cat_0000003>,
        <https://w3id.org/nfdi4cat/voc4cat_0000004>,
        <https://w3id.org/nfdi4cat/voc4cat_0000005>,
        <https://w3id.org/nfdi4cat/voc4cat_0000006>,
        <https://w3id.org/nfdi4cat/voc4cat_0000007>,
        <https://w3id.org/nfdi4cat/voc4cat_0000008>,
        <https://w3id.org/nfdi4cat/voc4cat_0000009>,
        <https://w3id.org/nfdi4cat/voc4cat_0000010>,
        <https://w3id.org/nfdi4cat/voc4cat_0000011>,
        <https://w3id.org/nfdi4cat/voc4cat_0000012>,
        <https://w3id.org/nfdi4cat/voc4cat_0000013>,
        <https://w3id.org/nfdi4cat/voc4cat_0000014>,
        <https://w3id.org/nfdi4cat/voc4cat_0000015>,
        <https://w3id.org/nfdi4cat/voc4cat_0000017>,
        <https://w3id.org/nfdi4cat/voc4cat_0000018>,
        <https://w3id.org/nfdi4cat/voc4cat_0000020>,
        <https://w3id.org/nfdi4cat/voc4cat_0000021>,
        <https://w3id.org/nfdi4cat/voc4cat_0000022>,
        <https://w3id.org/nfdi4cat/voc4cat_0000023>,
        <https://w3id.org/nfdi4cat/voc4cat_0000024>,
        <https://w3id.org/nfdi4cat/voc4cat_0000025>,
        <https://w3id.org/nfdi4cat/voc4cat_0000026>,
        <https://w3id.org/nfdi4cat/voc4cat_0000027>,
        <https://w3id.org/nfdi4cat/voc4cat_0000028>,
        <https://w3id.org/nfdi4cat/voc4cat_0000029>,
        <https://w3id.org/nfdi4cat/voc4cat_0000030>,
        <https://w3id.org/nfdi4cat/voc4cat_0000031>,
        <https://w3id.org/nfdi4cat/voc4cat_0000032>,
        <https://w3id.org/nfdi4cat/voc4cat_0000033>,
        <https://w3id.org/nfdi4cat/voc4cat_0000034>,
        <https://w3id.org/nfdi4cat/voc4cat_0000035>,
        <https://w3id.org/nfdi4cat/voc4cat_0000036>,
        <https://w3id.org/nfdi4cat/voc4cat_0000037>,
        <https://w3id.org/nfdi4cat/voc4cat_0000038>,
        <https://w3id.org/nfdi4cat/voc4cat_0000039>,
        <https://w3id.org/nfdi4cat/voc4cat_0000040>,
        <https://w3id.org/nfdi4cat/voc4cat_0000041>,
        <https://w3id.org/nfdi4cat/voc4cat_0000042>,
        <https://w3id.org/nfdi4cat/voc4cat_0000043>,
        <https://w3id.org/nfdi4cat/voc4cat_0000044>,
        <https://w3id.org/nfdi4cat/voc4cat_0000045>,
        <https://w3id.org/nfdi4cat/voc4cat_0000046>,
        <https://w3id.org/nfdi4cat/voc4cat_0000047>,
        <https://w3id.org/nfdi4cat/voc4cat_0000048>,
        <https://w3id.org/nfdi4cat/voc4cat_0000049>,
        <https://w3id.org/nfdi4cat/voc4cat_0000050>,
        <https://w3id.org/nfdi4cat/voc4cat_0000051>,
        <https://w3id.org/nfdi4cat/voc4cat_0000052>,
        <https://w3id.org/nfdi4cat/voc4cat_0000053>,
        <https://w3id.org/nfdi4cat/voc4cat_0000054>,
        <https://w3id.org/nfdi4cat/voc4cat_0000055>,
        <https://w3id.org/nfdi4cat/voc4cat_0000056>,
        <https://w3id.org/nfdi4cat/voc4cat_0000057>,
        <https://w3id.org/nfdi4cat/voc4cat_0000058>,
        <https://w3id.org/nfdi4cat/voc4cat_0000059>,
        <https://w3id.org/nfdi4cat/voc4cat_0000060>,
        <https://w3id.org/nfdi4cat/voc4cat_0000061>,
        <https://w3id.org/nfdi4cat/voc4cat_0000062>,
        <https://w3id.org/nfdi4cat/voc4cat_0000063>,
        <https://w3id.org/nfdi4cat/voc4cat_0000064>,
        <https://w3id.org/nfdi4cat/voc4cat_0000065>,
        <https://w3id.org/nfdi4cat/voc4cat_0000066>,
        <https://w3id.org/nfdi4cat/voc4cat_0000067>,
        <https://w3id.org/nfdi4cat/voc4cat_0000068>,
        <https://w3id.org/nfdi4cat/voc4cat_0000069>,
        <https://w3id.org/nfdi4cat/voc4cat_0000070>,
        <https://w3id.org/nfdi4cat/voc4cat_0000071>,
        <https://w3id.org/nfdi4cat/voc4cat_0000072>,
        <https://w3id.org/nfdi4cat/voc4cat_0000073>,
        <https://w3id.org/nfdi4cat/voc4cat_0000074>,
        <https://w3id.org/nfdi4cat/voc4cat_0000075>,
        <https://w3id.org/nfdi4cat/voc4cat_0000076>,
        <https://w3id.org/nfdi4cat/voc4cat_0000077>,
        <https://w3id.org/nfdi4cat/voc4cat_0000078>,
        <https://w3id.org/nfdi4cat/voc4cat_0000079>,
        <https://w3id.org/nfdi4cat/voc4cat_0000080>,
        <https://w3id.org/nfdi4cat/voc4cat_0000081>,
        <https://w3id.org/nfdi4cat/voc4cat_0000082>,
        <https://w3id.org/nfdi4cat/voc4cat_0000083>,
        <https://w3id.org/nfdi4cat/voc4cat_0000084>,
        <https://w3id.org/nfdi4cat/voc4cat_0000085>,
        <https://w3id.org/nfdi4cat/voc4cat_0000086>,
        <https://w3id.org/nfdi4cat/voc4cat_0000087>,
        <https://w3id.org/nfdi4cat/voc4cat_0000088>,
        <https://w3id.org/nfdi4cat/voc4cat_0000089>,
        <https://w3id.org/nfdi4cat/voc4cat_0000090>,
        <https://w3id.org/nfdi4cat/voc4cat_0000091>,
        <https://w3id.org/nfdi4cat/voc4cat_0000092>,
        <https://w3id.org/nfdi4cat/voc4cat_0000093>,
        <https://w3id.org/nfdi4cat/voc4cat_0000094>,
        <https://w3id.org/nfdi4cat/voc4cat_0000095>,
        <https://w3id.org/nfdi4cat/voc4cat_0000096>,
        <https://w3id.org/nfdi4cat/voc4cat_0000097>,
        <https://w3id.org/nfdi4cat/voc4cat_0000098>,
        <https://w3id.org/nfdi4cat/voc4cat_0000099>,
        <https://w3id.org/nfdi4cat/voc4cat_0000100>,
        <https://w3id.org/nfdi4cat/voc4cat_0000101>,
        <https://w3id.org/nfdi4cat/voc4cat_0000102>,
        <https://w3id.org/nfdi4cat/voc4cat_0000103>,
        <https://w3id.org/nfdi4cat/voc4cat_0000104>,
        <https://w3id.org/nfdi4cat/voc4cat_0000105>,
        <https://w3id.org/nfdi4cat/voc4cat_0000106>,
        <https://w3id.org/nfdi4cat/voc4cat_0000107>,
        <https://w3id.org/nfdi4cat/voc4cat_0000108>,
        <https://w3id.org/nfdi4cat/voc4cat_0000109>,
        <https://w3id.org/nfdi4cat/voc4cat_0000110>,
        <https://w3id.org/nfdi4cat/voc4cat_0000111>,
        <https://w3id.org/nfdi4cat/voc4cat_0000112>,
        <https://w3id.org/nfdi4cat/voc4cat_0000113>,
        <https://w3id.org/nfdi4cat/voc4cat_0000114>,
        <https://w3id.org/nfdi4cat/voc4cat_0000115>,
        <https://w3id.org/nfdi4cat/voc4cat_0000116>,
        <https://w3id.org/nfdi4cat/voc4cat_0000117>,
        <https://w3id.org/nfdi4cat/voc4cat_0000118>,
        <https://w3id.org/nfdi4cat/voc4cat_0000119>,
        <https://w3id.org/nfdi4cat/voc4cat_0000120>,
        <https://w3id.org/nfdi4cat/voc4cat_0000121>,
        <https://w3id.org/nfdi4cat/voc4cat_0000122>,
        <https://w3id.org/nfdi4cat/voc4cat_0000123>,
        <https://w3id.org/nfdi4cat/voc4cat_0000124>,
        <https://w3id.org/nfdi4cat/voc4cat_0000126>,
        <https://w3id.org/nfdi4cat/voc4cat_0000127>,
        <https://w3id.org/nfdi4cat/voc4cat_0000128>,
        <https://w3id.org/nfdi4cat/voc4cat_0000129>,
        <https://w3id.org/nfdi4cat/voc4cat_0000130>,
        <https://w3id.org/nfdi4cat/voc4cat_0000131>,
        <https://w3id.org/nfdi4cat/voc4cat_0000132>,
        <https://w3id.org/nfdi4cat/voc4cat_0000133>,
        <https://w3id.org/nfdi4cat/voc4cat_0000134>,
        <https://w3id.org/nfdi4cat/voc4cat_0000135>,
        <https://w3id.org/nfdi4cat/voc4cat_0000136>,
        <https://w3id.org/nfdi4cat/voc4cat_0000137>,
        <https://w3id.org/nfdi4cat/voc4cat_0000138>,
        <https://w3id.org/nfdi4cat/voc4cat_0000139>,
        <https://w3id.org/nfdi4cat/voc4cat_0000140>,
        <https://w3id.org/nfdi4cat/voc4cat_0000141>,
        <https://w3id.org/nfdi4cat/voc4cat_0000142>,
        <https://w3id.org/nfdi4cat/voc4cat_0000143>,
        <https://w3id.org/nfdi4cat/voc4cat_0000144>,
        <https://w3id.org/nfdi4cat/voc4cat_0000145>,
        <https://w3id.org/nfdi4cat/voc4cat_0000146>,
        <https://w3id.org/nfdi4cat/voc4cat_0000147>,
        <https://w3id.org/nfdi4cat/voc4cat_0000148>,
        <https://w3id.org/nfdi4cat/voc4cat_0000149>,
        <https://w3id.org/nfdi4cat/voc4cat_0000150>,
        <https://w3id.org/nfdi4cat/voc4cat_0000151>,
        <https://w3id.org/nfdi4cat/voc4cat_0000152>,
        <https://w3id.org/nfdi4cat/voc4cat_0000153>,
        <https://w3id.org/nfdi4cat/voc4cat_0000154>,
        <https://w3id.org/nfdi4cat/voc4cat_0000155>,
        <https://w3id.org/nfdi4cat/voc4cat_0000156>,
        <https://w3id.org/nfdi4cat/voc4cat_0000157>,
        <https://w3id.org/nfdi4cat/voc4cat_0000158>,
        <https://w3id.org/nfdi4cat/voc4cat_0000159>,
        <https://w3id.org/nfdi4cat/voc4cat_0000160>,
        <https://w3id.org/nfdi4cat/voc4cat_0000161>,
        <https://w3id.org/nfdi4cat/voc4cat_0000162>,
        <https://w3id.org/nfdi4cat/voc4cat_0000163>,
        <https://w3id.org/nfdi4cat/voc4cat_0000164>,
        <https://w3id.org/nfdi4cat/voc4cat_0000165>,
        <https://w3id.org/nfdi4cat/voc4cat_0000166>,
        <https://w3id.org/nfdi4cat/voc4cat_0000167>,
        <https://w3id.org/nfdi4cat/voc4cat_0000168>,
        <https://w3id.org/nfdi4cat/voc4cat_0000169>,
        <https://w3id.org/nfdi4cat/voc4cat_0000170>,
        <https://w3id.org/nfdi4cat/voc4cat_0000171>,
        <https://w3id.org/nfdi4cat/voc4cat_0000172>,
        <https://w3id.org/nfdi4cat/voc4cat_0000173>,
        <https://w3id.org/nfdi4cat/voc4cat_0000174>,
        <https://w3id.org/nfdi4cat/voc4cat_0000175>,
        <https://w3id.org/nfdi4cat/voc4cat_0000176>,
        <https://w3id.org/nfdi4cat/voc4cat_0000177>,
        <https://w3id.org/nfdi4cat/voc4cat_0000178>,
        <https://w3id.org/nfdi4cat/voc4cat_0000179> ;
    skos:prefLabel "Photocatalysis collection"@en .

<https://w3id.org/nfdi4cat/voc4cat_0005007> a skos:Concept ;
    dcterms:identifier "voc4cat_0005007"^^xsd:token ;
    skos:broader <https://w3id.org/nfdi4cat/voc4cat_0000186> ;
    skos:definition "Describes a transformation that changes the chemical composition of involved materials."@en ;
    skos:historyNote "0000-0002-5898-1820 David Linke created the resource"@en ;
    skos:inScheme <https://w3id.org/nfdi4cat/voc4cat> ;
    skos:prefLabel "chemical conversion"@en .

<https://w3id.org/nfdi4cat/voc4cat_0005008> a skos:Concept ;
    dcterms:identifier "voc4cat_0005008"^^xsd:token ;
    skos:broader <https://w3id.org/nfdi4cat/voc4cat_0000186> ;
    skos:definition "A quantity describing the progress of a chemical reaction. For any chemical entitiy taking part in the reaction it is defined by the amount of chemical entity formed devided by its stoichiometric number in the reaction."@en ;
    skos:historyNote "0000-0002-5898-1820 David Linke created the resource, 0000-0002-4041-0165 Julia Schumann modified the resource"@en ;
    skos:inScheme <https://w3id.org/nfdi4cat/voc4cat> ;
    skos:prefLabel "extent of reaction"@en .

<https://w3id.org/nfdi4cat/voc4cat_0005009> a skos:Concept ;
    dcterms:identifier "voc4cat_0005009"^^xsd:token ;
    skos:altLabel "formation rate"@en ;
    skos:broader <https://w3id.org/nfdi4cat/voc4cat_0000186> ;
    skos:definition "Is a quantity describing how fast a product is formed in a chemical reaction. It is defined by the amount of product formed per unit of time."@en ;
    skos:historyNote "0000-0002-5898-1820 David Linke created the resource"@en ;
    skos:inScheme <https://w3id.org/nfdi4cat/voc4cat> ;
    skos:prefLabel "rate of formation"@en .

<https://w3id.org/nfdi4cat/voc4cat_0005010> a skos:Concept ;
    dcterms:identifier "voc4cat_0005010"^^xsd:token ;
    skos:altLabel "consumption rate"@en ;
    skos:broader <https://w3id.org/nfdi4cat/voc4cat_0000186> ;
    skos:definition "Is a quantity describing how fast a reactant is consumed in a chemical reaction. It is defined by the amount of reactant consumed per unit of time."@en ;
    skos:historyNote "0000-0002-5898-1820 David Linke created the resource"@en ;
    skos:inScheme <https://w3id.org/nfdi4cat/voc4cat> ;
    skos:prefLabel "rate of consumption"@en .

<https://w3id.org/nfdi4cat/voc4cat_0005012> a skos:Concept ;
    dcterms:identifier "voc4cat_0005012"^^xsd:token ;
    skos:broader <https://w3id.org/nfdi4cat/voc4cat_0005011> ;
    skos:definition "A PID resource category for a collection, which is a group of resources and/or other collections."@en ;
    skos:historyNote "0000-0002-5898-1820 David Linke created the resource"@en ;
    skos:inScheme <https://w3id.org/nfdi4cat/voc4cat> ;
    skos:prefLabel "collection"@en .

<https://w3id.org/nfdi4cat/voc4cat_0005013> a skos:Concept ;
    dcterms:identifier "voc4cat_0005013"^^xsd:token ;
    skos:broader <https://w3id.org/nfdi4cat/voc4cat_0005011> ;
    skos:definition "A PID resource category for a material sample ([voc4cat:0005056](https://w3id.org/nfdi4cat/voc4cat_0005056))."@en ;
    skos:historyNote "0000-0002-5898-1820 David Linke created the resource"@en ;
    skos:inScheme <https://w3id.org/nfdi4cat/voc4cat> ;
    skos:prefLabel "sample"@en .

<https://w3id.org/nfdi4cat/voc4cat_0005014> a skos:Concept ;
    dcterms:identifier "voc4cat_0005014"^^xsd:token ;
    skos:broader <https://w3id.org/nfdi4cat/voc4cat_0005011> ;
    skos:definition "A PID resource category for a material used in the research process. Note that in the PID resource categorization, a \"material\" is distinct from \"sample\" ([voc4cat:0005013](https://w3id.org/nfdi4cat/voc4cat_0005013)) and distinct from \"device\" ([voc4cat:0005015](https://w3id.org/nfdi4cat/voc4cat_0005015)) ."@en ;
    skos:historyNote "0000-0002-5898-1820 David Linke created the resource"@en ;
    skos:inScheme <https://w3id.org/nfdi4cat/voc4cat> ;
    skos:prefLabel "material"@en .

<https://w3id.org/nfdi4cat/voc4cat_0005015> a skos:Concept ;
    dcterms:identifier "voc4cat_0005015"^^xsd:token ;
    skos:broader <https://w3id.org/nfdi4cat/voc4cat_0005011> ;
    skos:definition "A PID resource category for a physical device used in a research or manufacturing process."@en ;
    skos:historyNote "0000-0002-5898-1820 David Linke created the resource"@en ;
    skos:inScheme <https://w3id.org/nfdi4cat/voc4cat> ;
    skos:prefLabel "device"@en .

<https://w3id.org/nfdi4cat/voc4cat_0005016> a skos:Concept ;
    dcterms:identifier "voc4cat_0005016"^^xsd:token ;
    skos:broader <https://w3id.org/nfdi4cat/voc4cat_0005011> ;
    skos:definition "A PID resource category for a collection of data available for access or download. A data object might be a data file, a data set, a data collection."@en ;
    skos:historyNote "0000-0002-5898-1820 David Linke created the resource"@en ;
    skos:inScheme <https://w3id.org/nfdi4cat/voc4cat> ;
    skos:prefLabel "data object"@en .

<https://w3id.org/nfdi4cat/voc4cat_0005017> a skos:Concept ;
    dcterms:identifier "voc4cat_0005017"^^xsd:token ;
    skos:broader <https://w3id.org/nfdi4cat/voc4cat_0005011> ;
    skos:definition "A PID resource category for a data service, which is an organized system of operations that provide data processing functions or access to datasets."@en ;
    skos:historyNote "0000-0002-5898-1820 David Linke created the resource"@en ;
    skos:inScheme <https://w3id.org/nfdi4cat/voc4cat> ;
    skos:prefLabel "data service"@en .

<https://w3id.org/nfdi4cat/voc4cat_0005019> a skos:Concept ;
    dcterms:identifier "voc4cat_0005019"^^xsd:token ;
    skos:broader <https://w3id.org/nfdi4cat/voc4cat_0005018> ;
    skos:definition "The resource is cited by another resource."@en ;
    skos:historyNote "0000-0002-5898-1820 David Linke created the resource"@en ;
    skos:inScheme <https://w3id.org/nfdi4cat/voc4cat> ;
    skos:prefLabel "is cited by"@en .

<https://w3id.org/nfdi4cat/voc4cat_0005020> a skos:Concept ;
    dcterms:identifier "voc4cat_0005020"^^xsd:token ;
    skos:broader <https://w3id.org/nfdi4cat/voc4cat_0005018> ;
    skos:definition "The resource cites another resource."@en ;
    skos:historyNote "0000-0002-5898-1820 David Linke created the resource"@en ;
    skos:inScheme <https://w3id.org/nfdi4cat/voc4cat> ;
    skos:prefLabel "cites"@en .

<https://w3id.org/nfdi4cat/voc4cat_0005021> a skos:Concept ;
    dcterms:identifier "voc4cat_0005021"^^xsd:token ;
    skos:broader <https://w3id.org/nfdi4cat/voc4cat_0005018> ;
    skos:definition "The resource is supplemented by another resource."@en ;
    skos:historyNote "0000-0002-5898-1820 David Linke created the resource"@en ;
    skos:inScheme <https://w3id.org/nfdi4cat/voc4cat> ;
    skos:prefLabel "is supplement to"@en .

<https://w3id.org/nfdi4cat/voc4cat_0005022> a skos:Concept ;
    dcterms:identifier "voc4cat_0005022"^^xsd:token ;
    skos:broader <https://w3id.org/nfdi4cat/voc4cat_0005018> ;
    skos:definition "The resource supplements another resource."@en ;
    skos:historyNote "0000-0002-5898-1820 David Linke created the resource"@en ;
    skos:inScheme <https://w3id.org/nfdi4cat/voc4cat> ;
    skos:prefLabel "is supplemented by"@en .

<https://w3id.org/nfdi4cat/voc4cat_0005023> a skos:Concept ;
    dcterms:identifier "voc4cat_0005023"^^xsd:token ;
    skos:broader <https://w3id.org/nfdi4cat/voc4cat_0005018> ;
    skos:definition "The resource is continued by another resource."@en ;
    skos:historyNote "0000-0002-5898-1820 David Linke created the resource"@en ;
    skos:inScheme <https://w3id.org/nfdi4cat/voc4cat> ;
    skos:prefLabel "is continued by"@en .

<https://w3id.org/nfdi4cat/voc4cat_0005024> a skos:Concept ;
    dcterms:identifier "voc4cat_0005024"^^xsd:token ;
    skos:broader <https://w3id.org/nfdi4cat/voc4cat_0005018> ;
    skos:definition "The resource continues another resource."@en ;
    skos:historyNote "0000-0002-5898-1820 David Linke created the resource"@en ;
    skos:inScheme <https://w3id.org/nfdi4cat/voc4cat> ;
    skos:prefLabel "continues"@en .

<https://w3id.org/nfdi4cat/voc4cat_0005025> a skos:Concept ;
    dcterms:identifier "voc4cat_0005025"^^xsd:token ;
    skos:broader <https://w3id.org/nfdi4cat/voc4cat_0005018> ;
    skos:definition "The resource has metadata in another resource."@en ;
    skos:historyNote "0000-0002-5898-1820 David Linke created the resource"@en ;
    skos:inScheme <https://w3id.org/nfdi4cat/voc4cat> ;
    skos:prefLabel "has metadata"@en .

<https://w3id.org/nfdi4cat/voc4cat_0005026> a skos:Concept ;
    dcterms:identifier "voc4cat_0005026"^^xsd:token ;
    skos:broader <https://w3id.org/nfdi4cat/voc4cat_0005018> ;
    skos:definition "The resource is metadata for another resource."@en ;
    skos:historyNote "0000-0002-5898-1820 David Linke created the resource"@en ;
    skos:inScheme <https://w3id.org/nfdi4cat/voc4cat> ;
    skos:prefLabel "is metadata for"@en .

<https://w3id.org/nfdi4cat/voc4cat_0005027> a skos:Concept ;
    dcterms:identifier "voc4cat_0005027"^^xsd:token ;
    skos:broader <https://w3id.org/nfdi4cat/voc4cat_0005018> ;
    skos:definition "The resource has a version. This is useful to refer to different versions of an abstract resource, for example, \"Python has version Python 3.12.4\"."@en ;
    skos:historyNote "0000-0002-5898-1820 David Linke created the resource"@en ;
    skos:inScheme <https://w3id.org/nfdi4cat/voc4cat> ;
    skos:prefLabel "has version"@en .

<https://w3id.org/nfdi4cat/voc4cat_0005028> a skos:Concept ;
    dcterms:identifier "voc4cat_0005028"^^xsd:token ;
    skos:broader <https://w3id.org/nfdi4cat/voc4cat_0005018> ;
    skos:definition "The resource is a version of another resource. This is useful to refer to an abstract resource that has different versions, for example, \"Python 3.12.4 is version of Python\"."@en ;
    skos:historyNote "0000-0002-5898-1820 David Linke created the resource"@en ;
    skos:inScheme <https://w3id.org/nfdi4cat/voc4cat> ;
    skos:prefLabel "is version of"@en .

<https://w3id.org/nfdi4cat/voc4cat_0005029> a skos:Concept ;
    dcterms:identifier "voc4cat_0005029"^^xsd:token ;
    skos:broader <https://w3id.org/nfdi4cat/voc4cat_0005018> ;
    skos:definition "The resource is a new version of another versioned resource. This is useful to refer between versioned resources, for example, \"Python 3.12.1 is_new_version_of Python 3.12.0\"."@en ;
    skos:historyNote "0000-0002-5898-1820 David Linke created the resource"@en ;
    skos:inScheme <https://w3id.org/nfdi4cat/voc4cat> ;
    skos:prefLabel "is new version of"@en .

<https://w3id.org/nfdi4cat/voc4cat_0005030> a skos:Concept ;
    dcterms:identifier "voc4cat_0005030"^^xsd:token ;
    skos:broader <https://w3id.org/nfdi4cat/voc4cat_0005018> ;
    skos:definition "The resource is a previous version of another versioned resource. This is useful to refer between versioned resources, for example, \"Python 3.12.0 is_previous_version_of Python 3.12.1\"."@en ;
    skos:historyNote "0000-0002-5898-1820 David Linke created the resource"@en ;
    skos:inScheme <https://w3id.org/nfdi4cat/voc4cat> ;
    skos:prefLabel "is previous version of"@en .

<https://w3id.org/nfdi4cat/voc4cat_0005031> a skos:Concept ;
    dcterms:identifier "voc4cat_0005031"^^xsd:token ;
    skos:broader <https://w3id.org/nfdi4cat/voc4cat_0005018> ;
    skos:definition """The resource is part of another resource. This relation applies to container-contained type relationships.
If the relation refers to publishing one resource as part of another resource, use "IS_PUBLISHED_IN" instead. If the relation refers to a versioned resource and non-versioned resource, use "IS_VERSION_OF" instead."""@en ;
    skos:historyNote "0000-0002-5898-1820 David Linke created the resource"@en ;
    skos:inScheme <https://w3id.org/nfdi4cat/voc4cat> ;
    skos:prefLabel "is part of"@en .

<https://w3id.org/nfdi4cat/voc4cat_0005032> a skos:Concept ;
    dcterms:identifier "voc4cat_0005032"^^xsd:token ;
    skos:broader <https://w3id.org/nfdi4cat/voc4cat_0005018> ;
    skos:definition """The resource has part another resource. This relation applies to container-contained type relationships.
If the relation refers to publishing one resource as part of another resource, "IS_PUBLISHED_IN" instead. If the relation refers to a versioned resource and non-versioned resource, use "HAS_VERSION" instead."""@en ;
    skos:historyNote "0000-0002-5898-1820 David Linke created the resource"@en ;
    skos:inScheme <https://w3id.org/nfdi4cat/voc4cat> ;
    skos:prefLabel "has part"@en .

<https://w3id.org/nfdi4cat/voc4cat_0005033> a skos:Concept ;
    dcterms:identifier "voc4cat_0005033"^^xsd:token ;
    skos:broader <https://w3id.org/nfdi4cat/voc4cat_0005018> ;
    skos:definition """The resource is published in another resource.
A resource A that is_published_in a resource B is independent from other resources published in the same resource B."""@en ;
    skos:historyNote "0000-0002-5898-1820 David Linke created the resource"@en ;
    skos:inScheme <https://w3id.org/nfdi4cat/voc4cat> ;
    skos:prefLabel "is published in"@en .

<https://w3id.org/nfdi4cat/voc4cat_0005034> a skos:Concept ;
    dcterms:identifier "voc4cat_0005034"^^xsd:token ;
    skos:broader <https://w3id.org/nfdi4cat/voc4cat_0005018> ;
    skos:definition "The resource is referenced by another resource."@en ;
    skos:historyNote "0000-0002-5898-1820 David Linke created the resource"@en ;
    skos:inScheme <https://w3id.org/nfdi4cat/voc4cat> ;
    skos:prefLabel "is referenced by"@en .

<https://w3id.org/nfdi4cat/voc4cat_0005035> a skos:Concept ;
    dcterms:identifier "voc4cat_0005035"^^xsd:token ;
    skos:broader <https://w3id.org/nfdi4cat/voc4cat_0005018> ;
    skos:definition "The resource references another resource."@en ;
    skos:historyNote "0000-0002-5898-1820 David Linke created the resource"@en ;
    skos:inScheme <https://w3id.org/nfdi4cat/voc4cat> ;
    skos:prefLabel "references"@en .

<https://w3id.org/nfdi4cat/voc4cat_0005036> a skos:Concept ;
    dcterms:identifier "voc4cat_0005036"^^xsd:token ;
    skos:broader <https://w3id.org/nfdi4cat/voc4cat_0005018> ;
    skos:definition "The resource is documented by another resource."@en ;
    skos:historyNote "0000-0002-5898-1820 David Linke created the resource"@en ;
    skos:inScheme <https://w3id.org/nfdi4cat/voc4cat> ;
    skos:prefLabel "is documented by"@en .

<https://w3id.org/nfdi4cat/voc4cat_0005037> a skos:Concept ;
    dcterms:identifier "voc4cat_0005037"^^xsd:token ;
    skos:broader <https://w3id.org/nfdi4cat/voc4cat_0005018> ;
    skos:definition "The resource documents another resource."@en ;
    skos:historyNote "0000-0002-5898-1820 David Linke created the resource"@en ;
    skos:inScheme <https://w3id.org/nfdi4cat/voc4cat> ;
    skos:prefLabel "documents"@en .

<https://w3id.org/nfdi4cat/voc4cat_0005038> a skos:Concept ;
    dcterms:identifier "voc4cat_0005038"^^xsd:token ;
    skos:broader <https://w3id.org/nfdi4cat/voc4cat_0005018> ;
    skos:definition "The resource is compiled by another resource. Resources may be text or software. The compiler may be a computer program or a person."@en ;
    skos:historyNote "0000-0002-5898-1820 David Linke created the resource"@en ;
    skos:inScheme <https://w3id.org/nfdi4cat/voc4cat> ;
    skos:prefLabel "is compiled by"@en .

<https://w3id.org/nfdi4cat/voc4cat_0005039> a skos:Concept ;
    dcterms:identifier "voc4cat_0005039"^^xsd:token ;
    skos:broader <https://w3id.org/nfdi4cat/voc4cat_0005018> ;
    skos:definition "The resource compiles another resource. Resources may be text or software. The compiler may be a computer program or a person."@en ;
    skos:historyNote "0000-0002-5898-1820 David Linke created the resource"@en ;
    skos:inScheme <https://w3id.org/nfdi4cat/voc4cat> ;
    skos:prefLabel "compiles"@en .

<https://w3id.org/nfdi4cat/voc4cat_0005040> a skos:Concept ;
    dcterms:identifier "voc4cat_0005040"^^xsd:token ;
    skos:broader <https://w3id.org/nfdi4cat/voc4cat_0005018> ;
    skos:definition "The resource is variant form of another resource. This may be used e.g. for relating architecture-specific builds of a software program to a source-code release. It may also be used to express the relation between data in different formats (e.g. PNG, JPEG) of the same image."@en ;
    skos:historyNote "0000-0002-5898-1820 David Linke created the resource"@en ;
    skos:inScheme <https://w3id.org/nfdi4cat/voc4cat> ;
    skos:prefLabel "is variant form of"@en .

<https://w3id.org/nfdi4cat/voc4cat_0005041> a skos:Concept ;
    dcterms:identifier "voc4cat_0005041"^^xsd:token ;
    skos:broader <https://w3id.org/nfdi4cat/voc4cat_0005018> ;
    skos:definition "The resource is original form of another resource. This may be used e.g. for relating architecture-specific builds of a software program to a source-code release. It may also be used to express the relation between data in different formats (e.g. PNG, JPEG) of the same image."@en ;
    skos:historyNote "0000-0002-5898-1820 David Linke created the resource"@en ;
    skos:inScheme <https://w3id.org/nfdi4cat/voc4cat> ;
    skos:prefLabel "is original form of"@en .

<https://w3id.org/nfdi4cat/voc4cat_0005042> a skos:Concept ;
    dcterms:identifier "voc4cat_0005042"^^xsd:token ;
    skos:broader <https://w3id.org/nfdi4cat/voc4cat_0005018> ;
    skos:definition "The resource is identical to another resource. May be used to indicate the relationship between an exact copy of a resource that is published at another location."@en ;
    skos:historyNote "0000-0002-5898-1820 David Linke created the resource"@en ;
    skos:inScheme <https://w3id.org/nfdi4cat/voc4cat> ;
    skos:prefLabel "is identical to"@en .

<https://w3id.org/nfdi4cat/voc4cat_0005043> a skos:Concept ;
    dcterms:identifier "voc4cat_0005043"^^xsd:token ;
    skos:broader <https://w3id.org/nfdi4cat/voc4cat_0005018> ;
    skos:definition "The resource is derived from another resource. This may be used for relating a new dataset created by data processing to its original source dataset. For samples it may express the relation between the original sample and another sample derived from it by physical or chemical treatment."@en ;
    skos:historyNote "0000-0002-5898-1820 David Linke created the resource"@en ;
    skos:inScheme <https://w3id.org/nfdi4cat/voc4cat> ;
    skos:prefLabel "is derived from"@en .

<https://w3id.org/nfdi4cat/voc4cat_0005044> a skos:Concept ;
    dcterms:identifier "voc4cat_0005044"^^xsd:token ;
    skos:broader <https://w3id.org/nfdi4cat/voc4cat_0005018> ;
    skos:definition "The resource is source of another resource. This may be used for example to express the relation between a source dataset and a new dataset derived from it by data processing. For samples it may express the relation between a sample processed by physical or chemical treatment and the original sample."@en ;
    skos:historyNote "0000-0002-5898-1820 David Linke created the resource"@en ;
    skos:inScheme <https://w3id.org/nfdi4cat/voc4cat> ;
    skos:prefLabel "is source of"@en .

<https://w3id.org/nfdi4cat/voc4cat_0005045> a skos:Concept ;
    dcterms:identifier "voc4cat_0005045"^^xsd:token ;
    skos:broader <https://w3id.org/nfdi4cat/voc4cat_0005018> ;
    skos:definition "The resource is collected by another resource. May be used to indicate the relationship between a dataset and an instrument that is used to collect, measure, obtain, or observe data."@en ;
    skos:historyNote "0000-0002-5898-1820 David Linke created the resource"@en ;
    skos:inScheme <https://w3id.org/nfdi4cat/voc4cat> ;
    skos:prefLabel "is collected by"@en .

<https://w3id.org/nfdi4cat/voc4cat_0005046> a skos:Concept ;
    dcterms:identifier "voc4cat_0005046"^^xsd:token ;
    skos:broader <https://w3id.org/nfdi4cat/voc4cat_0005018> ;
    skos:definition """The resource collects another resource. May be used to indicate the relationship between an instrument and
where it has been used to collect, measure, obtain, or observe data."""@en ;
    skos:historyNote "0000-0002-5898-1820 David Linke created the resource"@en ;
    skos:inScheme <https://w3id.org/nfdi4cat/voc4cat> ;
    skos:prefLabel "collects"@en .

<https://w3id.org/nfdi4cat/voc4cat_0005047> a skos:Concept ;
    dcterms:identifier "voc4cat_0005047"^^xsd:token ;
    skos:broader <https://w3id.org/nfdi4cat/voc4cat_0005018> ;
    skos:definition "The resource is required by another resource."@en ;
    skos:historyNote "0000-0002-5898-1820 David Linke created the resource"@en ;
    skos:inScheme <https://w3id.org/nfdi4cat/voc4cat> ;
    skos:prefLabel "is required by"@en .

<https://w3id.org/nfdi4cat/voc4cat_0005048> a skos:Concept ;
    dcterms:identifier "voc4cat_0005048"^^xsd:token ;
    skos:broader <https://w3id.org/nfdi4cat/voc4cat_0005018> ;
    skos:definition "The resource requires another resource."@en ;
    skos:historyNote "0000-0002-5898-1820 David Linke created the resource"@en ;
    skos:inScheme <https://w3id.org/nfdi4cat/voc4cat> ;
    skos:prefLabel "requires"@en .

<https://w3id.org/nfdi4cat/voc4cat_0005049> a skos:Concept ;
    dcterms:identifier "voc4cat_0005049"^^xsd:token ;
    skos:broader <https://w3id.org/nfdi4cat/voc4cat_0005018> ;
    skos:definition "The resource is obsoleted by another resource."@en ;
    skos:historyNote "0000-0002-5898-1820 David Linke created the resource"@en ;
    skos:inScheme <https://w3id.org/nfdi4cat/voc4cat> ;
    skos:prefLabel "is obsoleted by"@en .

<https://w3id.org/nfdi4cat/voc4cat_0005050> a skos:Concept ;
    dcterms:identifier "voc4cat_0005050"^^xsd:token ;
    skos:broader <https://w3id.org/nfdi4cat/voc4cat_0005018> ;
    skos:definition "The resource obsoletes another resource."@en ;
    skos:historyNote "0000-0002-5898-1820 David Linke created the resource"@en ;
    skos:inScheme <https://w3id.org/nfdi4cat/voc4cat> ;
    skos:prefLabel "obsoletes"@en .

<https://w3id.org/nfdi4cat/voc4cat_0005052> a skos:Concept ;
    dcterms:identifier "voc4cat_0005052"^^xsd:token ;
    skos:broader <https://w3id.org/nfdi4cat/voc4cat_0005051> ;
    skos:definition "The persistent identifier is reserved but the resource is not yet linked."@en ;
    skos:historyNote "0000-0002-5898-1820 David Linke created the resource"@en ;
    skos:inScheme <https://w3id.org/nfdi4cat/voc4cat> ;
    skos:prefLabel "submitted"@en .

<https://w3id.org/nfdi4cat/voc4cat_0005053> a skos:Concept ;
    dcterms:identifier "voc4cat_0005053"^^xsd:token ;
    skos:broader <https://w3id.org/nfdi4cat/voc4cat_0005051> ;
    skos:definition "The persistent identifier is linked to a concrete resource."@en ;
    skos:historyNote "0000-0002-5898-1820 David Linke created the resource"@en ;
    skos:inScheme <https://w3id.org/nfdi4cat/voc4cat> ;
    skos:prefLabel "registered"@en .

<https://w3id.org/nfdi4cat/voc4cat_0005054> a skos:Concept ;
    dcterms:identifier "voc4cat_0005054"^^xsd:token ;
    skos:broader <https://w3id.org/nfdi4cat/voc4cat_0005051> ;
    skos:definition "The persistent identifier is obsolete, e.g. because the resource is referenced by another persistent identifier."@en ;
    skos:historyNote "0000-0002-5898-1820 David Linke created the resource"@en ;
    skos:inScheme <https://w3id.org/nfdi4cat/voc4cat> ;
    skos:prefLabel "obsoleted"@en .

<https://w3id.org/nfdi4cat/voc4cat_0005055> a skos:Concept ;
    dcterms:identifier "voc4cat_0005055"^^xsd:token ;
    skos:broader <https://w3id.org/nfdi4cat/voc4cat_0005051> ;
    skos:definition "The persistent identifier is deprecated, e.g. because the resource can no longer be found."@en ;
    skos:historyNote "0000-0002-5898-1820 David Linke created the resource"@en ;
    skos:inScheme <https://w3id.org/nfdi4cat/voc4cat> ;
    skos:prefLabel "deprecated"@en .

<https://w3id.org/nfdi4cat/voc4cat_0005056> a skos:Concept ;
    dcterms:identifier "voc4cat_0005056"^^xsd:token ;
    skos:altLabel "specimen"@en ;
    skos:broadMatch <https://www.w3.org/ns/sosa/Sample> ;
    skos:broader <https://w3id.org/nfdi4cat/voc4cat_0000190> ;
    skos:definition "A representative part of a material of interest on which observations are made."@en ;
    skos:historyNote "0000-0002-5898-1820 David Linke created the resource"@en ;
    skos:inScheme <https://w3id.org/nfdi4cat/voc4cat> ;
    skos:prefLabel "material sample"@en .

<https://w3id.org/nfdi4cat/voc4cat_0005057> a skos:Concept ;
    dcterms:identifier "voc4cat_0005057"^^xsd:token ;
    skos:broadMatch <https://www.w3.org/ns/sosa/Sample> ;
    skos:broader <https://w3id.org/nfdi4cat/voc4cat_0000182> ;
    skos:definition "A representative part of an entity of interest on which observations are made and which is created by time-based or spatial selection. It may have a lower dimension than the entity of interest. For example, an image may be a spatio-temporal sample of a 3D object."@en ;
    skos:historyNote "0000-0002-5898-1820 David Linke created the resource"@en ;
    skos:inScheme <https://w3id.org/nfdi4cat/voc4cat> ;
    skos:prefLabel "spatio-temporal sample"@en .

<https://w3id.org/nfdi4cat/voc4cat_0005058> a skos:Concept ;
    dcterms:identifier "voc4cat_0005058"^^xsd:token ;
    skos:broadMatch <https://www.w3.org/ns/sosa/Sample> ;
    skos:broader <https://w3id.org/nfdi4cat/voc4cat_0000181> ;
    skos:definition "A representative part of an entity of interest on which observations are made and which is created by statistical sampling or subset selection."@en ;
    skos:historyNote "0000-0002-5898-1820 David Linke created the resource"@en ;
    skos:inScheme <https://w3id.org/nfdi4cat/voc4cat> ;
    skos:prefLabel "statistical sample"@en .

<https://w3id.org/nfdi4cat/voc4cat_0005059> a skos:Concept ;
    dcterms:identifier "voc4cat_0005059"^^xsd:token ;
    skos:broader <https://w3id.org/nfdi4cat/voc4cat_0005018> ;
    skos:definition "An established standard to which the described resource conforms. This relation should be used to indicate the model, schema, ontology, or profile that the resource content conforms to."@en ;
    skos:historyNote "0000-0002-5898-1820 David Linke created the resource"@en ;
    skos:inScheme <https://w3id.org/nfdi4cat/voc4cat> ;
    skos:prefLabel "conforms to"@en .

<https://w3id.org/nfdi4cat/voc4cat_0007004> a skos:Concept ;
    dcterms:identifier "voc4cat_0007004"^^xsd:token ;
    skos:broader <https://w3id.org/nfdi4cat/voc4cat_0000186> ;
    skos:definition "The composition of chemical species fed to the inlet of a chemical reactor."@en ;
    skos:historyNote "0000-0002-4041-0165 Julia Schumann created the resource, 0000-0002-5898-1820 David Linke contributed to the definition of the resource"@en ;
    skos:inScheme <https://w3id.org/nfdi4cat/voc4cat> ;
    skos:prefLabel "reactor feed"@en .

<https://w3id.org/nfdi4cat/voc4cat_0007005> a skos:Concept ;
    dcterms:identifier "voc4cat_0007005"^^xsd:token ;
    skos:broader <https://w3id.org/nfdi4cat/voc4cat_0000181> ;
    skos:definition "A substance that is added to a chemical reaction."@en ;
    skos:historyNote "0000-0002-4041-0165 Julia Schumann created the resource"@en ;
    skos:inScheme <https://w3id.org/nfdi4cat/voc4cat> ;
    skos:prefLabel "reagent"@en .

<https://w3id.org/nfdi4cat/voc4cat_0007006> a skos:Concept ;
    dcterms:identifier "voc4cat_0007006"^^xsd:token ;
    skos:altLabel "active centre"@en ;
    skos:broader <https://w3id.org/nfdi4cat/voc4cat_0000181> ;
    skos:definition "Those sites for adsorption which are the effective sites for a particular heterogeneous catalytic reaction."@en ;
    skos:historyNote "0000-0002-4041-0165 Julia Schumann created the resource"@en ;
    skos:inScheme <https://w3id.org/nfdi4cat/voc4cat> ;
    skos:prefLabel "active site"@en .

<https://w3id.org/nfdi4cat/voc4cat_0007007> a skos:Concept ;
    dcterms:identifier "voc4cat_0007007"^^xsd:token ;
    skos:broader <https://w3id.org/nfdi4cat/voc4cat_0000184> ;
    skos:definition "A type of catalytic test, where the performance of the catalyst is measured over an extended time period. Not to be performed at full conversion to be able to see catalyst deactivation, but usually also not at differential conditions to see the effect of product concentration on the catalyst."@en ;
    skos:historyNote "0000-0002-4041-0165 Julia Schumann created the resource"@en ;
    skos:inScheme <https://w3id.org/nfdi4cat/voc4cat> ;
    skos:prefLabel "stability measurement"@en .

<https://w3id.org/nfdi4cat/voc4cat_0007008> a skos:Concept ;
    dcterms:identifier "voc4cat_0007008"^^xsd:token ;
    skos:broader <https://w3id.org/nfdi4cat/voc4cat_0000184> ;
    skos:definition "A type of catalytic test, where the depletion of formation of chemical substances is measured, usually performed under differential conditions"@en ;
    skos:historyNote "0000-0002-4041-0165 Julia Schumann created the resource"@en ;
    skos:inScheme <https://w3id.org/nfdi4cat/voc4cat> ;
    skos:prefLabel "kinetic measurement"@en .

<https://w3id.org/nfdi4cat/voc4cat_0007009> a skos:Concept ;
    dcterms:identifier "voc4cat_0007009"^^xsd:token ;
    skos:broader <https://w3id.org/nfdi4cat/voc4cat_0000186> ;
    skos:definition "A name for a chemical reaction which assigns the reactants and (desired) products."@en ;
    skos:historyNote "0000-0002-4041-0165 Julia Schumann created the resource"@en ;
    skos:inScheme <https://w3id.org/nfdi4cat/voc4cat> ;
    skos:prefLabel "reaction name"@en .

<https://w3id.org/nfdi4cat/voc4cat_0007010> a skos:Concept ;
    dcterms:identifier "voc4cat_0007010"^^xsd:token ;
    skos:altLabel "reaction class"@en ;
    skos:broader <https://w3id.org/nfdi4cat/voc4cat_0000186> ;
    skos:definition "A group of chemical reactions with common conditions or reactants, e.g. Oxidation, Hydrogenation, Reduction, Cracking."@en ;
    skos:historyNote "0000-0002-4041-0165 Julia Schumann created the resource"@en ;
    skos:inScheme <https://w3id.org/nfdi4cat/voc4cat> ;
    skos:prefLabel "reaction type"@en .

<https://w3id.org/nfdi4cat/voc4cat_0007012> a skos:Concept ;
    dcterms:identifier "voc4cat_0007012"^^xsd:token ;
    skos:broader <https://w3id.org/nfdi4cat/voc4cat_0000187> ;
    skos:definition "A definition of best practice procedures to measure consistent datasets."@en ;
    skos:historyNote "0000-0002-4041-0165 Julia Schumann created the resource"@en ;
    skos:inScheme <https://w3id.org/nfdi4cat/voc4cat> ;
    skos:prefLabel "handbook"@en .

<https://w3id.org/nfdi4cat/voc4cat_0007013> a skos:Concept ;
    dcterms:identifier "voc4cat_0007013"^^xsd:token ;
    skos:broader <https://w3id.org/nfdi4cat/voc4cat_0000186> ;
    skos:definition "The temperature at which a chemical reaction is happening."@en ;
    skos:historyNote "0000-0002-4041-0165 Julia Schumann created the resource, 0000-0002-5898-1820 David Linke contributed to the definition of the resource"@en ;
    skos:inScheme <https://w3id.org/nfdi4cat/voc4cat> ;
    skos:prefLabel "reaction temperature"@en .

<https://w3id.org/nfdi4cat/voc4cat_0007014> a skos:Concept ;
    dcterms:identifier "voc4cat_0007014"^^xsd:token ;
    skos:broader <https://w3id.org/nfdi4cat/voc4cat_0000186> ;
    skos:definition "Some characteristics that define the catalyst, which can be related to composition, active phase, or role."@en ;
    skos:historyNote "0000-0002-4041-0165 Julia Schumann created the resource"@en ;
    skos:inScheme <https://w3id.org/nfdi4cat/voc4cat> ;
    skos:prefLabel "catalyst type"@en .

<https://w3id.org/nfdi4cat/voc4cat_0007015> a skos:Concept ;
    dcterms:identifier "voc4cat_0007015"^^xsd:token ;
    skos:broader <https://w3id.org/nfdi4cat/voc4cat_0000194> ;
    skos:definition "A catalyst that consists mainly of the active ingredient or phase."@en ;
    skos:historyNote "0000-0002-4041-0165 Julia Schumann created the resource"@en ;
    skos:inScheme <https://w3id.org/nfdi4cat/voc4cat> ;
    skos:prefLabel "bulk catalyst"@en .

<https://w3id.org/nfdi4cat/voc4cat_0007016> a skos:Concept ;
    dcterms:identifier "voc4cat_0007016"^^xsd:token ;
    skos:broader <https://w3id.org/nfdi4cat/voc4cat_0000186> ;
    skos:definition "The main technique applied to make the catalyst material out of pure substances."@en ;
    skos:historyNote "0000-0002-4041-0165 Julia Schumann created the resource"@en ;
    skos:inScheme <https://w3id.org/nfdi4cat/voc4cat> ;
    skos:prefLabel "preparation method"@en .

<https://w3id.org/nfdi4cat/voc4cat_0007018> a skos:Concept ;
    dcterms:identifier "voc4cat_0007018"^^xsd:token ;
    skos:broader <https://w3id.org/nfdi4cat/voc4cat_0000186> ;
    skos:definition "A classification of chemical reactors based on the distinct design, configuration, and operational characteristics. Examples are stirred tank reactors, loop reactors, trickle beds, multitubular reactors, fluidized beds, and others. Each type is tailored to accomodate a specific combinations of reaction kinetics, thermodynamics, mass transfer requirements, and process variables."@en ;
    skos:historyNote "0000-0002-4041-0165 Julia Schumann created the resource, 0000-0002-5898-1820 David Linke provided the definition"@en ;
    skos:inScheme <https://w3id.org/nfdi4cat/voc4cat> ;
    skos:prefLabel "reactor design type"@en .

<https://w3id.org/nfdi4cat/voc4cat_0007019> a skos:Concept ;
    dcterms:identifier "voc4cat_0007019"^^xsd:token ;
    skos:altLabel "CSTR"@en ;
    skos:broader <https://w3id.org/nfdi4cat/voc4cat_0007036> ;
    skos:definition "A reaction vessel characterized by continuously fed reactnts, thorough mixing of fed reactants with the contents already present in the reactor by stirring and continous removal of a product stream from the system to maintain a constant volume."@en ;
    skos:historyNote "0000-0002-4041-0165 Julia Schumann created the resource, 0000-0002-5898-1820 David Linke contributed to the definition of the resource"@en ;
    skos:inScheme <https://w3id.org/nfdi4cat/voc4cat> ;
    skos:prefLabel "continuous stirred tank reactor"@en .

<https://w3id.org/nfdi4cat/voc4cat_0007020> a skos:Concept ;
    dcterms:identifier "voc4cat_0007020"^^xsd:token ;
    skos:broader <https://w3id.org/nfdi4cat/voc4cat_0000188> ;
    skos:definition "The part of the reactor where the catalyst is located, characterized by length, diameter, volume."@en ;
    skos:historyNote "0000-0002-4041-0165 Julia Schumann created the resource"@en ;
    skos:inScheme <https://w3id.org/nfdi4cat/voc4cat> ;
    skos:prefLabel "catalyst bed"@en .

<https://w3id.org/nfdi4cat/voc4cat_0007021> a skos:Concept ;
    dcterms:identifier "voc4cat_0007021"^^xsd:token ;
    skos:altLabel "apparent catalyst volume"@en ;
    skos:broader <https://w3id.org/nfdi4cat/voc4cat_0000186> ;
    skos:definition "The bulk volume taken up by the catalyst and potential diluent in a fixed bed reactor."@en ;
    skos:historyNote "0000-0002-4041-0165 Julia Schumann created the resource"@en ;
    skos:inScheme <https://w3id.org/nfdi4cat/voc4cat> ;
    skos:prefLabel "catalyst bed volume"@en .

<https://w3id.org/nfdi4cat/voc4cat_0007022> a skos:Concept ;
    dcterms:identifier "voc4cat_0007022"^^xsd:token ;
    skos:broader <https://w3id.org/nfdi4cat/voc4cat_0000186> ;
    skos:definition "The portion of a powder catalyst sample that passes through a standard sieve of specified number and is retained by some finer sieve."@en ;
    skos:historyNote "0000-0002-4041-0165 Julia Schumann created the resource"@en ;
    skos:inScheme <https://w3id.org/nfdi4cat/voc4cat> ;
    skos:prefLabel "sieve fraction"@en .

<https://w3id.org/nfdi4cat/voc4cat_0007023> a skos:Concept ;
    dcterms:identifier "voc4cat_0007023"^^xsd:token ;
    skos:altLabel "GHSV"@en ;
    skos:broader <https://w3id.org/nfdi4cat/voc4cat_0000186> ;
    skos:definition "A physical quantity given by the volumetric flow entering a control volume devided by the size of the control volume; the quantity must be given in the unit 1/hour.  In heterogeneous catalysis the volume of the undiluted catalyst bed is used as characteristic control volume. In case of gases the flow at reference conditions (0°C, 100 kPa = 1 bar) is used."@en ;
    skos:historyNote "0000-0002-4041-0165 Julia Schumann created the resource, 0000-0002-5898-1820 David Linke contributed to the definition of the resource"@en ;
    skos:inScheme <https://w3id.org/nfdi4cat/voc4cat> ;
    skos:prefLabel "gas hourly space velocity"@en .

<https://w3id.org/nfdi4cat/voc4cat_0007024> a skos:Concept ;
    dcterms:identifier "voc4cat_0007024"^^xsd:token ;
    skos:altLabel "rate of reaction"@en ;
    skos:broader <https://w3id.org/nfdi4cat/voc4cat_0000186> ;
    skos:definition "A physical quantity describing how fast a chemical reaction proceeds. It is defined by the change of the extend of reaction per unit of time."@en ;
    skos:historyNote "0000-0002-4041-0165 Julia Schumann created the resource, 0000-0002-5898-1820 David Linke contributed to the definition of the resource"@en ;
    skos:inScheme <https://w3id.org/nfdi4cat/voc4cat> ;
    skos:prefLabel "reaction rate"@en .

<https://w3id.org/nfdi4cat/voc4cat_0007025> a skos:Concept ;
    dcterms:identifier "voc4cat_0007025"^^xsd:token ;
    skos:broader <https://w3id.org/nfdi4cat/voc4cat_0000186> ;
    skos:definition "A reaction rate that is normalized either to mass of active ingredient, surface area or certain measured adsorption sites."@en ;
    skos:historyNote "0000-0002-4041-0165 Julia Schumann created the resource, 0000-0002-5898-1820 David Linke contributed to the definition of the resource"@en ;
    skos:inScheme <https://w3id.org/nfdi4cat/voc4cat> ;
    skos:prefLabel "specific reaction rate"@en .

<https://w3id.org/nfdi4cat/voc4cat_0007026> a skos:Concept ;
    dcterms:identifier "voc4cat_0007026"^^xsd:token ;
    skos:broader <https://w3id.org/nfdi4cat/voc4cat_0000186> ;
    skos:definition "The number of datapoints per unit of time. Inverse of sampling interval."@en ;
    skos:historyNote "0000-0002-4041-0165 Julia Schumann created the resource, 0000-0002-5898-1820 David Linke contributed to the definition of the resource"@en ;
    skos:inScheme <https://w3id.org/nfdi4cat/voc4cat> ;
    skos:prefLabel "sampling frequency"@en .

<https://w3id.org/nfdi4cat/voc4cat_0007027> a skos:Concept ;
    dcterms:identifier "voc4cat_0007027"^^xsd:token ;
    skos:broader <https://w3id.org/nfdi4cat/voc4cat_0000184> ;
    skos:definition "A synthesis method in which a solid material (a precipitate) sediments from a liquid solution in which the material is present in a concentration greater than its solubility in the liquid."@en ;
    skos:historyNote "0000-0002-4041-0165 Julia Schumann created the resource, 0000-0002-5898-1820 David Linke contributed to the definition of the resource"@en ;
    skos:inScheme <https://w3id.org/nfdi4cat/voc4cat> ;
    skos:prefLabel "precipitation"@en .

<https://w3id.org/nfdi4cat/voc4cat_0007028> a skos:Concept ;
    dcterms:identifier "voc4cat_0007028"^^xsd:token ;
    skos:broader <https://w3id.org/nfdi4cat/voc4cat_0000184> ;
    skos:definition "A synthesis method in which inorganic compounds are dissolved in a solvent and brought into contact with a solid support in order to deposit them completely or in parts onto the surface."@en ;
    skos:historyNote "0000-0002-4041-0165 Julia Schumann created the resource, 0000-0002-5898-1820 David Linke contributed to the definition of the resource"@en ;
    skos:inScheme <https://w3id.org/nfdi4cat/voc4cat> ;
    skos:prefLabel "impregnation"@en .

<https://w3id.org/nfdi4cat/voc4cat_0007029> a skos:Concept ;
    dcterms:identifier "voc4cat_0007029"^^xsd:token ;
    skos:broader <https://w3id.org/nfdi4cat/voc4cat_0000185> ;
    skos:definition "A synthesis method involving the thermal treatment of a mixture of substances in aqueous solution or in form of a slurry in water characterised by heating the mixture in a sealed  reaction vessel to a temperature greater than the boiling point at standard pressure ."@en ;
    skos:historyNote "0000-0002-4041-0165 Julia Schumann created the resource, 0000-0002-5898-1820 David Linke contributed to the definition of the resource"@en ;
    skos:inScheme <https://w3id.org/nfdi4cat/voc4cat> ;
    skos:prefLabel "hydrothermal synthesis"@en .

<https://w3id.org/nfdi4cat/voc4cat_0007030> a skos:Concept ;
    dcterms:identifier "voc4cat_0007030"^^xsd:token ;
    skos:broader <https://w3id.org/nfdi4cat/voc4cat_0000184> ;
    skos:definition "Treatment of a solid substance or mixtures of solids at elevated temperatures."@en ;
    skos:historyNote "0000-0002-4041-0165 Julia Schumann created the resource, 0000-0002-5898-1820 David Linke contributed to the definition of the resource"@en ;
    skos:inScheme <https://w3id.org/nfdi4cat/voc4cat> ;
    skos:prefLabel "calcination"@en .

<https://w3id.org/nfdi4cat/voc4cat_0007031> a skos:Concept ;
    dcterms:identifier "voc4cat_0007031"^^xsd:token ;
    skos:broader <https://w3id.org/nfdi4cat/voc4cat_0000185> ;
    skos:definition "A method to synthesize mixed oxide/non-oxide powders by combustion of liquid precursor droplets in a flame."@en ;
    skos:historyNote "0000-0002-4041-0165 Julia Schumann created the resource"@en ;
    skos:inScheme <https://w3id.org/nfdi4cat/voc4cat> ;
    skos:prefLabel "flame spray pyrolysis"@en .

<https://w3id.org/nfdi4cat/voc4cat_0007032> a skos:Concept ;
    dcterms:identifier "voc4cat_0007032"^^xsd:token ;
    skos:broader <https://w3id.org/nfdi4cat/voc4cat_0000186> ;
    skos:definition "A representative temperature value for the operating temperature of a reactor. In the special case of an isothermal chemical reactor, this is the same as the reaction temperature."@en ;
    skos:historyNote "0000-0002-4041-0165 Julia Schumann created the resource"@en ;
    skos:inScheme <https://w3id.org/nfdi4cat/voc4cat> ;
    skos:prefLabel "reactor temperature"@en .

<https://w3id.org/nfdi4cat/voc4cat_0007038> a skos:Concept ;
    dcterms:identifier "voc4cat_0007038"^^xsd:token ;
    skos:broader <https://w3id.org/nfdi4cat/voc4cat_0000186> ;
    skos:definition "The mass of a material sample."@en ;
    skos:historyNote "0000-0002-4041-0165 Julia Schumann created the resource, 0000-0002-5898-1820 David Linke contributed to the definition of the resource"@en ;
    skos:inScheme <https://w3id.org/nfdi4cat/voc4cat> ;
    skos:prefLabel "sample mass"@en .

<https://w3id.org/nfdi4cat/voc4cat_0007039> a skos:Concept ;
    dcterms:identifier "voc4cat_0007039"^^xsd:token ;
    skos:broader <https://w3id.org/nfdi4cat/voc4cat_0000186> ;
    skos:definition "Collection of environmental variables of a reaction such as temperature, pressure, reagent concentrations and flow rate."@en ;
    skos:historyNote "0000-0002-4041-0165 Julia Schumann created the resource"@en ;
    skos:inScheme <https://w3id.org/nfdi4cat/voc4cat> ;
    skos:prefLabel "reaction conditions"@en .

<https://w3id.org/nfdi4cat/voc4cat_0007040> a skos:Concept ;
    dcterms:identifier "voc4cat_0007040"^^xsd:token ;
    rdfs:isDefinedBy <https://doi.org/10.1351/goldbook.M03804> ;
    skos:altLabel "reaction mechanism"@en ;
    skos:broader <https://w3id.org/nfdi4cat/voc4cat_0000181> ;
    skos:definition "A detailed description of the process leading from the reactants to the products of a reaction, including a description as complete as possible of the composition, structure, energy and other properties of reaction intermediates, products and transition states."@en ;
    skos:historyNote "0000-0002-4041-0165 Julia Schumann created the resource"@en ;
    skos:inScheme <https://w3id.org/nfdi4cat/voc4cat> ;
    skos:prefLabel "chemical reaction mechanism"@en .

<https://w3id.org/nfdi4cat/voc4cat_0007041> a skos:Concept ;
    dcterms:identifier "voc4cat_0007041"^^xsd:token ;
    rdfs:isDefinedBy <https://doi.org/10.1351/goldbook.E02035> ;
    skos:altLabel "elementary step"@en ;
    skos:broader <https://w3id.org/nfdi4cat/voc4cat_0000181> ;
    skos:definition "A reaction for which no reaction intermediates have been detected or need to be postulated in order to describe the chemical reaction on a molecular scale. An elementary reaction is assumed to occur in a single step and to pass through a single transition state."@en ;
    skos:historyNote "0000-0002-4041-0165 Julia Schumann created the resource"@en ;
    skos:inScheme <https://w3id.org/nfdi4cat/voc4cat> ;
    skos:prefLabel "elementary reaction"@en .

<https://w3id.org/nfdi4cat/voc4cat_0007042> a skos:Concept ;
    dcterms:identifier "voc4cat_0007042"^^xsd:token ;
    skos:broader <https://w3id.org/nfdi4cat/voc4cat_0007045> ;
    skos:definition "The person carrying out a synthesis preparation."@en ;
    skos:historyNote "0000-0002-4041-0165 Julia Schumann created the resource"@en ;
    skos:inScheme <https://w3id.org/nfdi4cat/voc4cat> ;
    skos:prefLabel "preparator"@en .

<https://w3id.org/nfdi4cat/voc4cat_0007043> a skos:Concept ;
    dcterms:identifier "voc4cat_0007043"^^xsd:token ;
    skos:broader <https://w3id.org/nfdi4cat/voc4cat_0007045> ;
    skos:definition "The person starting or carrying out a planned process."@en ;
    skos:historyNote "0000-0002-4041-0165 Julia Schumann created the resource"@en ;
    skos:inScheme <https://w3id.org/nfdi4cat/voc4cat> ;
    skos:prefLabel "experimenter"@en .

<https://w3id.org/nfdi4cat/voc4cat_0007044> a skos:Concept ;
    dcterms:identifier "voc4cat_0007044"^^xsd:token ;
    skos:broader <https://w3id.org/nfdi4cat/voc4cat_0000186> ;
    skos:definition "The fractions of atoms of a specific chemical element located at the surface of a material versus the total number of atoms of this specific element in the material."@en ;
    skos:historyNote "0000-0002-4041-0165 Julia Schumann created the resource"@en ;
    skos:inScheme <https://w3id.org/nfdi4cat/voc4cat> ;
    skos:prefLabel "dispersion"@en .

<https://w3id.org/nfdi4cat/voc4cat_0007102> a skos:Concept ;
    dcterms:identifier "voc4cat_0007102"^^xsd:token ;
    skos:altLabel "PFR model"@en ;
    skos:broader <https://w3id.org/nfdi4cat/voc4cat_0007101> ;
    skos:definition "An abstract concept/ideal reactor model type in which a liquid flows uniformly through the tube, resulting in a straight wave/flow front. Each fluid element has the same residence time."@en ;
    skos:historyNote "0000-0001-5886-7860 Hendrik Borgelt created this resource, 0000-0002-5898-1820 David Linke contributed to the definition of the resource"@en ;
    skos:inScheme <https://w3id.org/nfdi4cat/voc4cat> ;
    skos:prefLabel "plug flow reactor model"@en .

<https://w3id.org/nfdi4cat/voc4cat_0007105> a skos:Concept ;
    dcterms:identifier "voc4cat_0007105"^^xsd:token ;
    skos:broader <https://w3id.org/nfdi4cat/voc4cat_0007104> ;
    skos:definition "An extension of the concept of the tubular reactor model, in that the fluid does not flow though a straight tube but through a tube with regular bends, e.g. a coiled tube, which modifies the residence time distribution as compared to a straight tube."@en ;
    skos:historyNote "0000-0001-5886-7860 Hendrik Borgelt created this resource, 0000-0002-5898-1820 David Linke contributed to the definition of the resource"@en ;
    skos:inScheme <https://w3id.org/nfdi4cat/voc4cat> ;
    skos:prefLabel "coiled tubular reactor model"@en .

<https://w3id.org/nfdi4cat/voc4cat_0007106> a skos:Concept ;
    dcterms:identifier "voc4cat_0007106"^^xsd:token ;
    skos:altLabel "CSTR model"@en ;
    skos:broader <https://w3id.org/nfdi4cat/voc4cat_0007103> ;
    skos:definition "A stirred tank reactor model with always present feed and effluent streams."@en ;
    skos:historyNote "0000-0001-5886-7860 Hendrik Borgelt created this resource, 0000-0002-5898-1820 David Linke contributed to the definition of the resource"@en ;
    skos:inScheme <https://w3id.org/nfdi4cat/voc4cat> ;
    skos:prefLabel "continuous stirred tank reactor model"@en .

<https://w3id.org/nfdi4cat/voc4cat_0007107> a skos:Concept ;
    dcterms:identifier "voc4cat_0007107"^^xsd:token ;
    skos:altLabel "batch stirred tank reactor model"@en ;
    skos:broader <https://w3id.org/nfdi4cat/voc4cat_0007103> ;
    skos:definition "A stirred tank reactor model characterized by the absence of either feed or effluent flows. Examples modes of operation are batch (neither feed nor effluent), feed batch (only feed) , or drained batch (only effluent)."@en ;
    skos:historyNote "0000-0001-5886-7860 Hendrik Borgelt created this resource, 0000-0002-5898-1820 David Linke contributed to the definition of the resource"@en ;
    skos:inScheme <https://w3id.org/nfdi4cat/voc4cat> ;
    skos:prefLabel "discontinuous stirred tank reactor model"@en .

<https://w3id.org/nfdi4cat/voc4cat_0007202> a skos:Concept ;
    dcterms:identifier "voc4cat_0007202"^^xsd:token ;
    skos:altLabel "WE"@en ;
    skos:broader <https://w3id.org/nfdi4cat/voc4cat_0007201> ;
    skos:definition "The electrode in a three-electrode cell where \"the action is\"."@en ;
    skos:historyNote "0009-0008-1278-8890 Michael Götte created the resource"@en ;
    skos:inScheme <https://w3id.org/nfdi4cat/voc4cat> ;
    skos:prefLabel "working electrode"@en .

<https://w3id.org/nfdi4cat/voc4cat_0007203> a skos:Concept ;
    dcterms:identifier "voc4cat_0007203"^^xsd:token ;
    skos:altLabel "CE"@en ;
    skos:broader <https://w3id.org/nfdi4cat/voc4cat_0007201> ;
    skos:definition "An electrode in a three-electrode cell that is used only to make an electrical connection to the electrolyte so that a current can be applied to the working electrode."@en ;
    skos:historyNote "0009-0008-1278-8890 Michael Götte created the resource"@en ;
    skos:inScheme <https://w3id.org/nfdi4cat/voc4cat> ;
    skos:prefLabel "counter electrode"@en .

<https://w3id.org/nfdi4cat/voc4cat_0007204> a skos:Concept ;
    dcterms:identifier "voc4cat_0007204"^^xsd:token ;
    skos:altLabel "reaction class"@en ;
    skos:broader <https://w3id.org/nfdi4cat/voc4cat_0007201> ;
    skos:definition "An electrode that has a well known and stable equilibrium electrode potential."@en ;
    skos:historyNote "0009-0008-1278-8890 Michael Götte created the resource"@en ;
    skos:inScheme <https://w3id.org/nfdi4cat/voc4cat> ;
    skos:prefLabel "reference electrode"@en .

<https://w3id.org/nfdi4cat/voc4cat_0007205> a skos:Concept ;
    dcterms:identifier "voc4cat_0007205"^^xsd:token ;
    skos:broader <https://w3id.org/nfdi4cat/voc4cat_0000187> ;
    skos:definition "An electronic instrument that controls the electrical potential difference between the working and reference electrodes of a three-electrode cell at a preset value."@en ;
    skos:historyNote "0009-0008-1278-8890 Michael Götte created the resource"@en ;
    skos:inScheme <https://w3id.org/nfdi4cat/voc4cat> ;
    skos:prefLabel "potentiostat"@en .

<https://w3id.org/nfdi4cat/voc4cat_0007207> a skos:Concept ;
    dcterms:identifier "voc4cat_0007207"^^xsd:token ;
    skos:altLabel "CA"@en ;
    skos:broader <https://w3id.org/nfdi4cat/voc4cat_0007237> ;
    skos:definition "An electrochemical measuring technique used for electrochemical analysis or for the determination of the kinetics and mechanism of electrode reactions. A fast-rising potential pulse is enforced on the working electrode of an electrochemical cell and the current flowing through this electrode is measured as a function of time."@en ;
    skos:historyNote "0009-0008-1278-8890 Michael Götte created the resource"@en ;
    skos:inScheme <https://w3id.org/nfdi4cat/voc4cat> ;
    skos:prefLabel "chronoamperometry"@en .

<https://w3id.org/nfdi4cat/voc4cat_0007208> a skos:Concept ;
    dcterms:identifier "voc4cat_0007208"^^xsd:token ;
    skos:altLabel "CP"@en ;
    skos:broader <https://w3id.org/nfdi4cat/voc4cat_0007206> ;
    skos:definition "An electrochemical measuring technique used for electrochemical analysis or for the determination of the kinetics and mechanism of electrode reactions. A fast-rising current pulse is enforced on the working electrode of an electrochemical cell and the potential of this electrode is measured against a reference electrode as a function of time."@en ;
    skos:historyNote "0009-0008-1278-8890 Michael Götte created the resource"@en ;
    skos:inScheme <https://w3id.org/nfdi4cat/voc4cat> ;
    skos:prefLabel "chronopotentiometry"@en .

<https://w3id.org/nfdi4cat/voc4cat_0007209> a skos:Concept ;
    dcterms:identifier "voc4cat_0007209"^^xsd:token ;
    skos:altLabel "EIS"@en ;
    skos:broader <https://w3id.org/nfdi4cat/voc4cat_0007206> ;
    skos:definition "A powerful tool for examining processes occurring at electrode surfaces. A small amplitude ac (sinusoidal) excitation signal (potential or current), covering a wide range of frequencies, is applied to the system under investigation and the response (current or voltage or another signal of interest) is measured. It is routinely used in electrode kinetics and mechanism investigations, and in the characterization of batteries, fuel cells, and corrosion phenomena."@en ;
    skos:historyNote "0009-0008-1278-8890 Michael Götte created the resource"@en ;
    skos:inScheme <https://w3id.org/nfdi4cat/voc4cat> ;
    skos:prefLabel "electrochemical impedance spectroscopy"@en .

<https://w3id.org/nfdi4cat/voc4cat_0007210> a skos:Concept ;
    dcterms:identifier "voc4cat_0007210"^^xsd:token ;
    skos:altLabel "OCV"@en ;
    skos:broader <https://w3id.org/nfdi4cat/voc4cat_0000186> ;
    skos:definition "The cell voltage under zero current conditions."@en ;
    skos:historyNote "0009-0008-1278-8890 Michael Götte created the resource"@en ;
    skos:inScheme <https://w3id.org/nfdi4cat/voc4cat> ;
    skos:prefLabel "open circuit voltage"@en .

<https://w3id.org/nfdi4cat/voc4cat_0007211> a skos:Concept ;
    dcterms:identifier "voc4cat_0007211"^^xsd:token ;
    skos:altLabel "LSV"@en ;
    skos:broader <https://w3id.org/nfdi4cat/voc4cat_0007237> ;
    skos:definition "A voltammetry where the voltage changes linearly over time from a initial potential to a final potential."@en ;
    skos:historyNote "0009-0008-1278-8890 Michael Götte created the resource"@en ;
    skos:inScheme <https://w3id.org/nfdi4cat/voc4cat> ;
    skos:prefLabel "linear sweep voltammetry"@en .

<https://w3id.org/nfdi4cat/voc4cat_0007212> a skos:Concept ;
    dcterms:identifier "voc4cat_0007212"^^xsd:token ;
    skos:altLabel "CC"@en ;
    skos:broader <https://w3id.org/nfdi4cat/voc4cat_0007206> ;
    skos:definition "An electrochemical measuring technique used for electrochemical analysis or for the determination of the kinetics and mechanism of electrode reactions. A fast-rising potential pulse is enforced on the working electrode of an electrochemical cell and the electrical charge passing through this electrode is measured as a function of time."@en ;
    skos:historyNote "0009-0008-1278-8890 Michael Götte created the resource"@en ;
    skos:inScheme <https://w3id.org/nfdi4cat/voc4cat> ;
    skos:prefLabel "chronocoulometry"@en .

<https://w3id.org/nfdi4cat/voc4cat_0007213> a skos:Concept ;
    dcterms:identifier "voc4cat_0007213"^^xsd:token ;
    skos:altLabel "sweep rate potential"@en ;
    skos:broader <https://w3id.org/nfdi4cat/voc4cat_0007219> ;
    skos:definition "In cyclic voltammetry, the rate at which the potential of the working electrode is varied, i.e., = (dE/dt). The value of is always cited as positive."@en ;
    skos:historyNote "0009-0008-1278-8890 Michael Götte created the resource"@en ;
    skos:inScheme <https://w3id.org/nfdi4cat/voc4cat> ;
    skos:prefLabel "scan rate potential"@en .

<https://w3id.org/nfdi4cat/voc4cat_0007214> a skos:Concept ;
    dcterms:identifier "voc4cat_0007214"^^xsd:token ;
    skos:broader <https://w3id.org/nfdi4cat/voc4cat_0007219> ;
    skos:definition "The minimal electrical potential in a cyclic voltammetry. This is where the sweep turns."@en ;
    skos:historyNote "0009-0008-1278-8890 Michael Götte created the resource"@en ;
    skos:inScheme <https://w3id.org/nfdi4cat/voc4cat> ;
    skos:prefLabel "lower limit potential"@en .

<https://w3id.org/nfdi4cat/voc4cat_0007215> a skos:Concept ;
    dcterms:identifier "voc4cat_0007215"^^xsd:token ;
    skos:broader <https://w3id.org/nfdi4cat/voc4cat_0007219> ;
    skos:definition "The maximal electrical potential in a cyclic voltammetry. This is where the sweep turns."@en ;
    skos:historyNote "0009-0008-1278-8890 Michael Götte created the resource"@en ;
    skos:inScheme <https://w3id.org/nfdi4cat/voc4cat> ;
    skos:prefLabel "upper limit potential"@en .

<https://w3id.org/nfdi4cat/voc4cat_0007216> a skos:Concept ;
    dcterms:identifier "voc4cat_0007216"^^xsd:token ;
    skos:broader <https://w3id.org/nfdi4cat/voc4cat_0007219> ;
    skos:definition "The electrical potential at which a linear sweep or cyclic voltammetry starts."@en ;
    skos:historyNote "0009-0008-1278-8890 Michael Götte created the resource"@en ;
    skos:inScheme <https://w3id.org/nfdi4cat/voc4cat> ;
    skos:prefLabel "initial potential"@en .

<https://w3id.org/nfdi4cat/voc4cat_0007217> a skos:Concept ;
    dcterms:identifier "voc4cat_0007217"^^xsd:token ;
    skos:broader <https://w3id.org/nfdi4cat/voc4cat_0007219> ;
    skos:definition "The electrical potential at which a linear sweep or cyclic voltammetry ends."@en ;
    skos:historyNote "0009-0008-1278-8890 Michael Götte created the resource"@en ;
    skos:inScheme <https://w3id.org/nfdi4cat/voc4cat> ;
    skos:prefLabel "final potential"@en .

<https://w3id.org/nfdi4cat/voc4cat_0007218> a skos:Concept ;
    dcterms:identifier "voc4cat_0007218"^^xsd:token ;
    skos:broader <https://w3id.org/nfdi4cat/voc4cat_0007219> ;
    skos:definition "The electrical potential difference at which the potential in a linear sweep or cyclic voltammetry is altered."@en ;
    skos:historyNote "0009-0008-1278-8890 Michael Götte created the resource"@en ;
    skos:inScheme <https://w3id.org/nfdi4cat/voc4cat> ;
    skos:prefLabel "step size potential"@en .

<https://w3id.org/nfdi4cat/voc4cat_0007221> a skos:Concept ;
    dcterms:identifier "voc4cat_0007221"^^xsd:token ;
    skos:broader <https://w3id.org/nfdi4cat/voc4cat_0000186> ;
    skos:definition "Current referred to the unit area of the electrode. Current divided by the true electrode area."@en ;
    skos:historyNote "0009-0008-1278-8890 Michael Götte created the resource"@en ;
    skos:inScheme <https://w3id.org/nfdi4cat/voc4cat> ;
    skos:prefLabel "current density"@en .

<https://w3id.org/nfdi4cat/voc4cat_0007222> a skos:Concept ;
    dcterms:identifier "voc4cat_0007222"^^xsd:token ;
    skos:broader <https://w3id.org/nfdi4cat/voc4cat_0000186> ;
    skos:definition "The measure of an electrical circuit element's inability to carry electrical current."@en ;
    skos:historyNote "0009-0008-1278-8890 Michael Götte created the resource"@en ;
    skos:inScheme <https://w3id.org/nfdi4cat/voc4cat> ;
    skos:prefLabel "resistance"@en .

<https://w3id.org/nfdi4cat/voc4cat_0007223> a skos:Concept ;
    dcterms:identifier "voc4cat_0007223"^^xsd:token ;
    skos:broader <https://w3id.org/nfdi4cat/voc4cat_0000186> ;
    skos:definition "The final environment in which the electrochemical reaction happens. Includes possibly purged electrolyte."@en ;
    skos:historyNote "0009-0008-1278-8890 Michael Götte created the resource"@en ;
    skos:inScheme <https://w3id.org/nfdi4cat/voc4cat> ;
    skos:prefLabel "electrochemical environment"@en .

<https://w3id.org/nfdi4cat/voc4cat_0007224> a skos:Concept ;
    dcterms:identifier "voc4cat_0007224"^^xsd:token ;
    skos:broader <https://w3id.org/nfdi4cat/voc4cat_0000187> ;
    skos:definition "A chemical compound (salt, acid, or base) that dissociates into electrically charged ions when dissolved in a solvent."@en ;
    skos:historyNote "0009-0008-1278-8890 Michael Götte created the resource"@en ;
    skos:inScheme <https://w3id.org/nfdi4cat/voc4cat> ;
    skos:prefLabel "electrolyte"@en .

<https://w3id.org/nfdi4cat/voc4cat_0007225> a skos:Concept ;
    dcterms:identifier "voc4cat_0007225"^^xsd:token ;
    skos:broader <https://w3id.org/nfdi4cat/voc4cat_0000184> ;
    skos:definition "The process of treating an electrolyte solution with gas."@en ;
    skos:historyNote "0009-0008-1278-8890 Michael Götte created the resource"@en ;
    skos:inScheme <https://w3id.org/nfdi4cat/voc4cat> ;
    skos:prefLabel "purging"@en .

<https://w3id.org/nfdi4cat/voc4cat_0007226> a skos:Concept ;
    dcterms:identifier "voc4cat_0007226"^^xsd:token ;
    skos:broader <https://w3id.org/nfdi4cat/voc4cat_0000186> ;
    skos:definition "Gas which is used in purging."@en ;
    skos:historyNote "0009-0008-1278-8890 Michael Götte created the resource"@en ;
    skos:inScheme <https://w3id.org/nfdi4cat/voc4cat> ;
    skos:prefLabel "purging gas"@en .

<https://w3id.org/nfdi4cat/voc4cat_0007227> a skos:Concept ;
    dcterms:identifier "voc4cat_0007227"^^xsd:token ;
    skos:broader <https://w3id.org/nfdi4cat/voc4cat_0000186> ;
    skos:definition "Temperature for which a gas is purged through the reaction chamber."@en ;
    skos:historyNote "0009-0008-1278-8890 Michael Götte created the resource"@en ;
    skos:inScheme <https://w3id.org/nfdi4cat/voc4cat> ;
    skos:prefLabel "purging temperature"@en .

<https://w3id.org/nfdi4cat/voc4cat_0007228> a skos:Concept ;
    dcterms:identifier "voc4cat_0007228"^^xsd:token ;
    skos:broader <https://w3id.org/nfdi4cat/voc4cat_0000186> ;
    skos:definition "The number of cycles in a measurement, such as a cyclic voltammetry."@en ;
    skos:historyNote "0009-0008-1278-8890 Michael Götte created the resource"@en ;
    skos:inScheme <https://w3id.org/nfdi4cat/voc4cat> ;
    skos:prefLabel "number of voltammetry cycles"@en .

<https://w3id.org/nfdi4cat/voc4cat_0007229> a skos:Concept ;
    dcterms:identifier "voc4cat_0007229"^^xsd:token ;
    skos:broader <https://w3id.org/nfdi4cat/voc4cat_0000186> ;
    skos:definition "The quotient of faradaic current to total current passed."@en ;
    skos:historyNote "0009-0008-1278-8890 Michael Götte created the resource"@en ;
    skos:inScheme <https://w3id.org/nfdi4cat/voc4cat> ;
    skos:prefLabel "faradaic efficiency"@en .

<https://w3id.org/nfdi4cat/voc4cat_0007230> a skos:Concept ;
    dcterms:identifier "voc4cat_0007230"^^xsd:token ;
    skos:broader <https://w3id.org/nfdi4cat/voc4cat_0000187> ;
    skos:definition "The collection of instruments and devices used in an electochemical reaction. Can include electrodes, flow cells, beaker, does not include the electrochemical environment."@en ;
    skos:historyNote "0009-0008-1278-8890 Michael Götte created the resource"@en ;
    skos:inScheme <https://w3id.org/nfdi4cat/voc4cat> ;
    skos:prefLabel "electrochemical setup"@en .

<https://w3id.org/nfdi4cat/voc4cat_0007231> a skos:Concept ;
    dcterms:identifier "voc4cat_0007231"^^xsd:token ;
    skos:altLabel "becker"@en,
        "beker"@en ;
    skos:broader <https://w3id.org/nfdi4cat/voc4cat_0000187> ;
    skos:definition "In laboratory equipment, a beaker is generally a cylindrical container with a flat bottom."@en ;
    skos:historyNote "0009-0008-1278-8890 Michael Götte created the resource"@en ;
    skos:inScheme <https://w3id.org/nfdi4cat/voc4cat> ;
    skos:prefLabel "beaker"@en .

<https://w3id.org/nfdi4cat/voc4cat_0007232> a skos:Concept ;
    dcterms:identifier "voc4cat_0007232"^^xsd:token ;
    skos:broader <https://w3id.org/nfdi4cat/voc4cat_0000187> ;
    skos:definition "Electrochemical cell in which analyte solution flows at a constant velocity through stationary tubular electrode(s)."@en ;
    skos:historyNote "0009-0008-1278-8890 Michael Götte created the resource"@en ;
    skos:inScheme <https://w3id.org/nfdi4cat/voc4cat> ;
    skos:prefLabel "flow cell"@en .

<https://w3id.org/nfdi4cat/voc4cat_0007233> a skos:Concept ;
    dcterms:identifier "voc4cat_0007233"^^xsd:token ;
    skos:broader <https://w3id.org/nfdi4cat/voc4cat_0000186> ;
    skos:definition "In voltammetry: a complementary pair of forward and reverse potential sweeps."@en ;
    skos:historyNote "0009-0008-1278-8890 Michael Götte created the resource"@en ;
    skos:inScheme <https://w3id.org/nfdi4cat/voc4cat> ;
    skos:prefLabel "voltammetry cycle"@en .

<https://w3id.org/nfdi4cat/voc4cat_0007234> a skos:Concept ;
    dcterms:identifier "voc4cat_0007234"^^xsd:token ;
    skos:broader <https://w3id.org/nfdi4cat/voc4cat_0000183> ;
    skos:definition "The phenomenon of movement (transportation) of electrical charge (that is, the electrical current) from one part of the electrochemical cell to another, occurring mainly as electromigration of ions, but it can also occur by diffusion of ions. See electrochemical potential."@en ;
    skos:historyNote "0009-0008-1278-8890 Michael Götte created the resource"@en ;
    skos:inScheme <https://w3id.org/nfdi4cat/voc4cat> ;
    skos:prefLabel "charge transport"@en .

<https://w3id.org/nfdi4cat/voc4cat_0007235> a skos:Concept ;
    dcterms:identifier "voc4cat_0007235"^^xsd:token ;
    skos:altLabel "separator"@en ;
    skos:broader <https://w3id.org/nfdi4cat/voc4cat_0000187> ;
    skos:definition "A thin structural material (usually a sheet) used to separate the electrolyte of a divided electrochemical cell into two or more compartments."@en ;
    skos:historyNote "0009-0008-1278-8890 Michael Götte created the resource"@en ;
    skos:inScheme <https://w3id.org/nfdi4cat/voc4cat> ;
    skos:prefLabel "membrane"@en .

<https://w3id.org/nfdi4cat/voc4cat_0007236> a skos:Concept ;
    dcterms:identifier "voc4cat_0007236"^^xsd:token ;
    skos:altLabel "H-cell"@en ;
    skos:broader <https://w3id.org/nfdi4cat/voc4cat_0000187> ;
    skos:definition "The H-Cell is a two-compartment electrochemical cell used for membrane testing, hydrogen permeation, or any other experiment where two separate electrode chambers are required."@en ;
    skos:historyNote "0009-0008-1278-8890 Michael Götte created the resource"@en ;
    skos:inScheme <https://w3id.org/nfdi4cat/voc4cat> ;
    skos:prefLabel "H cell"@en .

<https://w3id.org/nfdi4cat/voc4cat_0007238> a skos:Concept ;
    dcterms:identifier "voc4cat_0007238"^^xsd:token ;
    skos:broader <https://w3id.org/nfdi4cat/voc4cat_0000185> ;
    skos:definition "Graphical representation of the results of a voltammetric measurement."@en ;
    skos:historyNote "0009-0008-1278-8890 Michael Götte created the resource"@en ;
    skos:inScheme <https://w3id.org/nfdi4cat/voc4cat> ;
    skos:prefLabel "voltammogramm"@en .

<https://w3id.org/nfdi4cat/voc4cat_0007240> a skos:Concept ;
    dcterms:identifier "voc4cat_0007240"^^xsd:token ;
    skos:broader <https://w3id.org/nfdi4cat/voc4cat_0000186> ;
    skos:definition "Impedance is the analogue of the resistance when applied to alternating current. That is, it is a measure of a circuit element's inability to carry the electrical current."@en ;
    skos:historyNote "0009-0008-1278-8890 Michael Götte created the resource"@en ;
    skos:inScheme <https://w3id.org/nfdi4cat/voc4cat> ;
    skos:prefLabel "impedance"@en .

<https://w3id.org/nfdi4cat/voc4cat_0007241> a skos:Concept ;
    dcterms:identifier "voc4cat_0007241"^^xsd:token ;
    skos:broader <https://w3id.org/nfdi4cat/voc4cat_0007239> ;
    skos:definition "Initial frequency in for example an electrochemical impedance spectroscopy."@en ;
    skos:historyNote "0009-0008-1278-8890 Michael Götte created the resource"@en ;
    skos:inScheme <https://w3id.org/nfdi4cat/voc4cat> ;
    skos:prefLabel "initial frequency"@en .

<https://w3id.org/nfdi4cat/voc4cat_0007242> a skos:Concept ;
    dcterms:identifier "voc4cat_0007242"^^xsd:token ;
    skos:broader <https://w3id.org/nfdi4cat/voc4cat_0007239> ;
    skos:definition "Final frequency in for example an electrochemical impedance spectroscopy."@en ;
    skos:historyNote "0009-0008-1278-8890 Michael Götte created the resource"@en ;
    skos:inScheme <https://w3id.org/nfdi4cat/voc4cat> ;
    skos:prefLabel "final frequency"@en .

<https://w3id.org/nfdi4cat/voc4cat_0007243> a skos:Concept ;
    dcterms:identifier "voc4cat_0007243"^^xsd:token ;
    skos:altLabel "RHE"@en ;
    skos:broader <https://w3id.org/nfdi4cat/voc4cat_0007201> ;
    skos:definition "A commonly used reference electrode. A hydrogen electrode immersed directly into the electrolyte of the electrochemical cell and usually (unless otherwise stated) operated with one atmosphere pressure hydrogen gas. The equilibrium potential depends on the hydrogen ion concentration (strictly speaking, activity) of the cell electrolyte."@en ;
    skos:historyNote "0009-0008-1278-8890 Michael Götte created the resource"@en ;
    skos:inScheme <https://w3id.org/nfdi4cat/voc4cat> ;
    skos:prefLabel "reversible hydrogen electrode"@en .

<https://w3id.org/nfdi4cat/voc4cat_0007244> a skos:Concept ;
    dcterms:identifier "voc4cat_0007244"^^xsd:token ;
    skos:broader <https://w3id.org/nfdi4cat/voc4cat_0000186> ;
    skos:definition "The measure of the amount of dissolved material (solute) in a solution."@en ;
    skos:historyNote "0009-0008-1278-8890 Michael Götte created the resource"@en ;
    skos:inScheme <https://w3id.org/nfdi4cat/voc4cat> ;
    skos:prefLabel "concentration"@en .

<https://w3id.org/nfdi4cat/voc4cat_0007245> a skos:Concept ;
    dcterms:identifier "voc4cat_0007245"^^xsd:token ;
    skos:broader <https://w3id.org/nfdi4cat/voc4cat_0000186> ;
    skos:definition "The mass per area on a thin film sample, i.e. the working electrode."@en ;
    skos:historyNote "0009-0008-1278-8890 Michael Götte created the resource"@en ;
    skos:inScheme <https://w3id.org/nfdi4cat/voc4cat> ;
    skos:prefLabel "mass coverage"@en .

<https://w3id.org/nfdi4cat/voc4cat_0007246> a skos:Concept ;
    dcterms:identifier "voc4cat_0007246"^^xsd:token ;
    skos:broader <https://w3id.org/nfdi4cat/voc4cat_0000181> ;
    skos:definition "A liquid that dissolves another material."@en ;
    skos:historyNote "0009-0008-1278-8890 Michael Götte created the resource"@en ;
    skos:inScheme <https://w3id.org/nfdi4cat/voc4cat> ;
    skos:prefLabel "solvent"@en .

<https://w3id.org/nfdi4cat/voc4cat_0007247> a skos:Concept ;
    dcterms:identifier "voc4cat_0007247"^^xsd:token ;
    skos:broader <https://w3id.org/nfdi4cat/voc4cat_0000181> ;
    skos:definition "The dissolved species (e.g., a salt) in a solution."@en ;
    skos:historyNote "0009-0008-1278-8890 Michael Götte created the resource"@en ;
    skos:inScheme <https://w3id.org/nfdi4cat/voc4cat> ;
    skos:prefLabel "solute"@en .

<https://w3id.org/nfdi4cat/voc4cat_0007248> a skos:Concept ;
    dcterms:identifier "voc4cat_0007248"^^xsd:token ;
    skos:altLabel "RDE"@en,
        "rotating disk electrode"@en ;
    skos:broader <https://w3id.org/nfdi4cat/voc4cat_0007201> ;
    skos:definition "A specialized hydrodynamic electrode used in the study of the kinetics and mechanism of electrode reactions and in electroanalysis for ensuring a known and controllable flow of solution over the electrode."@en ;
    skos:historyNote "0009-0008-1278-8890 Michael Götte created the resource"@en ;
    skos:inScheme <https://w3id.org/nfdi4cat/voc4cat> ;
    skos:prefLabel "rotating-disk electrode"@en .

<https://w3id.org/nfdi4cat/voc4cat_0007250> a skos:Concept ;
    dcterms:identifier "voc4cat_0007250"^^xsd:token ;
    skos:broader <https://w3id.org/nfdi4cat/voc4cat_0000187> ;
    skos:definition "Equipment used in an electrochemical setup."@en ;
    skos:historyNote "0009-0008-1278-8890 Michael Götte created the resource"@en ;
    skos:inScheme <https://w3id.org/nfdi4cat/voc4cat> ;
    skos:prefLabel "electrochemical equipment"@en .

<https://w3id.org/nfdi4cat/voc4cat_0007251> a skos:Concept ;
    dcterms:identifier "voc4cat_0007251"^^xsd:token ;
    skos:altLabel "OCP measurement"@en,
        "OCV measurement"@en ;
    skos:broader <https://w3id.org/nfdi4cat/voc4cat_0000184> ;
    skos:definition "The measurement of the open circuit voltage of an electrochemical cell."@en ;
    skos:historyNote "0009-0008-1278-8890 Michael Götte created the resource"@en ;
    skos:inScheme <https://w3id.org/nfdi4cat/voc4cat> ;
    skos:prefLabel "open circuit voltage measurement"@en .

<https://w3id.org/nfdi4cat/voc4cat_0007252> a skos:Concept ;
    dcterms:identifier "voc4cat_0007252"^^xsd:token ;
    skos:broader <https://w3id.org/nfdi4cat/voc4cat_0000186> ;
    skos:definition "A basic property of matter that gives rise to all electric and magnetic forces and interactions."@en ;
    skos:historyNote "0009-0008-1278-8890 Michael Götte created the resource"@en ;
    skos:inScheme <https://w3id.org/nfdi4cat/voc4cat> ;
    skos:prefLabel "electrical charge"@en .

<https://w3id.org/nfdi4cat/voc4cat_0007253> a skos:Concept ;
    dcterms:identifier "voc4cat_0007253"^^xsd:token ;
    skos:broader <https://w3id.org/nfdi4cat/voc4cat_0000186> ;
    skos:definition "Charge referred to the unit area of the electrode. Charge divided by electrode area."@en ;
    skos:historyNote "0009-0008-1278-8890 Michael Götte created the resource"@en ;
    skos:inScheme <https://w3id.org/nfdi4cat/voc4cat> ;
    skos:prefLabel "electrical charge density"@en .

<https://w3id.org/nfdi4cat/voc4cat_0007254> a skos:Concept ;
    dcterms:identifier "voc4cat_0007254"^^xsd:token ;
    skos:broader <https://w3id.org/nfdi4cat/voc4cat_0007201> ;
    skos:definition "The electrode where reduction occurs in an electrochemical cell. It is the negative electrode in an electrolytic cell, while it is the positive electrode in a galvanic cell."@en ;
    skos:historyNote "0009-0008-1278-8890 Michael Götte created the resource"@en ;
    skos:inScheme <https://w3id.org/nfdi4cat/voc4cat> ;
    skos:prefLabel "cathode"@en .

<https://w3id.org/nfdi4cat/voc4cat_0007255> a skos:Concept ;
    dcterms:identifier "voc4cat_0007255"^^xsd:token ;
    skos:broader <https://w3id.org/nfdi4cat/voc4cat_0007201> ;
    skos:definition "The electrode where oxidation occurs in an electrochemical cell. It is the positive electrode in an electrolytic cell, while it is the negative electrode in a galvanic cell."@en ;
    skos:historyNote "0009-0008-1278-8890 Michael Götte created the resource"@en ;
    skos:inScheme <https://w3id.org/nfdi4cat/voc4cat> ;
    skos:prefLabel "anode"@en .

<https://w3id.org/nfdi4cat/voc4cat_0007256> a skos:Concept ;
    dcterms:identifier "voc4cat_0007256"^^xsd:token ;
    skos:broader <https://w3id.org/nfdi4cat/voc4cat_0007249> ;
    skos:definition "An electrochemical cell that converts chemical energy into electrical energy. A cell in which chemical reactions occur spontaneously at the electrodes when they are connected through an external circuit, producing an electrical current."@en ;
    skos:historyNote "0009-0008-1278-8890 Michael Götte created the resource"@en ;
    skos:inScheme <https://w3id.org/nfdi4cat/voc4cat> ;
    skos:prefLabel "galvanic cell"@en .

<https://w3id.org/nfdi4cat/voc4cat_0007257> a skos:Concept ;
    dcterms:identifier "voc4cat_0007257"^^xsd:token ;
    skos:broader <https://w3id.org/nfdi4cat/voc4cat_0007249> ;
    skos:definition "An electrochemical cell that converts electrical energy into chemical energy. The chemical reactions do not occur \"spontaneously\" at the electrodes when they are connected through an external circuit. The reaction must be forced by applying an external electrical current."@en ;
    skos:historyNote "0009-0008-1278-8890 Michael Götte created the resource"@en ;
    skos:inScheme <https://w3id.org/nfdi4cat/voc4cat> ;
    skos:prefLabel "electrolytic cell"@en .

<https://w3id.org/nfdi4cat/voc4cat_0007258> a skos:Concept ;
    dcterms:identifier "voc4cat_0007258"^^xsd:token ;
    skos:altLabel "true electrode area"@en ;
    skos:broader <https://w3id.org/nfdi4cat/voc4cat_0000186> ;
    skos:definition "In contrast to substrate area, the actual area of a sample or electrode which is active."@en ;
    skos:historyNote "0009-0008-1278-8890 Michael Götte created the resource"@en ;
    skos:inScheme <https://w3id.org/nfdi4cat/voc4cat> ;
    skos:prefLabel "active area"@en .

<https://w3id.org/nfdi4cat/voc4cat_0007259> a skos:Concept ;
    dcterms:identifier "voc4cat_0007259"^^xsd:token ;
    skos:broader <https://w3id.org/nfdi4cat/voc4cat_0007220> ;
    skos:definition "The current that is flowing through an electrochemical cell and is causing (or is caused by) chemical reactions (charge transfer) occurring at the electrode surfaces."@en ;
    skos:historyNote "0009-0008-1278-8890 Michael Götte created the resource"@en ;
    skos:inScheme <https://w3id.org/nfdi4cat/voc4cat> ;
    skos:prefLabel "faradaic current"@en .

<https://w3id.org/nfdi4cat/voc4cat_0007260> a skos:Concept ;
    dcterms:identifier "voc4cat_0007260"^^xsd:token ;
    skos:broader <https://w3id.org/nfdi4cat/voc4cat_0000186> ;
    skos:definition "A measure of the time taken for a solute to pass through a chromatography column. It is the mean of the residence time distribution; it is known as the first moment of the residence time distribution."@en ;
    skos:historyNote "0009-0008-1278-8890 Michael Götte created the resource"@en ;
    skos:inScheme <https://w3id.org/nfdi4cat/voc4cat> ;
    skos:prefLabel "retention time"@en .

<https://w3id.org/nfdi4cat/voc4cat_0007261> a skos:Concept ;
    dcterms:identifier "voc4cat_0007261"^^xsd:token ;
    skos:broader <https://w3id.org/nfdi4cat/voc4cat_0000186> ;
    skos:definition "A measure which is proportional to the amount of a product with a specific retention time. After calibration it is used to calculate gas concentrations of products of an chemical experiment."@en ;
    skos:historyNote "0009-0008-1278-8890 Michael Götte created the resource"@en ;
    skos:inScheme <https://w3id.org/nfdi4cat/voc4cat> ;
    skos:prefLabel "peak area"@en .

<https://w3id.org/nfdi4cat/voc4cat_0007262> a skos:Concept ;
    dcterms:identifier "voc4cat_0007262"^^xsd:token ;
    skos:broader <https://w3id.org/nfdi4cat/voc4cat_0000186> ;
    skos:definition "The thickness of the membrane."@en ;
    skos:historyNote "0009-0008-1278-8890 Michael Götte created the resource"@en ;
    skos:inScheme <https://w3id.org/nfdi4cat/voc4cat> ;
    skos:prefLabel "membrane thickness"@en .

<https://w3id.org/nfdi4cat/voc4cat_0007263> a skos:Concept ;
    dcterms:identifier "voc4cat_0007263"^^xsd:token ;
    skos:broader <https://w3id.org/nfdi4cat/voc4cat_0000186> ;
    skos:definition "The sum of all faradaic efficiencies in an experiment. If all current is accounted for should be 1."@en ;
    skos:historyNote "0009-0008-1278-8890 Michael Götte created the resource"@en ;
    skos:inScheme <https://w3id.org/nfdi4cat/voc4cat> ;
    skos:prefLabel "total faradaic efficiency"@en .

<https://w3id.org/nfdi4cat/> a schema:Organization ;
    schema:name "https://w3id.org/nfdi4cat/" ;
    schema:url "https://w3id.org/nfdi4cat/"^^xsd:anyURI .

<https://w3id.org/nfdi4cat/voc4cat_0000003> a skos:Concept ;
    dcterms:identifier "voc4cat_0000003"^^xsd:token ;
    skos:broader <https://w3id.org/nfdi4cat/voc4cat_0000190> ;
    skos:definition "A material with electrical conductivity between that of a conductor and an insulator."@en ;
    skos:historyNote "0000-0002-6242-2167 Nikolaos G. Moustakas created the resource"@en ;
    skos:inScheme <https://w3id.org/nfdi4cat/voc4cat> ;
    skos:prefLabel "semiconductor"@en .

<https://w3id.org/nfdi4cat/voc4cat_0000004> a skos:Concept ;
    dcterms:identifier "voc4cat_0000004"^^xsd:token ;
    skos:broader <https://w3id.org/nfdi4cat/voc4cat_0000186> ;
    skos:definition "Broad families of semiconducting materials (e.g., metal oxides) that can be used as catalysts in various applications."@en ;
    skos:historyNote "0000-0002-6242-2167 Nikolaos G. Moustakas created the resource"@en ;
    skos:inScheme <https://w3id.org/nfdi4cat/voc4cat> ;
    skos:prefLabel "categories of semiconductors"@en .

<https://w3id.org/nfdi4cat/voc4cat_0000005> a skos:Concept ;
    dcterms:identifier "voc4cat_0000005"^^xsd:token ;
    skos:broader <https://w3id.org/nfdi4cat/voc4cat_0000190> ;
    skos:definition "A chemical compound formed by the reaction of a metal with oxygen."@en ;
    skos:historyNote "0000-0002-6242-2167 Nikolaos G. Moustakas created the resource"@en ;
    skos:inScheme <https://w3id.org/nfdi4cat/voc4cat> ;
    skos:prefLabel "metal oxide"@en .

<https://w3id.org/nfdi4cat/voc4cat_0000006> a skos:Concept ;
    dcterms:identifier "voc4cat_0000006"^^xsd:token ;
    skos:broader <https://w3id.org/nfdi4cat/voc4cat_0000186> ;
    skos:definition "Characteristic properties of a semiconductor used in catalysis. These properties determine its performance in the studied catalytic application."@en ;
    skos:historyNote "0000-0002-6242-2167 Nikolaos G. Moustakas created the resource"@en ;
    skos:inScheme <https://w3id.org/nfdi4cat/voc4cat> ;
    skos:prefLabel "semiconductor property"@en .

<https://w3id.org/nfdi4cat/voc4cat_0000007> a skos:Concept ;
    dcterms:identifier "voc4cat_0000007"^^xsd:token ;
    skos:altLabel "EF"@en ;
    skos:broader <https://w3id.org/nfdi4cat/voc4cat_0000181> ;
    skos:definition "The energy level in a semiconductor where the probability of finding an electron is 0.5."@en ;
    skos:historyNote "0000-0002-6242-2167 Nikolaos G. Moustakas created the resource"@en ;
    skos:inScheme <https://w3id.org/nfdi4cat/voc4cat> ;
    skos:prefLabel "Fermi level"@en .

<https://w3id.org/nfdi4cat/voc4cat_0000008> a skos:Concept ;
    dcterms:identifier "voc4cat_0000008"^^xsd:token ;
    skos:broader <https://w3id.org/nfdi4cat/voc4cat_0000186> ;
    skos:definition "The degree of a three-dimensional structural order of atoms which constitute the crystal lattice of a material."@en ;
    skos:historyNote "0000-0002-6242-2167 Nikolaos G. Moustakas created the resource"@en ;
    skos:inScheme <https://w3id.org/nfdi4cat/voc4cat> ;
    skos:prefLabel "crystallinity"@en .

<https://w3id.org/nfdi4cat/voc4cat_0000009> a skos:Concept ;
    dcterms:identifier "voc4cat_0000009"^^xsd:token ;
    skos:broader <https://w3id.org/nfdi4cat/voc4cat_0000186> ;
    skos:definition "The range of pore sizes in a material."@en ;
    skos:historyNote "0000-0002-6242-2167 Nikolaos G. Moustakas created the resource"@en ;
    skos:inScheme <https://w3id.org/nfdi4cat/voc4cat> ;
    skos:prefLabel "pore size distribution"@en .

<https://w3id.org/nfdi4cat/voc4cat_0000010> a skos:Concept ;
    dcterms:identifier "voc4cat_0000010"^^xsd:token ;
    skos:altLabel "Eg"@en,
        "energy bandgap"@en ;
    skos:broader <https://w3id.org/nfdi4cat/voc4cat_0000186> ;
    skos:definition "The energy difference between a semiconductor’s valence band top and conduction band bottom, which is required to excite an electron from the former to the latter."@en ;
    skos:historyNote "0000-0002-6242-2167 Nikolaos G. Moustakas created the resource"@en ;
    skos:inScheme <https://w3id.org/nfdi4cat/voc4cat> ;
    skos:prefLabel "bandgap energy"@en .

<https://w3id.org/nfdi4cat/voc4cat_0000011> a skos:Concept ;
    dcterms:identifier "voc4cat_0000011"^^xsd:token ;
    skos:altLabel "VB"@en ;
    skos:broader <https://w3id.org/nfdi4cat/voc4cat_0000181> ;
    skos:definition "The band of energy levels in a solid fully occupied by electrons at 0 K (273.15 °C)."@en ;
    skos:historyNote "0000-0002-6242-2167 Nikolaos G. Moustakas created the resource"@en ;
    skos:inScheme <https://w3id.org/nfdi4cat/voc4cat> ;
    skos:prefLabel "valence band"@en .

<https://w3id.org/nfdi4cat/voc4cat_0000012> a skos:Concept ;
    dcterms:identifier "voc4cat_0000012"^^xsd:token ;
    skos:altLabel "CB"@en ;
    skos:broader <https://w3id.org/nfdi4cat/voc4cat_0000181> ;
    skos:definition "The energy band of electronic levels of partially or fully filled mobile electrons in a metal or a semiconductor."@en ;
    skos:historyNote "0000-0002-6242-2167 Nikolaos G. Moustakas created the resource"@en ;
    skos:inScheme <https://w3id.org/nfdi4cat/voc4cat> ;
    skos:prefLabel "conduction band"@en .

<https://w3id.org/nfdi4cat/voc4cat_0000013> a skos:Concept ;
    dcterms:identifier "voc4cat_0000013"^^xsd:token ;
    skos:altLabel "SSA"@en ;
    skos:broader <https://w3id.org/nfdi4cat/voc4cat_0000186> ;
    skos:definition "Α measure of the total surface area of a material per unit mass or volume."@en ;
    skos:historyNote "0000-0002-6242-2167 Nikolaos G. Moustakas created the resource"@en ;
    skos:inScheme <https://w3id.org/nfdi4cat/voc4cat> ;
    skos:prefLabel "specific surface area"@en .

<https://w3id.org/nfdi4cat/voc4cat_0000017> a skos:Concept ;
    dcterms:identifier "voc4cat_0000017"^^xsd:token ;
    skos:broader <https://w3id.org/nfdi4cat/voc4cat_0000194> ;
    skos:definition "A catalyst introduced to the reaction chamber in the form of a powder."@en ;
    skos:historyNote "0000-0002-6242-2167 Nikolaos G. Moustakas created the resource"@en ;
    skos:inScheme <https://w3id.org/nfdi4cat/voc4cat> ;
    skos:prefLabel "powdered catalyst"@en .

<https://w3id.org/nfdi4cat/voc4cat_0000018> a skos:Concept ;
    dcterms:identifier "voc4cat_0000018"^^xsd:token ;
    skos:broader <https://w3id.org/nfdi4cat/voc4cat_0000186> ;
    skos:definition "Mass of a powdered catalyst used for an experiment."@en ;
    skos:historyNote "0000-0002-6242-2167 Nikolaos G. Moustakas created the resource"@en ;
    skos:inScheme <https://w3id.org/nfdi4cat/voc4cat> ;
    skos:prefLabel "powder mass"@en .

<https://w3id.org/nfdi4cat/voc4cat_0000021> a skos:Concept ;
    dcterms:identifier "voc4cat_0000021"^^xsd:token ;
    skos:altLabel "spray-coating"@en ;
    skos:broader <https://w3id.org/nfdi4cat/voc4cat_0000020> ;
    skos:definition "A technique used to deposit uniform thin films onto a substrate by spraying a solution of the material onto the surface."@en ;
    skos:historyNote "0000-0002-6242-2167 Nikolaos G. Moustakas created the resource"@en ;
    skos:inScheme <https://w3id.org/nfdi4cat/voc4cat> ;
    skos:prefLabel "spray coating"@en .

<https://w3id.org/nfdi4cat/voc4cat_0000022> a skos:Concept ;
    dcterms:identifier "voc4cat_0000022"^^xsd:token ;
    skos:broader <https://w3id.org/nfdi4cat/voc4cat_0000020> ;
    skos:definition "A tape-casting method used to deposit thin films of a catalyst onto the surface of a substrate."@en ;
    skos:historyNote "0000-0002-6242-2167 Nikolaos G. Moustakas created the resource"@en ;
    skos:inScheme <https://w3id.org/nfdi4cat/voc4cat> ;
    skos:prefLabel "doctor blading"@en .

<https://w3id.org/nfdi4cat/voc4cat_0000023> a skos:Concept ;
    dcterms:identifier "voc4cat_0000023"^^xsd:token ;
    skos:altLabel "spin casting"@en,
        "spin-casting"@en,
        "spin-coating"@en ;
    skos:broader <https://w3id.org/nfdi4cat/voc4cat_0000020> ;
    skos:definition "A technique used to deposit uniform thin films onto a substrate (e.g., metal or glass) by spinning at high speeds a solution (paste) of the material onto the surface."@en ;
    skos:historyNote "0000-0002-6242-2167 Nikolaos G. Moustakas created the resource"@en ;
    skos:inScheme <https://w3id.org/nfdi4cat/voc4cat> ;
    skos:prefLabel "spin coating"@en .

<https://w3id.org/nfdi4cat/voc4cat_0000025> a skos:Concept ;
    dcterms:identifier "voc4cat_0000025"^^xsd:token ;
    skos:broader <https://w3id.org/nfdi4cat/voc4cat_0000186> ;
    skos:definition "The material that the substrate is made of. Common materials include: glass (conductive or not), ceramics and metal."@en ;
    skos:historyNote "0000-0002-6242-2167 Nikolaos G. Moustakas created the resource"@en ;
    skos:inScheme <https://w3id.org/nfdi4cat/voc4cat> ;
    skos:prefLabel "substrate material"@en .

<https://w3id.org/nfdi4cat/voc4cat_0000026> a skos:Concept ;
    dcterms:identifier "voc4cat_0000026"^^xsd:token ;
    skos:broader <https://w3id.org/nfdi4cat/voc4cat_0000024> ;
    skos:definition "A flat surface made of a metal (e.g., titanium, stainless steel) serving as a substrate for the deposition of a catalyst."@en ;
    skos:historyNote "0000-0002-6242-2167 Nikolaos G. Moustakas created the resource"@en ;
    skos:inScheme <https://w3id.org/nfdi4cat/voc4cat> ;
    skos:prefLabel "metallic substrate"@en .

<https://w3id.org/nfdi4cat/voc4cat_0000028> a skos:Concept ;
    dcterms:identifier "voc4cat_0000028"^^xsd:token ;
    skos:altLabel "FTO"@en,
        "FTO glass"@en ;
    skos:broader <https://w3id.org/nfdi4cat/voc4cat_0000027> ;
    skos:definition "Transparent conductive metal oxide (fluorine doped tin oxide) that can be used in the fabrication of transparent electrodes for thin films."@en ;
    skos:historyNote "0000-0002-6242-2167 Nikolaos G. Moustakas created the resource"@en ;
    skos:inScheme <https://w3id.org/nfdi4cat/voc4cat> ;
    skos:prefLabel "fluorine doped tin oxide coated glass"@en .

<https://w3id.org/nfdi4cat/voc4cat_0000029> a skos:Concept ;
    dcterms:identifier "voc4cat_0000029"^^xsd:token ;
    skos:altLabel "ITO"@en,
        "ITO glass"@en ;
    skos:broader <https://w3id.org/nfdi4cat/voc4cat_0000027> ;
    skos:definition "Transparent conductive metal oxide (indium tin oxide) that can be used in the fabrication of transparent electrodes for thin films."@en ;
    skos:historyNote "0000-0002-6242-2167 Nikolaos G. Moustakas created the resource"@en ;
    skos:inScheme <https://w3id.org/nfdi4cat/voc4cat> ;
    skos:prefLabel "indium tin oxide coated glass"@en .

<https://w3id.org/nfdi4cat/voc4cat_0000030> a skos:Concept ;
    dcterms:identifier "voc4cat_0000030"^^xsd:token ;
    skos:broader <https://w3id.org/nfdi4cat/voc4cat_0000027> ;
    skos:definition "A resistant to thermal shock type of glass, composed mainly of silica and boron trioxide."@en ;
    skos:historyNote "0000-0002-6242-2167 Nikolaos G. Moustakas created the resource"@en ;
    skos:inScheme <https://w3id.org/nfdi4cat/voc4cat> ;
    skos:prefLabel "borosilicate glass"@en .

<https://w3id.org/nfdi4cat/voc4cat_0000031> a skos:Concept ;
    dcterms:identifier "voc4cat_0000031"^^xsd:token ;
    skos:altLabel "quartz"@en ;
    skos:broader <https://w3id.org/nfdi4cat/voc4cat_0000027> ;
    skos:definition "A type of pure silicon dioxide, highly crystalline glass that allows the transmission of light in the UV wavelength range."@en ;
    skos:historyNote "0000-0002-6242-2167 Nikolaos G. Moustakas created the resource"@en ;
    skos:inScheme <https://w3id.org/nfdi4cat/voc4cat> ;
    skos:prefLabel "quartz glass"@en .

<https://w3id.org/nfdi4cat/voc4cat_0000032> a skos:Concept ;
    dcterms:identifier "voc4cat_0000032"^^xsd:token ;
    skos:broader <https://w3id.org/nfdi4cat/voc4cat_0000024> ;
    skos:definition "A surface made of a ceramic material (e.g., alumina) serving as a substrate for the deposition of a catalyst."@en ;
    skos:historyNote "0000-0002-6242-2167 Nikolaos G. Moustakas created the resource"@en ;
    skos:inScheme <https://w3id.org/nfdi4cat/voc4cat> ;
    skos:prefLabel "ceramic substrate"@en .

<https://w3id.org/nfdi4cat/voc4cat_0000034> a skos:Concept ;
    dcterms:identifier "voc4cat_0000034"^^xsd:token ;
    skos:broader <https://w3id.org/nfdi4cat/voc4cat_0000033> ;
    skos:definition "The width of the substrate."@en ;
    skos:historyNote "0000-0002-6242-2167 Nikolaos G. Moustakas created the resource"@en ;
    skos:inScheme <https://w3id.org/nfdi4cat/voc4cat> ;
    skos:prefLabel "substrate width"@en .

<https://w3id.org/nfdi4cat/voc4cat_0000035> a skos:Concept ;
    dcterms:identifier "voc4cat_0000035"^^xsd:token ;
    skos:broader <https://w3id.org/nfdi4cat/voc4cat_0000033> ;
    skos:definition "The depth of the substrate."@en ;
    skos:historyNote "0000-0002-6242-2167 Nikolaos G. Moustakas created the resource"@en ;
    skos:inScheme <https://w3id.org/nfdi4cat/voc4cat> ;
    skos:prefLabel "substrate depth"@en .

<https://w3id.org/nfdi4cat/voc4cat_0000036> a skos:Concept ;
    dcterms:identifier "voc4cat_0000036"^^xsd:token ;
    skos:broader <https://w3id.org/nfdi4cat/voc4cat_0000033> ;
    skos:definition "The thickness of the substrate."@en ;
    skos:historyNote "0000-0002-6242-2167 Nikolaos G. Moustakas created the resource"@en ;
    skos:inScheme <https://w3id.org/nfdi4cat/voc4cat> ;
    skos:prefLabel "substrate thickness"@en .

<https://w3id.org/nfdi4cat/voc4cat_0000038> a skos:Concept ;
    dcterms:identifier "voc4cat_0000038"^^xsd:token ;
    skos:broader <https://w3id.org/nfdi4cat/voc4cat_0000194> ;
    skos:definition "A thin film of the catalyst deposited on an appropriate for the application substrate."@en ;
    skos:historyNote "0000-0002-6242-2167 Nikolaos G. Moustakas created the resource"@en ;
    skos:inScheme <https://w3id.org/nfdi4cat/voc4cat> ;
    skos:prefLabel "deposited sample"@en .

<https://w3id.org/nfdi4cat/voc4cat_0000039> a skos:Concept ;
    dcterms:identifier "voc4cat_0000039"^^xsd:token ;
    skos:broader <https://w3id.org/nfdi4cat/voc4cat_0000186> ;
    skos:definition "Mass of catalyst deposited onto the surface of a substrate."@en ;
    skos:historyNote "0000-0002-6242-2167 Nikolaos G. Moustakas created the resource"@en ;
    skos:inScheme <https://w3id.org/nfdi4cat/voc4cat> ;
    skos:prefLabel "thin film mass"@en .

<https://w3id.org/nfdi4cat/voc4cat_0000041> a skos:Concept ;
    dcterms:identifier "voc4cat_0000041"^^xsd:token ;
    skos:broader <https://w3id.org/nfdi4cat/voc4cat_0000040> ;
    skos:definition "The width of the film of the deposited catalyst."@en ;
    skos:historyNote "0000-0002-6242-2167 Nikolaos G. Moustakas created the resource"@en ;
    skos:inScheme <https://w3id.org/nfdi4cat/voc4cat> ;
    skos:prefLabel "thin film width"@en .

<https://w3id.org/nfdi4cat/voc4cat_0000042> a skos:Concept ;
    dcterms:identifier "voc4cat_0000042"^^xsd:token ;
    skos:broader <https://w3id.org/nfdi4cat/voc4cat_0000040> ;
    skos:definition "The thickness of the film of the deposited catalyst."@en ;
    skos:historyNote "0000-0002-6242-2167 Nikolaos G. Moustakas created the resource"@en ;
    skos:inScheme <https://w3id.org/nfdi4cat/voc4cat> ;
    skos:prefLabel "thin film thickness"@en .

<https://w3id.org/nfdi4cat/voc4cat_0000043> a skos:Concept ;
    dcterms:identifier "voc4cat_0000043"^^xsd:token ;
    skos:broader <https://w3id.org/nfdi4cat/voc4cat_0000040> ;
    skos:definition "The depth of the film of the deposited catalyst."@en ;
    skos:historyNote "0000-0002-6242-2167 Nikolaos G. Moustakas created the resource"@en ;
    skos:inScheme <https://w3id.org/nfdi4cat/voc4cat> ;
    skos:prefLabel "thin film depth"@en .

<https://w3id.org/nfdi4cat/voc4cat_0000044> a skos:Concept ;
    dcterms:identifier "voc4cat_0000044"^^xsd:token ;
    skos:broader <https://w3id.org/nfdi4cat/voc4cat_0000040> ;
    skos:definition "The area of the substrate covered by the deposited catalyst."@en ;
    skos:historyNote "0000-0002-6242-2167 Nikolaos G. Moustakas created the resource"@en ;
    skos:inScheme <https://w3id.org/nfdi4cat/voc4cat> ;
    skos:prefLabel "thin film area"@en .

<https://w3id.org/nfdi4cat/voc4cat_0000045> a skos:Concept ;
    dcterms:identifier "voc4cat_0000045"^^xsd:token ;
    skos:broader <https://w3id.org/nfdi4cat/voc4cat_0000185> ;
    skos:definition "The process by which one or more chemical reactions are performed with the aim of converting a reactant or starting material into a product or multiple products."@en ;
    skos:historyNote "0000-0002-6242-2167 Nikolaos G. Moustakas created the resource"@en ;
    skos:inScheme <https://w3id.org/nfdi4cat/voc4cat> ;
    skos:prefLabel "synthesis"@en .

<https://w3id.org/nfdi4cat/voc4cat_0000047> a skos:Concept ;
    dcterms:identifier "voc4cat_0000047"^^xsd:token ;
    skos:broader <https://w3id.org/nfdi4cat/voc4cat_0000046> ;
    skos:definition "Assembly of literature research to include only the most relevant sources of information for the application / experiment / catalysts of interest."@en ;
    skos:historyNote "0000-0002-6242-2167 Nikolaos G. Moustakas created the resource"@en ;
    skos:inScheme <https://w3id.org/nfdi4cat/voc4cat> ;
    skos:prefLabel "literature collection"@en .

<https://w3id.org/nfdi4cat/voc4cat_0000048> a skos:Concept ;
    dcterms:identifier "voc4cat_0000048"^^xsd:token ;
    skos:broader <https://w3id.org/nfdi4cat/voc4cat_0000046> ;
    skos:definition "Addition and organization of relevant literature of interest using a citation management software (e.g., Mendeley, Zotero, EndNote etc.) allowing for easy access and categorization."@en ;
    skos:historyNote "0000-0002-6242-2167 Nikolaos G. Moustakas created the resource"@en ;
    skos:inScheme <https://w3id.org/nfdi4cat/voc4cat> ;
    skos:prefLabel "literature organization"@en .

<https://w3id.org/nfdi4cat/voc4cat_0000050> a skos:Concept ;
    dcterms:identifier "voc4cat_0000050"^^xsd:token ;
    skos:broader <https://w3id.org/nfdi4cat/voc4cat_0000186> ;
    skos:definition "Duration of each synthesis step needed to synthesize the desired catalyst."@en ;
    skos:historyNote "0000-0002-6242-2167 Nikolaos G. Moustakas created the resource"@en ;
    skos:inScheme <https://w3id.org/nfdi4cat/voc4cat> ;
    skos:prefLabel "synthesis duration"@en .

<https://w3id.org/nfdi4cat/voc4cat_0000051> a skos:Concept ;
    dcterms:identifier "voc4cat_0000051"^^xsd:token ;
    skos:broader <https://w3id.org/nfdi4cat/voc4cat_0000186> ;
    skos:definition "Temperature externally applied (if necessary) in any of the synthesis step. Higher temperature values can be observed if an exothermic reaction takes place during the synthesis."@en ;
    skos:historyNote "0000-0002-6242-2167 Nikolaos G. Moustakas created the resource"@en ;
    skos:inScheme <https://w3id.org/nfdi4cat/voc4cat> ;
    skos:prefLabel "synthesis temperature"@en .

<https://w3id.org/nfdi4cat/voc4cat_0000052> a skos:Concept ;
    dcterms:identifier "voc4cat_0000052"^^xsd:token ;
    skos:broader <https://w3id.org/nfdi4cat/voc4cat_0000186> ;
    skos:definition "The pH value in each of the synthesis steps."@en ;
    skos:historyNote "0000-0002-6242-2167 Nikolaos G. Moustakas created the resource"@en ;
    skos:inScheme <https://w3id.org/nfdi4cat/voc4cat> ;
    skos:prefLabel "synthesis pH"@en .

<https://w3id.org/nfdi4cat/voc4cat_0000053> a skos:Concept ;
    dcterms:identifier "voc4cat_0000053"^^xsd:token ;
    skos:broader <https://w3id.org/nfdi4cat/voc4cat_0000186> ;
    skos:definition "Pressure applied (if necessary) in any of the synthesis step. Changes in the pressure may be observed if variations in the temperature of the reaction occur (e.g., exothermic reaction)."@en ;
    skos:historyNote "0000-0002-6242-2167 Nikolaos G. Moustakas created the resource"@en ;
    skos:inScheme <https://w3id.org/nfdi4cat/voc4cat> ;
    skos:prefLabel "synthesis pressure"@en .

<https://w3id.org/nfdi4cat/voc4cat_0000054> a skos:Concept ;
    dcterms:identifier "voc4cat_0000054"^^xsd:token ;
    skos:altLabel "calcination"@en,
        "heat treatment"@en,
        "heat-treatment"@en ;
    skos:broader <https://w3id.org/nfdi4cat/voc4cat_0000186> ;
    skos:definition "Heat treatment to reach the desired final catalyst. The parameters of the heat treatment can vary between each calcination step."@en ;
    skos:historyNote "0000-0002-6242-2167 Nikolaos G. Moustakas created the resource"@en ;
    skos:inScheme <https://w3id.org/nfdi4cat/voc4cat> ;
    skos:prefLabel "calcination step"@en .

<https://w3id.org/nfdi4cat/voc4cat_0000055> a skos:Concept ;
    dcterms:identifier "voc4cat_0000055"^^xsd:token ;
    skos:altLabel "gaseous environment in calcination"@en ;
    skos:broader <https://w3id.org/nfdi4cat/voc4cat_0000181> ;
    skos:definition "A gas flow under which the calcination step takes place (e,g,, Ar or synthetic air)."@en ;
    skos:historyNote "0000-0002-6242-2167 Nikolaos G. Moustakas created the resource"@en ;
    skos:inScheme <https://w3id.org/nfdi4cat/voc4cat> ;
    skos:prefLabel "calcination gaseous environment"@en .

<https://w3id.org/nfdi4cat/voc4cat_0000056> a skos:Concept ;
    dcterms:identifier "voc4cat_0000056"^^xsd:token ;
    skos:altLabel "gas flow rate in calcination"@en ;
    skos:broader <https://w3id.org/nfdi4cat/voc4cat_0000186> ;
    skos:definition "The flow of gas (usually in ml min-1) used in the calcination steps during synthesis."@en ;
    skos:historyNote "0000-0002-6242-2167 Nikolaos G. Moustakas created the resource"@en ;
    skos:inScheme <https://w3id.org/nfdi4cat/voc4cat> ;
    skos:prefLabel "calcincation gas flow rate"@en .

<https://w3id.org/nfdi4cat/voc4cat_0000057> a skos:Concept ;
    dcterms:identifier "voc4cat_0000057"^^xsd:token ;
    skos:broader <https://w3id.org/nfdi4cat/voc4cat_0000186> ;
    skos:definition "Initial temperature of the calcination step."@en ;
    skos:historyNote "0000-0002-6242-2167 Nikolaos G. Moustakas created the resource"@en ;
    skos:inScheme <https://w3id.org/nfdi4cat/voc4cat> ;
    skos:prefLabel "calcination initial temperature"@en .

<https://w3id.org/nfdi4cat/voc4cat_0000058> a skos:Concept ;
    dcterms:identifier "voc4cat_0000058"^^xsd:token ;
    skos:broader <https://w3id.org/nfdi4cat/voc4cat_0000186> ;
    skos:definition "Final temperature of the calcination step."@en ;
    skos:historyNote "0000-0002-6242-2167 Nikolaos G. Moustakas created the resource"@en ;
    skos:inScheme <https://w3id.org/nfdi4cat/voc4cat> ;
    skos:prefLabel "calcination final temperature"@en .

<https://w3id.org/nfdi4cat/voc4cat_0000059> a skos:Concept ;
    dcterms:identifier "voc4cat_0000059"^^xsd:token ;
    skos:broader <https://w3id.org/nfdi4cat/voc4cat_0000186> ;
    skos:definition "Rate of increasing or decreasing the temperature during the calcination step. Usually mentioned in K min-1."@en ;
    skos:historyNote "0000-0002-6242-2167 Nikolaos G. Moustakas created the resource"@en ;
    skos:inScheme <https://w3id.org/nfdi4cat/voc4cat> ;
    skos:prefLabel "calcination heating rate"@en .

<https://w3id.org/nfdi4cat/voc4cat_0000060> a skos:Concept ;
    dcterms:identifier "voc4cat_0000060"^^xsd:token ;
    skos:broader <https://w3id.org/nfdi4cat/voc4cat_0000186> ;
    skos:definition "Time (usually in h) for which a desired temperature is held."@en ;
    skos:historyNote "0000-0002-6242-2167 Nikolaos G. Moustakas created the resource"@en ;
    skos:inScheme <https://w3id.org/nfdi4cat/voc4cat> ;
    skos:prefLabel "calcination dwelling time"@en .

<https://w3id.org/nfdi4cat/voc4cat_0000061> a skos:Concept ;
    dcterms:identifier "voc4cat_0000061"^^xsd:token ;
    skos:broader <https://w3id.org/nfdi4cat/voc4cat_0000187> ;
    skos:definition "Equipment used in each step of the synthesis of the catalysts. The equipment can include (but not limited to): crucibles, pH meters, condensers, volumetric cylinders, centrifuges, test tubes, flasks, beakers, mechanical shakers, pipettes, syringes, magnetic stirrers, heating plates, filters, funnels, and digital balances."@en ;
    skos:historyNote "0000-0002-6242-2167 Nikolaos G. Moustakas created the resource"@en ;
    skos:inScheme <https://w3id.org/nfdi4cat/voc4cat> ;
    skos:prefLabel "synthesis equipment"@en .

<https://w3id.org/nfdi4cat/voc4cat_0000062> a skos:Concept ;
    dcterms:identifier "voc4cat_0000062"^^xsd:token ;
    skos:broader <https://w3id.org/nfdi4cat/voc4cat_0000181> ;
    skos:definition "Chemical substances used in the synthesis process of a desired catalyst."@en ;
    skos:historyNote "0000-0002-6242-2167 Nikolaos G. Moustakas created the resource"@en ;
    skos:inScheme <https://w3id.org/nfdi4cat/voc4cat> ;
    skos:prefLabel "chemical substance for synthesis"@en .

<https://w3id.org/nfdi4cat/voc4cat_0000063> a skos:Concept ;
    dcterms:identifier "voc4cat_0000063"^^xsd:token ;
    skos:broader <https://w3id.org/nfdi4cat/voc4cat_0000186> ;
    skos:definition "Mass of chemicals used for synthesis."@en ;
    skos:historyNote "0000-0002-6242-2167 Nikolaos G. Moustakas created the resource"@en ;
    skos:inScheme <https://w3id.org/nfdi4cat/voc4cat> ;
    skos:prefLabel "mass of chemical substance for synthesis"@en .

<https://w3id.org/nfdi4cat/voc4cat_0000064> a skos:Concept ;
    dcterms:identifier "voc4cat_0000064"^^xsd:token ;
    skos:broader <https://w3id.org/nfdi4cat/voc4cat_0000186> ;
    skos:definition "Volume of chemicals used for synthesis."@en ;
    skos:historyNote "0000-0002-6242-2167 Nikolaos G. Moustakas created the resource"@en ;
    skos:inScheme <https://w3id.org/nfdi4cat/voc4cat> ;
    skos:prefLabel "volume of chemical substance for synthesis"@en .

<https://w3id.org/nfdi4cat/voc4cat_0000065> a skos:Concept ;
    dcterms:identifier "voc4cat_0000065"^^xsd:token ;
    skos:broader <https://w3id.org/nfdi4cat/voc4cat_0000186> ;
    skos:definition "Concentration of chemicals used for synthesis."@en ;
    skos:historyNote "0000-0002-6242-2167 Nikolaos G. Moustakas created the resource"@en ;
    skos:inScheme <https://w3id.org/nfdi4cat/voc4cat> ;
    skos:prefLabel "concentration of chemical substance for synthesis"@en .

<https://w3id.org/nfdi4cat/voc4cat_0000085> a skos:Concept ;
    dcterms:identifier "voc4cat_0000085"^^xsd:token ;
    skos:broader <https://w3id.org/nfdi4cat/voc4cat_0000084> ;
    skos:definition "Τhe lowest energy state of a system."@en ;
    skos:historyNote "0000-0002-6242-2167 Nikolaos G. Moustakas created the resource"@en ;
    skos:inScheme <https://w3id.org/nfdi4cat/voc4cat> ;
    skos:prefLabel "ground state"@en .

<https://w3id.org/nfdi4cat/voc4cat_0000086> a skos:Concept ;
    dcterms:identifier "voc4cat_0000086"^^xsd:token ;
    skos:broader <https://w3id.org/nfdi4cat/voc4cat_0000084> ;
    skos:definition "Τhe temporary state of a system with higher energy than its ground state caused by an external factor."@en ;
    skos:historyNote "0000-0002-6242-2167 Nikolaos G. Moustakas created the resource"@en ;
    skos:inScheme <https://w3id.org/nfdi4cat/voc4cat> ;
    skos:prefLabel "excited state"@en .

<https://w3id.org/nfdi4cat/voc4cat_0000087> a skos:Concept ;
    dcterms:identifier "voc4cat_0000087"^^xsd:token ;
    skos:broader <https://w3id.org/nfdi4cat/voc4cat_0000185> ;
    skos:definition "A multi-step process iniatiated by the absorption of photons by a photocatalyst. This process involves various sub-processes that include the photogeneration and transfer of electron and hole pairs."@en ;
    skos:historyNote "0000-0002-6242-2167 Nikolaos G. Moustakas created the resource"@en ;
    skos:inScheme <https://w3id.org/nfdi4cat/voc4cat> ;
    skos:prefLabel "photocatalytic process"@en .

<https://w3id.org/nfdi4cat/voc4cat_0000088> a skos:Concept ;
    dcterms:identifier "voc4cat_0000088"^^xsd:token ;
    skos:broader <https://w3id.org/nfdi4cat/voc4cat_0000183> ;
    skos:definition "The transfer of an electron initiated by the absorption of a photon of sufficient energy."@en ;
    skos:historyNote "0000-0002-6242-2167 Nikolaos G. Moustakas created the resource, 0000-0002-2367-1988 Norbert Kockmann edited the resource"@en ;
    skos:inScheme <https://w3id.org/nfdi4cat/voc4cat> ;
    skos:prefLabel "photoinduced electron transfer"@en .

<https://w3id.org/nfdi4cat/voc4cat_0000089> a skos:Concept ;
    dcterms:identifier "voc4cat_0000089"^^xsd:token ;
    skos:broader <https://w3id.org/nfdi4cat/voc4cat_0000183> ;
    skos:definition "The transfer of a hole initiated by the absorption of a photon of sufficient energy."@en ;
    skos:historyNote "0000-0002-6242-2167 Nikolaos G. Moustakas created the resource"@en ;
    skos:inScheme <https://w3id.org/nfdi4cat/voc4cat> ;
    skos:prefLabel "photoinduced hole transfer"@en .

<https://w3id.org/nfdi4cat/voc4cat_0000090> a skos:Concept ;
    dcterms:identifier "voc4cat_0000090"^^xsd:token ;
    skos:altLabel "charge photo-generation"@en,
        "charge photogeneration"@en,
        "electron excitation"@en,
        "electron-hole pair"@en,
        "photogenerated charges"@en ;
    skos:broader <https://w3id.org/nfdi4cat/voc4cat_0000183> ;
    skos:definition "The generation of electron - hole pairs in a semiconductor as a result of light absorption of sufficient energy to overcome the bandgap energy. Electrons (negative charge) get excited to the conduction band, while holes (positive charge) remain in the valence band."@en ;
    skos:historyNote "0000-0002-6242-2167 Nikolaos G. Moustakas created the resource"@en ;
    skos:inScheme <https://w3id.org/nfdi4cat/voc4cat> ;
    skos:prefLabel "photoinduced charge generation"@en .

<https://w3id.org/nfdi4cat/voc4cat_0000091> a skos:Concept ;
    dcterms:identifier "voc4cat_0000091"^^xsd:token ;
    skos:broader <https://w3id.org/nfdi4cat/voc4cat_0000183> ;
    skos:definition "The process by which photogenerated charges (electrons and holes) in a semiconductor recombine, resulting in the dissipation of energy in the form of e.g., heat or light."@en ;
    skos:historyNote "0000-0002-6242-2167 Nikolaos G. Moustakas created the resource"@en ;
    skos:inScheme <https://w3id.org/nfdi4cat/voc4cat> ;
    skos:prefLabel "charge recombination"@en .

<https://w3id.org/nfdi4cat/voc4cat_0000092> a skos:Concept ;
    dcterms:identifier "voc4cat_0000092"^^xsd:token ;
    skos:broader <https://w3id.org/nfdi4cat/voc4cat_0000183> ;
    skos:definition "Absorption is the process in which energy (e.g., photons) or an absorbent (e.g., a gas) is taken up by an absorbate."@en ;
    skos:historyNote "0000-0002-6242-2167 Nikolaos G. Moustakas created the resource"@en ;
    skos:inScheme <https://w3id.org/nfdi4cat/voc4cat> ;
    skos:prefLabel "absorption"@en .

<https://w3id.org/nfdi4cat/voc4cat_0000094> a skos:Concept ;
    dcterms:identifier "voc4cat_0000094"^^xsd:token ;
    skos:broader <https://w3id.org/nfdi4cat/voc4cat_0000183> ;
    skos:definition "The process under which reactants, intermediates and products are released from the surface of the catalyst. Desorption can be facilitated by an increase in temperature or a change in the pH."@en ;
    skos:historyNote "0000-0002-6242-2167 Nikolaos G. Moustakas created the resource"@en ;
    skos:inScheme <https://w3id.org/nfdi4cat/voc4cat> ;
    skos:prefLabel "desorption"@en .

<https://w3id.org/nfdi4cat/voc4cat_0000095> a skos:Concept ;
    dcterms:identifier "voc4cat_0000095"^^xsd:token ;
    skos:broader <https://w3id.org/nfdi4cat/voc4cat_0000183> ;
    skos:definition "The process of separating positive and negative charges in a semiconductor, typically as a result of an external force, (e.g., photoexcitation)."@en ;
    skos:historyNote "0000-0002-6242-2167 Nikolaos G. Moustakas created the resource"@en ;
    skos:inScheme <https://w3id.org/nfdi4cat/voc4cat> ;
    skos:prefLabel "charge separation"@en .

<https://w3id.org/nfdi4cat/voc4cat_0000096> a skos:Concept ;
    dcterms:identifier "voc4cat_0000096"^^xsd:token ;
    skos:altLabel "photo-excitation"@en ;
    skos:broader <https://w3id.org/nfdi4cat/voc4cat_0000183> ;
    skos:definition "The state caused by the transition of electrons from the valence band top to the conduction band bottom by absorption of photons of sufficient energy."@en ;
    skos:historyNote "0000-0002-6242-2167 Nikolaos G. Moustakas created the resource"@en ;
    skos:inScheme <https://w3id.org/nfdi4cat/voc4cat> ;
    skos:prefLabel "photoexcitation"@en .

<https://w3id.org/nfdi4cat/voc4cat_0000099> a skos:Concept ;
    dcterms:identifier "voc4cat_0000099"^^xsd:token ;
    skos:altLabel "CO2 photoreduction"@en,
        "artificial photosynthesis"@en,
        "carbon dioxide photoreduction"@en,
        "photocatalytic carbon dioxide reduction"@en ;
    skos:broader <https://w3id.org/nfdi4cat/voc4cat_0000185> ;
    skos:definition "The light-driven reduction (conversion) of carbon dioxide (CO2) to hydrocarbons and / or platform chemicals in presence of water. The absorption of light and the adsorption of the reactants is performed by a photocatalyst (usually a metal oxide)."@en ;
    skos:historyNote "0000-0002-6242-2167 Nikolaos G. Moustakas created the resource"@en ;
    skos:inScheme <https://w3id.org/nfdi4cat/voc4cat> ;
    skos:prefLabel "photocatalytic CO2 reduction"@en .

<https://w3id.org/nfdi4cat/voc4cat_0000100> a skos:Concept ;
    dcterms:identifier "voc4cat_0000100"^^xsd:token ;
    skos:broader <https://w3id.org/nfdi4cat/voc4cat_0000185> ;
    skos:definition "A lab-scale experiment performed to test the efficiency of a studied photocatalyst in a photocatalytic application."@en ;
    skos:historyNote "0000-0002-6242-2167 Nikolaos G. Moustakas created the resource"@en ;
    skos:inScheme <https://w3id.org/nfdi4cat/voc4cat> ;
    skos:prefLabel "photocatalytic experiment"@en .

<https://w3id.org/nfdi4cat/voc4cat_0000101> a skos:Concept ;
    dcterms:identifier "voc4cat_0000101"^^xsd:token ;
    skos:broader <https://w3id.org/nfdi4cat/voc4cat_0000181> ;
    skos:definition "A starting substance that undergoes a chemical reaction to produce a desired product."@en ;
    skos:historyNote "0000-0002-6242-2167 Nikolaos G. Moustakas created the resource"@en ;
    skos:inScheme <https://w3id.org/nfdi4cat/voc4cat> ;
    skos:prefLabel "reactant"@en .

<https://w3id.org/nfdi4cat/voc4cat_0000102> a skos:Concept ;
    dcterms:identifier "voc4cat_0000102"^^xsd:token ;
    skos:broader <https://w3id.org/nfdi4cat/voc4cat_0000186> ;
    skos:definition "Concentration of the reactants used to perform an experiment."@en ;
    skos:historyNote "0000-0002-6242-2167 Nikolaos G. Moustakas created the resource"@en ;
    skos:inScheme <https://w3id.org/nfdi4cat/voc4cat> ;
    skos:prefLabel "reactant concentration"@en .

<https://w3id.org/nfdi4cat/voc4cat_0000103> a skos:Concept ;
    dcterms:identifier "voc4cat_0000103"^^xsd:token ;
    skos:broader <https://w3id.org/nfdi4cat/voc4cat_0000186> ;
    skos:definition "Purity of reactants used in an experiment. Purity is a measure of the impurities contained in the reactants' supply. The highest purity reactants should be used to ensure the collection of reliable results."@en ;
    skos:historyNote "0000-0002-6242-2167 Nikolaos G. Moustakas created the resource"@en ;
    skos:inScheme <https://w3id.org/nfdi4cat/voc4cat> ;
    skos:prefLabel "reactant purity"@en .

<https://w3id.org/nfdi4cat/voc4cat_0000104> a skos:Concept ;
    dcterms:identifier "voc4cat_0000104"^^xsd:token ;
    skos:broader <https://w3id.org/nfdi4cat/voc4cat_0000186> ;
    skos:definition "The rate of flow of reactants (often in ml per min) in the photoreactor. Flow rates are usually controlled by mass flow controllers (MFCs)."@en ;
    skos:historyNote "0000-0002-6242-2167 Nikolaos G. Moustakas created the resource"@en ;
    skos:inScheme <https://w3id.org/nfdi4cat/voc4cat> ;
    skos:prefLabel "reactant flow rate"@en .

<https://w3id.org/nfdi4cat/voc4cat_0000106> a skos:Concept ;
    dcterms:identifier "voc4cat_0000106"^^xsd:token ;
    skos:broader <https://w3id.org/nfdi4cat/voc4cat_0000105> ;
    skos:definition "A molecule that accepts electrons from photoexcited species in a redox reaction and is subsequently consumed or degraded."@en ;
    skos:historyNote "0000-0002-6242-2167 Nikolaos G. Moustakas created the resource"@en ;
    skos:inScheme <https://w3id.org/nfdi4cat/voc4cat> ;
    skos:prefLabel "sacrificial acceptor"@en .

<https://w3id.org/nfdi4cat/voc4cat_0000107> a skos:Concept ;
    dcterms:identifier "voc4cat_0000107"^^xsd:token ;
    skos:broader <https://w3id.org/nfdi4cat/voc4cat_0000105> ;
    skos:definition "A molecule that donates electrons from photoexcited species in a redox reaction and is subsequently consumed or degraded."@en ;
    skos:historyNote "0000-0002-6242-2167 Nikolaos G. Moustakas created the resource"@en ;
    skos:inScheme <https://w3id.org/nfdi4cat/voc4cat> ;
    skos:prefLabel "sacrificial donor"@en .

<https://w3id.org/nfdi4cat/voc4cat_0000109> a skos:Concept ;
    dcterms:identifier "voc4cat_0000109"^^xsd:token ;
    skos:altLabel "continuous flow mode"@en,
        "continuous-flow mode"@en,
        "flow mode"@en,
        "flow-mode"@en ;
    skos:broader <https://w3id.org/nfdi4cat/voc4cat_0000108> ;
    skos:definition "Under flow conditions, a continuous flow of reactants is supplied to the reaction chamber and the formed products are removed and identified by an appropriate technique."@en ;
    skos:historyNote "0000-0002-6242-2167 Nikolaos G. Moustakas created the resource"@en ;
    skos:inScheme <https://w3id.org/nfdi4cat/voc4cat> ;
    skos:prefLabel "flow operation"@en .

<https://w3id.org/nfdi4cat/voc4cat_0000110> a skos:Concept ;
    dcterms:identifier "voc4cat_0000110"^^xsd:token ;
    skos:altLabel "batch mode"@en,
        "batch-mode"@en ;
    skos:broader <https://w3id.org/nfdi4cat/voc4cat_0000108> ;
    skos:definition "Operation mode in which the reaction chamber is filled with the (reactant) gas(es) up to a certain pressure, and the reaction products accummulate over time."@en ;
    skos:historyNote "0000-0002-6242-2167 Nikolaos G. Moustakas created the resource"@en ;
    skos:inScheme <https://w3id.org/nfdi4cat/voc4cat> ;
    skos:prefLabel "batch operation"@en .

<https://w3id.org/nfdi4cat/voc4cat_0000111> a skos:Concept ;
    dcterms:identifier "voc4cat_0000111"^^xsd:token ;
    skos:broader <https://w3id.org/nfdi4cat/voc4cat_0000186> ;
    skos:definition "The total duration of an experiment."@en ;
    skos:historyNote "0000-0002-6242-2167 Nikolaos G. Moustakas created the resource"@en ;
    skos:inScheme <https://w3id.org/nfdi4cat/voc4cat> ;
    skos:prefLabel "experiment duration"@en .

<https://w3id.org/nfdi4cat/voc4cat_0000112> a skos:Concept ;
    dcterms:identifier "voc4cat_0000112"^^xsd:token ;
    skos:broader <https://w3id.org/nfdi4cat/voc4cat_0000186> ;
    skos:definition "Time for which a gas is purged through the reaction chamber."@en ;
    skos:historyNote "0000-0002-6242-2167 Nikolaos G. Moustakas created the resource"@en ;
    skos:inScheme <https://w3id.org/nfdi4cat/voc4cat> ;
    skos:prefLabel "purging duration"@en .

<https://w3id.org/nfdi4cat/voc4cat_0000113> a skos:Concept ;
    dcterms:identifier "voc4cat_0000113"^^xsd:token ;
    skos:broader <https://w3id.org/nfdi4cat/voc4cat_0000186> ;
    skos:definition "The time in between the collection of two data points."@en ;
    skos:historyNote "0000-0002-6242-2167 Nikolaos G. Moustakas created the resource"@en ;
    skos:inScheme <https://w3id.org/nfdi4cat/voc4cat> ;
    skos:prefLabel "sampling interval"@en .

<https://w3id.org/nfdi4cat/voc4cat_0000114> a skos:Concept ;
    dcterms:identifier "voc4cat_0000114"^^xsd:token ;
    skos:broader <https://w3id.org/nfdi4cat/voc4cat_0000186> ;
    skos:definition "The total duration in which a catalyst is under irradiation by the selected light source."@en ;
    skos:historyNote "0000-0002-6242-2167 Nikolaos G. Moustakas created the resource"@en ;
    skos:inScheme <https://w3id.org/nfdi4cat/voc4cat> ;
    skos:prefLabel "irradiation duration"@en .

<https://w3id.org/nfdi4cat/voc4cat_0000116> a skos:Concept ;
    dcterms:identifier "voc4cat_0000116"^^xsd:token ;
    skos:broader <https://w3id.org/nfdi4cat/voc4cat_0000115> ;
    skos:definition "The temperature at the initiaton of the experiment."@en ;
    skos:historyNote "0000-0002-6242-2167 Nikolaos G. Moustakas created the resource"@en ;
    skos:inScheme <https://w3id.org/nfdi4cat/voc4cat> ;
    skos:prefLabel "experiment initial temperature"@en .

<https://w3id.org/nfdi4cat/voc4cat_0000117> a skos:Concept ;
    dcterms:identifier "voc4cat_0000117"^^xsd:token ;
    skos:broader <https://w3id.org/nfdi4cat/voc4cat_0000115> ;
    skos:definition "The temperature at the end of the experiment."@en ;
    skos:historyNote "0000-0002-6242-2167 Nikolaos G. Moustakas created the resource"@en ;
    skos:inScheme <https://w3id.org/nfdi4cat/voc4cat> ;
    skos:prefLabel "experiment final temperature"@en .

<https://w3id.org/nfdi4cat/voc4cat_0000119> a skos:Concept ;
    dcterms:identifier "voc4cat_0000119"^^xsd:token ;
    skos:broader <https://w3id.org/nfdi4cat/voc4cat_0000118> ;
    skos:definition "The pressure at the initiaton of the experiment or before a sampling event."@en ;
    skos:historyNote "0000-0002-6242-2167 Nikolaos G. Moustakas created the resource"@en ;
    skos:inScheme <https://w3id.org/nfdi4cat/voc4cat> ;
    skos:prefLabel "experiment initial pressure"@en .

<https://w3id.org/nfdi4cat/voc4cat_0000120> a skos:Concept ;
    dcterms:identifier "voc4cat_0000120"^^xsd:token ;
    skos:broader <https://w3id.org/nfdi4cat/voc4cat_0000118> ;
    skos:definition "The pressure at the end of the experiment or after a sampling event."@en ;
    skos:historyNote "0000-0002-6242-2167 Nikolaos G. Moustakas created the resource"@en ;
    skos:inScheme <https://w3id.org/nfdi4cat/voc4cat> ;
    skos:prefLabel "experiment final pressure"@en .

<https://w3id.org/nfdi4cat/voc4cat_0000121> a skos:Concept ;
    dcterms:identifier "voc4cat_0000121"^^xsd:token ;
    skos:broader <https://w3id.org/nfdi4cat/voc4cat_0000186> ;
    skos:definition "The pressure drop occurring when collecting a gaseous sample from the reaction chamber. This pressure drop should be taken into consideration when calculating the concentration of formed products."@en ;
    skos:historyNote "0000-0002-6242-2167 Nikolaos G. Moustakas created the resource"@en ;
    skos:inScheme <https://w3id.org/nfdi4cat/voc4cat> ;
    skos:prefLabel "experiment pressure drop"@en .

<https://w3id.org/nfdi4cat/voc4cat_0000122> a skos:Concept ;
    dcterms:identifier "voc4cat_0000122"^^xsd:token ;
    skos:altLabel "sample pretreatment"@en ;
    skos:broader <https://w3id.org/nfdi4cat/voc4cat_0000184> ;
    skos:definition "Pre-treatment of a catalyst before its introduction to the reaction chamber."@en ;
    skos:historyNote "0000-0002-6242-2167 Nikolaos G. Moustakas created the resource"@en ;
    skos:inScheme <https://w3id.org/nfdi4cat/voc4cat> ;
    skos:prefLabel "sample pre-treatment"@en .

<https://w3id.org/nfdi4cat/voc4cat_0000123> a skos:Concept ;
    dcterms:identifier "voc4cat_0000123"^^xsd:token ;
    skos:altLabel "control experiment"@en ;
    skos:broader <https://w3id.org/nfdi4cat/voc4cat_0000185> ;
    skos:definition "Measurements performed to ensure that the studied catalytic reaction occurs because of the interaction of the catalyst with the reactants under the selected experimental conditions, and not from the environment or the reactor."@en ;
    skos:historyNote "0000-0002-6242-2167 Nikolaos G. Moustakas created the resource"@en ;
    skos:inScheme <https://w3id.org/nfdi4cat/voc4cat> ;
    skos:prefLabel "blank experiment"@en .

<https://w3id.org/nfdi4cat/voc4cat_0000124> a skos:Concept ;
    dcterms:identifier "voc4cat_0000124"^^xsd:token ;
    skos:broader <https://w3id.org/nfdi4cat/voc4cat_0000184> ;
    skos:definition "Quantitative and qualitative evaluation of the outcome of a catalytic reaction. The evaluation can lead to changes in the synthesis of the catalyst and / or selecting different experimental parameters."@en ;
    skos:historyNote "0000-0002-6242-2167 Nikolaos G. Moustakas created the resource"@en ;
    skos:inScheme <https://w3id.org/nfdi4cat/voc4cat> ;
    skos:prefLabel "evaluation"@en .

<https://w3id.org/nfdi4cat/voc4cat_0000126> a skos:Concept ;
    dcterms:identifier "voc4cat_0000126"^^xsd:token ;
    skos:altLabel "AQY"@en,
        "AQY%"@en,
        "apparent photonic yield"@en ;
    skos:broader <https://w3id.org/nfdi4cat/voc4cat_0000186> ;
    skos:definition "A measure of the efficiency of a photocatalytic reaction. It is expressed as the number of consumed charge carriers divided by the number of incident photons."@en ;
    skos:historyNote "0000-0002-6242-2167 Nikolaos G. Moustakas created the resource"@en ;
    skos:inScheme <https://w3id.org/nfdi4cat/voc4cat> ;
    skos:prefLabel "apparent quantum yield"@en .

<https://w3id.org/nfdi4cat/voc4cat_0000127> a skos:Concept ;
    dcterms:identifier "voc4cat_0000127"^^xsd:token ;
    skos:broader <https://w3id.org/nfdi4cat/voc4cat_0000186> ;
    skos:definition "The concentration (usually in ppm or mol) of the products formed during a reaction."@en ;
    skos:historyNote "0000-0002-6242-2167 Nikolaos G. Moustakas created the resource"@en ;
    skos:inScheme <https://w3id.org/nfdi4cat/voc4cat> ;
    skos:prefLabel "product concentration"@en .

<https://w3id.org/nfdi4cat/voc4cat_0000128> a skos:Concept ;
    dcterms:identifier "voc4cat_0000128"^^xsd:token ;
    skos:altLabel "photoreactor engineering"@en,
        "reactor design"@en,
        "reactor engineering"@en ;
    skos:broader <https://w3id.org/nfdi4cat/voc4cat_0000181> ;
    skos:definition "Details describing the construction, physical dimensions, and operation of the photoreactor used to perform a photocatalytic reaction."@en ;
    skos:historyNote "0000-0002-6242-2167 Nikolaos G. Moustakas created the resource"@en ;
    skos:inScheme <https://w3id.org/nfdi4cat/voc4cat> ;
    skos:prefLabel "photoreactor design"@en .

<https://w3id.org/nfdi4cat/voc4cat_0000129> a skos:Concept ;
    dcterms:identifier "voc4cat_0000129"^^xsd:token ;
    skos:broader <https://w3id.org/nfdi4cat/voc4cat_0000186> ;
    skos:definition "Spectroscopic or chromatographic methods used to identify the products of the reaction qualitatively and quantitatively. Such devices are usually attached to the reactor, or a sample is being transferred to an identification method via another medium (e.g., gastight syringes)."@en ;
    skos:historyNote "0000-0002-6242-2167 Nikolaos G. Moustakas created the resource"@en ;
    skos:inScheme <https://w3id.org/nfdi4cat/voc4cat> ;
    skos:prefLabel "product identification method"@en .

<https://w3id.org/nfdi4cat/voc4cat_0000131> a skos:Concept ;
    dcterms:identifier "voc4cat_0000131"^^xsd:token ;
    skos:broader <https://w3id.org/nfdi4cat/voc4cat_0000191> ;
    skos:definition "Detectors of the gas chromatogragh used to identify the reaction products and intemediates."@en ;
    skos:historyNote "0000-0002-6242-2167 Nikolaos G. Moustakas created the resource"@en ;
    skos:inScheme <https://w3id.org/nfdi4cat/voc4cat> ;
    skos:prefLabel "gas chromatograph detector"@en .

<https://w3id.org/nfdi4cat/voc4cat_0000132> a skos:Concept ;
    dcterms:identifier "voc4cat_0000132"^^xsd:token ;
    skos:altLabel "FID"@en ;
    skos:broader <https://w3id.org/nfdi4cat/voc4cat_0000191> ;
    skos:definition "A type of gas chromatography detector that detects and quantifies the concentration of organic compounds in a gas sample emerging from a column, by measuring the electrical current generated by ionized gas constituents in a hydrogen flame."@en ;
    skos:historyNote "0000-0002-6242-2167 Nikolaos G. Moustakas created the resource"@en ;
    skos:inScheme <https://w3id.org/nfdi4cat/voc4cat> ;
    skos:prefLabel "flame ionization detector"@en .

<https://w3id.org/nfdi4cat/voc4cat_0000133> a skos:Concept ;
    dcterms:identifier "voc4cat_0000133"^^xsd:token ;
    skos:altLabel "TCD"@en ;
    skos:broader <https://w3id.org/nfdi4cat/voc4cat_0000191> ;
    skos:definition "A type of gas chromatography detector that measures the thermal conductivity of a gas sample and identifies its constituent molecules through changes in a filament’s temperature."@en ;
    skos:historyNote "0000-0002-6242-2167 Nikolaos G. Moustakas created the resource"@en ;
    skos:inScheme <https://w3id.org/nfdi4cat/voc4cat> ;
    skos:prefLabel "thermal conductivity detector"@en .

<https://w3id.org/nfdi4cat/voc4cat_0000134> a skos:Concept ;
    dcterms:identifier "voc4cat_0000134"^^xsd:token ;
    skos:altLabel "BID"@en ;
    skos:broader <https://w3id.org/nfdi4cat/voc4cat_0000191> ;
    skos:definition "Detector incorporating Ionization via a new dielectric barrier discharge He plasma."@en ;
    skos:historyNote "0000-0002-6242-2167 Nikolaos G. Moustakas created the resource"@en ;
    skos:inScheme <https://w3id.org/nfdi4cat/voc4cat> ;
    skos:prefLabel "dielectric-barrier discharge ionization detector"@en .

<https://w3id.org/nfdi4cat/voc4cat_0000135> a skos:Concept ;
    dcterms:identifier "voc4cat_0000135"^^xsd:token ;
    skos:broader <https://w3id.org/nfdi4cat/voc4cat_0000186> ;
    skos:definition "The minimum concentration of a product or intermediate that the gas chromatograph can identify."@en ;
    skos:historyNote "0000-0002-6242-2167 Nikolaos G. Moustakas created the resource"@en ;
    skos:inScheme <https://w3id.org/nfdi4cat/voc4cat> ;
    skos:prefLabel "gas chromatograph sensitivity"@en .

<https://w3id.org/nfdi4cat/voc4cat_0000136> a skos:Concept ;
    dcterms:identifier "voc4cat_0000136"^^xsd:token ;
    skos:broader <https://w3id.org/nfdi4cat/voc4cat_0000184> ;
    skos:definition "A process in which gaseous substances of known purity and concentration are introduced to the gas chromatograph and the respective area and retention time of the resulting peaks are identified. This process when concluded, allows for the calculation of concentrations of products and intermediates of the photoreaction."@en ;
    skos:historyNote "0000-0002-6242-2167 Nikolaos G. Moustakas created the resource"@en ;
    skos:inScheme <https://w3id.org/nfdi4cat/voc4cat> ;
    skos:prefLabel "gas chromatograph calibration"@en .

<https://w3id.org/nfdi4cat/voc4cat_0000138> a skos:Concept ;
    dcterms:identifier "voc4cat_0000138"^^xsd:token ;
    skos:broader <https://w3id.org/nfdi4cat/voc4cat_0000191> ;
    skos:definition "Detectors of the mass spectrometer used to identify the reaction products and intemediates."@en ;
    skos:historyNote "0000-0002-6242-2167 Nikolaos G. Moustakas created the resource"@en ;
    skos:inScheme <https://w3id.org/nfdi4cat/voc4cat> ;
    skos:prefLabel "mass spectrometer detector"@en .

<https://w3id.org/nfdi4cat/voc4cat_0000139> a skos:Concept ;
    dcterms:identifier "voc4cat_0000139"^^xsd:token ;
    skos:broader <https://w3id.org/nfdi4cat/voc4cat_0000186> ;
    skos:definition "The minimum concentration of a product or intermediate that the mass spectrometer can identify."@en ;
    skos:historyNote "0000-0002-6242-2167 Nikolaos G. Moustakas created the resource"@en ;
    skos:inScheme <https://w3id.org/nfdi4cat/voc4cat> ;
    skos:prefLabel "mass spectrometer sensitivity"@en .

<https://w3id.org/nfdi4cat/voc4cat_0000140> a skos:Concept ;
    dcterms:identifier "voc4cat_0000140"^^xsd:token ;
    skos:broader <https://w3id.org/nfdi4cat/voc4cat_0000184> ;
    skos:definition "A process in which gaseous substances of known purity and concentration are introduced to the mass spectrometer and the respective mass-to-charge ratios are identified. This process when concluded, allows for the calculation of concentrations of products and intermediates of the photoreaction."@en ;
    skos:historyNote "0000-0002-6242-2167 Nikolaos G. Moustakas created the resource"@en ;
    skos:inScheme <https://w3id.org/nfdi4cat/voc4cat> ;
    skos:prefLabel "mass spectrometer calibration"@en .

<https://w3id.org/nfdi4cat/voc4cat_0000144> a skos:Concept ;
    dcterms:identifier "voc4cat_0000144"^^xsd:token ;
    skos:broader <https://w3id.org/nfdi4cat/voc4cat_0000143> ;
    skos:definition "Maximum of operation pressure range within the reactor can operate safely."@en ;
    skos:historyNote "0000-0002-6242-2167 Nikolaos G. Moustakas created the resource"@en ;
    skos:inScheme <https://w3id.org/nfdi4cat/voc4cat> ;
    skos:prefLabel "maximum operation pressure"@en .

<https://w3id.org/nfdi4cat/voc4cat_0000145> a skos:Concept ;
    dcterms:identifier "voc4cat_0000145"^^xsd:token ;
    skos:broader <https://w3id.org/nfdi4cat/voc4cat_0000143> ;
    skos:definition "Minimum of operation pressure range within the reactor can operate safely."@en ;
    skos:historyNote "0000-0002-6242-2167 Nikolaos G. Moustakas created the resource"@en ;
    skos:inScheme <https://w3id.org/nfdi4cat/voc4cat> ;
    skos:prefLabel "minimum operation pressure"@en .

<https://w3id.org/nfdi4cat/voc4cat_0000147> a skos:Concept ;
    dcterms:identifier "voc4cat_0000147"^^xsd:token ;
    skos:broader <https://w3id.org/nfdi4cat/voc4cat_0000146> ;
    skos:definition "Α mechanical device that removes gas molecules from a sealed chamber reaching pressures lower than the atmospheric pressure."@en ;
    skos:historyNote "0000-0002-6242-2167 Nikolaos G. Moustakas created the resource"@en ;
    skos:inScheme <https://w3id.org/nfdi4cat/voc4cat> ;
    skos:prefLabel "vacuum pump"@en .

<https://w3id.org/nfdi4cat/voc4cat_0000149> a skos:Concept ;
    dcterms:identifier "voc4cat_0000149"^^xsd:token ;
    skos:broader <https://w3id.org/nfdi4cat/voc4cat_0000148> ;
    skos:definition "Maximum of operation temperature range within the reactor can operate safely."@en ;
    skos:historyNote "0000-0002-6242-2167 Nikolaos G. Moustakas created the resource"@en ;
    skos:inScheme <https://w3id.org/nfdi4cat/voc4cat> ;
    skos:prefLabel "maximum operation temperature"@en .

<https://w3id.org/nfdi4cat/voc4cat_0000150> a skos:Concept ;
    dcterms:identifier "voc4cat_0000150"^^xsd:token ;
    skos:broader <https://w3id.org/nfdi4cat/voc4cat_0000148> ;
    skos:definition "Minimum of operation temperature range within the reactor can operate safely."@en ;
    skos:historyNote "0000-0002-6242-2167 Nikolaos G. Moustakas created the resource"@en ;
    skos:inScheme <https://w3id.org/nfdi4cat/voc4cat> ;
    skos:prefLabel "minimum operation temperature"@en .

<https://w3id.org/nfdi4cat/voc4cat_0000151> a skos:Concept ;
    dcterms:identifier "voc4cat_0000151"^^xsd:token ;
    skos:altLabel "cooling device"@en,
        "heating device"@en,
        "temperature controller and monitor"@en,
        "temperature gauge"@en,
        "temperature monitor"@en ;
    skos:broader <https://w3id.org/nfdi4cat/voc4cat_0000187> ;
    skos:definition "Equipment used for controlling and/or monitoring the temperature in various parts of a reactor. This can include hot plates, heating elements and cryostats."@en ;
    skos:historyNote "0000-0002-6242-2167 Nikolaos G. Moustakas created the resource"@en ;
    skos:inScheme <https://w3id.org/nfdi4cat/voc4cat> ;
    skos:prefLabel "temperature controller"@en .

<https://w3id.org/nfdi4cat/voc4cat_0000152> a skos:Concept ;
    dcterms:identifier "voc4cat_0000152"^^xsd:token ;
    skos:altLabel "photoreaction chamber"@en ;
    skos:broader <https://w3id.org/nfdi4cat/voc4cat_0000188> ;
    skos:definition "A construction inside of which the catalyst and the reactants coexist, and the reaction takes place."@en ;
    skos:historyNote "0000-0002-6242-2167 Nikolaos G. Moustakas created the resource"@en ;
    skos:inScheme <https://w3id.org/nfdi4cat/voc4cat> ;
    skos:prefLabel "reaction chamber"@en .

<https://w3id.org/nfdi4cat/voc4cat_0000153> a skos:Concept ;
    dcterms:identifier "voc4cat_0000153"^^xsd:token ;
    skos:broader <https://w3id.org/nfdi4cat/voc4cat_0000186> ;
    skos:definition "Volume of the reaction chamber, calculated by its dimensions. Volume of pipes and valves connected to the reaction chamber should also be calculated and added to the total volume."@en ;
    skos:historyNote "0000-0002-6242-2167 Nikolaos G. Moustakas created the resource"@en ;
    skos:inScheme <https://w3id.org/nfdi4cat/voc4cat> ;
    skos:prefLabel "reaction chamber volume"@en .

<https://w3id.org/nfdi4cat/voc4cat_0000154> a skos:Concept ;
    dcterms:identifier "voc4cat_0000154"^^xsd:token ;
    skos:broader <https://w3id.org/nfdi4cat/voc4cat_0000186> ;
    skos:definition "Height, width and depth (in cubic- or rectangular- shaped reaction chambers) or diameter and height (in cylindrer - shaped reaction chambers)."@en ;
    skos:historyNote "0000-0002-6242-2167 Nikolaos G. Moustakas created the resource"@en ;
    skos:inScheme <https://w3id.org/nfdi4cat/voc4cat> ;
    skos:prefLabel "reaction chamber dimension"@en .

<https://w3id.org/nfdi4cat/voc4cat_0000155> a skos:Concept ;
    dcterms:identifier "voc4cat_0000155"^^xsd:token ;
    skos:broader <https://w3id.org/nfdi4cat/voc4cat_0000186> ;
    skos:definition "The shape of the reaction chamber. In gas-phase reactions, reaction chambers have usually a cylindrical, cubical or rectangular shape."@en ;
    skos:historyNote "0000-0002-6242-2167 Nikolaos G. Moustakas created the resource"@en ;
    skos:inScheme <https://w3id.org/nfdi4cat/voc4cat> ;
    skos:prefLabel "reaction chamber shape"@en .

<https://w3id.org/nfdi4cat/voc4cat_0000156> a skos:Concept ;
    dcterms:identifier "voc4cat_0000156"^^xsd:token ;
    skos:broader <https://w3id.org/nfdi4cat/voc4cat_0000186> ;
    skos:definition "Material used for the construction of the main body of the reaction chamber."@en ;
    skos:historyNote "0000-0002-6242-2167 Nikolaos G. Moustakas created the resource"@en ;
    skos:inScheme <https://w3id.org/nfdi4cat/voc4cat> ;
    skos:prefLabel "reaction chamber material"@en .

<https://w3id.org/nfdi4cat/voc4cat_0000157> a skos:Concept ;
    dcterms:identifier "voc4cat_0000157"^^xsd:token ;
    skos:broader <https://w3id.org/nfdi4cat/voc4cat_0000189> ;
    skos:definition "A transparent material optimized to allow the transmission of electromagnetic radiation with low reflectance and scattering."@en ;
    skos:historyNote "0000-0002-6242-2167 Nikolaos G. Moustakas created the resource"@en ;
    skos:inScheme <https://w3id.org/nfdi4cat/voc4cat> ;
    skos:prefLabel "optical window"@en .

<https://w3id.org/nfdi4cat/voc4cat_0000158> a skos:Concept ;
    dcterms:identifier "voc4cat_0000158"^^xsd:token ;
    skos:broader <https://w3id.org/nfdi4cat/voc4cat_0000186> ;
    skos:definition "Material that the optical window is made of. The window, usually attached to the lid sealing the reaction chamber, allows the incoming light to interact with the catalyst. The material of the window influences the wavelength range that the catalyst experiences."@en ;
    skos:historyNote "0000-0002-6242-2167 Nikolaos G. Moustakas created the resource"@en ;
    skos:inScheme <https://w3id.org/nfdi4cat/voc4cat> ;
    skos:prefLabel "optical window material"@en .

<https://w3id.org/nfdi4cat/voc4cat_0000160> a skos:Concept ;
    dcterms:identifier "voc4cat_0000160"^^xsd:token ;
    skos:broader <https://w3id.org/nfdi4cat/voc4cat_0000159> ;
    skos:definition "Diameter of the optical window allowing the incoming light to enter the reaction chamber and interact with the catalyst."@en ;
    skos:historyNote "0000-0002-6242-2167 Nikolaos G. Moustakas created the resource"@en ;
    skos:inScheme <https://w3id.org/nfdi4cat/voc4cat> ;
    skos:prefLabel "optical window diameter"@en .

<https://w3id.org/nfdi4cat/voc4cat_0000161> a skos:Concept ;
    dcterms:identifier "voc4cat_0000161"^^xsd:token ;
    skos:broader <https://w3id.org/nfdi4cat/voc4cat_0000159> ;
    skos:definition "Thickness of the optical window allowing the incoming light to enter the reaction chamber and interact with the catalyst."@en ;
    skos:historyNote "0000-0002-6242-2167 Nikolaos G. Moustakas created the resource"@en ;
    skos:inScheme <https://w3id.org/nfdi4cat/voc4cat> ;
    skos:prefLabel "optical window thickness"@en .

<https://w3id.org/nfdi4cat/voc4cat_0000162> a skos:Concept ;
    dcterms:identifier "voc4cat_0000162"^^xsd:token ;
    skos:altLabel "gas flow"@en ;
    skos:broader <https://w3id.org/nfdi4cat/voc4cat_0000186> ;
    skos:definition "Flow rates of gases used in an experiment. Gases can have either the role of a reactant (e.g., CO2) or be inert (e.g., Ar, He)."@en ;
    skos:historyNote "0000-0002-6242-2167 Nikolaos G. Moustakas created the resource"@en ;
    skos:inScheme <https://w3id.org/nfdi4cat/voc4cat> ;
    skos:prefLabel "gas feed"@en .

<https://w3id.org/nfdi4cat/voc4cat_0000164> a skos:Concept ;
    dcterms:identifier "voc4cat_0000164"^^xsd:token ;
    skos:altLabel "MFC"@en,
        "MFCs"@en ;
    skos:broader <https://w3id.org/nfdi4cat/voc4cat_0000163> ;
    skos:definition "A mass flow controller (MFC) is a device used to measure and control the flow of liquids and gases. A mass flow controller is designed and calibrated to control a specific type of liquid or gas at a particular range of flow rates."@en ;
    skos:historyNote "0000-0002-6242-2167 Nikolaos G. Moustakas created the resource"@en ;
    skos:inScheme <https://w3id.org/nfdi4cat/voc4cat> ;
    skos:prefLabel "mass flow controller"@en .

<https://w3id.org/nfdi4cat/voc4cat_0000167> a skos:Concept ;
    dcterms:identifier "voc4cat_0000167"^^xsd:token ;
    skos:altLabel "Hg-Xe lamp"@en,
        "Hg/Xe lamp"@en,
        "mercury xenon lamp"@en ;
    skos:broader <https://w3id.org/nfdi4cat/voc4cat_0000166> ;
    skos:definition "A lamp containing a mixture of mercury (Hg) and xenon (Xe) gases. Under electric current, the gas mixture gets ionized through a discharge electric charge creating a plasma generating UV and visible light."@en ;
    skos:historyNote "0000-0002-6242-2167 Nikolaos G. Moustakas created the resource"@en ;
    skos:inScheme <https://w3id.org/nfdi4cat/voc4cat> ;
    skos:prefLabel "mercury-xenon lamp"@en .

<https://w3id.org/nfdi4cat/voc4cat_0000168> a skos:Concept ;
    dcterms:identifier "voc4cat_0000168"^^xsd:token ;
    skos:altLabel "Xe lamp"@en,
        "Xe-lamp"@en ;
    skos:broader <https://w3id.org/nfdi4cat/voc4cat_0000166> ;
    skos:definition "A lamp containing pure xenon (Xe) gas. Under electric current, the gas mixture gets ionized through a discharge electric charge creating a plasma generating UV and visible light."@en ;
    skos:historyNote "0000-0002-6242-2167 Nikolaos G. Moustakas created the resource"@en ;
    skos:inScheme <https://w3id.org/nfdi4cat/voc4cat> ;
    skos:prefLabel "xenon lamp"@en .

<https://w3id.org/nfdi4cat/voc4cat_0000169> a skos:Concept ;
    dcterms:identifier "voc4cat_0000169"^^xsd:token ;
    skos:altLabel "LED"@en,
        "light-emitting diode"@en ;
    skos:broader <https://w3id.org/nfdi4cat/voc4cat_0000166> ;
    skos:definition "A solid-state semiconductor emitting light at highly controllable (narrow) wavelength ranges."@en ;
    skos:historyNote "0000-0002-6242-2167 Nikolaos G. Moustakas created the resource"@en ;
    skos:inScheme <https://w3id.org/nfdi4cat/voc4cat> ;
    skos:prefLabel "light emitting diode"@en .

<https://w3id.org/nfdi4cat/voc4cat_0000171> a skos:Concept ;
    dcterms:identifier "voc4cat_0000171"^^xsd:token ;
    skos:broader <https://w3id.org/nfdi4cat/voc4cat_0000170> ;
    skos:definition "The distance of the light source from the reaction chamber and the catalyst."@en ;
    skos:historyNote "0000-0002-6242-2167 Nikolaos G. Moustakas created the resource"@en ;
    skos:inScheme <https://w3id.org/nfdi4cat/voc4cat> ;
    skos:prefLabel "light source distance"@en .

<https://w3id.org/nfdi4cat/voc4cat_0000172> a skos:Concept ;
    dcterms:identifier "voc4cat_0000172"^^xsd:token ;
    skos:broader <https://w3id.org/nfdi4cat/voc4cat_0000170> ;
    skos:definition "The value of current (usually in A or mA) used to operate the selected light source."@en ;
    skos:historyNote "0000-0002-6242-2167 Nikolaos G. Moustakas created the resource"@en ;
    skos:inScheme <https://w3id.org/nfdi4cat/voc4cat> ;
    skos:prefLabel "light operation current"@en .

<https://w3id.org/nfdi4cat/voc4cat_0000173> a skos:Concept ;
    dcterms:identifier "voc4cat_0000173"^^xsd:token ;
    skos:broader <https://w3id.org/nfdi4cat/voc4cat_0000170> ;
    skos:definition "The value of voltage (usually in V or mV) used to operate the selected light source."@en ;
    skos:historyNote "0000-0002-6242-2167 Nikolaos G. Moustakas created the resource"@en ;
    skos:inScheme <https://w3id.org/nfdi4cat/voc4cat> ;
    skos:prefLabel "light operation voltage"@en .

<https://w3id.org/nfdi4cat/voc4cat_0000174> a skos:Concept ;
    dcterms:identifier "voc4cat_0000174"^^xsd:token ;
    skos:broader <https://w3id.org/nfdi4cat/voc4cat_0000170> ;
    skos:definition "The power of the light source (usually in W or mW). The power can be calculated by the multiplication of the current and voltage used to operate the light source."@en ;
    skos:historyNote "0000-0002-6242-2167 Nikolaos G. Moustakas created the resource"@en ;
    skos:inScheme <https://w3id.org/nfdi4cat/voc4cat> ;
    skos:prefLabel "light power output"@en .

<https://w3id.org/nfdi4cat/voc4cat_0000175> a skos:Concept ;
    dcterms:identifier "voc4cat_0000175"^^xsd:token ;
    skos:broader <https://w3id.org/nfdi4cat/voc4cat_0000170> ;
    skos:definition "The light intensity (usually in mW cm-2) of the selected light source. The light intensity should be measured at the same distance as the one between the light source and the reaction chamber / sample."@en ;
    skos:historyNote "0000-0002-6242-2167 Nikolaos G. Moustakas created the resource"@en ;
    skos:inScheme <https://w3id.org/nfdi4cat/voc4cat> ;
    skos:prefLabel "light intensity"@en .

<https://w3id.org/nfdi4cat/voc4cat_0000176> a skos:Concept ;
    dcterms:identifier "voc4cat_0000176"^^xsd:token ;
    skos:altLabel "λ"@en ;
    skos:broader <https://w3id.org/nfdi4cat/voc4cat_0000170> ;
    skos:definition "The distance between two successive peaks or troughs in a wave."@en ;
    skos:historyNote "0000-0002-6242-2167 Nikolaos G. Moustakas created the resource"@en ;
    skos:inScheme <https://w3id.org/nfdi4cat/voc4cat> ;
    skos:prefLabel "light wavelength"@en .

<https://w3id.org/nfdi4cat/voc4cat_0000177> a skos:Concept ;
    dcterms:identifier "voc4cat_0000177"^^xsd:token ;
    skos:altLabel "IR"@en,
        "Ir"@en ;
    skos:broader <https://w3id.org/nfdi4cat/voc4cat_0000181> ;
    skos:definition "Electromagnetic radiation with wavelengths typically in the range of 800 nm - 20000 nm."@en ;
    skos:historyNote "0000-0002-6242-2167 Nikolaos G. Moustakas created the resource"@en ;
    skos:inScheme <https://w3id.org/nfdi4cat/voc4cat> ;
    skos:prefLabel "infrared"@en .

<https://w3id.org/nfdi4cat/voc4cat_0000179> a skos:Concept ;
    dcterms:identifier "voc4cat_0000179"^^xsd:token ;
    skos:altLabel "UV"@en,
        "UV-A"@en,
        "UV-B"@en,
        "UV-C"@en,
        "VUV"@en ;
    skos:broader <https://w3id.org/nfdi4cat/voc4cat_0000181> ;
    skos:definition "Electromagnetic radiation with a wavelength typically in the range of 100-400 nanometers."@en ;
    skos:historyNote "0000-0002-6242-2167 Nikolaos G. Moustakas created the resource"@en ;
    skos:inScheme <https://w3id.org/nfdi4cat/voc4cat> ;
    skos:prefLabel "ultraviolet"@en .

<https://w3id.org/nfdi4cat/voc4cat_0000192> a skos:Concept ;
    dcterms:identifier "voc4cat_0000192"^^xsd:token ;
    skos:broader <https://w3id.org/nfdi4cat/voc4cat_0000187> ;
    skos:definition "A device that measures a specific physical or chemical property and converts it into readable signal, often for continuous monitoring."@en ;
    skos:historyNote "0000-0002-6242-2167 Nikolaos G. Moustakas created the resource"@en ;
    skos:inScheme <https://w3id.org/nfdi4cat/voc4cat> ;
    skos:narrower <https://w3id.org/nfdi4cat/voc4cat_0000191> ;
    skos:prefLabel "sensor"@en .

<https://w3id.org/nfdi4cat/voc4cat_0000197> a skos:Concept ;
    dcterms:identifier "voc4cat_0000197"^^xsd:token ;
    skos:altLabel "MOF"@en ;
    skos:broader <https://w3id.org/nfdi4cat/voc4cat_0000190> ;
    skos:definition "Porous crystalline materials composed of metal nodes or clusters connected by organic linkers, forming highly ordered one-, two-, or three-dimensional structures with tunable properties."@en ;
    skos:historyNote "0000-0002-6242-2167 Nikolaos G. Moustakas created the resource"@en ;
    skos:inScheme <https://w3id.org/nfdi4cat/voc4cat> ;
    skos:prefLabel "metal-organic framework"@en .

<https://w3id.org/nfdi4cat/voc4cat_0000198> a skos:Concept ;
    dcterms:identifier "voc4cat_0000198"^^xsd:token ;
    skos:broader <https://w3id.org/nfdi4cat/voc4cat_0000270> ;
    skos:definition "A porous solid material containing pores with width between 2 and 50 nm."@en ;
    skos:historyNote "0000-0002-6242-2167 Nikolaos G. Moustakas created the resource"@en ;
    skos:inScheme <https://w3id.org/nfdi4cat/voc4cat> ;
    skos:prefLabel "mesoporous material"@en .

<https://w3id.org/nfdi4cat/voc4cat_0000199> a skos:Concept ;
    dcterms:identifier "voc4cat_0000199"^^xsd:token ;
    skos:broader <https://w3id.org/nfdi4cat/voc4cat_0000181> ;
    skos:definition "A reaction mechanism is the step-by-step sequence of elementary reactions at the molecular level that explains how an overall chemical reaction proceeds."@en ;
    skos:historyNote "0000-0002-6242-2167 Nikolaos G. Moustakas created the resource"@en ;
    skos:inScheme <https://w3id.org/nfdi4cat/voc4cat> ;
    skos:prefLabel "reaction mechanism"@en .

<https://w3id.org/nfdi4cat/voc4cat_0000200> a skos:Concept ;
    dcterms:identifier "voc4cat_0000200"^^xsd:token ;
    skos:altLabel "sustainable chemistry"@en ;
    skos:broader <https://w3id.org/nfdi4cat/voc4cat_0000181> ;
    skos:definition "The science and technology of sustainable and environment friendly chemical processes and products that reduce or eliminate hazardous substances, while minimizing waste and energy consumption."@en ;
    skos:historyNote "0000-0002-6242-2167 Nikolaos G. Moustakas created the resource"@en ;
    skos:inScheme <https://w3id.org/nfdi4cat/voc4cat> ;
    skos:prefLabel "green chemistry"@en .

<https://w3id.org/nfdi4cat/voc4cat_0000201> a skos:Concept ;
    dcterms:identifier "voc4cat_0000201"^^xsd:token ;
    skos:altLabel "cross-coupling"@en ;
    skos:broader <https://w3id.org/nfdi4cat/voc4cat_0000181> ;
    skos:definition "A cross-coupling reaction is a catalytic, metal-mediated reaction that forms carbon-carbon or carbon-heteroatom bonds by joining two different molecular fragments, typically through the activation of electrophilic and nucleophilic partners."@en ;
    skos:historyNote "0000-0002-6242-2167 Nikolaos G. Moustakas created the resource"@en ;
    skos:inScheme <https://w3id.org/nfdi4cat/voc4cat> ;
    skos:prefLabel "cross-coupling reaction"@en .

<https://w3id.org/nfdi4cat/voc4cat_0000202> a skos:Concept ;
    dcterms:identifier "voc4cat_0000202"^^xsd:token ;
    skos:altLabel "C-H activation"@en,
        "C-H bond activation"@en,
        "carbon-hydrogen activation"@en,
        "carbon-hydrogen activation reaction"@en,
        "carbon-hydrogen bond activation"@en ;
    skos:broader <https://w3id.org/nfdi4cat/voc4cat_0000185> ;
    skos:definition "A type of organic reaction in which a stable carbon-hydrogen (C-H)  bond is cleaved and replaced with a C-X bond."@en ;
    skos:historyNote "0000-0002-6242-2167 Nikolaos G. Moustakas created the resource"@en ;
    skos:inScheme <https://w3id.org/nfdi4cat/voc4cat> ;
    skos:prefLabel "C-H activation reaction"@en .

<https://w3id.org/nfdi4cat/voc4cat_0000203> a skos:Concept ;
    dcterms:identifier "voc4cat_0000203"^^xsd:token ;
    skos:broader <https://w3id.org/nfdi4cat/voc4cat_0000181> ;
    skos:definition "A branch of chemistry studying chemical reactions and processes driven and affected by light and the absorption of photons."@en ;
    skos:historyNote "0000-0002-6242-2167 Nikolaos G. Moustakas created the resource"@en ;
    skos:inScheme <https://w3id.org/nfdi4cat/voc4cat> ;
    skos:prefLabel "photochemistry"@en .

<https://w3id.org/nfdi4cat/voc4cat_0000204> a skos:Concept ;
    dcterms:identifier "voc4cat_0000204"^^xsd:token ;
    skos:broader <https://w3id.org/nfdi4cat/voc4cat_0000196> ;
    skos:definition "A catalytic process catalyzed by the presence of biological entities."@en ;
    skos:historyNote "0000-0002-6242-2167 Nikolaos G. Moustakas created the resource"@en ;
    skos:inScheme <https://w3id.org/nfdi4cat/voc4cat> ;
    skos:prefLabel "biocatalysis"@en .

<https://w3id.org/nfdi4cat/voc4cat_0000205> a skos:Concept ;
    dcterms:identifier "voc4cat_0000205"^^xsd:token ;
    skos:broader <https://w3id.org/nfdi4cat/voc4cat_0000185> ;
    skos:definition "Epoxidation is the chemical process of converting an alkene into an epoxide, a three-membered cyclic ether, by adding a single oxygen atom across a carbon-carbon double bond."@en ;
    skos:historyNote "0000-0002-6242-2167 Nikolaos G. Moustakas created the resource"@en ;
    skos:inScheme <https://w3id.org/nfdi4cat/voc4cat> ;
    skos:prefLabel "epoxidation"@en .

<https://w3id.org/nfdi4cat/voc4cat_0000206> a skos:Concept ;
    dcterms:identifier "voc4cat_0000206"^^xsd:token ;
    skos:altLabel "H2O splitting"@en ;
    skos:broader <https://w3id.org/nfdi4cat/voc4cat_0000185> ;
    skos:definition "A chemical reaction in which water molecules are dissociated into gaseous hydrogen and oxygen, typically facilitted by catalysts and an external energy source."@en ;
    skos:historyNote "0000-0002-6242-2167 Nikolaos G. Moustakas created the resource"@en ;
    skos:inScheme <https://w3id.org/nfdi4cat/voc4cat> ;
    skos:prefLabel "water splitting"@en .

<https://w3id.org/nfdi4cat/voc4cat_0000207> a skos:Concept ;
    dcterms:identifier "voc4cat_0000207"^^xsd:token ;
    skos:broader <https://w3id.org/nfdi4cat/voc4cat_0000196> ;
    skos:definition "A biocatalytic process performed in the presence of an enzyme."@en ;
    skos:historyNote "0000-0002-6242-2167 Nikolaos G. Moustakas created the resource"@en ;
    skos:inScheme <https://w3id.org/nfdi4cat/voc4cat> ;
    skos:prefLabel "enzyme catalysis"@en .

<https://w3id.org/nfdi4cat/voc4cat_0000208> a skos:Concept ;
    dcterms:identifier "voc4cat_0000208"^^xsd:token ;
    skos:broader <https://w3id.org/nfdi4cat/voc4cat_0000196> ;
    skos:definition "A type of catalysis where the rate of a chemical reaction is increased by the addition of a substoichiometric quantity of an organic (non-metallic) compound."@en ;
    skos:historyNote "0000-0002-6242-2167 Nikolaos G. Moustakas created the resource"@en ;
    skos:inScheme <https://w3id.org/nfdi4cat/voc4cat> ;
    skos:prefLabel "organocatalysis"@en .

<https://w3id.org/nfdi4cat/voc4cat_0000209> a skos:Concept ;
    dcterms:identifier "voc4cat_0000209"^^xsd:token ;
    skos:broader <https://w3id.org/nfdi4cat/voc4cat_0007249> ;
    skos:definition "A fuel cell is an electrochemical device that converts the chemical energy of a fuel, often hydrogen, and an oxidizing agent, typically oxygen, into electrical energy, with water and heat as the main byproducts."@en ;
    skos:historyNote "0000-0002-6242-2167 Nikolaos G. Moustakas created the resource"@en ;
    skos:inScheme <https://w3id.org/nfdi4cat/voc4cat> ;
    skos:prefLabel "fuel cell"@en .

<https://w3id.org/nfdi4cat/voc4cat_0000210> a skos:Concept ;
    dcterms:identifier "voc4cat_0000210"^^xsd:token ;
    skos:broader <https://w3id.org/nfdi4cat/voc4cat_0000190> ;
    skos:definition "A hollow cylindrical tube-like material structure at the nanoscale."@en ;
    skos:historyNote "0000-0002-6242-2167 Nikolaos G. Moustakas created the resource"@en ;
    skos:inScheme <https://w3id.org/nfdi4cat/voc4cat> ;
    skos:prefLabel "nanotube"@en .

<https://w3id.org/nfdi4cat/voc4cat_0000211> a skos:Concept ;
    dcterms:identifier "voc4cat_0000211"^^xsd:token ;
    skos:broader <https://w3id.org/nfdi4cat/voc4cat_0000186> ;
    skos:definition "The property of a chemical reaction to occur at a specific reactive site on a molecule, leading to the preferential formation of one regiosomer over others."@en ;
    skos:historyNote "0000-0002-6242-2167 Nikolaos G. Moustakas created the resource"@en ;
    skos:inScheme <https://w3id.org/nfdi4cat/voc4cat> ;
    skos:prefLabel "regioselectivity"@en .

<https://w3id.org/nfdi4cat/voc4cat_0000212> a skos:Concept ;
    dcterms:identifier "voc4cat_0000212"^^xsd:token ;
    skos:broader <https://w3id.org/nfdi4cat/voc4cat_0000186> ;
    skos:definition "is the preference of a chemical reaction to selectively react with one functional group in the presence of other reactive groups, leaving the latter unaffected."@en ;
    skos:historyNote "0000-0002-6242-2167 Nikolaos G. Moustakas created the resource"@en ;
    skos:inScheme <https://w3id.org/nfdi4cat/voc4cat> ;
    skos:prefLabel "chemoselectivity"@en .

<https://w3id.org/nfdi4cat/voc4cat_0000213> a skos:Concept ;
    dcterms:identifier "voc4cat_0000213"^^xsd:token ;
    skos:broader <https://w3id.org/nfdi4cat/voc4cat_0000186> ;
    skos:definition "A one-, two-, or three-, dimensional structure that has at least one dimension in the nanometer scale."@en ;
    skos:historyNote "0000-0002-6242-2167 Nikolaos G. Moustakas created the resource"@en ;
    skos:inScheme <https://w3id.org/nfdi4cat/voc4cat> ;
    skos:prefLabel "nanostructure"@en .

<https://w3id.org/nfdi4cat/voc4cat_0000214> a skos:Concept ;
    dcterms:identifier "voc4cat_0000214"^^xsd:token ;
    skos:broader <https://w3id.org/nfdi4cat/voc4cat_0000186> ;
    skos:definition "The ability of a chemical reaction to differentiate between enantiomers, leading to the preferential formation of one stereoisomer, often controlled by a chiral catalyst or reagent."@en ;
    skos:historyNote "0000-0002-6242-2167 Nikolaos G. Moustakas created the resource"@en ;
    skos:inScheme <https://w3id.org/nfdi4cat/voc4cat> ;
    skos:prefLabel "enantioselectivity"@en .

<https://w3id.org/nfdi4cat/voc4cat_0000215> a skos:Concept ;
    dcterms:identifier "voc4cat_0000215"^^xsd:token ;
    skos:altLabel "DFT"@en ;
    skos:broader <https://w3id.org/nfdi4cat/voc4cat_0000181> ;
    skos:definition "A computational quantum mechanical modeling method used to investigate the electronic structure of atoms, molecules and solids, approximating their energy by using electron density as the key variable rather than wavefunctions."@en ;
    skos:historyNote "0000-0002-6242-2167 Nikolaos G. Moustakas created the resource"@en ;
    skos:inScheme <https://w3id.org/nfdi4cat/voc4cat> ;
    skos:prefLabel "density functional theory"@en .

<https://w3id.org/nfdi4cat/voc4cat_0000216> a skos:Concept ;
    dcterms:identifier "voc4cat_0000216"^^xsd:token ;
    skos:broader <https://w3id.org/nfdi4cat/voc4cat_0000196> ;
    skos:definition "A catalytic process that facilitates reactions by controlling charge transfer at the electrode-electrolyte interface."@en ;
    skos:historyNote "0000-0002-6242-2167 Nikolaos G. Moustakas created the resource"@en ;
    skos:inScheme <https://w3id.org/nfdi4cat/voc4cat> ;
    skos:prefLabel "electrocatalysis"@en .

<https://w3id.org/nfdi4cat/voc4cat_0000217> a skos:Concept ;
    dcterms:identifier "voc4cat_0000217"^^xsd:token ;
    skos:broader <https://w3id.org/nfdi4cat/voc4cat_0000196> ;
    skos:definition "Asymmetric catalysis is a catalytic process in which a chiral catalyst directs the formation of a chiral compound, preferentially producing one enantiomer over the other, thereby enhancing enantioselectivity in chemical reactions."@en ;
    skos:historyNote "0000-0002-6242-2167 Nikolaos G. Moustakas created the resource"@en ;
    skos:inScheme <https://w3id.org/nfdi4cat/voc4cat> ;
    skos:prefLabel "asymmetric catalysis"@en .

<https://w3id.org/nfdi4cat/voc4cat_0000218> a skos:Concept ;
    dcterms:identifier "voc4cat_0000218"^^xsd:token ;
    skos:broader <https://w3id.org/nfdi4cat/voc4cat_0000181> ;
    skos:definition "The branch of chemistry that studies the relationship between electrical potential and chemical transformations, focusing on electron transfer processes, particularly redox reactions at electrode interfaces."@en ;
    skos:historyNote "0000-0002-6242-2167 Nikolaos G. Moustakas created the resource"@en ;
    skos:inScheme <https://w3id.org/nfdi4cat/voc4cat> ;
    skos:prefLabel "electrochemistry"@en .

<https://w3id.org/nfdi4cat/voc4cat_0000219> a skos:Concept ;
    dcterms:identifier "voc4cat_0000219"^^xsd:token ;
    skos:altLabel "heterocyclic compound"@en ;
    skos:broader <https://w3id.org/nfdi4cat/voc4cat_0000181> ;
    skos:definition "A cyclic compound composed of at least one atom other than carbon in its ring structure."@en ;
    skos:historyNote "0000-0002-6242-2167 Nikolaos G. Moustakas created the resource"@en ;
    skos:inScheme <https://w3id.org/nfdi4cat/voc4cat> ;
    skos:prefLabel "heterocycle"@en .

<https://w3id.org/nfdi4cat/voc4cat_0000220> a skos:Concept ;
    dcterms:identifier "voc4cat_0000220"^^xsd:token ;
    skos:altLabel "cyclization"@en ;
    skos:broader <https://w3id.org/nfdi4cat/voc4cat_0000183> ;
    skos:definition "A chemical reaction in which an acyclic (open-chain) precursor molecule is transformed into a cyclic structure."@en ;
    skos:historyNote "0000-0002-6242-2167 Nikolaos G. Moustakas created the resource"@en ;
    skos:inScheme <https://w3id.org/nfdi4cat/voc4cat> ;
    skos:prefLabel "cyclization reaction"@en .

<https://w3id.org/nfdi4cat/voc4cat_0000221> a skos:Concept ;
    dcterms:identifier "voc4cat_0000221"^^xsd:token ;
    skos:broader <https://w3id.org/nfdi4cat/voc4cat_0000185> ;
    skos:definition "The process of designing and modifying protein structures via genetic or chemical alterations to improve their stability, activity, specificity, and functionality."@en ;
    skos:historyNote "0000-0002-6242-2167 Nikolaos G. Moustakas created the resource"@en ;
    skos:inScheme <https://w3id.org/nfdi4cat/voc4cat> ;
    skos:prefLabel "protein engineering"@en .

<https://w3id.org/nfdi4cat/voc4cat_0000222> a skos:Concept ;
    dcterms:identifier "voc4cat_0000222"^^xsd:token ;
    skos:altLabel "hydroformylation reaction"@en,
        "oxo process"@en,
        "oxo synthesis"@en ;
    skos:broader <https://w3id.org/nfdi4cat/voc4cat_0000183> ;
    skos:definition "A catalytic reaction for synthesizing an aldehyde from an alkene, by adding a formyl group (-CHO) and a hydrogen atom to a carbon-carbon double bond."@en ;
    skos:historyNote "0000-0002-6242-2167 Nikolaos G. Moustakas created the resource"@en ;
    skos:inScheme <https://w3id.org/nfdi4cat/voc4cat> ;
    skos:prefLabel "hydroformylation"@en .

<https://w3id.org/nfdi4cat/voc4cat_0000223> a skos:Concept ;
    dcterms:identifier "voc4cat_0000223"^^xsd:token ;
    skos:altLabel "C-C coupling"@en,
        "carbon-carbon coupling"@en,
        "carbon-carbon coupling reaction"@en ;
    skos:broader <https://w3id.org/nfdi4cat/voc4cat_0000183> ;
    skos:definition "A chemical reaction where a carbon-carbon bond is formed from two carbon-containing fragments."@en ;
    skos:historyNote "0000-0002-6242-2167 Nikolaos G. Moustakas created the resource"@en ;
    skos:inScheme <https://w3id.org/nfdi4cat/voc4cat> ;
    skos:prefLabel "C-C coupling reaction"@en .

<https://w3id.org/nfdi4cat/voc4cat_0000224> a skos:Concept ;
    dcterms:identifier "voc4cat_0000224"^^xsd:token ;
    skos:altLabel "catalytic hydrosilation"@en,
        "hydrosilation"@en,
        "hydrosilylation reaction"@en ;
    skos:broader <https://w3id.org/nfdi4cat/voc4cat_0000183> ;
    skos:definition "A chemical reaction where a silicon-hydrogen (Si-H) bond is added across an unsaturated bond typically catalyzed by a transition metal catalyst."@en ;
    skos:historyNote "0000-0002-6242-2167 Nikolaos G. Moustakas created the resource"@en ;
    skos:inScheme <https://w3id.org/nfdi4cat/voc4cat> ;
    skos:prefLabel "hydrosilylation"@en .

<https://w3id.org/nfdi4cat/voc4cat_0000225> a skos:Concept ;
    dcterms:identifier "voc4cat_0000225"^^xsd:token ;
    skos:altLabel "SAR"@en,
        "structure activity relationship"@en ;
    skos:broader <https://w3id.org/nfdi4cat/voc4cat_0000181> ;
    skos:definition "A study of the correlation between the chemical structure of a molecule, its functional properties and its biological activity."@en ;
    skos:historyNote "0000-0002-6242-2167 Nikolaos G. Moustakas created the resource"@en ;
    skos:inScheme <https://w3id.org/nfdi4cat/voc4cat> ;
    skos:prefLabel "structure-activity relationship"@en .

<https://w3id.org/nfdi4cat/voc4cat_0000226> a skos:Concept ;
    dcterms:identifier "voc4cat_0000226"^^xsd:token ;
    skos:altLabel "HDO"@en,
        "hydrodeoxygenation reaction"@en ;
    skos:broader <https://w3id.org/nfdi4cat/voc4cat_0000183> ;
    skos:definition "A catalytic process in which oxygen is removed from oxygenated organic compounds using hydrogen."@en ;
    skos:historyNote "0000-0002-6242-2167 Nikolaos G. Moustakas created the resource"@en ;
    skos:inScheme <https://w3id.org/nfdi4cat/voc4cat> ;
    skos:prefLabel "hydrodeoxygenation"@en .

<https://w3id.org/nfdi4cat/voc4cat_0000227> a skos:Concept ;
    dcterms:identifier "voc4cat_0000227"^^xsd:token ;
    skos:broader <https://w3id.org/nfdi4cat/voc4cat_0000185> ;
    skos:definition "The process by which molecules or particles spontaneously organize into structured, well-defined functional systems, without external stimuli, but driven by local interactions."@en ;
    skos:historyNote "0000-0002-6242-2167 Nikolaos G. Moustakas created the resource"@en ;
    skos:inScheme <https://w3id.org/nfdi4cat/voc4cat> ;
    skos:prefLabel "self-assembly"@en .

<https://w3id.org/nfdi4cat/voc4cat_0000228> a skos:Concept ;
    dcterms:identifier "voc4cat_0000228"^^xsd:token ;
    skos:broader <https://w3id.org/nfdi4cat/voc4cat_0000186> ;
    skos:definition "The property of an asymmetric molecule that makes it non-superposable on its mirror image, resulting in enantiomers with distinct chemical or biological properties."@en ;
    skos:historyNote "0000-0002-6242-2167 Nikolaos G. Moustakas created the resource"@en ;
    skos:inScheme <https://w3id.org/nfdi4cat/voc4cat> ;
    skos:prefLabel "chirality"@en .

<https://w3id.org/nfdi4cat/voc4cat_0000229> a skos:Concept ;
    dcterms:identifier "voc4cat_0000229"^^xsd:token ;
    skos:broader <https://w3id.org/nfdi4cat/voc4cat_0000181> ;
    skos:definition "A chemical species that contains at least one unpaired valence electron."@en ;
    skos:historyNote "0000-0002-6242-2167 Nikolaos G. Moustakas created the resource"@en ;
    skos:inScheme <https://w3id.org/nfdi4cat/voc4cat> ;
    skos:prefLabel "radical"@en .

<https://w3id.org/nfdi4cat/voc4cat_0000230> a skos:Concept ;
    dcterms:identifier "voc4cat_0000230"^^xsd:token ;
    skos:altLabel "cascade reaction"@en,
        "domino reaction"@en,
        "tandem reaction"@en ;
    skos:broader <https://w3id.org/nfdi4cat/voc4cat_0000183> ;
    skos:definition "A domino reaction is a chemical process of at least two consecutive sub-reactions occurring spontaneously in the same reaction vessel, without the need to add additional reagents, change reaction conditions and isolate intermediates. Each sub-reaction uses the product(s) already formed in the previous steps as reactant(s)."@en ;
    skos:historyNote "0000-0002-6242-2167 Nikolaos G. Moustakas created the resource"@en ;
    skos:inScheme <https://w3id.org/nfdi4cat/voc4cat> ;
    skos:prefLabel "sequential reaction"@en .

<https://w3id.org/nfdi4cat/voc4cat_0000231> a skos:Concept ;
    dcterms:identifier "voc4cat_0000231"^^xsd:token ;
    skos:broader <https://w3id.org/nfdi4cat/voc4cat_0000181> ;
    skos:definition "A natural resource that can be ecologically or artificially replenished at a rate faster than consumed and over a reasonable period on the human time scale."@en ;
    skos:historyNote "0000-0002-6242-2167 Nikolaos G. Moustakas created the resource"@en ;
    skos:inScheme <https://w3id.org/nfdi4cat/voc4cat> ;
    skos:prefLabel "renewable resource"@en .

<https://w3id.org/nfdi4cat/voc4cat_0000232> a skos:Concept ;
    dcterms:identifier "voc4cat_0000232"^^xsd:token ;
    skos:broader <https://w3id.org/nfdi4cat/voc4cat_0000196> ;
    skos:definition "A process in which an acid donates protons (protonation or electron withdrawal) or stabilizes reaction intermediates to accelerate a chemical reaction."@en ;
    skos:historyNote "0000-0002-6242-2167 Nikolaos G. Moustakas created the resource"@en ;
    skos:inScheme <https://w3id.org/nfdi4cat/voc4cat> ;
    skos:prefLabel "acid catalysis"@en .

<https://w3id.org/nfdi4cat/voc4cat_0000233> a skos:Concept ;
    dcterms:identifier "voc4cat_0000233"^^xsd:token ;
    skos:broader <https://w3id.org/nfdi4cat/voc4cat_0000196> ;
    skos:definition "A process in which base abstracts protons (deprotonation or electron donation) or stabilizes reaction intermediates to accelerate a chemical reaction."@en ;
    skos:historyNote "0000-0002-6242-2167 Nikolaos G. Moustakas created the resource"@en ;
    skos:inScheme <https://w3id.org/nfdi4cat/voc4cat> ;
    skos:prefLabel "base catalysis"@en .

<https://w3id.org/nfdi4cat/voc4cat_0000234> a skos:Concept ;
    dcterms:identifier "voc4cat_0000234"^^xsd:token ;
    skos:altLabel "micro-channel reactor"@en,
        "micro-reactor"@en,
        "micro-structured reactor"@en,
        "microchannel reactor"@en,
        "microstructured reactor"@en ;
    skos:broader <https://w3id.org/nfdi4cat/voc4cat_0000187> ;
    skos:definition "A small-scale chemical reactor, with lateral dimensions in the submillimeter range, typically employing microchannels to facilitate reactions within a well-controlled confined space."@en ;
    skos:historyNote "0000-0002-6242-2167 Nikolaos G. Moustakas created the resource"@en ;
    skos:inScheme <https://w3id.org/nfdi4cat/voc4cat> ;
    skos:prefLabel "microreactor"@en .

<https://w3id.org/nfdi4cat/voc4cat_0000235> a skos:Concept ;
    dcterms:identifier "voc4cat_0000235"^^xsd:token ;
    skos:broader <https://w3id.org/nfdi4cat/voc4cat_0000181> ;
    skos:definition "The interaction between at least two constituent parts (e.g., substances, processes, chemical species) to produce a combined effect greater than the sum of their individual effects, resulting in a more significant outcome than each part could achieve alone."@en ;
    skos:historyNote "0000-0002-6242-2167 Nikolaos G. Moustakas created the resource"@en ;
    skos:inScheme <https://w3id.org/nfdi4cat/voc4cat> ;
    skos:prefLabel "synergistic effect"@en .

<https://w3id.org/nfdi4cat/voc4cat_0000236> a skos:Concept ;
    dcterms:identifier "voc4cat_0000236"^^xsd:token ;
    skos:altLabel "OER"@en ;
    skos:broader <https://w3id.org/nfdi4cat/voc4cat_0000183> ;
    skos:definition "A chemical reaction of generating molecular oxygen in electrochemistry."@en ;
    skos:historyNote "0000-0002-6242-2167 Nikolaos G. Moustakas created the resource"@en ;
    skos:inScheme <https://w3id.org/nfdi4cat/voc4cat> ;
    skos:prefLabel "oxygen evolution reaction"@en .

<https://w3id.org/nfdi4cat/voc4cat_0000237> a skos:Concept ;
    dcterms:identifier "voc4cat_0000237"^^xsd:token ;
    skos:altLabel "ORR"@en ;
    skos:broader <https://w3id.org/nfdi4cat/voc4cat_0000183> ;
    skos:definition "The reduction half reaction where oxygen is reduced to water or hydrogen peroxide. In electrochemistry it takes place in the cathode."@en ;
    skos:historyNote "0000-0002-6242-2167 Nikolaos G. Moustakas created the resource"@en ;
    skos:inScheme <https://w3id.org/nfdi4cat/voc4cat> ;
    skos:prefLabel "oxygen reduction reaction"@en .

<https://w3id.org/nfdi4cat/voc4cat_0000238> a skos:Concept ;
    dcterms:identifier "voc4cat_0000238"^^xsd:token ;
    skos:broader <https://w3id.org/nfdi4cat/voc4cat_0000181> ;
    skos:definition "A chemical processes occurring at surfaces and interfaces."@en ;
    skos:historyNote "0000-0002-6242-2167 Nikolaos G. Moustakas created the resource"@en ;
    skos:inScheme <https://w3id.org/nfdi4cat/voc4cat> ;
    skos:prefLabel "surface chemistry"@en .

<https://w3id.org/nfdi4cat/voc4cat_0000239> a skos:Concept ;
    dcterms:identifier "voc4cat_0000239"^^xsd:token ;
    skos:altLabel "enantioselective synthesis"@en ;
    skos:broader <https://w3id.org/nfdi4cat/voc4cat_0000185> ;
    skos:definition "A chemical synthesis process yielding stereoisomeric (enantiomeric or diastereomeric) products in different rations."@en ;
    skos:historyNote "0000-0002-6242-2167 Nikolaos G. Moustakas created the resource"@en ;
    skos:inScheme <https://w3id.org/nfdi4cat/voc4cat> ;
    skos:prefLabel "asymmetric synthesis"@en .

<https://w3id.org/nfdi4cat/voc4cat_0000240> a skos:Concept ;
    dcterms:identifier "voc4cat_0000240"^^xsd:token ;
    skos:broader <https://w3id.org/nfdi4cat/voc4cat_0000181> ;
    skos:definition "Molecules with the same formula and atomic connectivity, but with different spatial arrangement of atoms."@en ;
    skos:historyNote "0000-0002-6242-2167 Nikolaos G. Moustakas created the resource"@en ;
    skos:inScheme <https://w3id.org/nfdi4cat/voc4cat> ;
    skos:prefLabel "stereoisomer"@en .

<https://w3id.org/nfdi4cat/voc4cat_0000241> a skos:Concept ;
    dcterms:identifier "voc4cat_0000241"^^xsd:token ;
    skos:altLabel "HER"@en ;
    skos:broader <https://w3id.org/nfdi4cat/voc4cat_0000183> ;
    skos:definition "A chemical reaction of generating molecular hydrogen in electrochemistry."@en ;
    skos:historyNote "0000-0002-6242-2167 Nikolaos G. Moustakas created the resource"@en ;
    skos:inScheme <https://w3id.org/nfdi4cat/voc4cat> ;
    skos:prefLabel "hydrogen evolution reaction"@en .

<https://w3id.org/nfdi4cat/voc4cat_0000242> a skos:Concept ;
    dcterms:identifier "voc4cat_0000242"^^xsd:token ;
    skos:altLabel "amination reaction"@en ;
    skos:broader <https://w3id.org/nfdi4cat/voc4cat_0000183> ;
    skos:definition "The chemical reaction of adding an amino (-NH2) into a molecule to generate an amine."@en ;
    skos:historyNote "0000-0002-6242-2167 Nikolaos G. Moustakas created the resource"@en ;
    skos:inScheme <https://w3id.org/nfdi4cat/voc4cat> ;
    skos:prefLabel "amination"@en .

<https://w3id.org/nfdi4cat/voc4cat_0000243> a skos:Concept ;
    dcterms:identifier "voc4cat_0000243"^^xsd:token ;
    skos:altLabel "cycloaddition reaction"@en ;
    skos:broader <https://w3id.org/nfdi4cat/voc4cat_0000183> ;
    skos:definition "A chemical reaction where two or more unsaturated molecules unite to form a ring-shaped (cyclic) compound."@en ;
    skos:historyNote "0000-0002-6242-2167 Nikolaos G. Moustakas created the resource"@en ;
    skos:inScheme <https://w3id.org/nfdi4cat/voc4cat> ;
    skos:prefLabel "cycloaddition"@en .

<https://w3id.org/nfdi4cat/voc4cat_0000244> a skos:Concept ;
    dcterms:identifier "voc4cat_0000244"^^xsd:token ;
    skos:altLabel "hydrogen transfer"@en,
        "transfer hydrogenation reaction"@en ;
    skos:broader <https://w3id.org/nfdi4cat/voc4cat_0000183> ;
    skos:definition "A chemical reaction in which hydrogen (not directly from molecular hydrogen) is transferred to a molecule."@en ;
    skos:historyNote "0000-0002-6242-2167 Nikolaos G. Moustakas created the resource"@en ;
    skos:inScheme <https://w3id.org/nfdi4cat/voc4cat> ;
    skos:prefLabel "transfer hydrogenation"@en .

<https://w3id.org/nfdi4cat/voc4cat_0000245> a skos:Concept ;
    dcterms:identifier "voc4cat_0000245"^^xsd:token ;
    skos:altLabel "metathesis reaction"@en ;
    skos:broader <https://w3id.org/nfdi4cat/voc4cat_0000183> ;
    skos:definition "A chemical reaction in which double bonds between atoms in two molecules are rearranged, yielding products formed by the exchange of molecular fragments between the reactants while keeping the number of double bonds the same."@en ;
    skos:historyNote "0000-0002-6242-2167 Nikolaos G. Moustakas created the resource"@en ;
    skos:inScheme <https://w3id.org/nfdi4cat/voc4cat> ;
    skos:prefLabel "metathesis"@en .

<https://w3id.org/nfdi4cat/voc4cat_0000246> a skos:Concept ;
    dcterms:identifier "voc4cat_0000246"^^xsd:token ;
    skos:broader <https://w3id.org/nfdi4cat/voc4cat_0000196> ;
    skos:definition "The application of materials with dimensions in the nanoscale, to catalyze chemical reactions."@en ;
    skos:historyNote "0000-0002-6242-2167 Nikolaos G. Moustakas created the resource"@en ;
    skos:inScheme <https://w3id.org/nfdi4cat/voc4cat> ;
    skos:prefLabel "nanocatalysis"@en .

<https://w3id.org/nfdi4cat/voc4cat_0000247> a skos:Concept ;
    dcterms:identifier "voc4cat_0000247"^^xsd:token ;
    skos:altLabel "carbonylation reaction"@en ;
    skos:broader <https://w3id.org/nfdi4cat/voc4cat_0000183> ;
    skos:definition "A chemical reaction in which a carbonyl group (C=O) is introduced into a molecule, typically through the addition of carbon monoxide (CO) to a substrate."@en ;
    skos:historyNote "0000-0002-6242-2167 Nikolaos G. Moustakas created the resource"@en ;
    skos:inScheme <https://w3id.org/nfdi4cat/voc4cat> ;
    skos:prefLabel "carbonylation"@en .

<https://w3id.org/nfdi4cat/voc4cat_0000248> a skos:Concept ;
    dcterms:identifier "voc4cat_0000248"^^xsd:token ;
    skos:broader <https://w3id.org/nfdi4cat/voc4cat_0000185> ;
    skos:definition "The modification of chemical compounds by biological entities (e.g., enzymes) to yield more biologically active products."@en ;
    skos:historyNote "0000-0002-6242-2167 Nikolaos G. Moustakas created the resource"@en ;
    skos:inScheme <https://w3id.org/nfdi4cat/voc4cat> ;
    skos:prefLabel "biotransformation"@en .

<https://w3id.org/nfdi4cat/voc4cat_0000249> a skos:Concept ;
    dcterms:identifier "voc4cat_0000249"^^xsd:token ;
    skos:broader <https://w3id.org/nfdi4cat/voc4cat_0000185> ;
    skos:definition "A process of separating two enantiomers of a chiral compound in a racemic mixture based on their different reaction rates in a chemical reaction."@en ;
    skos:historyNote "0000-0002-6242-2167 Nikolaos G. Moustakas created the resource"@en ;
    skos:inScheme <https://w3id.org/nfdi4cat/voc4cat> ;
    skos:prefLabel "kinetic resolution"@en .

<https://w3id.org/nfdi4cat/voc4cat_0000250> a skos:Concept ;
    dcterms:identifier "voc4cat_0000250"^^xsd:token ;
    skos:altLabel "water oxidation reaction"@en ;
    skos:broader <https://w3id.org/nfdi4cat/voc4cat_0000185> ;
    skos:definition "The reaction in which water is converted (usually electrochemically or photocatalytically) into oxygen and protons."@en ;
    skos:historyNote "0000-0002-6242-2167 Nikolaos G. Moustakas created the resource"@en ;
    skos:inScheme <https://w3id.org/nfdi4cat/voc4cat> ;
    skos:prefLabel "water oxidation"@en .

<https://w3id.org/nfdi4cat/voc4cat_0000251> a skos:Concept ;
    dcterms:identifier "voc4cat_0000251"^^xsd:token ;
    skos:altLabel "MCR"@en ;
    skos:broader <https://w3id.org/nfdi4cat/voc4cat_0000185> ;
    skos:definition "A synthesis process where three or more compounds react in the same reactor (one-pot reaction) to form a structurally complex single product that incorporates most of the atoms of the starting compounds."@en ;
    skos:historyNote "0000-0002-6242-2167 Nikolaos G. Moustakas created the resource"@en ;
    skos:inScheme <https://w3id.org/nfdi4cat/voc4cat> ;
    skos:prefLabel "multicomponent reaction"@en .

<https://w3id.org/nfdi4cat/voc4cat_0000252> a skos:Concept ;
    dcterms:identifier "voc4cat_0000252"^^xsd:token ;
    skos:altLabel "arylation reaction"@en ;
    skos:broader <https://w3id.org/nfdi4cat/voc4cat_0000183> ;
    skos:definition "A chemical reaction in which one or more aryl groups are added into a molecule, commonly facilitated by a catalyst."@en ;
    skos:historyNote "0000-0002-6242-2167 Nikolaos G. Moustakas created the resource"@en ;
    skos:inScheme <https://w3id.org/nfdi4cat/voc4cat> ;
    skos:prefLabel "arylation"@en .

<https://w3id.org/nfdi4cat/voc4cat_0000253> a skos:Concept ;
    dcterms:identifier "voc4cat_0000253"^^xsd:token ;
    skos:altLabel "hydrogenolysis reaction"@en ;
    skos:broader <https://w3id.org/nfdi4cat/voc4cat_0000183> ;
    skos:definition "A chemical reaction which involves the cleavage of a chemical bond in the presence of hydrogen, often performed catalytically."@en ;
    skos:historyNote "0000-0002-6242-2167 Nikolaos G. Moustakas created the resource"@en ;
    skos:inScheme <https://w3id.org/nfdi4cat/voc4cat> ;
    skos:prefLabel "hydrogenolysis"@en .

<https://w3id.org/nfdi4cat/voc4cat_0000254> a skos:Concept ;
    dcterms:identifier "voc4cat_0000254"^^xsd:token ;
    skos:broader <https://w3id.org/nfdi4cat/voc4cat_0000194> ;
    skos:definition "A material which directs and accelerates an electrochemical reaction while remaining unchanged in the process."@en ;
    skos:historyNote "0000-0002-6242-2167 Nikolaos G. Moustakas created the resource"@en ;
    skos:inScheme <https://w3id.org/nfdi4cat/voc4cat> ;
    skos:prefLabel "electrocatalyst"@en .

<https://w3id.org/nfdi4cat/voc4cat_0000255> a skos:Concept ;
    dcterms:identifier "voc4cat_0000255"^^xsd:token ;
    skos:broader <https://w3id.org/nfdi4cat/voc4cat_0000181> ;
    skos:definition "The characteristics of a material or substance that determine how it interacts or responds to a magnetic field."@en ;
    skos:historyNote "0000-0002-6242-2167 Nikolaos G. Moustakas created the resource, 0000-0002-5898-1820 David Linke edited the definition"@en ;
    skos:inScheme <https://w3id.org/nfdi4cat/voc4cat> ;
    skos:prefLabel "magnetic property"@en .

<https://w3id.org/nfdi4cat/voc4cat_0000256> a skos:Concept ;
    dcterms:identifier "voc4cat_0000256"^^xsd:token ;
    skos:broader <https://w3id.org/nfdi4cat/voc4cat_0000185> ;
    skos:definition "A process that utilizes physical, chemical, or biological processes to turn organic substances, like plant material and animal waste, into high-value products and energy forms (e.g., biofuels)."@en ;
    skos:historyNote "0000-0002-6242-2167 Nikolaos G. Moustakas created the resource"@en ;
    skos:inScheme <https://w3id.org/nfdi4cat/voc4cat> ;
    skos:prefLabel "biomass conversion"@en .

<https://w3id.org/nfdi4cat/voc4cat_0000257> a skos:Concept ;
    dcterms:identifier "voc4cat_0000257"^^xsd:token ;
    skos:broader <https://w3id.org/nfdi4cat/voc4cat_0000181> ;
    skos:definition "The effects a solvent exerts on chemical reactions and molecular properties."@en ;
    skos:historyNote "0000-0002-6242-2167 Nikolaos G. Moustakas created the resource"@en ;
    skos:inScheme <https://w3id.org/nfdi4cat/voc4cat> ;
    skos:prefLabel "solvent effect"@en .

<https://w3id.org/nfdi4cat/voc4cat_0000258> a skos:Concept ;
    dcterms:identifier "voc4cat_0000258"^^xsd:token ;
    skos:altLabel "hydroxylation reaction"@en ;
    skos:broader <https://w3id.org/nfdi4cat/voc4cat_0000183> ;
    skos:definition "The addition of a hydroxyl group (-OH) to a molecule, typically by replacing a hydrogen atom."@en ;
    skos:historyNote "0000-0002-6242-2167 Nikolaos G. Moustakas created the resource"@en ;
    skos:inScheme <https://w3id.org/nfdi4cat/voc4cat> ;
    skos:prefLabel "hydroxylation"@en .

<https://w3id.org/nfdi4cat/voc4cat_0000259> a skos:Concept ;
    dcterms:identifier "voc4cat_0000259"^^xsd:token ;
    skos:altLabel "CO hydrogenation reaction"@en,
        "carbon dioxide hydrogenation"@en,
        "carbon dioxide hydrogenation reaction"@en ;
    skos:broader <https://w3id.org/nfdi4cat/voc4cat_0000183> ;
    skos:definition "The reaction of carbon dioxide (CO2) with molecular hydrogen (H2) to produce value-added hydrocarbons or alcohols."@en ;
    skos:historyNote "0000-0002-6242-2167 Nikolaos G. Moustakas created the resource"@en ;
    skos:inScheme <https://w3id.org/nfdi4cat/voc4cat> ;
    skos:prefLabel "CO2 hydrogenation"@en .

<https://w3id.org/nfdi4cat/voc4cat_0000260> a skos:Concept ;
    dcterms:identifier "voc4cat_0000260"^^xsd:token ;
    skos:altLabel "hydrogenation reaction"@en ;
    skos:broader <https://w3id.org/nfdi4cat/voc4cat_0000183> ;
    skos:definition "A chemical reaction of molecular hydrogen (H2) and another chemical species, typically facilitated by a catalyst."@en ;
    skos:historyNote "0000-0002-6242-2167 Nikolaos G. Moustakas created the resource"@en ;
    skos:inScheme <https://w3id.org/nfdi4cat/voc4cat> ;
    skos:prefLabel "hydrogenation"@en .

<https://w3id.org/nfdi4cat/voc4cat_0000261> a skos:Concept ;
    dcterms:identifier "voc4cat_0000261"^^xsd:token ;
    skos:altLabel "selective oxidation reaction"@en ;
    skos:broader <https://w3id.org/nfdi4cat/voc4cat_0000183> ;
    skos:definition "The targeted oxidation of a specific bond or functional group in a molecule leaving other sites unaffected, often directed by a catalyst."@en ;
    skos:historyNote "0000-0002-6242-2167 Nikolaos G. Moustakas created the resource"@en ;
    skos:inScheme <https://w3id.org/nfdi4cat/voc4cat> ;
    skos:prefLabel "selective oxidation"@en .

<https://w3id.org/nfdi4cat/voc4cat_0000262> a skos:Concept ;
    dcterms:identifier "voc4cat_0000262"^^xsd:token ;
    skos:altLabel "reductive amination reaction"@en ;
    skos:broader <https://w3id.org/nfdi4cat/voc4cat_0000185> ;
    skos:definition "The typically catalyzed reduction of carbonyl groups to form primary and secondary amines, through an imine intermediate."@en ;
    skos:historyNote "0000-0002-6242-2167 Nikolaos G. Moustakas created the resource"@en ;
    skos:inScheme <https://w3id.org/nfdi4cat/voc4cat> ;
    skos:prefLabel "reductive amination"@en .

<https://w3id.org/nfdi4cat/voc4cat_0000263> a skos:Concept ;
    dcterms:identifier "voc4cat_0000263"^^xsd:token ;
    skos:broader <https://w3id.org/nfdi4cat/voc4cat_0000181> ;
    skos:definition "The tendency of a reaction to yield one stereoisomer preferentially over another."@en ;
    skos:historyNote "0000-0002-6242-2167 Nikolaos G. Moustakas created the resource"@en ;
    skos:inScheme <https://w3id.org/nfdi4cat/voc4cat> ;
    skos:prefLabel "stereoselectivity"@en .

<https://w3id.org/nfdi4cat/voc4cat_0000264> a skos:Concept ;
    dcterms:identifier "voc4cat_0000264"^^xsd:token ;
    skos:broader <https://w3id.org/nfdi4cat/voc4cat_0000181> ;
    skos:definition "A field of chemistry focused in solving chemical problems through the use of mathematical modelling, chemical theory and computational techniques."@en ;
    skos:historyNote "0000-0002-6242-2167 Nikolaos G. Moustakas created the resource"@en ;
    skos:inScheme <https://w3id.org/nfdi4cat/voc4cat> ;
    skos:prefLabel "computational chemistry"@en .

<https://w3id.org/nfdi4cat/voc4cat_0000265> a skos:Concept ;
    dcterms:identifier "voc4cat_0000265"^^xsd:token ;
    skos:broader <https://w3id.org/nfdi4cat/voc4cat_0000185> ;
    skos:definition "The application of analytical techniques (e.g., spectroscopy and microscopy) to examine the composition, structure, and properties of surfaces."@en ;
    skos:historyNote "0000-0002-6242-2167 Nikolaos G. Moustakas created the resource"@en ;
    skos:inScheme <https://w3id.org/nfdi4cat/voc4cat> ;
    skos:prefLabel "surface analysis"@en .

<https://w3id.org/nfdi4cat/voc4cat_0000266> a skos:Concept ;
    dcterms:identifier "voc4cat_0000266"^^xsd:token ;
    skos:altLabel "DE"@en ;
    skos:broader <https://w3id.org/nfdi4cat/voc4cat_0000185> ;
    skos:definition "A process of accelerating natural evolution of biological molecules (e.g., proteins, enzymes, nucleic acids) and systems by random mutagenesis and selective screening leading to tailored properties and functionality."@en ;
    skos:historyNote "0000-0002-6242-2167 Nikolaos G. Moustakas created the resource"@en ;
    skos:inScheme <https://w3id.org/nfdi4cat/voc4cat> ;
    skos:prefLabel "directed evolution"@en .

<https://w3id.org/nfdi4cat/voc4cat_0000267> a skos:Concept ;
    dcterms:identifier "voc4cat_0000267"^^xsd:token ;
    skos:broader <https://w3id.org/nfdi4cat/voc4cat_0000181> ;
    skos:definition "A single catalyst, integrating two distinct active sites with complementary functionalities, that participate synergistically in a chemical reaction."@en ;
    skos:historyNote "0000-0002-6242-2167 Nikolaos G. Moustakas created the resource"@en ;
    skos:inScheme <https://w3id.org/nfdi4cat/voc4cat> ;
    skos:prefLabel "bifunctional catalyst"@en .

<https://w3id.org/nfdi4cat/voc4cat_0000268> a skos:Concept ;
    dcterms:identifier "voc4cat_0000268"^^xsd:token ;
    skos:altLabel "syngas"@en ;
    skos:broader <https://w3id.org/nfdi4cat/voc4cat_0000190> ;
    skos:definition "A gas mixture comprised primarily of hydrogen (H2) and carbon monoxide (CO) in various ratios."@en ;
    skos:historyNote "0000-0002-6242-2167 Nikolaos G. Moustakas created the resource"@en ;
    skos:inScheme <https://w3id.org/nfdi4cat/voc4cat> ;
    skos:prefLabel "synthesis gas"@en .

<https://w3id.org/nfdi4cat/voc4cat_0000269> a skos:Concept ;
    dcterms:identifier "voc4cat_0000269"^^xsd:token ;
    skos:altLabel "continuous flow chemistry"@en ;
    skos:broader <https://w3id.org/nfdi4cat/voc4cat_0000185> ;
    skos:definition "A chemical reaction that is performed in a continuous flow stream of reagents."@en ;
    skos:historyNote "0000-0002-6242-2167 Nikolaos G. Moustakas created the resource"@en ;
    skos:inScheme <https://w3id.org/nfdi4cat/voc4cat> ;
    skos:prefLabel "flow chemistry"@en .

<https://w3id.org/nfdi4cat/voc4cat_0000271> a skos:Concept ;
    dcterms:identifier "voc4cat_0000271"^^xsd:token ;
    skos:broader <https://w3id.org/nfdi4cat/voc4cat_0000270> ;
    skos:definition "A porous solid material containing pores with width smaller than 2nm."@en ;
    skos:historyNote "0000-0002-6242-2167 Nikolaos G. Moustakas created the resource"@en ;
    skos:inScheme <https://w3id.org/nfdi4cat/voc4cat> ;
    skos:prefLabel "microporous material"@en .

<https://w3id.org/nfdi4cat/voc4cat_0000272> a skos:Concept ;
    dcterms:identifier "voc4cat_0000272"^^xsd:token ;
    skos:broader <https://w3id.org/nfdi4cat/voc4cat_0000270> ;
    skos:definition "A porous solid material containing pores with width larger than 50nm"@en ;
    skos:historyNote "0000-0002-6242-2167 Nikolaos G. Moustakas created the resource"@en ;
    skos:inScheme <https://w3id.org/nfdi4cat/voc4cat> ;
    skos:prefLabel "macroporous material"@en .

<https://w3id.org/nfdi4cat/voc4cat_0000273> a skos:Concept ;
    dcterms:identifier "voc4cat_0000273"^^xsd:token ;
    skos:broader <https://w3id.org/nfdi4cat/voc4cat_0000185> ;
    skos:definition "A technique of synthesizing substances from high-temperature and high-pressure aqueous solutions, typically performed in a sealed vessel."@en ;
    skos:historyNote "0000-0002-6242-2167 Nikolaos G. Moustakas created the resource"@en ;
    skos:inScheme <https://w3id.org/nfdi4cat/voc4cat> ;
    skos:prefLabel "hydrothermal synthesis"@en .

<https://w3id.org/nfdi4cat/voc4cat_0000274> a skos:Concept ;
    dcterms:identifier "voc4cat_0000274"^^xsd:token ;
    skos:broader <https://w3id.org/nfdi4cat/voc4cat_0000181> ;
    skos:definition "The ability of a chemical action to differentiate between diastereoisomers, leading to the preferential formation of one diastereoisomers over another."@en ;
    skos:historyNote "0000-0002-6242-2167 Nikolaos G. Moustakas created the resource"@en ;
    skos:inScheme <https://w3id.org/nfdi4cat/voc4cat> ;
    skos:prefLabel "diastereoselectivity"@en .

<https://w3id.org/nfdi4cat/voc4cat_0000275> a skos:Concept ;
    dcterms:identifier "voc4cat_0000275"^^xsd:token ;
    skos:broader <https://w3id.org/nfdi4cat/voc4cat_0000181> ;
    skos:definition "The study of water’s properties and its interactions with other substances in chemical reactions."@en ;
    skos:historyNote "0000-0002-6242-2167 Nikolaos G. Moustakas created the resource"@en ;
    skos:inScheme <https://w3id.org/nfdi4cat/voc4cat> ;
    skos:prefLabel "water chemistry"@en .

<https://w3id.org/nfdi4cat/voc4cat_0000276> a skos:Concept ;
    dcterms:identifier "voc4cat_0000276"^^xsd:token ;
    skos:broader <https://w3id.org/nfdi4cat/voc4cat_0000183> ;
    skos:definition "A carbon-carbon bond-forming reaction between the carbonyl groups of two compounds (typically aldehydes or ketones). A carbonyl group of one compound and the α-position of another carbonyl molecule react to form a β-hydroxycarbonyl compound."@en ;
    skos:historyNote "0000-0002-6242-2167 Nikolaos G. Moustakas created the resource"@en ;
    skos:inScheme <https://w3id.org/nfdi4cat/voc4cat> ;
    skos:prefLabel "aldol reaction"@en .

<https://w3id.org/nfdi4cat/voc4cat_0000277> a skos:Concept ;
    dcterms:identifier "voc4cat_0000277"^^xsd:token ;
    skos:altLabel "carbon-hydrogen functionalization"@en ;
    skos:broader <https://w3id.org/nfdi4cat/voc4cat_0000181> ;
    skos:definition "The process of introducing new functional groups by cleaving and modifying a carbon-hydrogen (C-H) bond into C-X (X=heteroatom or functional group)."@en ;
    skos:historyNote "0000-0002-6242-2167 Nikolaos G. Moustakas created the resource"@en ;
    skos:inScheme <https://w3id.org/nfdi4cat/voc4cat> ;
    skos:prefLabel "C-H functionalization"@en .

<https://w3id.org/nfdi4cat/voc4cat_0000278> a skos:Concept ;
    dcterms:identifier "voc4cat_0000278"^^xsd:token ;
    skos:altLabel "Michael addition reaction"@en,
        "Michael reaction"@en ;
    skos:broader <https://w3id.org/nfdi4cat/voc4cat_0000183> ;
    skos:definition "A C-C (or C-X) bond forming reaction in which a nucleophile (typically an enolate), reacts with an α,β-unsaturated carbonyl compound."@en ;
    skos:historyNote "0000-0002-6242-2167 Nikolaos G. Moustakas created the resource"@en ;
    skos:inScheme <https://w3id.org/nfdi4cat/voc4cat> ;
    skos:prefLabel "Michael addition"@en .

<https://w3id.org/nfdi4cat/voc4cat_0000279> a skos:Concept ;
    dcterms:identifier "voc4cat_0000279"^^xsd:token ;
    skos:altLabel "OV"@en ;
    skos:broader <https://w3id.org/nfdi4cat/voc4cat_0000181> ;
    skos:definition "A type of a structural point defect in a crystal lattice where an oxygen atom is missing from its expected position."@en ;
    skos:historyNote "0000-0002-6242-2167 Nikolaos G. Moustakas created the resource"@en ;
    skos:inScheme <https://w3id.org/nfdi4cat/voc4cat> ;
    skos:prefLabel "oxygen vacancy"@en .

<https://w3id.org/nfdi4cat/voc4cat_0000280> a skos:Concept ;
    dcterms:identifier "voc4cat_0000280"^^xsd:token ;
    skos:broader <https://w3id.org/nfdi4cat/voc4cat_0000183> ;
    skos:definition "A catalytic chemical reaction in which a mixture of carbon monoxide (CO) and hydrogen (H2), is converted via a chain-growth mechanism into long-chain hydrocarbons (e.g., alkanes, alkenes or alcohols)—typically using iron or cobalt catalysts under moderate to high pressures and temperatures."@en ;
    skos:historyNote "0000-0002-6242-2167 Nikolaos G. Moustakas created the resource"@en ;
    skos:inScheme <https://w3id.org/nfdi4cat/voc4cat> ;
    skos:prefLabel "Fischer-Tropsch synthesis"@en .

<https://w3id.org/nfdi4cat/voc4cat_0000281> a skos:Concept ;
    dcterms:identifier "voc4cat_0000281"^^xsd:token ;
    skos:broader <https://w3id.org/nfdi4cat/voc4cat_0000185> ;
    skos:definition "The industrial implementation of Fischer–Tropsch synthesis, encompassing in addition the associated engineering, reactor design, feedstock preparation, heat management, and product upgrading steps required for large-scale operation."@en ;
    skos:historyNote "0000-0002-6242-2167 Nikolaos G. Moustakas created the resource"@en ;
    skos:inScheme <https://w3id.org/nfdi4cat/voc4cat> ;
    skos:prefLabel "Fischer-Tropsch process"@en .

<https://w3id.org/nfdi4cat/voc4cat_0000282> a skos:Concept ;
    dcterms:identifier "voc4cat_0000282"^^xsd:token ;
    skos:altLabel "density functional theory calculation"@en ;
    skos:broader <https://w3id.org/nfdi4cat/voc4cat_0000184> ;
    skos:definition "The application of density functional theory (DFT) to compute the electonic structure of atoms, molecules and solids."@en ;
    skos:historyNote "0000-0002-6242-2167 Nikolaos G. Moustakas created the resource"@en ;
    skos:inScheme <https://w3id.org/nfdi4cat/voc4cat> ;
    skos:prefLabel "DFT calculation"@en .

<https://w3id.org/nfdi4cat/voc4cat_0000283> a skos:Concept ;
    dcterms:identifier "voc4cat_0000283"^^xsd:token ;
    skos:broader <https://w3id.org/nfdi4cat/voc4cat_0000183> ;
    skos:definition "The relocation of an electron from one donor chemical species (atom, ion, or molecule) to another chemical entity (acceptor) changing their oxidation states in the process."@en ;
    skos:historyNote "0000-0002-6242-2167 Nikolaos G. Moustakas created the resource"@en ;
    skos:inScheme <https://w3id.org/nfdi4cat/voc4cat> ;
    skos:prefLabel "electron transfer"@en .

<https://w3id.org/nfdi4cat/voc4cat_0000284> a skos:Concept ;
    dcterms:identifier "voc4cat_0000284"^^xsd:token ;
    skos:broader <https://w3id.org/nfdi4cat/voc4cat_0000181> ;
    skos:definition "A ring-shaped compound that contains at least one nitrogen atom as part of its cyclic structure along with carbon atoms."@en ;
    skos:historyNote "0000-0002-6242-2167 Nikolaos G. Moustakas created the resource"@en ;
    skos:inScheme <https://w3id.org/nfdi4cat/voc4cat> ;
    skos:prefLabel "nitrogen heterocycle"@en .

<https://w3id.org/nfdi4cat/voc4cat_0000285> a skos:Concept ;
    dcterms:identifier "voc4cat_0000285"^^xsd:token ;
    skos:broader <https://w3id.org/nfdi4cat/voc4cat_0000185> ;
    skos:definition "The chemical or enzymatic incorporation of carbon dioxide into organic compounds (typically carbohydrates)."@en ;
    skos:historyNote "0000-0002-6242-2167 Nikolaos G. Moustakas created the resource"@en ;
    skos:inScheme <https://w3id.org/nfdi4cat/voc4cat> ;
    skos:prefLabel "carbon dioxide fixation"@en .

<https://w3id.org/nfdi4cat/voc4cat_0000286> a skos:Concept ;
    dcterms:identifier "voc4cat_0000286"^^xsd:token ;
    skos:altLabel "XAS"@en ;
    skos:broader <https://w3id.org/nfdi4cat/voc4cat_0000066> ;
    skos:definition "An element- and orbital- specific analytical technique that probes the energy-dependent absorption of X-rays from synchrotron radiation, to study the electronic and geometric properties of materials."@en ;
    skos:historyNote "0000-0002-6242-2167 Nikolaos G. Moustakas created the resource"@en ;
    skos:inScheme <https://w3id.org/nfdi4cat/voc4cat> ;
    skos:prefLabel "X-ray absorption spectroscopy"@en .

<https://w3id.org/nfdi4cat/voc4cat_0000287> a skos:Concept ;
    dcterms:identifier "voc4cat_0000287"^^xsd:token ;
    skos:broader <https://w3id.org/nfdi4cat/voc4cat_0000181> ;
    skos:definition "An ion or molecule that binds to a central atom through electron pair donation, to form a coordination complex compound."@en ;
    skos:historyNote "0000-0002-6242-2167 Nikolaos G. Moustakas created the resource"@en ;
    skos:inScheme <https://w3id.org/nfdi4cat/voc4cat> ;
    skos:prefLabel "ligand"@en .

<https://w3id.org/nfdi4cat/voc4cat_0000288> a skos:Concept ;
    dcterms:identifier "voc4cat_0000288"^^xsd:token ;
    skos:broader <https://w3id.org/nfdi4cat/voc4cat_0000066> ;
    skos:definition "A microscopy technique that uses an electron beam as a source of sample illumination."@en ;
    skos:historyNote "0000-0002-6242-2167 Nikolaos G. Moustakas created the resource"@en ;
    skos:inScheme <https://w3id.org/nfdi4cat/voc4cat> ;
    skos:prefLabel "electron microscopy"@en .

<https://w3id.org/nfdi4cat/voc4cat_0000289> a skos:Concept ;
    dcterms:identifier "voc4cat_0000289"^^xsd:token ;
    skos:altLabel "CO oxidation reaction"@en,
        "carbon monoxide oxidation"@en,
        "carbon monoxide oxidation reaction"@en ;
    skos:broader <https://w3id.org/nfdi4cat/voc4cat_0000183> ;
    skos:definition "The reaction in which carbon monoxide (CO) is converted to carbon dioxide (CO₂) through interaction with an oxidizing agent, typically oxygen (O₂)."@en ;
    skos:historyNote "0000-0002-6242-2167 Nikolaos G. Moustakas created the resource"@en ;
    skos:inScheme <https://w3id.org/nfdi4cat/voc4cat> ;
    skos:prefLabel "CO oxidation"@en .

<https://w3id.org/nfdi4cat/voc4cat_0000290> a skos:Concept ;
    dcterms:identifier "voc4cat_0000290"^^xsd:token ;
    skos:altLabel "CO2 reduction reaction"@en,
        "carbon dioxide reduction"@en,
        "carbon dioxide reduction reaction"@en ;
    skos:broader <https://w3id.org/nfdi4cat/voc4cat_0000183> ;
    skos:definition "The chemical reaction in which carbon dioxide (CO₂) is converted into value-added chemicals or fuels through electron and proton transfer, typically facilitated by a catalyst under electrochemical, photochemical, or thermochemical conditions."@en ;
    skos:historyNote "0000-0002-6242-2167 Nikolaos G. Moustakas created the resource"@en ;
    skos:inScheme <https://w3id.org/nfdi4cat/voc4cat> ;
    skos:prefLabel "CO2 reduction"@en .

<https://w3id.org/nfdi4cat/voc4cat_0000291> a skos:Concept ;
    dcterms:identifier "voc4cat_0000291"^^xsd:token ;
    skos:broader <https://w3id.org/nfdi4cat/voc4cat_0000185> ;
    skos:definition "The generation of molecular hydrogen (H2) through chemical transformations."@en ;
    skos:historyNote "0000-0002-6242-2167 Nikolaos G. Moustakas created the resource"@en ;
    skos:inScheme <https://w3id.org/nfdi4cat/voc4cat> ;
    skos:prefLabel "hydrogen production"@en .

<https://w3id.org/nfdi4cat/voc4cat_0000292> a skos:Concept ;
    dcterms:identifier "voc4cat_0000292"^^xsd:token ;
    skos:broader <https://w3id.org/nfdi4cat/voc4cat_0000181> ;
    skos:definition "An industrial term that covers the Fischer-Tropsch process and all the systems, equipment, and engineering methods used to apply it at commercial scale. This includes reactors, control systems, and plant designs used to produce synthetic fuels using the Fischer-Tropsch synthesis."@en ;
    skos:historyNote "0000-0002-6242-2167 Nikolaos G. Moustakas created the resource, 0000-0001-6434-6623 Aleksandr Fedorov defined the resource"@en ;
    skos:inScheme <https://w3id.org/nfdi4cat/voc4cat> ;
    skos:prefLabel "Fischer-Tropsch technology"@en .

<https://w3id.org/nfdi4cat/voc4cat_0000293> a skos:Concept ;
    dcterms:identifier "voc4cat_0000293"^^xsd:token ;
    skos:broader <https://w3id.org/nfdi4cat/voc4cat_0000190> ;
    skos:definition "A particle with dimensions in the nanoscale range."@en ;
    skos:historyNote "0000-0002-6242-2167 Nikolaos G. Moustakas created the resource"@en ;
    skos:inScheme <https://w3id.org/nfdi4cat/voc4cat> ;
    skos:prefLabel "nanoparticle"@en .

<https://w3id.org/nfdi4cat/voc4cat_0000294> a skos:Concept ;
    dcterms:identifier "voc4cat_0000294"^^xsd:token ;
    skos:broader <https://w3id.org/nfdi4cat/voc4cat_0000196> ;
    skos:definition "A catalytic process where the catalytic species is present in the same physical phase as the reactants, typically in a sinlge liquid phase."@en ;
    skos:historyNote "0000-0002-6242-2167 Nikolaos G. Moustakas created the resource"@en ;
    skos:inScheme <https://w3id.org/nfdi4cat/voc4cat> ;
    skos:prefLabel "homogeneous catalysis"@en .

<https://w3id.org/nfdi4cat/voc4cat_0000295> a skos:Concept ;
    dcterms:identifier "voc4cat_0000295"^^xsd:token ;
    skos:broader <https://w3id.org/nfdi4cat/voc4cat_0000190> ;
    skos:definition "Organic mass of biological origin."@en ;
    skos:historyNote "0000-0002-6242-2167 Nikolaos G. Moustakas created the resource, 0000-0002-2367-1988 Norbert Kockmann defined the resource"@en ;
    skos:inScheme <https://w3id.org/nfdi4cat/voc4cat> ;
    skos:prefLabel "biomass"@en .

<https://w3id.org/nfdi4cat/voc4cat_0000296> a skos:Concept ;
    dcterms:identifier "voc4cat_0000296"^^xsd:token ;
    skos:broader <https://w3id.org/nfdi4cat/voc4cat_0000196> ;
    skos:definition "Acceleration of a chemical reaction induced by the presence of material that is chemically unchanged at the end of the reaction."@en ;
    skos:historyNote "0000-0002-6242-2167 Nikolaos G. Moustakas created the resource"@en ;
    skos:inScheme <https://w3id.org/nfdi4cat/voc4cat> ;
    skos:prefLabel "catalysis"@en .

<https://w3id.org/nfdi4cat/voc4cat_0000297> a skos:Concept ;
    dcterms:identifier "voc4cat_0000297"^^xsd:token ;
    skos:altLabel "dehydrogenation reaction"@en ;
    skos:broader <https://w3id.org/nfdi4cat/voc4cat_0000183> ;
    skos:definition "A chemical reaction that involves the removal of two or more hydrogen atoms from a molecule."@en ;
    skos:historyNote "0000-0002-6242-2167 Nikolaos G. Moustakas created the resource"@en ;
    skos:inScheme <https://w3id.org/nfdi4cat/voc4cat> ;
    skos:prefLabel "dehydrogenation"@en .

<https://w3id.org/nfdi4cat/voc4cat_0000298> a skos:Concept ;
    dcterms:identifier "voc4cat_0000298"^^xsd:token ;
    skos:broader <https://w3id.org/nfdi4cat/voc4cat_0000181> ;
    skos:definition "The study and characterization of the temporal progression of physical and (bio-)chemical processes, with particular emphasis on the rates and mechanisms by which chemical transformations occur."@en ;
    skos:historyNote "0000-0002-6242-2167 Nikolaos G. Moustakas created the resource"@en ;
    skos:inScheme <https://w3id.org/nfdi4cat/voc4cat> ;
    skos:prefLabel "kinetics"@en .

<https://w3id.org/nfdi4cat/voc4cat_0000299> a skos:Concept ;
    dcterms:identifier "voc4cat_0000299"^^xsd:token ;
    skos:broader <https://w3id.org/nfdi4cat/voc4cat_0000186> ;
    skos:definition "Measure of the acidic strength of a solution."@en ;
    skos:historyNote "0000-0002-6242-2167 Nikolaos G. Moustakas created the resource, 0000-0002-2367-1988 Norbert Kockmann defined the resource"@en ;
    skos:inScheme <https://w3id.org/nfdi4cat/voc4cat> ;
    skos:prefLabel "acidity"@en .

<https://w3id.org/nfdi4cat/voc4cat_0000300> a skos:Concept ;
    dcterms:identifier "voc4cat_0000300"^^xsd:token ;
    skos:broader <https://w3id.org/nfdi4cat/voc4cat_0000190> ;
    skos:definition "Mixture of metals with certain (often improved) mechanical, chemical, electrical, magnetic or other properties."@en ;
    skos:historyNote "0000-0002-6242-2167 Nikolaos G. Moustakas created the resource, 0000-0002-2367-1988 Norbert Kockmann defined the resource"@en ;
    skos:inScheme <https://w3id.org/nfdi4cat/voc4cat> ;
    skos:prefLabel "alloy"@en .

<https://w3id.org/nfdi4cat/voc4cat_0000301> a skos:Concept ;
    dcterms:identifier "voc4cat_0000301"^^xsd:token ;
    skos:broader <https://w3id.org/nfdi4cat/voc4cat_0000181> ;
    skos:definition "A Lewis acid is a molecular entity that functions as an electron-pair acceptor, forming a coordinate covalent bond with a Lewis base through interaction with its lone electron pair."@en ;
    skos:historyNote "0000-0002-6242-2167 Nikolaos G. Moustakas created the resource"@en ;
    skos:inScheme <https://w3id.org/nfdi4cat/voc4cat> ;
    skos:prefLabel "Lewis acid"@en .

<https://w3id.org/nfdi4cat/voc4cat_0000302> a skos:Concept ;
    dcterms:identifier "voc4cat_0000302"^^xsd:token ;
    skos:altLabel "isomerisation reaction"@en,
        "isomerization"@en,
        "isomerization reaction"@en ;
    skos:broader <https://w3id.org/nfdi4cat/voc4cat_0000183> ;
    skos:definition "A chemical reaction in which the main product is an isomer of the main reactant, entailing a change in molecular structure without altering the overall molecular composition."@en ;
    skos:historyNote "0000-0002-6242-2167 Nikolaos G. Moustakas created the resource"@en ;
    skos:inScheme <https://w3id.org/nfdi4cat/voc4cat> ;
    skos:prefLabel "isomerisation"@en .

<https://w3id.org/nfdi4cat/voc4cat_0000303> a skos:Concept ;
    dcterms:identifier "voc4cat_0000303"^^xsd:token ;
    skos:broader <https://w3id.org/nfdi4cat/voc4cat_0000183> ;
    skos:definition "A chemical reaction where one or more alkyl groups is introduced into a molecular structure via covalent bond formation."@en ;
    skos:historyNote "0000-0002-6242-2167 Nikolaos G. Moustakas created the resource"@en ;
    skos:inScheme <https://w3id.org/nfdi4cat/voc4cat> ;
    skos:prefLabel "alkylation"@en .

<https://w3id.org/nfdi4cat/voc4cat_0000304> a skos:Concept ;
    dcterms:identifier "voc4cat_0000304"^^xsd:token ;
    skos:altLabel "polymerisation reaction"@en,
        "polymerization"@en,
        "polymerization reaction"@en ;
    skos:broader <https://w3id.org/nfdi4cat/voc4cat_0000185> ;
    skos:definition "A process in which low molecular weight monomers (of the same or different kind) are combined forming a long-chain or three-dimensional, high molecular weight polymer molecule."@en ;
    skos:historyNote "0000-0002-6242-2167 Nikolaos G. Moustakas created the resource"@en ;
    skos:inScheme <https://w3id.org/nfdi4cat/voc4cat> ;
    skos:prefLabel "polymerisation"@en .

<https://w3id.org/nfdi4cat/voc4cat_0000305> a skos:Concept ;
    dcterms:identifier "voc4cat_0000305"^^xsd:token ;
    skos:broader <https://w3id.org/nfdi4cat/voc4cat_0000186> ;
    skos:definition "The quality of being free from change or variation or not taking part in chemical change."@en ;
    skos:historyNote "0000-0002-6242-2167 Nikolaos G. Moustakas created the resource"@en ;
    skos:inScheme <https://w3id.org/nfdi4cat/voc4cat> ;
    skos:prefLabel "stability"@en .

<https://w3id.org/nfdi4cat/voc4cat_0000306> a skos:Concept ;
    dcterms:identifier "voc4cat_0000306"^^xsd:token ;
    skos:altLabel "hydrolysis reaction"@en ;
    skos:broader <https://w3id.org/nfdi4cat/voc4cat_0000183> ;
    skos:definition "A solvolysis reaction where the solvent material is water."@en ;
    skos:historyNote "0000-0002-6242-2167 Nikolaos G. Moustakas created the resource"@en ;
    skos:inScheme <https://w3id.org/nfdi4cat/voc4cat> ;
    skos:prefLabel "hydrolysis"@en .

<https://w3id.org/nfdi4cat/voc4cat_0000307> a skos:Concept ;
    dcterms:identifier "voc4cat_0000307"^^xsd:token ;
    skos:altLabel "POM"@en ;
    skos:broader <https://w3id.org/nfdi4cat/voc4cat_0000190> ;
    skos:definition "An anionic metal-oxygen cluster composed of early transition metals in high oxidation states, interconnected by shared oxygen atoms to form a closed 3-dimensional framework."@en ;
    skos:historyNote "0000-0002-6242-2167 Nikolaos G. Moustakas created the resource"@en ;
    skos:inScheme <https://w3id.org/nfdi4cat/voc4cat> ;
    skos:prefLabel "polyoxometalate"@en .

<https://w3id.org/nfdi4cat/voc4cat_0000308> a skos:Concept ;
    dcterms:identifier "voc4cat_0000308"^^xsd:token ;
    skos:broader <https://w3id.org/nfdi4cat/voc4cat_0000186> ;
    skos:definition "Measure of the basic strength from OH- ions of a solution."@en ;
    skos:historyNote "0000-0002-6242-2167 Nikolaos G. Moustakas created the resource, 0000-0002-2367-1988 Norbert Kockmann defined the resource"@en ;
    skos:inScheme <https://w3id.org/nfdi4cat/voc4cat> ;
    skos:prefLabel "basicity"@en .

<https://w3id.org/nfdi4cat/voc4cat_0000309> a skos:Concept ;
    dcterms:identifier "voc4cat_0000309"^^xsd:token ;
    skos:broader <https://w3id.org/nfdi4cat/voc4cat_0000181> ;
    skos:definition "A chemical element in the d-block of the periodic table with a partially filled d-orbital."@en ;
    skos:historyNote "0000-0002-6242-2167 Nikolaos G. Moustakas created the resource"@en ;
    skos:inScheme <https://w3id.org/nfdi4cat/voc4cat> ;
    skos:prefLabel "transition metal"@en .

<https://w3id.org/nfdi4cat/voc4cat_0007001> a skos:Concept ;
    dcterms:identifier "voc4cat_0007001"^^xsd:token ;
    skos:broader <https://w3id.org/nfdi4cat/voc4cat_0000196> ;
    skos:definition "A process during which a chemical reaction is accelerated by the presence of a catalyst in a different phase than the reactant. The reaction generally proceeds at the interface."@en ;
    skos:historyNote "0000-0002-4041-0165 Julia Schumann created the resource"@en ;
    skos:inScheme <https://w3id.org/nfdi4cat/voc4cat> ;
    skos:prefLabel "heterogeneous catalysis"@en .

<https://w3id.org/nfdi4cat/voc4cat_0007002> a skos:Concept ;
    dcterms:identifier "voc4cat_0007002"^^xsd:token ;
    skos:broader <https://w3id.org/nfdi4cat/voc4cat_0000196> ;
    skos:definition "A process, during which elevated temperature is applied to increase the reaction rate of a reaction in presence of a catalyst."@en ;
    skos:historyNote "0000-0002-4041-0165 Julia Schumann created the resource"@en ;
    skos:inScheme <https://w3id.org/nfdi4cat/voc4cat> ;
    skos:prefLabel "thermal catalysis"@en .

<https://w3id.org/nfdi4cat/voc4cat_0007003> a skos:Concept ;
    dcterms:identifier "voc4cat_0007003"^^xsd:token ;
    skos:broader <https://w3id.org/nfdi4cat/voc4cat_0000194> ;
    skos:definition "A substance that increases the rate of a chemical reaction that is in a different phase than the reagents."@en ;
    skos:historyNote "0000-0002-4041-0165 Julia Schumann created the resource"@en ;
    skos:inScheme <https://w3id.org/nfdi4cat/voc4cat> ;
    skos:prefLabel "heterogeneous catalyst"@en .

<https://w3id.org/nfdi4cat/voc4cat_0007034> a skos:Concept ;
    dcterms:identifier "voc4cat_0007034"^^xsd:token ;
    skos:broader <https://w3id.org/nfdi4cat/voc4cat_0000194> ;
    skos:definition "A catalyst where the active material is usually the minority phase and fixed on a high surface area, relatively inert solid."@en ;
    skos:historyNote "0000-0002-4041-0165 Julia Schumann created the resource"@en ;
    skos:inScheme <https://w3id.org/nfdi4cat/voc4cat> ;
    skos:prefLabel "supported catalyst"@en .

<https://w3id.org/nfdi4cat/voc4cat_0007035> a skos:Concept ;
    dcterms:identifier "voc4cat_0007035"^^xsd:token ;
    skos:broader <https://w3id.org/nfdi4cat/voc4cat_0007017> ;
    skos:definition "A device designed for the controlled execution of chemical reactions."@en ;
    skos:historyNote "0000-0002-4041-0165 Julia Schumann created the resource"@en ;
    skos:inScheme <https://w3id.org/nfdi4cat/voc4cat> ;
    skos:narrower <https://w3id.org/nfdi4cat/voc4cat_0007036> ;
    skos:prefLabel "chemical reactor"@en .

<https://w3id.org/nfdi4cat/voc4cat_0007104> a skos:Concept ;
    dcterms:identifier "voc4cat_0007104"^^xsd:token ;
    skos:broader <https://w3id.org/nfdi4cat/voc4cat_0007101> ;
    skos:definition "A reactor model, in which opposing to the ideal plug flow behavior, friction is acting on the fluid, thus creating a residence time distribution."@en ;
    skos:historyNote "0000-0001-5886-7860 Hendrik Borgelt created this resource, 0000-0002-5898-1820 David Linke contributed to the definition of the resource"@en ;
    skos:inScheme <https://w3id.org/nfdi4cat/voc4cat> ;
    skos:narrower <https://w3id.org/nfdi4cat/voc4cat_0007105> ;
    skos:prefLabel "tubular reactor model"@en .

<https://w3id.org/nfdi4cat/voc4cat_0007220> a skos:Concept ;
    dcterms:identifier "voc4cat_0007220"^^xsd:token ;
    skos:broader <https://w3id.org/nfdi4cat/voc4cat_0000186> ;
    skos:definition "The movement of electrical charges in a conductor; carried by electrons in an electronic conductor (electronic current) or by ions in an ionic conductor (ionic current)."@en ;
    skos:historyNote "0009-0008-1278-8890 Michael Götte created the resource"@en ;
    skos:inScheme <https://w3id.org/nfdi4cat/voc4cat> ;
    skos:narrower <https://w3id.org/nfdi4cat/voc4cat_0007259> ;
    skos:prefLabel "current"@en .

<https://w3id.org/nfdi4cat/voc4cat_0000001> a skos:Concept ;
    dcterms:identifier "voc4cat_0000001"^^xsd:token ;
    skos:broader <https://w3id.org/nfdi4cat/voc4cat_0000196> ;
    skos:definition "A process which catalyzes a chemical reaction through the absorption of sufficient light energy by a photocatalyst."@en ;
    skos:historyNote "0000-0002-6242-2167 Nikolaos G. Moustakas created the resource"@en ;
    skos:inScheme <https://w3id.org/nfdi4cat/voc4cat> ;
    skos:prefLabel "photocatalysis"@en .

<https://w3id.org/nfdi4cat/voc4cat_0000002> a skos:Concept ;
    dcterms:identifier "voc4cat_0000002"^^xsd:token ;
    skos:altLabel "photocatalytic material"@en ;
    skos:broader <https://w3id.org/nfdi4cat/voc4cat_0000194> ;
    skos:definition "A material that absorbs photons (light) of appropriate energy and initiates or accelerates a photochemical reaction, while it regenerates itself after each reaction cycle."@en ;
    skos:historyNote "0000-0002-6242-2167 Nikolaos G. Moustakas created the resource"@en ;
    skos:inScheme <https://w3id.org/nfdi4cat/voc4cat> ;
    skos:prefLabel "photocatalyst"@en .

<https://w3id.org/nfdi4cat/voc4cat_0000014> a skos:Concept ;
    dcterms:identifier "voc4cat_0000014"^^xsd:token ;
    skos:broader <https://w3id.org/nfdi4cat/voc4cat_0000185> ;
    skos:definition "Techniques used to modify the properties of a catalyst, with the aim to increase its efficiency in a catalytic application."@en ;
    skos:historyNote "0000-0002-6242-2167 Nikolaos G. Moustakas created the resource"@en ;
    skos:inScheme <https://w3id.org/nfdi4cat/voc4cat> ;
    skos:narrower <https://w3id.org/nfdi4cat/voc4cat_0000015> ;
    skos:prefLabel "modification technique"@en .

<https://w3id.org/nfdi4cat/voc4cat_0000015> a skos:Concept ;
    dcterms:identifier "voc4cat_0000015"^^xsd:token ;
    skos:broader <https://w3id.org/nfdi4cat/voc4cat_0000014> ;
    skos:definition "The introduction of foreign atoms into a semiconductor leading to the formation of new energy levels and charge concentrations."@en ;
    skos:historyNote "0000-0002-6242-2167 Nikolaos G. Moustakas created the resource"@en ;
    skos:inScheme <https://w3id.org/nfdi4cat/voc4cat> ;
    skos:prefLabel "doping"@en .

<https://w3id.org/nfdi4cat/voc4cat_0000037> a skos:Concept ;
    dcterms:identifier "voc4cat_0000037"^^xsd:token ;
    skos:altLabel "substrate surface area"@en ;
    skos:broader <https://w3id.org/nfdi4cat/voc4cat_0000033>,
        <https://w3id.org/nfdi4cat/voc4cat_0000186> ;
    skos:definition "The surface area of the substrate."@en ;
    skos:historyNote "0000-0002-6242-2167 Nikolaos G. Moustakas created the resource"@en ;
    skos:inScheme <https://w3id.org/nfdi4cat/voc4cat> ;
    skos:prefLabel "substrate area"@en .

<https://w3id.org/nfdi4cat/voc4cat_0000049> a skos:Concept ;
    dcterms:identifier "voc4cat_0000049"^^xsd:token ;
    skos:altLabel "synthesis design"@en,
        "synthetic method"@en ;
    skos:broader <https://w3id.org/nfdi4cat/voc4cat_0000185> ;
    skos:definition "Necessary steps needed to follow to reach the desired catalyst."@en ;
    skos:historyNote "0000-0002-6242-2167 Nikolaos G. Moustakas created the resource"@en ;
    skos:inScheme <https://w3id.org/nfdi4cat/voc4cat> ;
    skos:prefLabel "synthesis procedure"@en .

<https://w3id.org/nfdi4cat/voc4cat_0000067> a skos:Concept ;
    dcterms:identifier "voc4cat_0000067"^^xsd:token ;
    skos:altLabel "X-ray emission spectrometry"@en,
        "X-ray fluorescence spectrometry"@en,
        "X-ray fluorescence spectroscopy"@en,
        "XES"@en,
        "XRES"@en,
        "XRF"@en,
        "XRF spectrometry"@en,
        "XRF spectroscopy"@en ;
    skos:broader <https://w3id.org/nfdi4cat/voc4cat_0000066> ;
    skos:definition "A non-destructive analytical technique which uses a high-energy X-ray source to expose a material and monitors the emitted characteristic fluorescent X-Rays."@en ;
    skos:historyNote "0000-0002-6242-2167 Nikolaos G. Moustakas created the resource"@en ;
    skos:inScheme <https://w3id.org/nfdi4cat/voc4cat> ;
    skos:prefLabel "X-ray fluorescence"@en .

<https://w3id.org/nfdi4cat/voc4cat_0000068> a skos:Concept ;
    dcterms:identifier "voc4cat_0000068"^^xsd:token ;
    skos:altLabel "EELS"@en ;
    skos:broader <https://w3id.org/nfdi4cat/voc4cat_0000066> ;
    skos:definition "An analytical technique used to measure the energy loss of electrons passing through a sample."@en ;
    skos:historyNote "0000-0002-6242-2167 Nikolaos G. Moustakas created the resource"@en ;
    skos:inScheme <https://w3id.org/nfdi4cat/voc4cat> ;
    skos:prefLabel "electron energy loss spectroscopy"@en .

<https://w3id.org/nfdi4cat/voc4cat_0000070> a skos:Concept ;
    dcterms:identifier "voc4cat_0000070"^^xsd:token ;
    skos:altLabel "AFM"@en,
        "SFM"@en,
        "atomic force imaging"@en,
        "atomic-force microscopy"@en,
        "scanning force microscopy"@en ;
    skos:broader <https://w3id.org/nfdi4cat/voc4cat_0000066> ;
    skos:definition "A high-resolution imaging technique that measures the interaction between a sharp probe and the sample’s surface to create a three-dimensional image of the surface’s morphology."@en ;
    skos:historyNote "0000-0002-6242-2167 Nikolaos G. Moustakas created the resource"@en ;
    skos:inScheme <https://w3id.org/nfdi4cat/voc4cat> ;
    skos:prefLabel "atomic force microscopy"@en .

<https://w3id.org/nfdi4cat/voc4cat_0000071> a skos:Concept ;
    dcterms:identifier "voc4cat_0000071"^^xsd:token ;
    skos:altLabel "DSC"@en,
        "differential scanning calorimetric (DSC) analysis"@en,
        "differential scanning calorimetric analysis"@en ;
    skos:broader <https://w3id.org/nfdi4cat/voc4cat_0000066> ;
    skos:definition "A thermal analysis technique which compares the heat flow in a sample and a reference material under controlled applied temperature profiles."@en ;
    skos:historyNote "0000-0002-6242-2167 Nikolaos G. Moustakas created the resource"@en ;
    skos:inScheme <https://w3id.org/nfdi4cat/voc4cat> ;
    skos:prefLabel "differential scanning calorimetry"@en .

<https://w3id.org/nfdi4cat/voc4cat_0000072> a skos:Concept ;
    dcterms:identifier "voc4cat_0000072"^^xsd:token ;
    skos:altLabel "TG"@en,
        "TG analysis"@en,
        "TG measurements"@en,
        "TGA"@en,
        "thermal gravimetric analysis"@en,
        "thermo-gravimetric analysis"@en,
        "thermogravimetric (TG) analyses"@en,
        "thermogravimetric (TG) analysis"@en ;
    skos:broader <https://w3id.org/nfdi4cat/voc4cat_0000066> ;
    skos:definition "A thermal analysis technique used to measure the change of a sample’s mass under the influence of controlled applied temperature profiles."@en ;
    skos:historyNote "0000-0002-6242-2167 Nikolaos G. Moustakas created the resource"@en ;
    skos:inScheme <https://w3id.org/nfdi4cat/voc4cat> ;
    skos:prefLabel "thermogravimetric analysis"@en .

<https://w3id.org/nfdi4cat/voc4cat_0000074> a skos:Concept ;
    dcterms:identifier "voc4cat_0000074"^^xsd:token ;
    skos:altLabel "PL"@en ;
    skos:broader <https://w3id.org/nfdi4cat/voc4cat_0000066> ;
    skos:definition "Light emission of lower energy photons from a sample upon its photoexcitation."@en ;
    skos:historyNote "0000-0002-6242-2167 Nikolaos G. Moustakas created the resource"@en ;
    skos:inScheme <https://w3id.org/nfdi4cat/voc4cat> ;
    skos:prefLabel "photoluminescence"@en .

<https://w3id.org/nfdi4cat/voc4cat_0000075> a skos:Concept ;
    dcterms:identifier "voc4cat_0000075"^^xsd:token ;
    skos:altLabel "SEM"@en ;
    skos:broader <https://w3id.org/nfdi4cat/voc4cat_0000066> ;
    skos:definition "An electron microscopy technique that produces high-resolution images under high magnification of a sample's surface by assessing the secondary and back-scattered electrons produced by a focused electron beam."@en ;
    skos:historyNote "0000-0002-6242-2167 Nikolaos G. Moustakas created the resource"@en ;
    skos:inScheme <https://w3id.org/nfdi4cat/voc4cat> ;
    skos:prefLabel "scanning electron microscopy"@en .

<https://w3id.org/nfdi4cat/voc4cat_0000076> a skos:Concept ;
    dcterms:identifier "voc4cat_0000076"^^xsd:token ;
    skos:altLabel "XPS"@en ;
    skos:broader <https://w3id.org/nfdi4cat/voc4cat_0000066> ;
    skos:definition "A technique that analyzes the chemical composition of an X-ray irradiated sample by measuring the energies of the emitted electrons."@en ;
    skos:historyNote "0000-0002-6242-2167 Nikolaos G. Moustakas created the resource"@en ;
    skos:inScheme <https://w3id.org/nfdi4cat/voc4cat> ;
    skos:prefLabel "X-ray photoelectron spectroscopy"@en .

<https://w3id.org/nfdi4cat/voc4cat_0000077> a skos:Concept ;
    dcterms:identifier "voc4cat_0000077"^^xsd:token ;
    skos:altLabel "X-ray analysis"@en,
        "X-ray crystallographic analysis"@en,
        "X-ray crystallography"@en,
        "X-ray diffraction analysis"@en,
        "X-ray diffractometry"@en,
        "X-ray structure determination"@en,
        "XRD"@en ;
    skos:broader <https://w3id.org/nfdi4cat/voc4cat_0000066> ;
    skos:definition "A technique which analyses the diffraction pattern produced when X-rays are scattered by a sample bombarded by a focused electron beam."@en ;
    skos:historyNote "0000-0002-6242-2167 Nikolaos G. Moustakas created the resource"@en ;
    skos:inScheme <https://w3id.org/nfdi4cat/voc4cat> ;
    skos:prefLabel "X-ray diffraction"@en .

<https://w3id.org/nfdi4cat/voc4cat_0000078> a skos:Concept ;
    dcterms:identifier "voc4cat_0000078"^^xsd:token ;
    skos:altLabel "TEM"@en ;
    skos:broader <https://w3id.org/nfdi4cat/voc4cat_0000066> ;
    skos:definition "Transmission electron microscopy is a technique that produces high-resolution images if the internal structure of a sample by using a beam of electrons to bombard the thin sample and measuring the intensity of the scattered transmitted electrons."@en ;
    skos:historyNote "0000-0002-6242-2167 Nikolaos G. Moustakas created the resource"@en ;
    skos:inScheme <https://w3id.org/nfdi4cat/voc4cat> ;
    skos:prefLabel "transmission electron microscopy"@en .

<https://w3id.org/nfdi4cat/voc4cat_0000079> a skos:Concept ;
    dcterms:identifier "voc4cat_0000079"^^xsd:token ;
    skos:altLabel "UV-Vis"@en ;
    skos:broader <https://w3id.org/nfdi4cat/voc4cat_0000066> ;
    skos:definition "A technique used to measure the absorption, transmission or reflectance of light by a sample in the ultraviolet and visible regions of the electromagnetic spectrum."@en ;
    skos:historyNote "0000-0002-6242-2167 Nikolaos G. Moustakas created the resource"@en ;
    skos:inScheme <https://w3id.org/nfdi4cat/voc4cat> ;
    skos:prefLabel "ultraviolet-visible spectroscopy"@en .

<https://w3id.org/nfdi4cat/voc4cat_0000081> a skos:Concept ;
    dcterms:identifier "voc4cat_0000081"^^xsd:token ;
    skos:altLabel "BET"@en ;
    skos:broader <https://w3id.org/nfdi4cat/voc4cat_0000066> ;
    skos:definition "The study of physical adsorption of gas molecules on a solid surface for the calculation of the specific surface area of materials."@en ;
    skos:historyNote "0000-0002-6242-2167 Nikolaos G. Moustakas created the resource"@en ;
    skos:inScheme <https://w3id.org/nfdi4cat/voc4cat> ;
    skos:prefLabel "Brunauer-Emmett-Teller surface area analysis"@en .

<https://w3id.org/nfdi4cat/voc4cat_0000082> a skos:Concept ;
    dcterms:identifier "voc4cat_0000082"^^xsd:token ;
    skos:altLabel "CV"@en,
        "cyclovoltammetry"@en ;
    skos:broader <https://w3id.org/nfdi4cat/voc4cat_0007237> ;
    skos:definition "An electrochemical technique used to study the redox properties of a sample by measuring the current produced by an applied voltage sweep."@en ;
    skos:historyNote "0000-0002-6242-2167 Nikolaos G. Moustakas created the resource"@en ;
    skos:inScheme <https://w3id.org/nfdi4cat/voc4cat> ;
    skos:prefLabel "cyclic voltammetry"@en .

<https://w3id.org/nfdi4cat/voc4cat_0000083> a skos:Concept ;
    dcterms:identifier "voc4cat_0000083"^^xsd:token ;
    skos:broader <https://w3id.org/nfdi4cat/voc4cat_0000066> ;
    skos:definition "A method used in cyclic voltammetry to determine the charge carrier concentration and the flat-band potential of an electrochemical system by measuring the capacitance as a function of applied voltage."@en ;
    skos:historyNote "0000-0002-6242-2167 Nikolaos G. Moustakas created the resource"@en ;
    skos:inScheme <https://w3id.org/nfdi4cat/voc4cat> ;
    skos:prefLabel "Mott-Schottky analysis"@en .

<https://w3id.org/nfdi4cat/voc4cat_0000093> a skos:Concept ;
    dcterms:identifier "voc4cat_0000093"^^xsd:token ;
    skos:broader <https://w3id.org/nfdi4cat/voc4cat_0000183> ;
    skos:definition "The adhesion of a gas, liquid or dissolved solid chemical of interest onto a solid surface."@en ;
    skos:historyNote "0000-0002-6242-2167 Nikolaos G. Moustakas created the resource"@en ;
    skos:inScheme <https://w3id.org/nfdi4cat/voc4cat> ;
    skos:prefLabel "adsorption"@en .

<https://w3id.org/nfdi4cat/voc4cat_0000097> a skos:Concept ;
    dcterms:identifier "voc4cat_0000097"^^xsd:token ;
    skos:broader <https://w3id.org/nfdi4cat/voc4cat_0000183> ;
    skos:definition "The loss of electrons or an increase in the oxidation state of a species."@en ;
    skos:historyNote "0000-0002-6242-2167 Nikolaos G. Moustakas created the resource"@en ;
    skos:inScheme <https://w3id.org/nfdi4cat/voc4cat> ;
    skos:prefLabel "oxidation"@en .

<https://w3id.org/nfdi4cat/voc4cat_0000098> a skos:Concept ;
    dcterms:identifier "voc4cat_0000098"^^xsd:token ;
    skos:broader <https://w3id.org/nfdi4cat/voc4cat_0000183> ;
    skos:definition "The gain of electrons or a decrease in the oxidation state of a species."@en ;
    skos:historyNote "0000-0002-6242-2167 Nikolaos G. Moustakas created the resource"@en ;
    skos:inScheme <https://w3id.org/nfdi4cat/voc4cat> ;
    skos:prefLabel "reduction"@en .

<https://w3id.org/nfdi4cat/voc4cat_0000130> a skos:Concept ;
    dcterms:identifier "voc4cat_0000130"^^xsd:token ;
    skos:altLabel "GC"@en ;
    skos:broader <https://w3id.org/nfdi4cat/voc4cat_0000185> ;
    skos:definition "An analytical technique that separates and analyzes the components of a gas mixture by passing it though a stationary phase."@en ;
    skos:historyNote "0000-0002-6242-2167 Nikolaos G. Moustakas created the resource"@en ;
    skos:inScheme <https://w3id.org/nfdi4cat/voc4cat> ;
    skos:prefLabel "gas chromatography"@en .

<https://w3id.org/nfdi4cat/voc4cat_0000137> a skos:Concept ;
    dcterms:identifier "voc4cat_0000137"^^xsd:token ;
    skos:altLabel "MS"@en ;
    skos:broader <https://w3id.org/nfdi4cat/voc4cat_0000185> ;
    skos:definition "An analytical technique which determines the mass-to-charge ratio of ions in a sample to give information about the composition of the sample."@en ;
    skos:historyNote "0000-0002-6242-2167 Nikolaos G. Moustakas created the resource"@en ;
    skos:inScheme <https://w3id.org/nfdi4cat/voc4cat> ;
    skos:prefLabel "mass spectrometry"@en .

<https://w3id.org/nfdi4cat/voc4cat_0000141> a skos:Concept ;
    dcterms:identifier "voc4cat_0000141"^^xsd:token ;
    skos:altLabel "LC"@en ;
    skos:broader <https://w3id.org/nfdi4cat/voc4cat_0000185> ;
    skos:definition "A sepation technique that uses a liquid mobile phase to separate the components of a mixture based on their interactions with a stationary phase and a mobile phase."@en ;
    skos:historyNote "0000-0002-6242-2167 Nikolaos G. Moustakas created the resource"@en ;
    skos:inScheme <https://w3id.org/nfdi4cat/voc4cat> ;
    skos:prefLabel "liquid chromatography"@en .

<https://w3id.org/nfdi4cat/voc4cat_0000146> a skos:Concept ;
    dcterms:identifier "voc4cat_0000146"^^xsd:token ;
    skos:altLabel "pressure controller"@en,
        "pressure controller and monitor"@en,
        "pressure gauge"@en,
        "pressure monitor"@en ;
    skos:broader <https://w3id.org/nfdi4cat/voc4cat_0000187> ;
    skos:definition "Equipment (e.g., a vacuum pump) used for controlling and / or monitoring the pressure in various parts of a reactor."@en ;
    skos:historyNote "0000-0002-6242-2167 Nikolaos G. Moustakas created the resource"@en ;
    skos:inScheme <https://w3id.org/nfdi4cat/voc4cat> ;
    skos:narrower <https://w3id.org/nfdi4cat/voc4cat_0000147> ;
    skos:prefLabel "pressure controller"@en .

<https://w3id.org/nfdi4cat/voc4cat_0000163> a skos:Concept ;
    dcterms:identifier "voc4cat_0000163"^^xsd:token ;
    skos:altLabel "gas flow controller and monitor"@en ;
    skos:broader <https://w3id.org/nfdi4cat/voc4cat_0000187> ;
    skos:definition "Equipment used for controlling and / or monitoring the flow of gases (reactant or inert) needed for a catalytic experiment. Mass flow controllers (MFCs) are commonly used to control gas flows."@en ;
    skos:historyNote "0000-0002-6242-2167 Nikolaos G. Moustakas created the resource"@en ;
    skos:inScheme <https://w3id.org/nfdi4cat/voc4cat> ;
    skos:narrower <https://w3id.org/nfdi4cat/voc4cat_0000164> ;
    skos:prefLabel "gas flow controller"@en .

<https://w3id.org/nfdi4cat/voc4cat_0000165> a skos:Concept ;
    dcterms:identifier "voc4cat_0000165"^^xsd:token ;
    skos:broader <https://w3id.org/nfdi4cat/voc4cat_0000189> ;
    skos:definition "All the necessary equipment needed to perform a catalytic experiment involving irradiation. The system apart from the light source can include, filters, power units, lamp cooling devices etc.."@en ;
    skos:historyNote "0000-0002-6242-2167 Nikolaos G. Moustakas created the resource"@en ;
    skos:inScheme <https://w3id.org/nfdi4cat/voc4cat> ;
    skos:narrower <https://w3id.org/nfdi4cat/voc4cat_0000166> ;
    skos:prefLabel "irradiation system"@en .

<https://w3id.org/nfdi4cat/voc4cat_0000178> a skos:Concept ;
    dcterms:identifier "voc4cat_0000178"^^xsd:token ;
    skos:altLabel "VIS"@en,
        "Vis"@en,
        "visible light"@en ;
    skos:broader <https://w3id.org/nfdi4cat/voc4cat_0000181> ;
    skos:definition "Electromagnetic radiation with wavelengths visible to the human eye, typically in the range of 400-800 nm."@en ;
    skos:historyNote "0000-0002-6242-2167 Nikolaos G. Moustakas created the resource"@en ;
    skos:inScheme <https://w3id.org/nfdi4cat/voc4cat> ;
    skos:prefLabel "visible"@en .

<https://w3id.org/nfdi4cat/voc4cat_0000188> a skos:Concept ;
    dcterms:identifier "voc4cat_0000188"^^xsd:token ;
    skos:broader <https://w3id.org/nfdi4cat/voc4cat_0000187> ;
    skos:definition "Components being integral parts of a catalytic reactor."@en ;
    skos:historyNote "0000-0002-6242-2167 Nikolaos G. Moustakas created the resource"@en ;
    skos:inScheme <https://w3id.org/nfdi4cat/voc4cat> ;
    skos:narrower <https://w3id.org/nfdi4cat/voc4cat_0000152>,
        <https://w3id.org/nfdi4cat/voc4cat_0007020> ;
    skos:prefLabel "reactor equipment"@en .

<https://w3id.org/nfdi4cat/voc4cat_0000189> a skos:Concept ;
    dcterms:identifier "voc4cat_0000189"^^xsd:token ;
    skos:broader <https://w3id.org/nfdi4cat/voc4cat_0000187> ;
    skos:definition "Optical systems involved in light irradiation."@en ;
    skos:historyNote "0000-0002-6242-2167 Nikolaos G. Moustakas created the resource"@en ;
    skos:inScheme <https://w3id.org/nfdi4cat/voc4cat> ;
    skos:narrower <https://w3id.org/nfdi4cat/voc4cat_0000157>,
        <https://w3id.org/nfdi4cat/voc4cat_0000165> ;
    skos:prefLabel "optical equipment"@en .

<https://w3id.org/nfdi4cat/voc4cat_0005004> a skos:Concept ;
    dcterms:identifier "voc4cat_0005004"^^xsd:token ;
    skos:broader <https://w3id.org/nfdi4cat/voc4cat_0005001>,
        <https://w3id.org/nfdi4cat/voc4cat_0005002>,
        <https://w3id.org/nfdi4cat/voc4cat_0005003> ;
    skos:definition "A dimensionless physical quantity describing the fraction of a reactant that reacts in a chemical conversion. If a reactant is consumed completely its conversion is 1 (or 100 %)."@en ;
    skos:historyNote "0000-0002-5898-1820 David Linke created the resource"@en ;
    skos:inScheme <https://w3id.org/nfdi4cat/voc4cat> ;
    skos:prefLabel "conversion"@en .

<https://w3id.org/nfdi4cat/voc4cat_0005005> a skos:Concept ;
    dcterms:identifier "voc4cat_0005005"^^xsd:token ;
    skos:broader <https://w3id.org/nfdi4cat/voc4cat_0005001>,
        <https://w3id.org/nfdi4cat/voc4cat_0005002>,
        <https://w3id.org/nfdi4cat/voc4cat_0005003> ;
    skos:definition "A dimensionless physical quantity describing the fraction of a product B that is formed from a reactant A taking into account the stoichiometry. If A fully reacts to B without side-reactions, the yield of product B is 1 (or 100 %)."@en ;
    skos:historyNote "0000-0002-5898-1820 David Linke created the resource"@en ;
    skos:inScheme <https://w3id.org/nfdi4cat/voc4cat> ;
    skos:prefLabel "yield"@en .

<https://w3id.org/nfdi4cat/voc4cat_0005006> a skos:Concept ;
    dcterms:identifier "voc4cat_0005006"^^xsd:token ;
    skos:broader <https://w3id.org/nfdi4cat/voc4cat_0005001>,
        <https://w3id.org/nfdi4cat/voc4cat_0005002>,
        <https://w3id.org/nfdi4cat/voc4cat_0005003> ;
    skos:definition """A physical quantity that describes the amount of product produced per unit of time and unit of producing entity. The producing entity is for example the volume of a chemical reactor or in catalysis the mass or volume or moles of catalyst.
Example unit: kg{product} / (hour * cubicmeter{catalyst})"""@en ;
    skos:historyNote "0000-0002-5898-1820 David Linke created the resource"@en ;
    skos:inScheme <https://w3id.org/nfdi4cat/voc4cat> ;
    skos:prefLabel "space-time yield"@en .

<https://w3id.org/nfdi4cat/voc4cat_0007036> a skos:Concept ;
    dcterms:identifier "voc4cat_0007036"^^xsd:token ;
    skos:broader <https://w3id.org/nfdi4cat/voc4cat_0007017>,
        <https://w3id.org/nfdi4cat/voc4cat_0007035> ;
    skos:definition "A chemical reactor in which the reaction is carried out in the presence of a catalyst."@en ;
    skos:historyNote "0000-0002-4041-0165 Julia Schumann created the resource"@en ;
    skos:inScheme <https://w3id.org/nfdi4cat/voc4cat> ;
    skos:narrower <https://w3id.org/nfdi4cat/voc4cat_0007019> ;
    skos:prefLabel "catalytic reactor"@en .

<https://w3id.org/nfdi4cat/voc4cat_0007045> a skos:Concept ;
    dcterms:identifier "voc4cat_0007045"^^xsd:token ;
    skos:broader <https://w3id.org/nfdi4cat/voc4cat_0000180> ;
    skos:definition "A physical entity which is a human beeing."@en ;
    skos:historyNote "0000-0002-4041-0165 Julia Schumann created the resource"@en ;
    skos:inScheme <https://w3id.org/nfdi4cat/voc4cat> ;
    skos:narrower <https://w3id.org/nfdi4cat/voc4cat_0007042>,
        <https://w3id.org/nfdi4cat/voc4cat_0007043> ;
    skos:prefLabel "person"@en .

<https://w3id.org/nfdi4cat/voc4cat_0007103> a skos:Concept ;
    dcterms:identifier "voc4cat_0007103"^^xsd:token ;
    skos:broader <https://w3id.org/nfdi4cat/voc4cat_0007101> ;
    skos:definition "An abstract concept/ideal reactor model type, in which the volume of fluid in the reaction vessel is considered to be perfectly mixed which results in the same concentration of all components in the whole reaction volume."@en ;
    skos:historyNote "0000-0001-5886-7860 Hendrik Borgelt created this resource, 0000-0002-5898-1820 David Linke contributed to the definition of the resource"@en ;
    skos:inScheme <https://w3id.org/nfdi4cat/voc4cat> ;
    skos:narrower <https://w3id.org/nfdi4cat/voc4cat_0007106>,
        <https://w3id.org/nfdi4cat/voc4cat_0007107> ;
    skos:prefLabel "stirred tank reactor model"@en .

<https://w3id.org/nfdi4cat/voc4cat_0007239> a skos:Concept ;
    dcterms:identifier "voc4cat_0007239"^^xsd:token ;
    skos:broader <https://w3id.org/nfdi4cat/voc4cat_0000186> ;
    skos:definition "The frequency of an alternating (ac) current is a measure of how many times the direction of the current flow changes, in the same direction, per second. As the direction of flow changes back and forth, the total number of directional changes, per second, is twice the frequency."@en ;
    skos:historyNote "0009-0008-1278-8890 Michael Götte created the resource"@en ;
    skos:inScheme <https://w3id.org/nfdi4cat/voc4cat> ;
    skos:narrower <https://w3id.org/nfdi4cat/voc4cat_0007241>,
        <https://w3id.org/nfdi4cat/voc4cat_0007242> ;
    skos:prefLabel "frequency"@en .

<https://w3id.org/nfdi4cat/voc4cat_0000046> a skos:Concept ;
    dcterms:identifier "voc4cat_0000046"^^xsd:token ;
    skos:broader <https://w3id.org/nfdi4cat/voc4cat_0000184> ;
    skos:definition "Thorough search of available literature on the research topic of interest using online research platforms (e.g, Scopus, Google Scholar, Web of Science, Research Gate etc.) and / or libraries. Relevant literature can be found in the form of publications, books, abstracts and conference presentations."@en ;
    skos:historyNote "0000-0002-6242-2167 Nikolaos G. Moustakas created the resource"@en ;
    skos:inScheme <https://w3id.org/nfdi4cat/voc4cat> ;
    skos:narrower <https://w3id.org/nfdi4cat/voc4cat_0000047>,
        <https://w3id.org/nfdi4cat/voc4cat_0000048> ;
    skos:prefLabel "literature research"@en .

<https://w3id.org/nfdi4cat/voc4cat_0000069> a skos:Concept ;
    dcterms:identifier "voc4cat_0000069"^^xsd:token ;
    skos:altLabel "RAMAN"@en,
        "Raman"@en,
        "Raman scattering spectrometry"@en,
        "Raman spectrometry"@en,
        "raman scattering spectroscopy"@en ;
    skos:broader <https://w3id.org/nfdi4cat/voc4cat_0000066> ;
    skos:definition "A spectroscopy technique studying the vibrational modes of molecules, by measuring the intensity and frequency of scattered by the sample of monochromatic light."@en ;
    skos:historyNote "0000-0002-6242-2167 Nikolaos G. Moustakas created the resource"@en ;
    skos:inScheme <https://w3id.org/nfdi4cat/voc4cat> ;
    skos:prefLabel "Raman spectroscopy"@en .

<https://w3id.org/nfdi4cat/voc4cat_0000073> a skos:Concept ;
    dcterms:identifier "voc4cat_0000073"^^xsd:token ;
    skos:altLabel "NMR"@en ;
    skos:broader <https://w3id.org/nfdi4cat/voc4cat_0000066> ;
    skos:definition "A spectroscopic technique that uses a static magnetic field and radiofrequency radiation to measure the magnetic resonance of atomic nuclei protons or electrons."@en ;
    skos:historyNote "0000-0002-6242-2167 Nikolaos G. Moustakas created the resource"@en ;
    skos:inScheme <https://w3id.org/nfdi4cat/voc4cat> ;
    skos:prefLabel "nuclear magnetic resonance spectroscopy"@en .

<https://w3id.org/nfdi4cat/voc4cat_0000080> a skos:Concept ;
    dcterms:identifier "voc4cat_0000080"^^xsd:token ;
    skos:altLabel "FT-IR"@en,
        "FT-IR spectroscopy"@en,
        "FTIR"@en,
        "FTIR spectrometry"@en,
        "FTIR spectroscopy"@en,
        "Fourier transform infra-red absoprtion spectroscopy"@en,
        "Fourier transform infra-red spectrometry"@en,
        "Fourier transform infrared (FT-IR)"@en,
        "Fourier transform infrared (FT-IR) spectroscopy"@en,
        "Fourier-transform infra-red absorption spectrometry"@en,
        "Fourier-transform infrared (FTIR) absorption spectroscopy"@en ;
    skos:broader <https://w3id.org/nfdi4cat/voc4cat_0000066> ;
    skos:definition "A spectroscopic technique used to study the vibrational modes of chemical bonds of a sample using infrared radiation."@en ;
    skos:historyNote "0000-0002-6242-2167 Nikolaos G. Moustakas created the resource"@en ;
    skos:inScheme <https://w3id.org/nfdi4cat/voc4cat> ;
    skos:prefLabel "Fourier transform infrared spectroscopy"@en .

<https://w3id.org/nfdi4cat/voc4cat_0000084> a skos:Concept ;
    dcterms:identifier "voc4cat_0000084"^^xsd:token ;
    skos:broader <https://w3id.org/nfdi4cat/voc4cat_0000181> ;
    skos:definition "The energy state occupied by an electron in a catalyst. This state can affect the electron's ability to participate in a catalytic reaction."@en ;
    skos:historyNote "0000-0002-6242-2167 Nikolaos G. Moustakas created the resource"@en ;
    skos:inScheme <https://w3id.org/nfdi4cat/voc4cat> ;
    skos:narrower <https://w3id.org/nfdi4cat/voc4cat_0000085>,
        <https://w3id.org/nfdi4cat/voc4cat_0000086> ;
    skos:prefLabel "electronic state"@en .

<https://w3id.org/nfdi4cat/voc4cat_0000105> a skos:Concept ;
    dcterms:identifier "voc4cat_0000105"^^xsd:token ;
    skos:broader <https://w3id.org/nfdi4cat/voc4cat_0000181> ;
    skos:definition "Electron donors or hole scavengers used to reduce the recombination tendency of electrons and holes. Sacrificial reagents are used in catalysis to study an oxidation or reduction reaction separately."@en ;
    skos:historyNote "0000-0002-6242-2167 Nikolaos G. Moustakas created the resource"@en ;
    skos:inScheme <https://w3id.org/nfdi4cat/voc4cat> ;
    skos:narrower <https://w3id.org/nfdi4cat/voc4cat_0000106>,
        <https://w3id.org/nfdi4cat/voc4cat_0000107> ;
    skos:prefLabel "sacrificial reagant"@en .

<https://w3id.org/nfdi4cat/voc4cat_0000108> a skos:Concept ;
    dcterms:identifier "voc4cat_0000108"^^xsd:token ;
    skos:broader <https://w3id.org/nfdi4cat/voc4cat_0000186> ;
    skos:definition "Operation mode under the which the experiment takes place: batch of continuous flow mode."@en ;
    skos:historyNote "0000-0002-6242-2167 Nikolaos G. Moustakas created the resource"@en ;
    skos:inScheme <https://w3id.org/nfdi4cat/voc4cat> ;
    skos:narrower <https://w3id.org/nfdi4cat/voc4cat_0000109>,
        <https://w3id.org/nfdi4cat/voc4cat_0000110> ;
    skos:prefLabel "operation mode"@en .

<https://w3id.org/nfdi4cat/voc4cat_0000115> a skos:Concept ;
    dcterms:identifier "voc4cat_0000115"^^xsd:token ;
    skos:broader <https://w3id.org/nfdi4cat/voc4cat_0000186> ;
    skos:definition "The temperature (range) under which the catalytic reaction takes place."@en ;
    skos:historyNote "0000-0002-6242-2167 Nikolaos G. Moustakas created the resource"@en ;
    skos:inScheme <https://w3id.org/nfdi4cat/voc4cat> ;
    skos:narrower <https://w3id.org/nfdi4cat/voc4cat_0000116>,
        <https://w3id.org/nfdi4cat/voc4cat_0000117> ;
    skos:prefLabel "experiment temperature"@en .

<https://w3id.org/nfdi4cat/voc4cat_0000118> a skos:Concept ;
    dcterms:identifier "voc4cat_0000118"^^xsd:token ;
    skos:broader <https://w3id.org/nfdi4cat/voc4cat_0000186> ;
    skos:definition "The pressure (range) under which the catalytic reaction takes place."@en ;
    skos:historyNote "0000-0002-6242-2167 Nikolaos G. Moustakas created the resource"@en ;
    skos:inScheme <https://w3id.org/nfdi4cat/voc4cat> ;
    skos:narrower <https://w3id.org/nfdi4cat/voc4cat_0000119>,
        <https://w3id.org/nfdi4cat/voc4cat_0000120> ;
    skos:prefLabel "experiment pressure"@en .

<https://w3id.org/nfdi4cat/voc4cat_0000125> a skos:Concept ;
    dcterms:identifier "voc4cat_0000125"^^xsd:token ;
    skos:broader <https://w3id.org/nfdi4cat/voc4cat_0005001>,
        <https://w3id.org/nfdi4cat/voc4cat_0005002>,
        <https://w3id.org/nfdi4cat/voc4cat_0005003> ;
    skos:definition "A dimensionless physical quantity describing how effective a reactant is converted to the desired product in a chemical conversion. It is calculated as the ratio between the amount of the desired product and the amount of the desired product that could have been formed if all reactants were converted to the desired product. The selectivity is 1 (or 100 %) if no other than the desired product is formed."@en ;
    skos:historyNote "0000-0002-6242-2167 Nikolaos G. Moustakas created the resource, 0000-0002-5898-1820 David Linke generalized the definition"@en ;
    skos:inScheme <https://w3id.org/nfdi4cat/voc4cat> ;
    skos:prefLabel "selectivity"@en .

<https://w3id.org/nfdi4cat/voc4cat_0000142> a skos:Concept ;
    dcterms:identifier "voc4cat_0000142"^^xsd:token ;
    skos:broader <https://w3id.org/nfdi4cat/voc4cat_0000186> ;
    skos:definition "The range of parameters, critical for the safe operation of a reactor."@en ;
    skos:historyNote "0000-0002-6242-2167 Nikolaos G. Moustakas created the resource"@en ;
    skos:inScheme <https://w3id.org/nfdi4cat/voc4cat> ;
    skos:narrower <https://w3id.org/nfdi4cat/voc4cat_0000143>,
        <https://w3id.org/nfdi4cat/voc4cat_0000148> ;
    skos:prefLabel "operation parameters"@en .

<https://w3id.org/nfdi4cat/voc4cat_0000143> a skos:Concept ;
    dcterms:identifier "voc4cat_0000143"^^xsd:token ;
    skos:altLabel "operation pressure range"@en,
        "pressure range"@en,
        "range of operation pressure"@en ;
    skos:broader <https://w3id.org/nfdi4cat/voc4cat_0000142> ;
    skos:definition "Maximum and minimum of operation pressure range within the reactor can operate safely. Higher operation temperatures can lead to higher pressure values."@en ;
    skos:historyNote "0000-0002-6242-2167 Nikolaos G. Moustakas created the resource"@en ;
    skos:inScheme <https://w3id.org/nfdi4cat/voc4cat> ;
    skos:narrower <https://w3id.org/nfdi4cat/voc4cat_0000144>,
        <https://w3id.org/nfdi4cat/voc4cat_0000145> ;
    skos:prefLabel "operation pressure"@en .

<https://w3id.org/nfdi4cat/voc4cat_0000148> a skos:Concept ;
    dcterms:identifier "voc4cat_0000148"^^xsd:token ;
    skos:altLabel "operation temperature range"@en,
        "range of operation temperature"@en,
        "temperature range"@en ;
    skos:broader <https://w3id.org/nfdi4cat/voc4cat_0000142> ;
    skos:definition "Maximum and minimum of operation temperature range within the reactor can operate safely."@en ;
    skos:historyNote "0000-0002-6242-2167 Nikolaos G. Moustakas created the resource"@en ;
    skos:inScheme <https://w3id.org/nfdi4cat/voc4cat> ;
    skos:narrower <https://w3id.org/nfdi4cat/voc4cat_0000149>,
        <https://w3id.org/nfdi4cat/voc4cat_0000150> ;
    skos:prefLabel "operation temperature"@en .

<https://w3id.org/nfdi4cat/voc4cat_0000159> a skos:Concept ;
    dcterms:identifier "voc4cat_0000159"^^xsd:token ;
    skos:broader <https://w3id.org/nfdi4cat/voc4cat_0000186> ;
    skos:definition "The dimension of the optical window (diameter / thickness) allowing the incoming light to enter the reaction chamber and interact with the catalyst."@en ;
    skos:historyNote "0000-0002-6242-2167 Nikolaos G. Moustakas created the resource"@en ;
    skos:inScheme <https://w3id.org/nfdi4cat/voc4cat> ;
    skos:narrower <https://w3id.org/nfdi4cat/voc4cat_0000160>,
        <https://w3id.org/nfdi4cat/voc4cat_0000161> ;
    skos:prefLabel "optical window dimensions"@en .

<https://w3id.org/nfdi4cat/voc4cat_0007017> a skos:Concept ;
    dcterms:identifier "voc4cat_0007017"^^xsd:token ;
    skos:broader <https://w3id.org/nfdi4cat/voc4cat_0000180> ;
    skos:definition "An apparatus or system designed for the controlled execution of reactions, encompassing a wide range of processes including chemical, nuclear, biochemical, or other physical transformations."@en ;
    skos:historyNote "0000-0002-4041-0165 Julia Schumann created the resource, 0000-0002-5898-1820 David Linke contributed to the definition of the resource"@en ;
    skos:inScheme <https://w3id.org/nfdi4cat/voc4cat> ;
    skos:narrower <https://w3id.org/nfdi4cat/voc4cat_0000193>,
        <https://w3id.org/nfdi4cat/voc4cat_0007035>,
        <https://w3id.org/nfdi4cat/voc4cat_0007036> ;
    skos:prefLabel "reactor"@en .

<https://w3id.org/nfdi4cat/voc4cat_0007101> a skos:Concept ;
    dcterms:identifier "voc4cat_0007101"^^xsd:token ;
    skos:broader <https://w3id.org/nfdi4cat/voc4cat_0000181> ;
    skos:definition "Chemical reactors are often classified by their abstract concept. The reactor model type characterizes the basic physicochemical behavior of a reactor and thus creates a level of comparability between reactors. Different reactor model types are often used in simulation to simplify complex equations and physical behaviors."@en ;
    skos:historyNote "0000-0001-5886-7860 Hendrik Borgelt created this resource, 0000-0002-5898-1820 David Linke contributed to the definition of the resource"@en ;
    skos:inScheme <https://w3id.org/nfdi4cat/voc4cat> ;
    skos:narrower <https://w3id.org/nfdi4cat/voc4cat_0007102>,
        <https://w3id.org/nfdi4cat/voc4cat_0007103>,
        <https://w3id.org/nfdi4cat/voc4cat_0007104> ;
    skos:prefLabel "reactor model type"@en .

<https://w3id.org/nfdi4cat/voc4cat_0007237> a skos:Concept ;
    dcterms:identifier "voc4cat_0007237"^^xsd:token ;
    skos:broader <https://w3id.org/nfdi4cat/voc4cat_0007206> ;
    skos:definition "An electrochemical measuring technique used for electrochemical analysis, for the determination of the kinetics and mechanism of electrode reactions, and for corrosion studies. \"Voltammetry\" is a family of techniques with the common characteristics that the potential of the working electrode is controlled (typically with a potentiostat) and the current flowing through the electrode is measured."@en ;
    skos:historyNote "0009-0008-1278-8890 Michael Götte created the resource"@en ;
    skos:inScheme <https://w3id.org/nfdi4cat/voc4cat> ;
    skos:narrower <https://w3id.org/nfdi4cat/voc4cat_0000082>,
        <https://w3id.org/nfdi4cat/voc4cat_0007207>,
        <https://w3id.org/nfdi4cat/voc4cat_0007211> ;
    skos:prefLabel "voltammetry"@en .

<https://w3id.org/nfdi4cat/voc4cat_0007249> a skos:Concept ;
    dcterms:identifier "voc4cat_0007249"^^xsd:token ;
    skos:broader <https://w3id.org/nfdi4cat/voc4cat_0000187> ;
    skos:definition "A device that converts chemical energy into electrical energy or vice versa when a chemical reaction is occurring in the cell. Typically, it consists of two metal electrodes immersed into an aqueous solution (electrolyte) with electrode reactions occurring at the electrode-solution surfaces. See also galvanic cell and electrolytic cell."@en ;
    skos:historyNote "0009-0008-1278-8890 Michael Götte created the resource"@en ;
    skos:inScheme <https://w3id.org/nfdi4cat/voc4cat> ;
    skos:narrower <https://w3id.org/nfdi4cat/voc4cat_0000209>,
        <https://w3id.org/nfdi4cat/voc4cat_0007256>,
        <https://w3id.org/nfdi4cat/voc4cat_0007257> ;
    skos:prefLabel "electrochemical cell"@en .

<https://w3id.org/nfdi4cat/voc4cat_0000024> a skos:Concept ;
    dcterms:identifier "voc4cat_0000024"^^xsd:token ;
    skos:broader <https://w3id.org/nfdi4cat/voc4cat_0000190> ;
    skos:definition "The substate onto which a (powdered) catalyst is deposited. Such substrates include glass surfaces (e.g., borosilicate glass or conductive glass like ITO and FTO), ceramic substrates (e.g., alumina) or metal substrates (e.g., Ti foils, stainless steel etc.)."@en ;
    skos:historyNote "0000-0002-6242-2167 Nikolaos G. Moustakas created the resource"@en ;
    skos:inScheme <https://w3id.org/nfdi4cat/voc4cat> ;
    skos:narrower <https://w3id.org/nfdi4cat/voc4cat_0000026>,
        <https://w3id.org/nfdi4cat/voc4cat_0000027>,
        <https://w3id.org/nfdi4cat/voc4cat_0000032> ;
    skos:prefLabel "substrate"@en .

<https://w3id.org/nfdi4cat/voc4cat_0000166> a skos:Concept ;
    dcterms:identifier "voc4cat_0000166"^^xsd:token ;
    skos:broader <https://w3id.org/nfdi4cat/voc4cat_0000165> ;
    skos:definition "Source used to irradiate a catalyst in a reaction chamber. These include sources with various intensities, power, and wavelength ranges, including Hg/Xe lamps, Xe lamps and LEDs."@en ;
    skos:historyNote "0000-0002-6242-2167 Nikolaos G. Moustakas created the resource"@en ;
    skos:inScheme <https://w3id.org/nfdi4cat/voc4cat> ;
    skos:narrower <https://w3id.org/nfdi4cat/voc4cat_0000167>,
        <https://w3id.org/nfdi4cat/voc4cat_0000168>,
        <https://w3id.org/nfdi4cat/voc4cat_0000169> ;
    skos:prefLabel "light source"@en .

<https://w3id.org/nfdi4cat/voc4cat_0000180> a skos:Concept ;
    dcterms:identifier "voc4cat_0000180"^^xsd:token ;
    skos:definition "Entity with a concrete and physical nature."@en ;
    skos:historyNote "0000-0002-6242-2167 Nikolaos G. Moustakas and 0000-0002-5898-1820 David Linke created the resource"@en ;
    skos:inScheme <https://w3id.org/nfdi4cat/voc4cat> ;
    skos:narrower <https://w3id.org/nfdi4cat/voc4cat_0000187>,
        <https://w3id.org/nfdi4cat/voc4cat_0000190>,
        <https://w3id.org/nfdi4cat/voc4cat_0007017>,
        <https://w3id.org/nfdi4cat/voc4cat_0007045> ;
    skos:prefLabel "physical entity"@en ;
    skos:topConceptOf <https://w3id.org/nfdi4cat/voc4cat> .

<https://w3id.org/nfdi4cat/voc4cat_0000182> a skos:Concept ;
    dcterms:identifier "voc4cat_0000182"^^xsd:token ;
    skos:definition "Anything that has a temporal dimension, whether it is an instantaneous point in time, a duration, or a sequence of events."@en ;
    skos:historyNote "0000-0002-6242-2167 Nikolaos G. Moustakas and 0000-0002-5898-1820 David Linke created the resource"@en ;
    skos:inScheme <https://w3id.org/nfdi4cat/voc4cat> ;
    skos:narrower <https://w3id.org/nfdi4cat/voc4cat_0000183>,
        <https://w3id.org/nfdi4cat/voc4cat_0000184>,
        <https://w3id.org/nfdi4cat/voc4cat_0000185>,
        <https://w3id.org/nfdi4cat/voc4cat_0005057> ;
    skos:prefLabel "temporal abstract entity"@en ;
    skos:topConceptOf <https://w3id.org/nfdi4cat/voc4cat> .

<https://w3id.org/nfdi4cat/voc4cat_0000270> a skos:Concept ;
    dcterms:identifier "voc4cat_0000270"^^xsd:token ;
    skos:altLabel "porous media"@en ;
    skos:broader <https://w3id.org/nfdi4cat/voc4cat_0000190> ;
    skos:definition "A solid substance featuring pores, the size, arrangement and shape of which govern the material’s permeability, adsorption properties, and mechanical properties."@en ;
    skos:historyNote "0000-0002-6242-2167 Nikolaos G. Moustakas created the resource"@en ;
    skos:inScheme <https://w3id.org/nfdi4cat/voc4cat> ;
    skos:narrower <https://w3id.org/nfdi4cat/voc4cat_0000198>,
        <https://w3id.org/nfdi4cat/voc4cat_0000271>,
        <https://w3id.org/nfdi4cat/voc4cat_0000272> ;
    skos:prefLabel "porous material"@en .

<https://w3id.org/nfdi4cat/voc4cat_0005001> a skos:Concept ;
    dcterms:identifier "voc4cat_0005001"^^xsd:token ;
    skos:broader <https://w3id.org/nfdi4cat/voc4cat_0000186> ;
    skos:definition "A measure to quantify how fast and selective a chemical conversion occurs in a reactor. A chemical conversion may include multiple reactions."@en ;
    skos:historyNote "0000-0002-5898-1820 David Linke created the resource"@en ;
    skos:inScheme <https://w3id.org/nfdi4cat/voc4cat> ;
    skos:narrower <https://w3id.org/nfdi4cat/voc4cat_0000125>,
        <https://w3id.org/nfdi4cat/voc4cat_0005004>,
        <https://w3id.org/nfdi4cat/voc4cat_0005005>,
        <https://w3id.org/nfdi4cat/voc4cat_0005006> ;
    skos:prefLabel "reactor performance measure"@en .

<https://w3id.org/nfdi4cat/voc4cat_0005002> a skos:Concept ;
    dcterms:identifier "voc4cat_0005002"^^xsd:token ;
    skos:broader <https://w3id.org/nfdi4cat/voc4cat_0000186> ;
    skos:definition "A measure to quantify how fast and selective a chemical conversion occurs. A chemical conversion may include multiple reactions."@en ;
    skos:historyNote "0000-0002-5898-1820 David Linke created the resource"@en ;
    skos:inScheme <https://w3id.org/nfdi4cat/voc4cat> ;
    skos:narrower <https://w3id.org/nfdi4cat/voc4cat_0000125>,
        <https://w3id.org/nfdi4cat/voc4cat_0005004>,
        <https://w3id.org/nfdi4cat/voc4cat_0005005>,
        <https://w3id.org/nfdi4cat/voc4cat_0005006> ;
    skos:prefLabel "chemical conversion performance measure"@en .

<https://w3id.org/nfdi4cat/voc4cat_0005003> a skos:Concept ;
    dcterms:identifier "voc4cat_0005003"^^xsd:token ;
    skos:broader <https://w3id.org/nfdi4cat/voc4cat_0000186> ;
    skos:definition "A measure to quantify how fast and selective a chemical conversion occurs over in presence of a catalyst.  A chemical conversion may include multiple reactions."@en ;
    skos:historyNote "0000-0002-5898-1820 David Linke created the resource"@en ;
    skos:inScheme <https://w3id.org/nfdi4cat/voc4cat> ;
    skos:narrower <https://w3id.org/nfdi4cat/voc4cat_0000125>,
        <https://w3id.org/nfdi4cat/voc4cat_0005004>,
        <https://w3id.org/nfdi4cat/voc4cat_0005005>,
        <https://w3id.org/nfdi4cat/voc4cat_0005006> ;
    skos:prefLabel "catalyst performance measure"@en .

<https://w3id.org/nfdi4cat/voc4cat_0005051> a skos:Concept ;
    dcterms:identifier "voc4cat_0005051"^^xsd:token ;
    skos:broader <https://w3id.org/nfdi4cat/voc4cat_0000181> ;
    skos:definition "A usage status of a pid4cat persistent identifier (PID)."@en ;
    skos:historyNote "0000-0002-5898-1820 David Linke created the resource"@en ;
    skos:inScheme <https://w3id.org/nfdi4cat/voc4cat> ;
    skos:narrower <https://w3id.org/nfdi4cat/voc4cat_0005052>,
        <https://w3id.org/nfdi4cat/voc4cat_0005053>,
        <https://w3id.org/nfdi4cat/voc4cat_0005054>,
        <https://w3id.org/nfdi4cat/voc4cat_0005055> ;
    skos:prefLabel "pid4cat status"@en .

<https://w3id.org/nfdi4cat/voc4cat_0007206> a skos:Concept ;
    dcterms:identifier "voc4cat_0007206"^^xsd:token ;
    skos:broader <https://w3id.org/nfdi4cat/voc4cat_0000185> ;
    skos:definition "An electroanalytical technique based on the measurement of the electromotive force of an electrochemical cell comprised of a measuring and a reference electrode."@en ;
    skos:historyNote "0009-0008-1278-8890 Michael Götte created the resource"@en ;
    skos:inScheme <https://w3id.org/nfdi4cat/voc4cat> ;
    skos:narrower <https://w3id.org/nfdi4cat/voc4cat_0007208>,
        <https://w3id.org/nfdi4cat/voc4cat_0007209>,
        <https://w3id.org/nfdi4cat/voc4cat_0007212>,
        <https://w3id.org/nfdi4cat/voc4cat_0007237> ;
    skos:prefLabel "potentiometry"@en .

<https://w3id.org/nfdi4cat/voc4cat_0000020> a skos:Concept ;
    dcterms:identifier "voc4cat_0000020"^^xsd:token ;
    skos:altLabel "immobilization"@en,
        "immobilization technique"@en ;
    skos:broader <https://w3id.org/nfdi4cat/voc4cat_0000185> ;
    skos:definition "A technique used to deposit (immobilize) a (powdered) catalyst on a substate. These techniques include (but are not limited to): doctor blading, spin coating, spray coating, etc.."@en ;
    skos:historyNote "0000-0002-6242-2167 Nikolaos G. Moustakas created the resource"@en ;
    skos:inScheme <https://w3id.org/nfdi4cat/voc4cat> ;
    skos:narrower <https://w3id.org/nfdi4cat/voc4cat_0000021>,
        <https://w3id.org/nfdi4cat/voc4cat_0000022>,
        <https://w3id.org/nfdi4cat/voc4cat_0000023> ;
    skos:prefLabel "deposition technique"@en .

<https://w3id.org/nfdi4cat/voc4cat_0000027> a skos:Concept ;
    dcterms:identifier "voc4cat_0000027"^^xsd:token ;
    skos:broader <https://w3id.org/nfdi4cat/voc4cat_0000024> ;
    skos:definition "A flat surface made of glass serving as a substrate for the deposition of a catalyst."@en ;
    skos:historyNote "0000-0002-6242-2167 Nikolaos G. Moustakas created the resource"@en ;
    skos:inScheme <https://w3id.org/nfdi4cat/voc4cat> ;
    skos:narrower <https://w3id.org/nfdi4cat/voc4cat_0000028>,
        <https://w3id.org/nfdi4cat/voc4cat_0000029>,
        <https://w3id.org/nfdi4cat/voc4cat_0000030>,
        <https://w3id.org/nfdi4cat/voc4cat_0000031> ;
    skos:prefLabel "glass substrate"@en .

<https://w3id.org/nfdi4cat/voc4cat_0000033> a skos:Concept ;
    dcterms:identifier "voc4cat_0000033"^^xsd:token ;
    skos:broader <https://w3id.org/nfdi4cat/voc4cat_0000186> ;
    skos:definition "The diamensions of the substrate."@en ;
    skos:historyNote "0000-0002-6242-2167 Nikolaos G. Moustakas created the resource"@en ;
    skos:inScheme <https://w3id.org/nfdi4cat/voc4cat> ;
    skos:narrower <https://w3id.org/nfdi4cat/voc4cat_0000034>,
        <https://w3id.org/nfdi4cat/voc4cat_0000035>,
        <https://w3id.org/nfdi4cat/voc4cat_0000036>,
        <https://w3id.org/nfdi4cat/voc4cat_0000037> ;
    skos:prefLabel "substrate dimension"@en .

<https://w3id.org/nfdi4cat/voc4cat_0000040> a skos:Concept ;
    dcterms:identifier "voc4cat_0000040"^^xsd:token ;
    skos:broader <https://w3id.org/nfdi4cat/voc4cat_0000186> ;
    skos:definition "The diamensions of the - deposited on the substrate - thin film."@en ;
    skos:historyNote "0000-0002-6242-2167 Nikolaos G. Moustakas created the resource"@en ;
    skos:inScheme <https://w3id.org/nfdi4cat/voc4cat> ;
    skos:narrower <https://w3id.org/nfdi4cat/voc4cat_0000041>,
        <https://w3id.org/nfdi4cat/voc4cat_0000042>,
        <https://w3id.org/nfdi4cat/voc4cat_0000043>,
        <https://w3id.org/nfdi4cat/voc4cat_0000044> ;
    skos:prefLabel "thin film dimension"@en .

<https://w3id.org/nfdi4cat/voc4cat_0000191> a skos:Concept ;
    dcterms:identifier "voc4cat_0000191"^^xsd:token ;
    skos:broader <https://w3id.org/nfdi4cat/voc4cat_0000192> ;
    skos:definition "A device designed to identify a measurable change or signal in a system, often providing a binary (detected / not detected) or a qualitative response."@en ;
    skos:historyNote "0000-0002-6242-2167 Nikolaos G. Moustakas created the resource"@en ;
    skos:inScheme <https://w3id.org/nfdi4cat/voc4cat> ;
    skos:narrower <https://w3id.org/nfdi4cat/voc4cat_0000131>,
        <https://w3id.org/nfdi4cat/voc4cat_0000132>,
        <https://w3id.org/nfdi4cat/voc4cat_0000133>,
        <https://w3id.org/nfdi4cat/voc4cat_0000134>,
        <https://w3id.org/nfdi4cat/voc4cat_0000138> ;
    skos:prefLabel "detector"@en .

<https://w3id.org/nfdi4cat/voc4cat_0005011> a skos:Concept ;
    dcterms:identifier "voc4cat_0005011"^^xsd:token ;
    skos:broader <https://w3id.org/nfdi4cat/voc4cat_0000181> ;
    skos:definition "A collection of the resource categories used in pid4cat. Resource categories classify for which type of resource the PID is used, e.g. if the PID is for a sample or a device."@en ;
    skos:historyNote "0000-0002-5898-1820 David Linke created the resource"@en ;
    skos:inScheme <https://w3id.org/nfdi4cat/voc4cat> ;
    skos:narrower <https://w3id.org/nfdi4cat/voc4cat_0005012>,
        <https://w3id.org/nfdi4cat/voc4cat_0005013>,
        <https://w3id.org/nfdi4cat/voc4cat_0005014>,
        <https://w3id.org/nfdi4cat/voc4cat_0005015>,
        <https://w3id.org/nfdi4cat/voc4cat_0005016>,
        <https://w3id.org/nfdi4cat/voc4cat_0005017> ;
    skos:prefLabel "PID resource categories"@en .

<https://w3id.org/nfdi4cat/voc4cat_0007219> a skos:Concept ;
    dcterms:identifier "voc4cat_0007219"^^xsd:token ;
    skos:altLabel "voltage"@en ;
    skos:broader <https://w3id.org/nfdi4cat/voc4cat_0000186> ;
    skos:definition "Defined as the amount of work needed per unit of electric charge to move the charge from a reference point to a specific point in an electric field. By definition, the electric potential at the reference point is zero units. A typical reference point is earth (ground)."@en ;
    skos:historyNote "0009-0008-1278-8890 Michael Götte created the resource"@en ;
    skos:inScheme <https://w3id.org/nfdi4cat/voc4cat> ;
    skos:narrower <https://w3id.org/nfdi4cat/voc4cat_0007213>,
        <https://w3id.org/nfdi4cat/voc4cat_0007214>,
        <https://w3id.org/nfdi4cat/voc4cat_0007215>,
        <https://w3id.org/nfdi4cat/voc4cat_0007216>,
        <https://w3id.org/nfdi4cat/voc4cat_0007217>,
        <https://w3id.org/nfdi4cat/voc4cat_0007218> ;
    skos:prefLabel "electrical potential"@en .

<https://w3id.org/nfdi4cat/voc4cat_0000170> a skos:Concept ;
    dcterms:identifier "voc4cat_0000170"^^xsd:token ;
    skos:broader <https://w3id.org/nfdi4cat/voc4cat_0000186> ;
    skos:definition "Specific of properties of the light source dictating its operation and its adequacy in the studied catalytic reaction."@en ;
    skos:historyNote "0000-0002-6242-2167 Nikolaos G. Moustakas created the resource"@en ;
    skos:inScheme <https://w3id.org/nfdi4cat/voc4cat> ;
    skos:narrower <https://w3id.org/nfdi4cat/voc4cat_0000171>,
        <https://w3id.org/nfdi4cat/voc4cat_0000172>,
        <https://w3id.org/nfdi4cat/voc4cat_0000173>,
        <https://w3id.org/nfdi4cat/voc4cat_0000174>,
        <https://w3id.org/nfdi4cat/voc4cat_0000175>,
        <https://w3id.org/nfdi4cat/voc4cat_0000176> ;
    skos:prefLabel "light source property"@en .

<https://w3id.org/nfdi4cat/voc4cat_0007201> a skos:Concept ;
    dcterms:identifier "voc4cat_0007201"^^xsd:token ;
    skos:broader <https://w3id.org/nfdi4cat/voc4cat_0000187> ;
    skos:definition "The two electronically conducting parts of an electrochemical cell."@en ;
    skos:historyNote "0009-0008-1278-8890 Michael Götte created the resource"@en ;
    skos:inScheme <https://w3id.org/nfdi4cat/voc4cat> ;
    skos:narrower <https://w3id.org/nfdi4cat/voc4cat_0007202>,
        <https://w3id.org/nfdi4cat/voc4cat_0007203>,
        <https://w3id.org/nfdi4cat/voc4cat_0007204>,
        <https://w3id.org/nfdi4cat/voc4cat_0007243>,
        <https://w3id.org/nfdi4cat/voc4cat_0007248>,
        <https://w3id.org/nfdi4cat/voc4cat_0007254>,
        <https://w3id.org/nfdi4cat/voc4cat_0007255> ;
    skos:prefLabel "electrode"@en .

<https://w3id.org/nfdi4cat/voc4cat_0000194> a skos:Concept ;
    dcterms:identifier "voc4cat_0000194"^^xsd:token ;
    skos:broader <https://w3id.org/nfdi4cat/voc4cat_0000190> ;
    skos:definition "A material that initiates or increases the rate of a catalytic reaction, without it being consumed in the process."@en ;
    skos:historyNote "0000-0002-6242-2167 Nikolaos G. Moustakas created the resource"@en ;
    skos:inScheme <https://w3id.org/nfdi4cat/voc4cat> ;
    skos:narrower <https://w3id.org/nfdi4cat/voc4cat_0000002>,
        <https://w3id.org/nfdi4cat/voc4cat_0000017>,
        <https://w3id.org/nfdi4cat/voc4cat_0000019>,
        <https://w3id.org/nfdi4cat/voc4cat_0000038>,
        <https://w3id.org/nfdi4cat/voc4cat_0000254>,
        <https://w3id.org/nfdi4cat/voc4cat_0007003>,
        <https://w3id.org/nfdi4cat/voc4cat_0007015>,
        <https://w3id.org/nfdi4cat/voc4cat_0007034> ;
    skos:prefLabel "catalyst"@en .

<https://w3id.org/nfdi4cat/voc4cat_0000184> a skos:Concept ;
    dcterms:identifier "voc4cat_0000184"^^xsd:token ;
    skos:broader <https://w3id.org/nfdi4cat/voc4cat_0000182> ;
    skos:definition "Temporal entities that have a duration and occur at specific points in time."@en ;
    skos:historyNote "0000-0002-6242-2167 Nikolaos G. Moustakas and 0000-0002-5898-1820 David Linke created the resource"@en ;
    skos:inScheme <https://w3id.org/nfdi4cat/voc4cat> ;
    skos:narrower <https://w3id.org/nfdi4cat/voc4cat_0000046>,
        <https://w3id.org/nfdi4cat/voc4cat_0000122>,
        <https://w3id.org/nfdi4cat/voc4cat_0000124>,
        <https://w3id.org/nfdi4cat/voc4cat_0000136>,
        <https://w3id.org/nfdi4cat/voc4cat_0000140>,
        <https://w3id.org/nfdi4cat/voc4cat_0000282>,
        <https://w3id.org/nfdi4cat/voc4cat_0007007>,
        <https://w3id.org/nfdi4cat/voc4cat_0007008>,
        <https://w3id.org/nfdi4cat/voc4cat_0007027>,
        <https://w3id.org/nfdi4cat/voc4cat_0007028>,
        <https://w3id.org/nfdi4cat/voc4cat_0007030>,
        <https://w3id.org/nfdi4cat/voc4cat_0007225>,
        <https://w3id.org/nfdi4cat/voc4cat_0007251> ;
    skos:prefLabel "actions"@en .

<https://w3id.org/nfdi4cat/voc4cat_0000190> a skos:Concept ;
    dcterms:identifier "voc4cat_0000190"^^xsd:token ;
    skos:broader <https://w3id.org/nfdi4cat/voc4cat_0000180> ;
    skos:definition "Substances used as catalysts, supports, or reactants in catalytic processes."@en ;
    skos:historyNote "0000-0002-6242-2167 Nikolaos G. Moustakas created the resource"@en ;
    skos:inScheme <https://w3id.org/nfdi4cat/voc4cat> ;
    skos:narrower <https://w3id.org/nfdi4cat/voc4cat_0000003>,
        <https://w3id.org/nfdi4cat/voc4cat_0000005>,
        <https://w3id.org/nfdi4cat/voc4cat_0000024>,
        <https://w3id.org/nfdi4cat/voc4cat_0000194>,
        <https://w3id.org/nfdi4cat/voc4cat_0000197>,
        <https://w3id.org/nfdi4cat/voc4cat_0000210>,
        <https://w3id.org/nfdi4cat/voc4cat_0000268>,
        <https://w3id.org/nfdi4cat/voc4cat_0000270>,
        <https://w3id.org/nfdi4cat/voc4cat_0000293>,
        <https://w3id.org/nfdi4cat/voc4cat_0000295>,
        <https://w3id.org/nfdi4cat/voc4cat_0000300>,
        <https://w3id.org/nfdi4cat/voc4cat_0000307>,
        <https://w3id.org/nfdi4cat/voc4cat_0005056> ;
    skos:prefLabel "material"@en .

<https://w3id.org/nfdi4cat/voc4cat_0000196> a skos:Concept ;
    dcterms:identifier "voc4cat_0000196"^^xsd:token ;
    skos:altLabel "catalysis domain"@en ;
    skos:broader <https://w3id.org/nfdi4cat/voc4cat_0000181> ;
    skos:definition "An area of study, focusing in a specific sub-section of the general field of catalysis."@en ;
    skos:historyNote "0000-0002-6242-2167 Nikolaos G. Moustakas created the resource"@en ;
    skos:inScheme <https://w3id.org/nfdi4cat/voc4cat> ;
    skos:narrower <https://w3id.org/nfdi4cat/voc4cat_0000001>,
        <https://w3id.org/nfdi4cat/voc4cat_0000204>,
        <https://w3id.org/nfdi4cat/voc4cat_0000207>,
        <https://w3id.org/nfdi4cat/voc4cat_0000208>,
        <https://w3id.org/nfdi4cat/voc4cat_0000216>,
        <https://w3id.org/nfdi4cat/voc4cat_0000217>,
        <https://w3id.org/nfdi4cat/voc4cat_0000232>,
        <https://w3id.org/nfdi4cat/voc4cat_0000233>,
        <https://w3id.org/nfdi4cat/voc4cat_0000246>,
        <https://w3id.org/nfdi4cat/voc4cat_0000294>,
        <https://w3id.org/nfdi4cat/voc4cat_0000296>,
        <https://w3id.org/nfdi4cat/voc4cat_0007001>,
        <https://w3id.org/nfdi4cat/voc4cat_0007002> ;
    skos:prefLabel "catalysis research field"@en .

<https://w3id.org/nfdi4cat/voc4cat_0000066> a skos:Concept ;
    dcterms:identifier "voc4cat_0000066"^^xsd:token ;
    skos:altLabel "characterization"@en ;
    skos:broader <https://w3id.org/nfdi4cat/voc4cat_0000185> ;
    skos:definition "Techniques used to identify the (physico)chemical, morphological, structural, mechanical, optical and electrical properties of the syntesized catalysts. Characterization is performed after the synthesis of the catalysts to evaluate the success of the synthetic approach, but also after the completion of the evaluation of the materials in a reaction to ensure their stability under the selected experimental parameters."@en ;
    skos:historyNote "0000-0002-6242-2167 Nikolaos G. Moustakas created the resource"@en ;
    skos:inScheme <https://w3id.org/nfdi4cat/voc4cat> ;
    skos:narrower <https://w3id.org/nfdi4cat/voc4cat_0000067>,
        <https://w3id.org/nfdi4cat/voc4cat_0000068>,
        <https://w3id.org/nfdi4cat/voc4cat_0000069>,
        <https://w3id.org/nfdi4cat/voc4cat_0000070>,
        <https://w3id.org/nfdi4cat/voc4cat_0000071>,
        <https://w3id.org/nfdi4cat/voc4cat_0000072>,
        <https://w3id.org/nfdi4cat/voc4cat_0000073>,
        <https://w3id.org/nfdi4cat/voc4cat_0000074>,
        <https://w3id.org/nfdi4cat/voc4cat_0000075>,
        <https://w3id.org/nfdi4cat/voc4cat_0000076>,
        <https://w3id.org/nfdi4cat/voc4cat_0000077>,
        <https://w3id.org/nfdi4cat/voc4cat_0000078>,
        <https://w3id.org/nfdi4cat/voc4cat_0000079>,
        <https://w3id.org/nfdi4cat/voc4cat_0000080>,
        <https://w3id.org/nfdi4cat/voc4cat_0000081>,
        <https://w3id.org/nfdi4cat/voc4cat_0000083>,
        <https://w3id.org/nfdi4cat/voc4cat_0000286>,
        <https://w3id.org/nfdi4cat/voc4cat_0000288> ;
    skos:prefLabel "characterization technique"@en .

<https://w3id.org/nfdi4cat/voc4cat_0000187> a skos:Concept ;
    dcterms:identifier "voc4cat_0000187"^^xsd:token ;
    skos:broader <https://w3id.org/nfdi4cat/voc4cat_0000180> ;
    skos:definition "Apparatus, devices, and instruments employed in the construction and operation of experimental setups and the analysis of catalytic reactions and materials."@en ;
    skos:historyNote "0000-0002-6242-2167 Nikolaos G. Moustakas created the resource"@en ;
    skos:inScheme <https://w3id.org/nfdi4cat/voc4cat> ;
    skos:narrower <https://w3id.org/nfdi4cat/voc4cat_0000061>,
        <https://w3id.org/nfdi4cat/voc4cat_0000146>,
        <https://w3id.org/nfdi4cat/voc4cat_0000151>,
        <https://w3id.org/nfdi4cat/voc4cat_0000163>,
        <https://w3id.org/nfdi4cat/voc4cat_0000188>,
        <https://w3id.org/nfdi4cat/voc4cat_0000189>,
        <https://w3id.org/nfdi4cat/voc4cat_0000192>,
        <https://w3id.org/nfdi4cat/voc4cat_0000234>,
        <https://w3id.org/nfdi4cat/voc4cat_0007012>,
        <https://w3id.org/nfdi4cat/voc4cat_0007201>,
        <https://w3id.org/nfdi4cat/voc4cat_0007205>,
        <https://w3id.org/nfdi4cat/voc4cat_0007224>,
        <https://w3id.org/nfdi4cat/voc4cat_0007230>,
        <https://w3id.org/nfdi4cat/voc4cat_0007231>,
        <https://w3id.org/nfdi4cat/voc4cat_0007232>,
        <https://w3id.org/nfdi4cat/voc4cat_0007235>,
        <https://w3id.org/nfdi4cat/voc4cat_0007236>,
        <https://w3id.org/nfdi4cat/voc4cat_0007249>,
        <https://w3id.org/nfdi4cat/voc4cat_0007250> ;
    skos:prefLabel "equipment"@en .

<https://w3id.org/nfdi4cat/voc4cat_0005018> a skos:Concept ;
    dcterms:identifier "voc4cat_0005018"^^xsd:token ;
    skos:broader <https://w3id.org/nfdi4cat/voc4cat_0000181> ;
    skos:definition "The type of relation between two resources. These relations are for example used to express relations between resources identified by their persistent identifiers."@en ;
    skos:historyNote "0000-0002-5898-1820 David Linke created the resource"@en ;
    skos:inScheme <https://w3id.org/nfdi4cat/voc4cat> ;
    skos:narrower <https://w3id.org/nfdi4cat/voc4cat_0005019>,
        <https://w3id.org/nfdi4cat/voc4cat_0005020>,
        <https://w3id.org/nfdi4cat/voc4cat_0005021>,
        <https://w3id.org/nfdi4cat/voc4cat_0005022>,
        <https://w3id.org/nfdi4cat/voc4cat_0005023>,
        <https://w3id.org/nfdi4cat/voc4cat_0005024>,
        <https://w3id.org/nfdi4cat/voc4cat_0005025>,
        <https://w3id.org/nfdi4cat/voc4cat_0005026>,
        <https://w3id.org/nfdi4cat/voc4cat_0005027>,
        <https://w3id.org/nfdi4cat/voc4cat_0005028>,
        <https://w3id.org/nfdi4cat/voc4cat_0005029>,
        <https://w3id.org/nfdi4cat/voc4cat_0005030>,
        <https://w3id.org/nfdi4cat/voc4cat_0005031>,
        <https://w3id.org/nfdi4cat/voc4cat_0005032>,
        <https://w3id.org/nfdi4cat/voc4cat_0005033>,
        <https://w3id.org/nfdi4cat/voc4cat_0005034>,
        <https://w3id.org/nfdi4cat/voc4cat_0005035>,
        <https://w3id.org/nfdi4cat/voc4cat_0005036>,
        <https://w3id.org/nfdi4cat/voc4cat_0005037>,
        <https://w3id.org/nfdi4cat/voc4cat_0005038>,
        <https://w3id.org/nfdi4cat/voc4cat_0005039>,
        <https://w3id.org/nfdi4cat/voc4cat_0005040>,
        <https://w3id.org/nfdi4cat/voc4cat_0005041>,
        <https://w3id.org/nfdi4cat/voc4cat_0005042>,
        <https://w3id.org/nfdi4cat/voc4cat_0005043>,
        <https://w3id.org/nfdi4cat/voc4cat_0005044>,
        <https://w3id.org/nfdi4cat/voc4cat_0005045>,
        <https://w3id.org/nfdi4cat/voc4cat_0005046>,
        <https://w3id.org/nfdi4cat/voc4cat_0005047>,
        <https://w3id.org/nfdi4cat/voc4cat_0005048>,
        <https://w3id.org/nfdi4cat/voc4cat_0005049>,
        <https://w3id.org/nfdi4cat/voc4cat_0005050>,
        <https://w3id.org/nfdi4cat/voc4cat_0005059> ;
    skos:prefLabel "resource relation"@en .

<https://w3id.org/nfdi4cat/voc4cat_0000185> a skos:Concept ;
    dcterms:identifier "voc4cat_0000185"^^xsd:token ;
    skos:broader <https://w3id.org/nfdi4cat/voc4cat_0000182> ;
    skos:definition "A series of temporal entities, like actions, events, changes, or functions that are not isolated but rather a connected sequence of activities. Processes often involve the transformation of inputs into outputs and can be conceptualized as workflows."@en ;
    skos:historyNote "0000-0002-6242-2167 Nikolaos G. Moustakas and 0000-0002-5898-1820 David Linke created the resource"@en ;
    skos:inScheme <https://w3id.org/nfdi4cat/voc4cat> ;
    skos:narrower <https://w3id.org/nfdi4cat/voc4cat_0000014>,
        <https://w3id.org/nfdi4cat/voc4cat_0000020>,
        <https://w3id.org/nfdi4cat/voc4cat_0000045>,
        <https://w3id.org/nfdi4cat/voc4cat_0000049>,
        <https://w3id.org/nfdi4cat/voc4cat_0000066>,
        <https://w3id.org/nfdi4cat/voc4cat_0000087>,
        <https://w3id.org/nfdi4cat/voc4cat_0000099>,
        <https://w3id.org/nfdi4cat/voc4cat_0000100>,
        <https://w3id.org/nfdi4cat/voc4cat_0000123>,
        <https://w3id.org/nfdi4cat/voc4cat_0000130>,
        <https://w3id.org/nfdi4cat/voc4cat_0000137>,
        <https://w3id.org/nfdi4cat/voc4cat_0000141>,
        <https://w3id.org/nfdi4cat/voc4cat_0000202>,
        <https://w3id.org/nfdi4cat/voc4cat_0000205>,
        <https://w3id.org/nfdi4cat/voc4cat_0000206>,
        <https://w3id.org/nfdi4cat/voc4cat_0000221>,
        <https://w3id.org/nfdi4cat/voc4cat_0000227>,
        <https://w3id.org/nfdi4cat/voc4cat_0000239>,
        <https://w3id.org/nfdi4cat/voc4cat_0000248>,
        <https://w3id.org/nfdi4cat/voc4cat_0000249>,
        <https://w3id.org/nfdi4cat/voc4cat_0000250>,
        <https://w3id.org/nfdi4cat/voc4cat_0000251>,
        <https://w3id.org/nfdi4cat/voc4cat_0000256>,
        <https://w3id.org/nfdi4cat/voc4cat_0000262>,
        <https://w3id.org/nfdi4cat/voc4cat_0000265>,
        <https://w3id.org/nfdi4cat/voc4cat_0000266>,
        <https://w3id.org/nfdi4cat/voc4cat_0000269>,
        <https://w3id.org/nfdi4cat/voc4cat_0000273>,
        <https://w3id.org/nfdi4cat/voc4cat_0000281>,
        <https://w3id.org/nfdi4cat/voc4cat_0000285>,
        <https://w3id.org/nfdi4cat/voc4cat_0000291>,
        <https://w3id.org/nfdi4cat/voc4cat_0000304>,
        <https://w3id.org/nfdi4cat/voc4cat_0007029>,
        <https://w3id.org/nfdi4cat/voc4cat_0007031>,
        <https://w3id.org/nfdi4cat/voc4cat_0007206>,
        <https://w3id.org/nfdi4cat/voc4cat_0007238> ;
    skos:prefLabel "processes"@en .

<https://w3id.org/nfdi4cat/voc4cat_0000183> a skos:Concept ;
    dcterms:identifier "voc4cat_0000183"^^xsd:token ;
    skos:broader <https://w3id.org/nfdi4cat/voc4cat_0000182> ;
    skos:definition "An occurrence or happening, marked by a specific point in time. Events can be observed, recorded, and may have an impact on the state of the system or entities involved."@en ;
    skos:historyNote "0000-0002-6242-2167 Nikolaos G. Moustakas and 0000-0002-5898-1820 David Linke created the resource"@en ;
    skos:inScheme <https://w3id.org/nfdi4cat/voc4cat> ;
    skos:narrower <https://w3id.org/nfdi4cat/voc4cat_0000088>,
        <https://w3id.org/nfdi4cat/voc4cat_0000089>,
        <https://w3id.org/nfdi4cat/voc4cat_0000090>,
        <https://w3id.org/nfdi4cat/voc4cat_0000091>,
        <https://w3id.org/nfdi4cat/voc4cat_0000092>,
        <https://w3id.org/nfdi4cat/voc4cat_0000093>,
        <https://w3id.org/nfdi4cat/voc4cat_0000094>,
        <https://w3id.org/nfdi4cat/voc4cat_0000095>,
        <https://w3id.org/nfdi4cat/voc4cat_0000096>,
        <https://w3id.org/nfdi4cat/voc4cat_0000097>,
        <https://w3id.org/nfdi4cat/voc4cat_0000098>,
        <https://w3id.org/nfdi4cat/voc4cat_0000220>,
        <https://w3id.org/nfdi4cat/voc4cat_0000222>,
        <https://w3id.org/nfdi4cat/voc4cat_0000223>,
        <https://w3id.org/nfdi4cat/voc4cat_0000224>,
        <https://w3id.org/nfdi4cat/voc4cat_0000226>,
        <https://w3id.org/nfdi4cat/voc4cat_0000230>,
        <https://w3id.org/nfdi4cat/voc4cat_0000236>,
        <https://w3id.org/nfdi4cat/voc4cat_0000237>,
        <https://w3id.org/nfdi4cat/voc4cat_0000241>,
        <https://w3id.org/nfdi4cat/voc4cat_0000242>,
        <https://w3id.org/nfdi4cat/voc4cat_0000243>,
        <https://w3id.org/nfdi4cat/voc4cat_0000244>,
        <https://w3id.org/nfdi4cat/voc4cat_0000245>,
        <https://w3id.org/nfdi4cat/voc4cat_0000247>,
        <https://w3id.org/nfdi4cat/voc4cat_0000252>,
        <https://w3id.org/nfdi4cat/voc4cat_0000253>,
        <https://w3id.org/nfdi4cat/voc4cat_0000258>,
        <https://w3id.org/nfdi4cat/voc4cat_0000259>,
        <https://w3id.org/nfdi4cat/voc4cat_0000260>,
        <https://w3id.org/nfdi4cat/voc4cat_0000261>,
        <https://w3id.org/nfdi4cat/voc4cat_0000276>,
        <https://w3id.org/nfdi4cat/voc4cat_0000278>,
        <https://w3id.org/nfdi4cat/voc4cat_0000280>,
        <https://w3id.org/nfdi4cat/voc4cat_0000283>,
        <https://w3id.org/nfdi4cat/voc4cat_0000289>,
        <https://w3id.org/nfdi4cat/voc4cat_0000290>,
        <https://w3id.org/nfdi4cat/voc4cat_0000297>,
        <https://w3id.org/nfdi4cat/voc4cat_0000302>,
        <https://w3id.org/nfdi4cat/voc4cat_0000303>,
        <https://w3id.org/nfdi4cat/voc4cat_0000306>,
        <https://w3id.org/nfdi4cat/voc4cat_0007234> ;
    skos:prefLabel "events"@en .

<https://w3id.org/nfdi4cat/voc4cat_0000181> a skos:Concept ;
    dcterms:identifier "voc4cat_0000181"^^xsd:token ;
    skos:definition "Any entity that cannot be located in space-time. E.g., mathematical entities, formal semantics elements, regions within dimensional spaces, ideas, conceptual models."@en ;
    skos:historyNote "0000-0002-6242-2167 Nikolaos G. Moustakas and 0000-0002-5898-1820 David Linke created the resource"@en ;
    skos:inScheme <https://w3id.org/nfdi4cat/voc4cat> ;
    skos:narrower <https://w3id.org/nfdi4cat/voc4cat_0000007>,
        <https://w3id.org/nfdi4cat/voc4cat_0000011>,
        <https://w3id.org/nfdi4cat/voc4cat_0000012>,
        <https://w3id.org/nfdi4cat/voc4cat_0000055>,
        <https://w3id.org/nfdi4cat/voc4cat_0000062>,
        <https://w3id.org/nfdi4cat/voc4cat_0000084>,
        <https://w3id.org/nfdi4cat/voc4cat_0000101>,
        <https://w3id.org/nfdi4cat/voc4cat_0000105>,
        <https://w3id.org/nfdi4cat/voc4cat_0000128>,
        <https://w3id.org/nfdi4cat/voc4cat_0000177>,
        <https://w3id.org/nfdi4cat/voc4cat_0000178>,
        <https://w3id.org/nfdi4cat/voc4cat_0000179>,
        <https://w3id.org/nfdi4cat/voc4cat_0000196>,
        <https://w3id.org/nfdi4cat/voc4cat_0000199>,
        <https://w3id.org/nfdi4cat/voc4cat_0000200>,
        <https://w3id.org/nfdi4cat/voc4cat_0000201>,
        <https://w3id.org/nfdi4cat/voc4cat_0000203>,
        <https://w3id.org/nfdi4cat/voc4cat_0000215>,
        <https://w3id.org/nfdi4cat/voc4cat_0000218>,
        <https://w3id.org/nfdi4cat/voc4cat_0000219>,
        <https://w3id.org/nfdi4cat/voc4cat_0000225>,
        <https://w3id.org/nfdi4cat/voc4cat_0000229>,
        <https://w3id.org/nfdi4cat/voc4cat_0000231>,
        <https://w3id.org/nfdi4cat/voc4cat_0000235>,
        <https://w3id.org/nfdi4cat/voc4cat_0000238>,
        <https://w3id.org/nfdi4cat/voc4cat_0000240>,
        <https://w3id.org/nfdi4cat/voc4cat_0000255>,
        <https://w3id.org/nfdi4cat/voc4cat_0000257>,
        <https://w3id.org/nfdi4cat/voc4cat_0000263>,
        <https://w3id.org/nfdi4cat/voc4cat_0000264>,
        <https://w3id.org/nfdi4cat/voc4cat_0000267>,
        <https://w3id.org/nfdi4cat/voc4cat_0000274>,
        <https://w3id.org/nfdi4cat/voc4cat_0000275>,
        <https://w3id.org/nfdi4cat/voc4cat_0000277>,
        <https://w3id.org/nfdi4cat/voc4cat_0000279>,
        <https://w3id.org/nfdi4cat/voc4cat_0000284>,
        <https://w3id.org/nfdi4cat/voc4cat_0000287>,
        <https://w3id.org/nfdi4cat/voc4cat_0000292>,
        <https://w3id.org/nfdi4cat/voc4cat_0000298>,
        <https://w3id.org/nfdi4cat/voc4cat_0000301>,
        <https://w3id.org/nfdi4cat/voc4cat_0000309>,
        <https://w3id.org/nfdi4cat/voc4cat_0005011>,
        <https://w3id.org/nfdi4cat/voc4cat_0005018>,
        <https://w3id.org/nfdi4cat/voc4cat_0005051>,
        <https://w3id.org/nfdi4cat/voc4cat_0005058>,
        <https://w3id.org/nfdi4cat/voc4cat_0007005>,
        <https://w3id.org/nfdi4cat/voc4cat_0007006>,
        <https://w3id.org/nfdi4cat/voc4cat_0007040>,
        <https://w3id.org/nfdi4cat/voc4cat_0007041>,
        <https://w3id.org/nfdi4cat/voc4cat_0007101>,
        <https://w3id.org/nfdi4cat/voc4cat_0007246>,
        <https://w3id.org/nfdi4cat/voc4cat_0007247> ;
    skos:prefLabel "non-temporal abstract entity"@en ;
    skos:topConceptOf <https://w3id.org/nfdi4cat/voc4cat> .

<https://w3id.org/nfdi4cat/voc4cat_0000186> a skos:Concept ;
    dcterms:identifier "voc4cat_0000186"^^xsd:token ;
    skos:definition "A characteristic of an entity that is intrinsic to and cannot exist without the entity. E.g., properties, characteristics, qualities of things, states."@en ;
    skos:historyNote "0000-0002-6242-2167 Nikolaos G. Moustakas and 0000-0002-5898-1820 David Linke created the resource"@en ;
    skos:inScheme <https://w3id.org/nfdi4cat/voc4cat> ;
    skos:narrower <https://w3id.org/nfdi4cat/voc4cat_0000004>,
        <https://w3id.org/nfdi4cat/voc4cat_0000006>,
        <https://w3id.org/nfdi4cat/voc4cat_0000008>,
        <https://w3id.org/nfdi4cat/voc4cat_0000009>,
        <https://w3id.org/nfdi4cat/voc4cat_0000010>,
        <https://w3id.org/nfdi4cat/voc4cat_0000013>,
        <https://w3id.org/nfdi4cat/voc4cat_0000016>,
        <https://w3id.org/nfdi4cat/voc4cat_0000018>,
        <https://w3id.org/nfdi4cat/voc4cat_0000025>,
        <https://w3id.org/nfdi4cat/voc4cat_0000033>,
        <https://w3id.org/nfdi4cat/voc4cat_0000037>,
        <https://w3id.org/nfdi4cat/voc4cat_0000039>,
        <https://w3id.org/nfdi4cat/voc4cat_0000040>,
        <https://w3id.org/nfdi4cat/voc4cat_0000050>,
        <https://w3id.org/nfdi4cat/voc4cat_0000051>,
        <https://w3id.org/nfdi4cat/voc4cat_0000052>,
        <https://w3id.org/nfdi4cat/voc4cat_0000053>,
        <https://w3id.org/nfdi4cat/voc4cat_0000054>,
        <https://w3id.org/nfdi4cat/voc4cat_0000056>,
        <https://w3id.org/nfdi4cat/voc4cat_0000057>,
        <https://w3id.org/nfdi4cat/voc4cat_0000058>,
        <https://w3id.org/nfdi4cat/voc4cat_0000059>,
        <https://w3id.org/nfdi4cat/voc4cat_0000060>,
        <https://w3id.org/nfdi4cat/voc4cat_0000063>,
        <https://w3id.org/nfdi4cat/voc4cat_0000064>,
        <https://w3id.org/nfdi4cat/voc4cat_0000065>,
        <https://w3id.org/nfdi4cat/voc4cat_0000102>,
        <https://w3id.org/nfdi4cat/voc4cat_0000103>,
        <https://w3id.org/nfdi4cat/voc4cat_0000104>,
        <https://w3id.org/nfdi4cat/voc4cat_0000108>,
        <https://w3id.org/nfdi4cat/voc4cat_0000111>,
        <https://w3id.org/nfdi4cat/voc4cat_0000112>,
        <https://w3id.org/nfdi4cat/voc4cat_0000113>,
        <https://w3id.org/nfdi4cat/voc4cat_0000114>,
        <https://w3id.org/nfdi4cat/voc4cat_0000115>,
        <https://w3id.org/nfdi4cat/voc4cat_0000118>,
        <https://w3id.org/nfdi4cat/voc4cat_0000121>,
        <https://w3id.org/nfdi4cat/voc4cat_0000126>,
        <https://w3id.org/nfdi4cat/voc4cat_0000127>,
        <https://w3id.org/nfdi4cat/voc4cat_0000129>,
        <https://w3id.org/nfdi4cat/voc4cat_0000135>,
        <https://w3id.org/nfdi4cat/voc4cat_0000139>,
        <https://w3id.org/nfdi4cat/voc4cat_0000142>,
        <https://w3id.org/nfdi4cat/voc4cat_0000153>,
        <https://w3id.org/nfdi4cat/voc4cat_0000154>,
        <https://w3id.org/nfdi4cat/voc4cat_0000155>,
        <https://w3id.org/nfdi4cat/voc4cat_0000156>,
        <https://w3id.org/nfdi4cat/voc4cat_0000158>,
        <https://w3id.org/nfdi4cat/voc4cat_0000159>,
        <https://w3id.org/nfdi4cat/voc4cat_0000162>,
        <https://w3id.org/nfdi4cat/voc4cat_0000170>,
        <https://w3id.org/nfdi4cat/voc4cat_0000211>,
        <https://w3id.org/nfdi4cat/voc4cat_0000212>,
        <https://w3id.org/nfdi4cat/voc4cat_0000213>,
        <https://w3id.org/nfdi4cat/voc4cat_0000214>,
        <https://w3id.org/nfdi4cat/voc4cat_0000228>,
        <https://w3id.org/nfdi4cat/voc4cat_0000299>,
        <https://w3id.org/nfdi4cat/voc4cat_0000305>,
        <https://w3id.org/nfdi4cat/voc4cat_0000308>,
        <https://w3id.org/nfdi4cat/voc4cat_0005001>,
        <https://w3id.org/nfdi4cat/voc4cat_0005002>,
        <https://w3id.org/nfdi4cat/voc4cat_0005003>,
        <https://w3id.org/nfdi4cat/voc4cat_0005007>,
        <https://w3id.org/nfdi4cat/voc4cat_0005008>,
        <https://w3id.org/nfdi4cat/voc4cat_0005009>,
        <https://w3id.org/nfdi4cat/voc4cat_0005010>,
        <https://w3id.org/nfdi4cat/voc4cat_0007004>,
        <https://w3id.org/nfdi4cat/voc4cat_0007009>,
        <https://w3id.org/nfdi4cat/voc4cat_0007010>,
        <https://w3id.org/nfdi4cat/voc4cat_0007013>,
        <https://w3id.org/nfdi4cat/voc4cat_0007014>,
        <https://w3id.org/nfdi4cat/voc4cat_0007016>,
        <https://w3id.org/nfdi4cat/voc4cat_0007018>,
        <https://w3id.org/nfdi4cat/voc4cat_0007021>,
        <https://w3id.org/nfdi4cat/voc4cat_0007022>,
        <https://w3id.org/nfdi4cat/voc4cat_0007023>,
        <https://w3id.org/nfdi4cat/voc4cat_0007024>,
        <https://w3id.org/nfdi4cat/voc4cat_0007025>,
        <https://w3id.org/nfdi4cat/voc4cat_0007026>,
        <https://w3id.org/nfdi4cat/voc4cat_0007032>,
        <https://w3id.org/nfdi4cat/voc4cat_0007038>,
        <https://w3id.org/nfdi4cat/voc4cat_0007039>,
        <https://w3id.org/nfdi4cat/voc4cat_0007044>,
        <https://w3id.org/nfdi4cat/voc4cat_0007210>,
        <https://w3id.org/nfdi4cat/voc4cat_0007219>,
        <https://w3id.org/nfdi4cat/voc4cat_0007220>,
        <https://w3id.org/nfdi4cat/voc4cat_0007221>,
        <https://w3id.org/nfdi4cat/voc4cat_0007222>,
        <https://w3id.org/nfdi4cat/voc4cat_0007223>,
        <https://w3id.org/nfdi4cat/voc4cat_0007226>,
        <https://w3id.org/nfdi4cat/voc4cat_0007227>,
        <https://w3id.org/nfdi4cat/voc4cat_0007228>,
        <https://w3id.org/nfdi4cat/voc4cat_0007229>,
        <https://w3id.org/nfdi4cat/voc4cat_0007233>,
        <https://w3id.org/nfdi4cat/voc4cat_0007239>,
        <https://w3id.org/nfdi4cat/voc4cat_0007240>,
        <https://w3id.org/nfdi4cat/voc4cat_0007244>,
        <https://w3id.org/nfdi4cat/voc4cat_0007245>,
        <https://w3id.org/nfdi4cat/voc4cat_0007252>,
        <https://w3id.org/nfdi4cat/voc4cat_0007253>,
        <https://w3id.org/nfdi4cat/voc4cat_0007258>,
        <https://w3id.org/nfdi4cat/voc4cat_0007260>,
        <https://w3id.org/nfdi4cat/voc4cat_0007261>,
        <https://w3id.org/nfdi4cat/voc4cat_0007262>,
        <https://w3id.org/nfdi4cat/voc4cat_0007263> ;
    skos:prefLabel "attributes"@en ;
    skos:topConceptOf <https://w3id.org/nfdi4cat/voc4cat> .

<https://w3id.org/nfdi4cat/voc4cat> a skos:ConceptScheme ;
    dcterms:created "2023-06-29"^^xsd:date ;
    dcterms:creator <https://w3id.org/nfdi4cat/> ;
    dcterms:hasPart <https://w3id.org/nfdi4cat/voc4cat_0000195>,
        <https://w3id.org/nfdi4cat/voc4cat_0001900>,
        <https://w3id.org/nfdi4cat/voc4cat_0001901> ;
    dcterms:identifier "voc4cat"^^xsd:token ;
    dcterms:modified "2025-05-22"^^xsd:date ;
    dcterms:publisher <https://w3id.org/nfdi4cat/> ;
    owl:versionInfo "v2025-05-22" ;
    skos:definition """The Voc4Cat vocabulary is a collection of concepts (or "terms") from the field of catalysis and related disciplines such as chemical engineering or materials science. For each concept, Voc4Cat provides a unique resolvable persistent identifier and a carefully written textual definition, which reflects the community’s shared understanding of the concept’s meaning.

By using the identifiers provided by Voc4Cat to annotate data, rather than just words and symbols, ambiguity as to what is meant is avoided. Producing Voc4Cat-annotated data contributes to realising the vision of machine-actionability described as the ultimate goal of the FAIR principles.

See also [voc4cat help](https://nfdi4cat.github.io/voc4cat/)."""@en ;
    skos:hasTopConcept <https://w3id.org/nfdi4cat/voc4cat_0000180>,
        <https://w3id.org/nfdi4cat/voc4cat_0000181>,
        <https://w3id.org/nfdi4cat/voc4cat_0000182>,
        <https://w3id.org/nfdi4cat/voc4cat_0000186> ;
    skos:historyNote "https://orcid.org/0000-0002-5898-1820 David Linke, https://orcid.org/0000-0002-6242-2167 Nikolaos G. Moustakas"@en ;
    skos:prefLabel "Voc4Cat - A SKOS vocabulary for Catalysis."@en ;
    dcat:contactPoint "David Linke (orcid:0000-0002-5898-1820), Nikolaos G. Moustakas (orcid:0000-0002-6242-2167)" .

